@prefix rdf:	<http://www.w3.org/1999/02/22-rdf-syntax-ns#>.
@prefix skos:	<http://www.w3.org/2004/02/skos/core#>.
@prefix owl:	<http://www.w3.org/2002/07/owl#>.
@prefix subj:	<http://cv.iptc.org/newscodes/subjectcode/>
		
<http://cv.iptc.org/newscodes/subjectcode/> 
	rdf:type skos:ConceptScheme;
	skos:HasTopConcept		subj:01000000;
	skos:HasTopConcept		subj:02000000;
	skos:HasTopConcept		subj:03000000;
	skos:HasTopConcept		subj:04000000;
	skos:HasTopConcept		subj:05000000;
	skos:HasTopConcept		subj:06000000;
	skos:HasTopConcept		subj:07000000;
	skos:HasTopConcept		subj:08000000;
	skos:HasTopConcept		subj:09000000;
	skos:HasTopConcept		subj:10000000;
	skos:HasTopConcept		subj:11000000;
	skos:HasTopConcept		subj:12000000;
	skos:HasTopConcept		subj:13000000;
	skos:HasTopConcept		subj:14000000;
	skos:HasTopConcept		subj:15000000;
	skos:HasTopConcept		subj:16000000;
	skos:HasTopConcept		subj:17000000.

subj:01000000
	rdf:type skos:Concept;
	skos:prefLabel	"arts, culture and entertainment"@en-GB;
	skos:definition	"Matters pertaining to the advancement and refinement of the human mind, of interests, skills, tastes and emotions "@en-GB;
	skos:inScheme <http://cv.iptc.org/newscodes/subjectcode/>;
	skos:exactMatch medtop:01000000;
	skos:narrower	subj:01001000;
	skos:narrower	subj:01002000;
	skos:narrower	subj:01003000;
	skos:narrower	subj:01004000;
	skos:narrower	subj:01005000;
	skos:narrower	subj:01006000;
	skos:narrower	subj:01007000;
	skos:narrower	subj:01008000;
	skos:narrower	subj:01009000;
	skos:narrower	subj:01010000;
	skos:narrower	subj:01011000;
	skos:narrower	subj:01012000;
	skos:narrower	subj:01013000;
	skos:narrower	subj:01014000;
	skos:narrower	subj:01015000;
	skos:narrower	subj:01016000;
	skos:narrower	subj:01017000;
	skos:narrower	subj:01018000;
	skos:narrower	subj:01019000;
	skos:narrower	subj:01020000;
	skos:narrower	subj:01021000;
	skos:narrower	subj:01022000;
	skos:narrower	subj:01023000;
	skos:narrower	subj:01024000;
	skos:narrower	subj:01025000;
	skos:narrower	subj:01026000;
	skos:narrower	subj:01027000;
	skos:narrower	subj:01028000.

subj:01001000
	rdf:type skos:Concept;
	skos:prefLabel	"archaeology"@en-GB;
	skos:definition	"Probing the past through ruins and artefacts "@en-GB;
	skos:inScheme <http://cv.iptc.org/newscodes/subjectcode/>;
	skos:exactMatch medtop:20000744;
	skos:broader	subj:01000000.

subj:01002000
	rdf:type skos:Concept;
	skos:prefLabel	"architecture"@en-GB;
	skos:definition	"Designing of buildings, monuments and the spaces around them "@en-GB;
	skos:inScheme <http://cv.iptc.org/newscodes/subjectcode/>;
	skos:exactMatch medtop:20000032;
	skos:broader	subj:01000000.

subj:01003000
	rdf:type skos:Concept;
	skos:prefLabel	"bullfighting"@en-GB;
	skos:definition	"Classical contest pitting man against the bull "@en-GB;
	skos:inScheme <http://cv.iptc.org/newscodes/subjectcode/>;
	skos:exactMatch medtop:20000875;
	skos:broader	subj:01000000.

subj:01004000
	rdf:type skos:Concept;
	skos:prefLabel	"festive event (including carnival)"@en-GB;
	skos:definition	"Parades, parties, celebrations and the like not necessarily tied to a fixed occasion or date "@en-GB;
	skos:inScheme <http://cv.iptc.org/newscodes/subjectcode/>;
	skos:exactMatch medtop:20000041;
	skos:broader	subj:01000000.

subj:01005000
	rdf:type skos:Concept;
	skos:prefLabel	"cinema"@en-GB;
	skos:definition	"Cinema as art and entertainment "@en-GB;
	skos:inScheme <http://cv.iptc.org/newscodes/subjectcode/>;
	skos:exactMatch medtop:20000005;
	skos:broader	subj:01000000;
	skos:narrower	subj:01005001.

subj:01005001
	rdf:type skos:Concept;
	skos:prefLabel	"film festival"@en-GB;
	skos:definition	"National and international motion pictures festivals, selections, festival juries, nominations, awards etc. "@en-GB;
	skos:inScheme <http://cv.iptc.org/newscodes/subjectcode/>;
	skos:exactMatch medtop:20000006;
	skos:broader	subj:01005000.

subj:01006000
	rdf:type skos:Concept;
	skos:prefLabel	"dance"@en-GB;
	skos:definition	"The expression of emotion or message through movement "@en-GB;
	skos:inScheme <http://cv.iptc.org/newscodes/subjectcode/>;
	skos:exactMatch medtop:20000007;
	skos:broader	subj:01000000.

subj:01007000
	rdf:type skos:Concept;
	skos:prefLabel	"fashion"@en-GB;
	skos:definition	"The design of clothing and accessories "@en-GB;
	skos:inScheme <http://cv.iptc.org/newscodes/subjectcode/>;
	skos:exactMatch medtop:20000011;
	skos:broader	subj:01000000;
	skos:narrower	subj:01007001.

subj:01007001
	rdf:type skos:Concept;
	skos:prefLabel	"jewelry"@en-GB;
	skos:definition	"Accessories to clothing "@en-GB;
	skos:inScheme <http://cv.iptc.org/newscodes/subjectcode/>;
	skos:exactMatch medtop:20000012;
	skos:broader	subj:01007000.

subj:01008000
	rdf:type skos:Concept;
	skos:prefLabel	"language"@en-GB;
	skos:definition	"The means by which people communicate with each other "@en-GB;
	skos:inScheme <http://cv.iptc.org/newscodes/subjectcode/>;
	skos:exactMatch medtop:20000042;
	skos:broader	subj:01000000.

subj:01009000
	rdf:type skos:Concept;
	skos:prefLabel	"library and museum"@en-GB;
	skos:definition	"Edifices used to house collections of books, music, art, or objects from the past and present for public use and display "@en-GB;
	skos:inScheme <http://cv.iptc.org/newscodes/subjectcode/>;
	skos:exactMatch medtop:20000043;
	skos:broader	subj:01000000.

subj:01010000
	rdf:type skos:Concept;
	skos:prefLabel	"literature"@en-GB;
	skos:definition	"The use of pamphlets, books or other printed matter to convey ideas, stories or other messages for the public "@en-GB;
	skos:inScheme <http://cv.iptc.org/newscodes/subjectcode/>;
	skos:exactMatch medtop:20000013;
	skos:broader	subj:01000000;
	skos:narrower	subj:01010001;
	skos:narrower	subj:01010002.

subj:01010001
	rdf:type skos:Concept;
	skos:prefLabel	"fiction"@en-GB;
	skos:definition	"Structured stories that are usually not based on fact but are the creation of the authors imagination "@en-GB;
	skos:inScheme <http://cv.iptc.org/newscodes/subjectcode/>;
	skos:exactMatch medtop:20000015;
	skos:broader	subj:01010000.

subj:01010002
	rdf:type skos:Concept;
	skos:prefLabel	"poetry"@en-GB;
	skos:definition	"The art, structure, forms of poetic expression "@en-GB;
	skos:inScheme <http://cv.iptc.org/newscodes/subjectcode/>;
	skos:exactMatch medtop:20000017;
	skos:broader	subj:01010000.

subj:01011000
	rdf:type skos:Concept;
	skos:prefLabel	"music"@en-GB;
	skos:definition	"Expressing emotion or message through instruments or voice using different sounds, tones, harmonies and the like "@en-GB;
	skos:inScheme <http://cv.iptc.org/newscodes/subjectcode/>;
	skos:exactMatch medtop:20000018;
	skos:broader	subj:01000000;
	skos:narrower	subj:01011001;
	skos:narrower	subj:01011002;
	skos:narrower	subj:01011003;
	skos:narrower	subj:01011004;
	skos:narrower	subj:01011005;
	skos:narrower	subj:01011006;
	skos:narrower	subj:01011007.

subj:01011001
	rdf:type skos:Concept;
	skos:prefLabel	"classical music"@en-GB;
	skos:definition	"Music that follows classic structures of rhythm and harmony "@en-GB;
	skos:inScheme <http://cv.iptc.org/newscodes/subjectcode/>;
	skos:exactMatch medtop:20000022;
	skos:broader	subj:01011000.

subj:01011002
	rdf:type skos:Concept;
	skos:prefLabel	"folk music"@en-GB;
	skos:definition	"Music that developed from folk cultures, often based on story-telling "@en-GB;
	skos:inScheme <http://cv.iptc.org/newscodes/subjectcode/>;
	skos:exactMatch medtop:20000024;
	skos:broader	subj:01011000.

subj:01011003
	rdf:type skos:Concept;
	skos:prefLabel	"jazz music"@en-GB;
	skos:definition	"A music of diverse harmonics, often improvised "@en-GB;
	skos:inScheme <http://cv.iptc.org/newscodes/subjectcode/>;
	skos:exactMatch medtop:20000025;
	skos:broader	subj:01011000.

subj:01011004
	rdf:type skos:Concept;
	skos:prefLabel	"popular music"@en-GB;
	skos:definition	"The latest fad in music, generally aimed at the younger generation "@en-GB;
	skos:inScheme <http://cv.iptc.org/newscodes/subjectcode/>;
	skos:exactMatch medtop:20000026;
	skos:broader	subj:01011000.

subj:01011005
	rdf:type skos:Concept;
	skos:prefLabel	"country music"@en-GB;
	skos:definition	"Similar to folk but is unique to the United States and is less about story telling than about loves sought and lost "@en-GB;
	skos:inScheme <http://cv.iptc.org/newscodes/subjectcode/>;
	skos:exactMatch medtop:20000023;
	skos:broader	subj:01011000.

subj:01011006
	rdf:type skos:Concept;
	skos:prefLabel	"rock and roll music"@en-GB;
	skos:definition	"Popular dance music developed in the 1950s "@en-GB;
	skos:inScheme <http://cv.iptc.org/newscodes/subjectcode/>;
	skos:exactMatch medtop:20000027;
	skos:broader	subj:01011000.

subj:01011007
	rdf:type skos:Concept;
	skos:prefLabel	"hip-hop"@en-GB;
	skos:definition	"A contemporary urban music originating in the 1970s. "@en-GB;
	skos:inScheme <http://cv.iptc.org/newscodes/subjectcode/>;
	skos:broadMatch medtop:20000018;
	skos:broader	subj:01011000.

subj:01012000
	rdf:type skos:Concept;
	skos:prefLabel	"painting"@en-GB;
	skos:definition	"Using the mediums of oils, watercolour, pastel, pencils, chalk, crayon etc on various grounds to express emotion or message "@en-GB;
	skos:inScheme <http://cv.iptc.org/newscodes/subjectcode/>;
	skos:exactMatch medtop:20000035;
	skos:broader	subj:01000000.

subj:01013000
	rdf:type skos:Concept;
	skos:prefLabel	"photography"@en-GB;
	skos:definition	"Mechanical means of creating images of objects by use of light and light sensitive materials with chemicals or by digitals means "@en-GB;
	skos:inScheme <http://cv.iptc.org/newscodes/subjectcode/>;
	skos:exactMatch medtop:20000036;
	skos:broader	subj:01000000.

subj:01014000
	rdf:type skos:Concept;
	skos:prefLabel	"radio"@en-GB;
	skos:definition	"Radio as art and entertainment "@en-GB;
	skos:inScheme <http://cv.iptc.org/newscodes/subjectcode/>;
	skos:exactMatch medtop:20000050;
	skos:broader	subj:01000000.

subj:01015000
	rdf:type skos:Concept;
	skos:prefLabel	"sculpture"@en-GB;
	skos:definition	"Representation of forms in clays, stone, woods, metals or other materials "@en-GB;
	skos:inScheme <http://cv.iptc.org/newscodes/subjectcode/>;
	skos:exactMatch medtop:20000037;
	skos:broader	subj:01000000;
	skos:narrower	subj:01015001.

subj:01015001
	rdf:type skos:Concept;
	skos:prefLabel	"plastic art"@en-GB;
	skos:definition	"Forms of hand created art including installations "@en-GB;
	skos:inScheme <http://cv.iptc.org/newscodes/subjectcode/>;
	skos:closeMatch medtop:20000031;
	skos:broader	subj:01015000.

subj:01016000
	rdf:type skos:Concept;
	skos:prefLabel	"television"@en-GB;
	skos:definition	"Television as art and entertainment "@en-GB;
	skos:inScheme <http://cv.iptc.org/newscodes/subjectcode/>;
	skos:exactMatch medtop:20000051;
	skos:broader	subj:01000000;
	skos:narrower	subj:01016001.

subj:01016001
	rdf:type skos:Concept;
	skos:prefLabel	"soap opera"@en-GB;
	skos:definition	"Episodic TV drama or saga, normally aired during daytime "@en-GB;
	skos:inScheme <http://cv.iptc.org/newscodes/subjectcode/>;
	skos:broadMatch medtop:20000051;
	skos:broader	subj:01016000.

subj:01017000
	rdf:type skos:Concept;
	skos:prefLabel	"theatre"@en-GB;
	skos:definition	"Telling of a story or idea through dialogue, music and physical expression in a space or building designed for it "@en-GB;
	skos:inScheme <http://cv.iptc.org/newscodes/subjectcode/>;
	skos:exactMatch medtop:20000029;
	skos:broader	subj:01000000;
	skos:narrower	subj:01017001.

subj:01017001
	rdf:type skos:Concept;
	skos:prefLabel	"music theatre"@en-GB;
	skos:definition	"Opera, operetta, music revues etc "@en-GB;
	skos:inScheme <http://cv.iptc.org/newscodes/subjectcode/>;
	skos:exactMatch medtop:20000030;
	skos:broader	subj:01017000.

subj:01018000
	rdf:type skos:Concept;
	skos:prefLabel	"monument and heritage site"@en-GB;
	skos:definition	"Areas containing commemorative objects for historical people or events "@en-GB;
	skos:inScheme <http://cv.iptc.org/newscodes/subjectcode/>;
	skos:exactMatch medtop:20000044;
	skos:broader	subj:01000000;
	skos:narrower	subj:01018001.

subj:01018001
	rdf:type skos:Concept;
	skos:prefLabel	"institution-DEPRECATED"@en-GB;
	skos:definition	"NA"@en-GB;
	skos:historyNote	"DEPRECATED in V 14 - term moved to 04018001 "@en-GB;
	skos:inScheme <http://cv.iptc.org/newscodes/subjectcode/>;
	skos:broader	subj:01018000.

subj:01019000
	rdf:type skos:Concept;
	skos:prefLabel	"customs and tradition"@en-GB;
	skos:definition	"A particular way of behaving, or observances that have developed over time by a group of people "@en-GB;
	skos:inScheme <http://cv.iptc.org/newscodes/subjectcode/>;
	skos:exactMatch medtop:20000040;
	skos:broader	subj:01000000.

subj:01020000
	rdf:type skos:Concept;
	skos:prefLabel	"arts (general)"@en-GB;
	skos:definition	"The collective expression of message or emotion through music, literature, painting, theatre or other means "@en-GB;
	skos:inScheme <http://cv.iptc.org/newscodes/subjectcode/>;
	skos:broadMatch medtop:20000002;
	skos:broader	subj:01000000.

subj:01021000
	rdf:type skos:Concept;
	skos:prefLabel	"entertainment (general)"@en-GB;
	skos:definition	"The collective use of television, radio, theatre, music and the like for the amusement of people "@en-GB;
	skos:inScheme <http://cv.iptc.org/newscodes/subjectcode/>;
	skos:broadMatch medtop:20000002;
	skos:broader	subj:01000000;
	skos:narrower	subj:01021001.

subj:01021001
	rdf:type skos:Concept;
	skos:prefLabel	"entertainment award"@en-GB;
	skos:definition	"Awards for achievement in the entertainment industry, such as the Oscars for film, the Booker Prize for Literature, the Grammys for music, or induction into halls of fame. "@en-GB;
	skos:inScheme <http://cv.iptc.org/newscodes/subjectcode/>;
	skos:broadMatch medtop:20000002;
	skos:broader	subj:01021000.

subj:01022000
	rdf:type skos:Concept;
	skos:prefLabel	"culture (general)"@en-GB;
	skos:definition	"The ideas, customs, arts, skills of a particular group "@en-GB;
	skos:inScheme <http://cv.iptc.org/newscodes/subjectcode/>;
	skos:exactMatch medtop:20000038;
	skos:broader	subj:01000000;
	skos:narrower	subj:01022001.

subj:01022001
	rdf:type skos:Concept;
	skos:prefLabel	"cultural development"@en-GB;
	skos:definition	"The history of the development of art and culture such as the rise of cave paintings, pre-Colombian art, Chinese paper-making, anything non-political "@en-GB;
	skos:inScheme <http://cv.iptc.org/newscodes/subjectcode/>;
	skos:exactMatch medtop:20000039;
	skos:broader	subj:01022000.

subj:01023000
	rdf:type skos:Concept;
	skos:prefLabel	"nightclub"@en-GB;
	skos:definition	"A commercial establishment providing music, or other entertainment along with food and drink to selected clientele "@en-GB;
	skos:inScheme <http://cv.iptc.org/newscodes/subjectcode/>;
	skos:exactMatch medtop:20000557;
	skos:broader	subj:01000000.

subj:01024000
	rdf:type skos:Concept;
	skos:prefLabel	"cartoon"@en-GB;
	skos:definition	"Still images such as editorial cartoons and comic strips "@en-GB;
	skos:inScheme <http://cv.iptc.org/newscodes/subjectcode/>;
	skos:exactMatch medtop:20000004;
	skos:broader	subj:01000000.

subj:01025000
	rdf:type skos:Concept;
	skos:prefLabel	"animation"@en-GB;
	skos:definition	"Animation, including full-length and short cinema, artists and merchandising of goods featuring animation characters. "@en-GB;
	skos:inScheme <http://cv.iptc.org/newscodes/subjectcode/>;
	skos:exactMatch medtop:20000003;
	skos:broader	subj:01000000.

subj:01026000
	rdf:type skos:Concept;
	skos:prefLabel	"mass media"@en-GB;
	skos:definition	"Television, radio, magazines, newspapers etc "@en-GB;
	skos:inScheme <http://cv.iptc.org/newscodes/subjectcode/>;
	skos:exactMatch medtop:20000045;
	skos:broader	subj:01000000;
	skos:narrower	subj:01026001;
	skos:narrower	subj:01026002;
	skos:narrower	subj:01026003;
	skos:narrower	subj:01026004.

subj:01026001
	rdf:type skos:Concept;
	skos:prefLabel	"periodicals"@en-GB;
	skos:definition	"Written material that is usually published weekly, bi-weekly, monthly or annually for a long time "@en-GB;
	skos:inScheme <http://cv.iptc.org/newscodes/subjectcode/>;
	skos:exactMatch medtop:20000049;
	skos:broader	subj:01026000.

subj:01026002
	rdf:type skos:Concept;
	skos:prefLabel	"news media"@en-GB;
	skos:definition	"Television, wire services, radio that collect facts about incidents, developing and presenting them to audiences as a whole story "@en-GB;
	skos:inScheme <http://cv.iptc.org/newscodes/subjectcode/>;
	skos:exactMatch medtop:20000046;
	skos:broader	subj:01026000.

subj:01026003
	rdf:type skos:Concept;
	skos:prefLabel	"newspapers"@en-GB;
	skos:definition	"Daily or weekly publications that present the day to day history of the world, as well as features, comics etc "@en-GB;
	skos:inScheme <http://cv.iptc.org/newscodes/subjectcode/>;
	skos:exactMatch medtop:20000047;
	skos:broader	subj:01026000.

subj:01026004
	rdf:type skos:Concept;
	skos:prefLabel	"reviews"@en-GB;
	skos:definition	"A critical look at someone else's work, whether film, theatre or writing "@en-GB;
	skos:inScheme <http://cv.iptc.org/newscodes/subjectcode/>;
	skos:broadMatch medtop:20000002;
	skos:broader	subj:01026000.

subj:01027000
	rdf:type skos:Concept;
	skos:prefLabel	"internet"@en-GB;
	skos:definition	"Internet as art and entertainment "@en-GB;
	skos:inScheme <http://cv.iptc.org/newscodes/subjectcode/>;
	skos:closeMatch medtop:20000048;
	skos:broader	subj:01000000.

subj:01028000
	rdf:type skos:Concept;
	skos:prefLabel	"history"@en-GB;
	skos:definition	"Issues connected with the past; discoveries, repair, conservation or display of artifacts; anniversaries of historic events "@en-GB;
	skos:inScheme <http://cv.iptc.org/newscodes/subjectcode/>;
	skos:exactMatch medtop:20000747;
	skos:broader	subj:01000000.

subj:02000000
	rdf:type skos:Concept;
	skos:prefLabel	"crime, law and justice"@en-GB;
	skos:definition	"Establishment and/or statement of the rules of behaviour in society, the enforcement of these rules, breaches of the rules and the punishment of offenders. Organizations and bodies involved in these activities. "@en-GB;
	skos:inScheme <http://cv.iptc.org/newscodes/subjectcode/>;
	skos:exactMatch medtop:02000000;
	skos:narrower	subj:02001000;
	skos:narrower	subj:02002000;
	skos:narrower	subj:02003000;
	skos:narrower	subj:02004000;
	skos:narrower	subj:02005000;
	skos:narrower	subj:02006000;
	skos:narrower	subj:02007000;
	skos:narrower	subj:02008000;
	skos:narrower	subj:02009000;
	skos:narrower	subj:02010000;
	skos:narrower	subj:02011000;
	skos:narrower	subj:02012000;
	skos:narrower	subj:02013000;
	skos:narrower	subj:02014000;
	skos:narrower	subj:02015000;
	skos:narrower	subj:02016000.

subj:02001000
	rdf:type skos:Concept;
	skos:prefLabel	"crime"@en-GB;
	skos:definition	"Violation of established laws by individuals, companies or organizations "@en-GB;
	skos:inScheme <http://cv.iptc.org/newscodes/subjectcode/>;
	skos:exactMatch medtop:20000082;
	skos:broader	subj:02000000;
	skos:narrower	subj:02001001;
	skos:narrower	subj:02001002;
	skos:narrower	subj:02001003;
	skos:narrower	subj:02001004;
	skos:narrower	subj:02001005;
	skos:narrower	subj:02001006;
	skos:narrower	subj:02001007;
	skos:narrower	subj:02001008;
	skos:narrower	subj:02001009;
	skos:narrower	subj:02001010.

subj:02001001
	rdf:type skos:Concept;
	skos:prefLabel	"homicide"@en-GB;
	skos:definition	"Killing of one person by another "@en-GB;
	skos:inScheme <http://cv.iptc.org/newscodes/subjectcode/>;
	skos:exactMatch medtop:20000099;
	skos:broader	subj:02001000.

subj:02001002
	rdf:type skos:Concept;
	skos:prefLabel	"computer crime"@en-GB;
	skos:definition	"Theft or destructive behaviour using a computer "@en-GB;
	skos:inScheme <http://cv.iptc.org/newscodes/subjectcode/>;
	skos:exactMatch medtop:20000086;
	skos:broader	subj:02001000.

subj:02001003
	rdf:type skos:Concept;
	skos:prefLabel	"theft"@en-GB;
	skos:definition	"Unlawful taking "@en-GB;
	skos:inScheme <http://cv.iptc.org/newscodes/subjectcode/>;
	skos:exactMatch medtop:20000104;
	skos:broader	subj:02001000.

subj:02001004
	rdf:type skos:Concept;
	skos:prefLabel	"drug trafficking"@en-GB;
	skos:definition	"Dealing in illicit often harmful substances "@en-GB;
	skos:inScheme <http://cv.iptc.org/newscodes/subjectcode/>;
	skos:exactMatch medtop:20000096;
	skos:broader	subj:02001000.

subj:02001005
	rdf:type skos:Concept;
	skos:prefLabel	"sexual assault"@en-GB;
	skos:definition	"Sexual battery of one sex against another "@en-GB;
	skos:inScheme <http://cv.iptc.org/newscodes/subjectcode/>;
	skos:exactMatch medtop:20000085;
	skos:broader	subj:02001000.

subj:02001006
	rdf:type skos:Concept;
	skos:prefLabel	"assault (general)"@en-GB;
	skos:definition	"Battery, slugfests, brawls and threatening behaviour "@en-GB;
	skos:inScheme <http://cv.iptc.org/newscodes/subjectcode/>;
	skos:exactMatch medtop:20000084;
	skos:broader	subj:02001000.

subj:02001007
	rdf:type skos:Concept;
	skos:prefLabel	"kidnapping"@en-GB;
	skos:definition	"To seize and detain or carry away a person against that person's will by unlawful threat, force or fraud "@en-GB;
	skos:inScheme <http://cv.iptc.org/newscodes/subjectcode/>;
	skos:exactMatch medtop:20000100;
	skos:broader	subj:02001000.

subj:02001008
	rdf:type skos:Concept;
	skos:prefLabel	"arson"@en-GB;
	skos:definition	"Intentional setting of fires with criminal intent "@en-GB;
	skos:inScheme <http://cv.iptc.org/newscodes/subjectcode/>;
	skos:exactMatch medtop:20000083;
	skos:broader	subj:02001000.

subj:02001009
	rdf:type skos:Concept;
	skos:prefLabel	"gang activity"@en-GB;
	skos:definition	"Criminal activities by groups of individuals, usually in urban areas, who are allied by common territories, languages, ethnic backgrounds but generally are loosely organized. "@en-GB;
	skos:inScheme <http://cv.iptc.org/newscodes/subjectcode/>;
	skos:exactMatch medtop:20000102;
	skos:broader	subj:02001000.

subj:02001010
	rdf:type skos:Concept;
	skos:prefLabel	"terrorism"@en-GB;
	skos:definition	"Violence against people to create fear in order to achieve political or ideological objectives "@en-GB;
	skos:inScheme <http://cv.iptc.org/newscodes/subjectcode/>;
	skos:exactMatch medtop:20000103;
	skos:broader	subj:02001000.

subj:02002000
	rdf:type skos:Concept;
	skos:prefLabel	"judiciary (system of justice)"@en-GB;
	skos:definition	"The system set up to deal with crime and those who do them "@en-GB;
	skos:inScheme <http://cv.iptc.org/newscodes/subjectcode/>;
	skos:exactMatch medtop:20000106;
	skos:broader	subj:02000000;
	skos:narrower	subj:02002001;
	skos:narrower	subj:02002002;
	skos:narrower	subj:02002003.

subj:02002001
	rdf:type skos:Concept;
	skos:prefLabel	"lawyer"@en-GB;
	skos:definition	"Anyone legally able to represent another person or entity in a legal matter, such as a lawyer, solicitor, barrister, procurator, notary. "@en-GB;
	skos:inScheme <http://cv.iptc.org/newscodes/subjectcode/>;
	skos:broadMatch medtop:20000282;
	skos:broader	subj:02002000.

subj:02002002
	rdf:type skos:Concept;
	skos:prefLabel	"judge"@en-GB;
	skos:definition	"Members of the bench that sit in judgement "@en-GB;
	skos:inScheme <http://cv.iptc.org/newscodes/subjectcode/>;
	skos:exactMatch medtop:20000110;
	skos:broader	subj:02002000.

subj:02002003
	rdf:type skos:Concept;
	skos:prefLabel	"court administration"@en-GB;
	skos:definition	"Court clerks, bailiffs, stenographers etc. "@en-GB;
	skos:inScheme <http://cv.iptc.org/newscodes/subjectcode/>;
	skos:exactMatch medtop:20000109;
	skos:broader	subj:02002000.

subj:02003000
	rdf:type skos:Concept;
	skos:prefLabel	"police"@en-GB;
	skos:definition	"Agents of the legal system set up enforce the laws "@en-GB;
	skos:inScheme <http://cv.iptc.org/newscodes/subjectcode/>;
	skos:exactMatch medtop:20000133;
	skos:broader	subj:02000000;
	skos:narrower	subj:02003001;
	skos:narrower	subj:02003002;
	skos:narrower	subj:02003003.

subj:02003001
	rdf:type skos:Concept;
	skos:prefLabel	"law enforcement"@en-GB;
	skos:definition	"Agencies involved in attempts to prevent disobedience to established laws, or to bring to justice those that disobey those laws "@en-GB;
	skos:inScheme <http://cv.iptc.org/newscodes/subjectcode/>;
	skos:exactMatch medtop:20000129;
	skos:broader	subj:02003000.

subj:02003002
	rdf:type skos:Concept;
	skos:prefLabel	"investigation"@en-GB;
	skos:definition	"Process of inquiry of a possible crime up to the point of arrest "@en-GB;
	skos:inScheme <http://cv.iptc.org/newscodes/subjectcode/>;
	skos:exactMatch medtop:20000131;
	skos:broader	subj:02003000.

subj:02003003
	rdf:type skos:Concept;
	skos:prefLabel	"arrest"@en-GB;
	skos:definition	"Detention of a suspect of a crime "@en-GB;
	skos:inScheme <http://cv.iptc.org/newscodes/subjectcode/>;
	skos:exactMatch medtop:20000130;
	skos:broader	subj:02003000.

subj:02004000
	rdf:type skos:Concept;
	skos:prefLabel	"punishment"@en-GB;
	skos:definition	"The retribution handed out to those who break the laws "@en-GB;
	skos:inScheme <http://cv.iptc.org/newscodes/subjectcode/>;
	skos:exactMatch medtop:20000134;
	skos:broader	subj:02000000;
	skos:narrower	subj:02004001;
	skos:narrower	subj:02004002.

subj:02004001
	rdf:type skos:Concept;
	skos:prefLabel	"fine"@en-GB;
	skos:definition	"Monetary punishment "@en-GB;
	skos:inScheme <http://cv.iptc.org/newscodes/subjectcode/>;
	skos:exactMatch medtop:20000136;
	skos:broader	subj:02004000.

subj:02004002
	rdf:type skos:Concept;
	skos:prefLabel	"execution"@en-GB;
	skos:definition	"The carrying out of executions by a government or state, not by extralegal groups/organisations "@en-GB;
	skos:inScheme <http://cv.iptc.org/newscodes/subjectcode/>;
	skos:broadMatch medtop:20000134;
	skos:broader	subj:02004000.

subj:02005000
	rdf:type skos:Concept;
	skos:prefLabel	"prison"@en-GB;
	skos:definition	"Also know as jails, lockups, calaboose, etc. for keeping law breakers from society "@en-GB;
	skos:inScheme <http://cv.iptc.org/newscodes/subjectcode/>;
	skos:exactMatch medtop:20000137;
	skos:broader	subj:02000000.

subj:02006000
	rdf:type skos:Concept;
	skos:prefLabel	"laws"@en-GB;
	skos:definition	"The codification of rules of behaviour "@en-GB;
	skos:inScheme <http://cv.iptc.org/newscodes/subjectcode/>;
	skos:exactMatch medtop:20000121;
	skos:broader	subj:02000000;
	skos:narrower	subj:02006001;
	skos:narrower	subj:02006002.

subj:02006001
	rdf:type skos:Concept;
	skos:prefLabel	"criminal"@en-GB;
	skos:definition	"The criminal code system "@en-GB;
	skos:inScheme <http://cv.iptc.org/newscodes/subjectcode/>;
	skos:exactMatch medtop:20000125;
	skos:broader	subj:02006000.

subj:02006002
	rdf:type skos:Concept;
	skos:prefLabel	"civil"@en-GB;
	skos:definition	"The civil code system "@en-GB;
	skos:inScheme <http://cv.iptc.org/newscodes/subjectcode/>;
	skos:exactMatch medtop:20000122;
	skos:broader	subj:02006000.

subj:02007000
	rdf:type skos:Concept;
	skos:prefLabel	"justice and rights"@en-GB;
	skos:definition	"The equitable administration of laws and regulations "@en-GB;
	skos:inScheme <http://cv.iptc.org/newscodes/subjectcode/>;
	skos:exactMatch medtop:20000119;
	skos:broader	subj:02000000;
	skos:narrower	subj:02007001.

subj:02007001
	rdf:type skos:Concept;
	skos:prefLabel	"civil rights"@en-GB;
	skos:definition	"Rights of individuals under civil law "@en-GB;
	skos:inScheme <http://cv.iptc.org/newscodes/subjectcode/>;
	skos:exactMatch medtop:20000120;
	skos:broader	subj:02007000.

subj:02008000
	rdf:type skos:Concept;
	skos:prefLabel	"trials"@en-GB;
	skos:definition	"The process by which guilt or innocence, or right or wrong is determined and adjudged "@en-GB;
	skos:inScheme <http://cv.iptc.org/newscodes/subjectcode/>;
	skos:exactMatch medtop:20000111;
	skos:broader	subj:02000000;
	skos:narrower	subj:02008001;
	skos:narrower	subj:02008002;
	skos:narrower	subj:02008003.

subj:02008001
	rdf:type skos:Concept;
	skos:prefLabel	"litigation"@en-GB;
	skos:definition	"Taking disputed issues to court for settlement by judge and/or jury "@en-GB;
	skos:inScheme <http://cv.iptc.org/newscodes/subjectcode/>;
	skos:exactMatch medtop:20000114;
	skos:broader	subj:02008000.

subj:02008002
	rdf:type skos:Concept;
	skos:prefLabel	"arbitration"@en-GB;
	skos:definition	"Resolution of disputed issues by a neutral panel "@en-GB;
	skos:inScheme <http://cv.iptc.org/newscodes/subjectcode/>;
	skos:exactMatch medtop:20000117;
	skos:broader	subj:02008000.

subj:02008003
	rdf:type skos:Concept;
	skos:prefLabel	"court preliminary"@en-GB;
	skos:definition	"Pre-trial events including pleas, bail, motions, discovery, depositions. "@en-GB;
	skos:inScheme <http://cv.iptc.org/newscodes/subjectcode/>;
	skos:exactMatch medtop:20000112;
	skos:broader	subj:02008000.

subj:02009000
	rdf:type skos:Concept;
	skos:prefLabel	"prosecution"@en-GB;
	skos:definition	"Stories regarding activities and investigations by public prosecutors. "@en-GB;
	skos:inScheme <http://cv.iptc.org/newscodes/subjectcode/>;
	skos:exactMatch medtop:20000118;
	skos:broader	subj:02000000;
	skos:narrower	subj:02009001;
	skos:narrower	subj:02009002.

subj:02009001
	rdf:type skos:Concept;
	skos:prefLabel	"defendant"@en-GB;
	skos:definition	"The person on trial "@en-GB;
	skos:inScheme <http://cv.iptc.org/newscodes/subjectcode/>;
	skos:exactMatch medtop:20000113;
	skos:broader	subj:02009000.

subj:02009002
	rdf:type skos:Concept;
	skos:prefLabel	"witness"@en-GB;
	skos:definition	"A person who testifies "@en-GB;
	skos:inScheme <http://cv.iptc.org/newscodes/subjectcode/>;
	skos:exactMatch medtop:20000115;
	skos:broader	subj:02009000.

subj:02010000
	rdf:type skos:Concept;
	skos:prefLabel	"organized crime"@en-GB;
	skos:definition	"Crimes committed by gangs or criminal groups. "@en-GB;
	skos:inScheme <http://cv.iptc.org/newscodes/subjectcode/>;
	skos:exactMatch medtop:20000101;
	skos:broader	subj:02000000.

subj:02011000
	rdf:type skos:Concept;
	skos:prefLabel	"international law"@en-GB;
	skos:definition	"The system of laws embraced by all nations, such as the Geneva Convention, the International Law of the Seas, etc. "@en-GB;
	skos:inScheme <http://cv.iptc.org/newscodes/subjectcode/>;
	skos:exactMatch medtop:20000126;
	skos:broader	subj:02000000;
	skos:narrower	subj:02011001;
	skos:narrower	subj:02011002.

subj:02011001
	rdf:type skos:Concept;
	skos:prefLabel	"international court or tribunal"@en-GB;
	skos:definition	"The activities of international tribunals such as European court for human rights, Hague tribunal, International Court of Justice etc "@en-GB;
	skos:inScheme <http://cv.iptc.org/newscodes/subjectcode/>;
	skos:exactMatch medtop:20000128;
	skos:broader	subj:02011000.

subj:02011002
	rdf:type skos:Concept;
	skos:prefLabel	"extradition"@en-GB;
	skos:definition	"Legal transfer of criminals or suspects between countries "@en-GB;
	skos:inScheme <http://cv.iptc.org/newscodes/subjectcode/>;
	skos:exactMatch medtop:20000127;
	skos:broader	subj:02011000.

subj:02012000
	rdf:type skos:Concept;
	skos:prefLabel	"corporate crime"@en-GB;
	skos:definition	"Misdeeds of corporations and corporate officers "@en-GB;
	skos:inScheme <http://cv.iptc.org/newscodes/subjectcode/>;
	skos:exactMatch medtop:20000087;
	skos:broader	subj:02000000;
	skos:narrower	subj:02012001;
	skos:narrower	subj:02012002;
	skos:narrower	subj:02012003;
	skos:narrower	subj:02012004;
	skos:narrower	subj:02012005;
	skos:narrower	subj:02012006;
	skos:narrower	subj:02012007.

subj:02012001
	rdf:type skos:Concept;
	skos:prefLabel	"fraud"@en-GB;
	skos:definition	"Intentional deception that causes others to give up rights or property "@en-GB;
	skos:inScheme <http://cv.iptc.org/newscodes/subjectcode/>;
	skos:exactMatch medtop:20000097;
	skos:broader	subj:02012000.

subj:02012002
	rdf:type skos:Concept;
	skos:prefLabel	"embezzlement"@en-GB;
	skos:definition	"The intentional theft of money left in one's care "@en-GB;
	skos:inScheme <http://cv.iptc.org/newscodes/subjectcode/>;
	skos:exactMatch medtop:20000090;
	skos:broader	subj:02012000.

subj:02012003
	rdf:type skos:Concept;
	skos:prefLabel	"restraint of trade"@en-GB;
	skos:definition	"Interference in free competition in business and trade "@en-GB;
	skos:inScheme <http://cv.iptc.org/newscodes/subjectcode/>;
	skos:exactMatch medtop:20000092;
	skos:broader	subj:02012000.

subj:02012004
	rdf:type skos:Concept;
	skos:prefLabel	"breach of contract"@en-GB;
	skos:definition	"Rupture of legal agreements between companies, and with customers "@en-GB;
	skos:inScheme <http://cv.iptc.org/newscodes/subjectcode/>;
	skos:exactMatch medtop:20000089;
	skos:broader	subj:02012000.

subj:02012005
	rdf:type skos:Concept;
	skos:prefLabel	"anti-trust crime"@en-GB;
	skos:definition	"Violations of laws against monopolies "@en-GB;
	skos:inScheme <http://cv.iptc.org/newscodes/subjectcode/>;
	skos:exactMatch medtop:20000088;
	skos:broader	subj:02012000.

subj:02012006
	rdf:type skos:Concept;
	skos:prefLabel	"corruption"@en-GB;
	skos:definition	"General business misbehaviour "@en-GB;
	skos:inScheme <http://cv.iptc.org/newscodes/subjectcode/>;
	skos:exactMatch medtop:20000093;
	skos:broader	subj:02012000.

subj:02012007
	rdf:type skos:Concept;
	skos:prefLabel	"bribery"@en-GB;
	skos:definition	"Payments or benefits to influence the outcome of a legal case "@en-GB;
	skos:inScheme <http://cv.iptc.org/newscodes/subjectcode/>;
	skos:exactMatch medtop:20000094;
	skos:broader	subj:02012000.

subj:02013000
	rdf:type skos:Concept;
	skos:prefLabel	"war crime"@en-GB;
	skos:definition	"Crimes committed during a war or armed conflict, usually against civilians or POW's, including the prosecution of such crimes "@en-GB;
	skos:inScheme <http://cv.iptc.org/newscodes/subjectcode/>;
	skos:exactMatch medtop:20000105;
	skos:broader	subj:02000000.

subj:02014000
	rdf:type skos:Concept;
	skos:prefLabel	"inquest"@en-GB;
	skos:definition	"Formal investigation of sudden or unexpected death and the hearing to decide cause of death. "@en-GB;
	skos:inScheme <http://cv.iptc.org/newscodes/subjectcode/>;
	skos:broadMatch medtop:20000131;
	skos:broader	subj:02000000.

subj:02015000
	rdf:type skos:Concept;
	skos:prefLabel	"inquiry"@en-GB;
	skos:definition	"Formal hearing involving a disaster, political event etc. Eg rail crash, drug prescription scandal. "@en-GB;
	skos:inScheme <http://cv.iptc.org/newscodes/subjectcode/>;
	skos:broadMatch medtop:20000111;
	skos:broader	subj:02000000.

subj:02016000
	rdf:type skos:Concept;
	skos:prefLabel	"tribunal"@en-GB;
	skos:definition	"Formal hearing usually involving employment issues, property etc. "@en-GB;
	skos:inScheme <http://cv.iptc.org/newscodes/subjectcode/>;
	skos:broadMatch medtop:20000111;
	skos:broader	subj:02000000.

subj:03000000
	rdf:type skos:Concept;
	skos:prefLabel	"disaster and accident"@en-GB;
	skos:definition	"Man made and natural events resulting in loss of life or injury to living creatures and/or damage to inanimate objects or property. "@en-GB;
	skos:inScheme <http://cv.iptc.org/newscodes/subjectcode/>;
	skos:exactMatch medtop:03000000;
	skos:narrower	subj:03001000;
	skos:narrower	subj:03002000;
	skos:narrower	subj:03003000;
	skos:narrower	subj:03004000;
	skos:narrower	subj:03005000;
	skos:narrower	subj:03006000;
	skos:narrower	subj:03007000;
	skos:narrower	subj:03008000;
	skos:narrower	subj:03009000;
	skos:narrower	subj:03010000;
	skos:narrower	subj:03011000;
	skos:narrower	subj:03012000;
	skos:narrower	subj:03013000;
	skos:narrower	subj:03014000;
	skos:narrower	subj:03015000;
	skos:narrower	subj:03016000;
	skos:narrower	subj:03017000.

subj:03001000
	rdf:type skos:Concept;
	skos:prefLabel	"drought"@en-GB;
	skos:definition	"A severe lack of water over a period of time "@en-GB;
	skos:inScheme <http://cv.iptc.org/newscodes/subjectcode/>;
	skos:exactMatch medtop:20000152;
	skos:broader	subj:03000000.

subj:03002000
	rdf:type skos:Concept;
	skos:prefLabel	"earthquake"@en-GB;
	skos:definition	"The shifting of the tectonic plates of the Earth, creating in some cases damage to structures "@en-GB;
	skos:inScheme <http://cv.iptc.org/newscodes/subjectcode/>;
	skos:exactMatch medtop:20000153;
	skos:broader	subj:03000000.

subj:03003000
	rdf:type skos:Concept;
	skos:prefLabel	"famine"@en-GB;
	skos:definition	"Severe lack of food for a large population "@en-GB;
	skos:inScheme <http://cv.iptc.org/newscodes/subjectcode/>;
	skos:exactMatch medtop:20000149;
	skos:broader	subj:03000000.

subj:03004000
	rdf:type skos:Concept;
	skos:prefLabel	"fire"@en-GB;
	skos:definition	"Ignition and consumption of materials through a combination of high heat and oxygen "@en-GB;
	skos:inScheme <http://cv.iptc.org/newscodes/subjectcode/>;
	skos:exactMatch medtop:20000150;
	skos:broader	subj:03000000.

subj:03005000
	rdf:type skos:Concept;
	skos:prefLabel	"flood"@en-GB;
	skos:definition	"Surfeit of water, caused by heavy rains or melting snow, usually in places where it's not wanted "@en-GB;
	skos:inScheme <http://cv.iptc.org/newscodes/subjectcode/>;
	skos:exactMatch medtop:20000154;
	skos:broader	subj:03000000.

subj:03006000
	rdf:type skos:Concept;
	skos:prefLabel	"industrial accident"@en-GB;
	skos:definition	"A mishap in a factory, a shop or an office, potentially harmful to humans "@en-GB;
	skos:inScheme <http://cv.iptc.org/newscodes/subjectcode/>;
	skos:exactMatch medtop:20000141;
	skos:broader	subj:03000000;
	skos:narrower	subj:03006001.

subj:03006001
	rdf:type skos:Concept;
	skos:prefLabel	"structural failures"@en-GB;
	skos:definition	"When a building, bridge or other structures collapse because of unexpected forces or poor design "@en-GB;
	skos:inScheme <http://cv.iptc.org/newscodes/subjectcode/>;
	skos:exactMatch medtop:20000161;
	skos:broader	subj:03006000.

subj:03007000
	rdf:type skos:Concept;
	skos:prefLabel	"meteorological disaster"@en-GB;
	skos:definition	"A weather-related disaster "@en-GB;
	skos:inScheme <http://cv.iptc.org/newscodes/subjectcode/>;
	skos:exactMatch medtop:20000157;
	skos:broader	subj:03000000;
	skos:narrower	subj:03007001.

subj:03007001
	rdf:type skos:Concept;
	skos:prefLabel	"windstorms"@en-GB;
	skos:definition	"A storm of high velocity but non-hurricane force movements of air with little or no rain or hail. Often highly destructive "@en-GB;
	skos:inScheme <http://cv.iptc.org/newscodes/subjectcode/>;
	skos:exactMatch medtop:20000158;
	skos:broader	subj:03007000.

subj:03008000
	rdf:type skos:Concept;
	skos:prefLabel	"nuclear accident"@en-GB;
	skos:definition	"A mishap involving radioactive materials "@en-GB;
	skos:inScheme <http://cv.iptc.org/newscodes/subjectcode/>;
	skos:exactMatch medtop:20000142;
	skos:broader	subj:03000000.

subj:03009000
	rdf:type skos:Concept;
	skos:prefLabel	"pollution"@en-GB;
	skos:definition	"Emissions of unwanted materials in areas where it can be harmful "@en-GB;
	skos:inScheme <http://cv.iptc.org/newscodes/subjectcode/>;
	skos:closeMatch medtop:20000424;
	skos:broader	subj:03000000.

subj:03010000
	rdf:type skos:Concept;
	skos:prefLabel	"transport accident"@en-GB;
	skos:definition	"An accident involving one or more vehicles "@en-GB;
	skos:inScheme <http://cv.iptc.org/newscodes/subjectcode/>;
	skos:exactMatch medtop:20000143;
	skos:broader	subj:03000000;
	skos:narrower	subj:03010001;
	skos:narrower	subj:03010002;
	skos:narrower	subj:03010003;
	skos:narrower	subj:03010004.

subj:03010001
	rdf:type skos:Concept;
	skos:prefLabel	"road accident"@en-GB;
	skos:definition	"Accidents on roads. "@en-GB;
	skos:inScheme <http://cv.iptc.org/newscodes/subjectcode/>;
	skos:exactMatch medtop:20000147;
	skos:broader	subj:03010000.

subj:03010002
	rdf:type skos:Concept;
	skos:prefLabel	"railway accident"@en-GB;
	skos:definition	"Accidents involving trains. "@en-GB;
	skos:inScheme <http://cv.iptc.org/newscodes/subjectcode/>;
	skos:exactMatch medtop:20000146;
	skos:broader	subj:03010000.

subj:03010003
	rdf:type skos:Concept;
	skos:prefLabel	"air and space accident"@en-GB;
	skos:definition	"Accidents involving craft in air or space. "@en-GB;
	skos:inScheme <http://cv.iptc.org/newscodes/subjectcode/>;
	skos:exactMatch medtop:20000144;
	skos:broader	subj:03010000.

subj:03010004
	rdf:type skos:Concept;
	skos:prefLabel	"maritime accident"@en-GB;
	skos:definition	"Accidents involving marine vessels. "@en-GB;
	skos:inScheme <http://cv.iptc.org/newscodes/subjectcode/>;
	skos:exactMatch medtop:20000145;
	skos:broader	subj:03010000.

subj:03011000
	rdf:type skos:Concept;
	skos:prefLabel	"volcanic eruption"@en-GB;
	skos:definition	"A rupture in the skin of the Earth allowing molten material to escape to the surface "@en-GB;
	skos:inScheme <http://cv.iptc.org/newscodes/subjectcode/>;
	skos:exactMatch medtop:20000159;
	skos:broader	subj:03000000.

subj:03012000
	rdf:type skos:Concept;
	skos:prefLabel	"relief and aid organisation"@en-GB;
	skos:definition	"Organizations set up to provide help to those in need because of lack of food, water or shelter "@en-GB;
	skos:inScheme <http://cv.iptc.org/newscodes/subjectcode/>;
	skos:closeMatch medtop:20000168;
	skos:broader	subj:03000000.

subj:03013000
	rdf:type skos:Concept;
	skos:prefLabel	"accident (general)"@en-GB;
	skos:definition	"Any unplanned event that causes unwanted consequences "@en-GB;
	skos:inScheme <http://cv.iptc.org/newscodes/subjectcode/>;
	skos:exactMatch medtop:20000139;
	skos:broader	subj:03000000.

subj:03014000
	rdf:type skos:Concept;
	skos:prefLabel	"emergency incident"@en-GB;
	skos:definition	"A sudden, unexpected event that requires immediate action "@en-GB;
	skos:inScheme <http://cv.iptc.org/newscodes/subjectcode/>;
	skos:exactMatch medtop:20000160;
	skos:broader	subj:03000000;
	skos:narrower	subj:03014001.

subj:03014001
	rdf:type skos:Concept;
	skos:prefLabel	"explosion"@en-GB;
	skos:definition	"Sudden eruptions, usually of chemical substances "@en-GB;
	skos:inScheme <http://cv.iptc.org/newscodes/subjectcode/>;
	skos:exactMatch medtop:20000140;
	skos:broader	subj:03014000.

subj:03015000
	rdf:type skos:Concept;
	skos:prefLabel	"disaster (general)"@en-GB;
	skos:definition	"Serious or sudden misfortune "@en-GB;
	skos:inScheme <http://cv.iptc.org/newscodes/subjectcode/>;
	skos:exactMatch medtop:20000148;
	skos:broader	subj:03000000;
	skos:narrower	subj:03015001;
	skos:narrower	subj:03015002.

subj:03015001
	rdf:type skos:Concept;
	skos:prefLabel	"natural disasters"@en-GB;
	skos:definition	"Destructive incidents caused by the very nature of nature -- hurricanes, earthquakes, floods etc "@en-GB;
	skos:inScheme <http://cv.iptc.org/newscodes/subjectcode/>;
	skos:exactMatch medtop:20000151;
	skos:broader	subj:03015000.

subj:03015002
	rdf:type skos:Concept;
	skos:prefLabel	"avalanche/landslide"@en-GB;
	skos:definition	"Sudden dislodging of massive amounts of snow or soil. "@en-GB;
	skos:inScheme <http://cv.iptc.org/newscodes/subjectcode/>;
	skos:closeMatch medtop:20000155;
	skos:broader	subj:03015000.

subj:03016000
	rdf:type skos:Concept;
	skos:prefLabel	"emergency planning"@en-GB;
	skos:definition	"Planning for actions to deal with sudden, unplanned events "@en-GB;
	skos:inScheme <http://cv.iptc.org/newscodes/subjectcode/>;
	skos:exactMatch medtop:20000167;
	skos:broader	subj:03000000.

subj:03017000
	rdf:type skos:Concept;
	skos:prefLabel	"rescue"@en-GB;
	skos:definition	"An operation to save people, animals or property from harm or danger. "@en-GB;
	skos:inScheme <http://cv.iptc.org/newscodes/subjectcode/>;
	skos:broadMatch medtop:20000168;
	skos:broader	subj:03000000.

subj:04000000
	rdf:type skos:Concept;
	skos:prefLabel	"economy, business and finance"@en-GB;
	skos:definition	"All matters concerning the planning, production and exchange of wealth. "@en-GB;
	skos:inScheme <http://cv.iptc.org/newscodes/subjectcode/>;
	skos:exactMatch medtop:04000000;
	skos:narrower	subj:04001000;
	skos:narrower	subj:04002000;
	skos:narrower	subj:04003000;
	skos:narrower	subj:04004000;
	skos:narrower	subj:04005000;
	skos:narrower	subj:04006000;
	skos:narrower	subj:04007000;
	skos:narrower	subj:04008000;
	skos:narrower	subj:04009000;
	skos:narrower	subj:04010000;
	skos:narrower	subj:04011000;
	skos:narrower	subj:04012000;
	skos:narrower	subj:04013000;
	skos:narrower	subj:04014000;
	skos:narrower	subj:04015000;
	skos:narrower	subj:04016000;
	skos:narrower	subj:04017000;
	skos:narrower	subj:04018000;
	skos:narrower	subj:04019000.

subj:04001000
	rdf:type skos:Concept;
	skos:prefLabel	"agriculture"@en-GB;
	skos:definition	"The process of producing natural materials for consumption "@en-GB;
	skos:inScheme <http://cv.iptc.org/newscodes/subjectcode/>;
	skos:exactMatch medtop:20000210;
	skos:broader	subj:04000000;
	skos:narrower	subj:04001001;
	skos:narrower	subj:04001002;
	skos:narrower	subj:04001003;
	skos:narrower	subj:04001004;
	skos:narrower	subj:04001005;
	skos:narrower	subj:04001006.

subj:04001001
	rdf:type skos:Concept;
	skos:prefLabel	"arable farming"@en-GB;
	skos:definition	"Production of food in the ground "@en-GB;
	skos:inScheme <http://cv.iptc.org/newscodes/subjectcode/>;
	skos:exactMatch medtop:20000212;
	skos:broader	subj:04001000.

subj:04001002
	rdf:type skos:Concept;
	skos:prefLabel	"fishing industry"@en-GB;
	skos:definition	"Raising or gathering of fish "@en-GB;
	skos:inScheme <http://cv.iptc.org/newscodes/subjectcode/>;
	skos:exactMatch medtop:20000213;
	skos:broader	subj:04001000.

subj:04001003
	rdf:type skos:Concept;
	skos:prefLabel	"forestry and timber"@en-GB;
	skos:definition	"Production and collection and preparation of wood products for future use "@en-GB;
	skos:inScheme <http://cv.iptc.org/newscodes/subjectcode/>;
	skos:exactMatch medtop:20000214;
	skos:broader	subj:04001000.

subj:04001004
	rdf:type skos:Concept;
	skos:prefLabel	"livestock farming"@en-GB;
	skos:definition	"Raising of animals for food "@en-GB;
	skos:inScheme <http://cv.iptc.org/newscodes/subjectcode/>;
	skos:exactMatch medtop:20000215;
	skos:broader	subj:04001000.

subj:04001005
	rdf:type skos:Concept;
	skos:prefLabel	"viniculture"@en-GB;
	skos:definition	"Production of wines from the vines to the finish products "@en-GB;
	skos:inScheme <http://cv.iptc.org/newscodes/subjectcode/>;
	skos:exactMatch medtop:20000216;
	skos:broader	subj:04001000.

subj:04001006
	rdf:type skos:Concept;
	skos:prefLabel	"aquaculture"@en-GB;
	skos:definition	"Growing plants or animals in water for human consumption "@en-GB;
	skos:inScheme <http://cv.iptc.org/newscodes/subjectcode/>;
	skos:exactMatch medtop:20000211;
	skos:broader	subj:04001000.

subj:04002000
	rdf:type skos:Concept;
	skos:prefLabel	"chemicals"@en-GB;
	skos:definition	"Natural or manmade materials used to produce other materials "@en-GB;
	skos:inScheme <http://cv.iptc.org/newscodes/subjectcode/>;
	skos:exactMatch medtop:20000217;
	skos:broader	subj:04000000;
	skos:narrower	subj:04002001;
	skos:narrower	subj:04002002;
	skos:narrower	subj:04002003;
	skos:narrower	subj:04002004;
	skos:narrower	subj:04002005;
	skos:narrower	subj:04002006;
	skos:narrower	subj:04002007.

subj:04002001
	rdf:type skos:Concept;
	skos:prefLabel	"biotechnology"@en-GB;
	skos:definition	"The business of using engineering technology to study and solved problems of living organisms "@en-GB;
	skos:inScheme <http://cv.iptc.org/newscodes/subjectcode/>;
	skos:exactMatch medtop:20000218;
	skos:broader	subj:04002000.

subj:04002002
	rdf:type skos:Concept;
	skos:prefLabel	"fertiliser"@en-GB;
	skos:definition	"Natural or manmade materials used to encourage the growth of plants "@en-GB;
	skos:inScheme <http://cv.iptc.org/newscodes/subjectcode/>;
	skos:exactMatch medtop:20000219;
	skos:broader	subj:04002000.

subj:04002003
	rdf:type skos:Concept;
	skos:prefLabel	"health and beauty product"@en-GB;
	skos:definition	"Compilation of chemicals and other substances for use in enhancing ones looks or smell "@en-GB;
	skos:inScheme <http://cv.iptc.org/newscodes/subjectcode/>;
	skos:exactMatch medtop:20000220;
	skos:broader	subj:04002000.

subj:04002004
	rdf:type skos:Concept;
	skos:prefLabel	"inorganic chemical"@en-GB;
	skos:definition	"The branch of chemistry dealing with minerals and metals "@en-GB;
	skos:inScheme <http://cv.iptc.org/newscodes/subjectcode/>;
	skos:exactMatch medtop:20000221;
	skos:broader	subj:04002000.

subj:04002005
	rdf:type skos:Concept;
	skos:prefLabel	"organic chemical"@en-GB;
	skos:definition	"The branch of chemistry dealing with human, animal or carbon-based substances "@en-GB;
	skos:inScheme <http://cv.iptc.org/newscodes/subjectcode/>;
	skos:exactMatch medtop:20000222;
	skos:broader	subj:04002000.

subj:04002006
	rdf:type skos:Concept;
	skos:prefLabel	"pharmaceutical"@en-GB;
	skos:definition	"The production of medicines from various chemicals and natural substances "@en-GB;
	skos:inScheme <http://cv.iptc.org/newscodes/subjectcode/>;
	skos:exactMatch medtop:20000223;
	skos:broader	subj:04002000.

subj:04002007
	rdf:type skos:Concept;
	skos:prefLabel	"synthetic and plastic"@en-GB;
	skos:definition	"Chemicals used to produce plastics and other artificial substances to be used in manufacturing "@en-GB;
	skos:inScheme <http://cv.iptc.org/newscodes/subjectcode/>;
	skos:exactMatch medtop:20000224;
	skos:broader	subj:04002000.

subj:04003000
	rdf:type skos:Concept;
	skos:prefLabel	"computing and information technology"@en-GB;
	skos:definition	"Anything to do with the computing and/or transmission of information from one point to another. "@en-GB;
	skos:inScheme <http://cv.iptc.org/newscodes/subjectcode/>;
	skos:exactMatch medtop:20000225;
	skos:broader	subj:04000000;
	skos:narrower	subj:04003001;
	skos:narrower	subj:04003002;
	skos:narrower	subj:04003003;
	skos:narrower	subj:04003004;
	skos:narrower	subj:04003005;
	skos:narrower	subj:04003006;
	skos:narrower	subj:04003007;
	skos:narrower	subj:04003008;
	skos:narrower	subj:04003009.

subj:04003001
	rdf:type skos:Concept;
	skos:prefLabel	"hardware"@en-GB;
	skos:definition	"The physical devices used to provide computer services, such as monitors, hard drives, keyboards etc. but can also be used for equipment such as routers, servers and other network devices. "@en-GB;
	skos:inScheme <http://cv.iptc.org/newscodes/subjectcode/>;
	skos:broadMatch medtop:20000222;
	skos:broader	subj:04003000.

subj:04003002
	rdf:type skos:Concept;
	skos:prefLabel	"networking"@en-GB;
	skos:definition	"The interconnectivity between hardware that provides the medium for the transmission of data. "@en-GB;
	skos:inScheme <http://cv.iptc.org/newscodes/subjectcode/>;
	skos:exactMatch medtop:20000227;
	skos:broader	subj:04003000.

subj:04003003
	rdf:type skos:Concept;
	skos:prefLabel	"satellite technology"@en-GB;
	skos:definition	"Hardware and software that enables groundbased devices to send signals to each other via an orbiting satellite. "@en-GB;
	skos:inScheme <http://cv.iptc.org/newscodes/subjectcode/>;
	skos:exactMatch medtop:20000228;
	skos:broader	subj:04003000.

subj:04003004
	rdf:type skos:Concept;
	skos:prefLabel	"semiconductors and active components"@en-GB;
	skos:definition	"The basic components that together create working electronic devices such as computers "@en-GB;
	skos:inScheme <http://cv.iptc.org/newscodes/subjectcode/>;
	skos:exactMatch medtop:20000230;
	skos:broader	subj:04003000.

subj:04003005
	rdf:type skos:Concept;
	skos:prefLabel	"software"@en-GB;
	skos:definition	"Programming sets that, when installed on hardware, perform specified functions. "@en-GB;
	skos:inScheme <http://cv.iptc.org/newscodes/subjectcode/>;
	skos:exactMatch medtop:20000231;
	skos:broader	subj:04003000.

subj:04003006
	rdf:type skos:Concept;
	skos:prefLabel	"telecommunication equipment"@en-GB;
	skos:definition	"Devices such as telephone sets, voice/data switches, modems etc that facilitate point-to-point voice/data transmissions "@en-GB;
	skos:inScheme <http://cv.iptc.org/newscodes/subjectcode/>;
	skos:exactMatch medtop:20000232;
	skos:broader	subj:04003000.

subj:04003007
	rdf:type skos:Concept;
	skos:prefLabel	"telecommunication service"@en-GB;
	skos:definition	"Services provided by commercial companies that facilitate connections between telephones, pagers, computers "@en-GB;
	skos:historyNote	"typo fixed in Explanation "@en-GB;
	skos:inScheme <http://cv.iptc.org/newscodes/subjectcode/>;
	skos:exactMatch medtop:20000233;
	skos:broader	subj:04003000.

subj:04003008
	rdf:type skos:Concept;
	skos:prefLabel	"security"@en-GB;
	skos:definition	"To encompass technical developments in hardware and software, basic research and related areas such as cyber security "@en-GB;
	skos:inScheme <http://cv.iptc.org/newscodes/subjectcode/>;
	skos:exactMatch medtop:20000229;
	skos:broader	subj:04003000.

subj:04003009
	rdf:type skos:Concept;
	skos:prefLabel	"wireless technology"@en-GB;
	skos:definition	"Transmission of information through means other than point-to-point wired hookups "@en-GB;
	skos:inScheme <http://cv.iptc.org/newscodes/subjectcode/>;
	skos:exactMatch medtop:20000234;
	skos:broader	subj:04003000.

subj:04004000
	rdf:type skos:Concept;
	skos:prefLabel	"construction and property"@en-GB;
	skos:definition	"All items pertaining to the construction and sale of property "@en-GB;
	skos:inScheme <http://cv.iptc.org/newscodes/subjectcode/>;
	skos:exactMatch medtop:20000235;
	skos:broader	subj:04000000;
	skos:narrower	subj:04004001;
	skos:narrower	subj:04004002;
	skos:narrower	subj:04004003;
	skos:narrower	subj:04004004;
	skos:narrower	subj:04004005;
	skos:narrower	subj:04004006;
	skos:narrower	subj:04004007.

subj:04004001
	rdf:type skos:Concept;
	skos:prefLabel	"heavy construction"@en-GB;
	skos:definition	"Large scale construction projects, construction of roads, dams, office/factory buildings, offshore and onshore structures, large sport stadiums "@en-GB;
	skos:historyNote	"Explanation changed in V 15 "@en-GB;
	skos:inScheme <http://cv.iptc.org/newscodes/subjectcode/>;
	skos:exactMatch medtop:20000238;
	skos:broader	subj:04004000.

subj:04004002
	rdf:type skos:Concept;
	skos:prefLabel	"house building"@en-GB;
	skos:definition	"Construction of residences, for private use "@en-GB;
	skos:inScheme <http://cv.iptc.org/newscodes/subjectcode/>;
	skos:exactMatch medtop:20000239;
	skos:broader	subj:04004000.

subj:04004003
	rdf:type skos:Concept;
	skos:prefLabel	"real estate"@en-GB;
	skos:definition	"The buying and selling of properties of all types "@en-GB;
	skos:inScheme <http://cv.iptc.org/newscodes/subjectcode/>;
	skos:exactMatch medtop:20000241;
	skos:broader	subj:04004000.

subj:04004004
	rdf:type skos:Concept;
	skos:prefLabel	"farms"@en-GB;
	skos:definition	"Agricultural areas for the production of foodstuffs, including dairy products, fruits and livestock, such as cattle and fish "@en-GB;
	skos:inScheme <http://cv.iptc.org/newscodes/subjectcode/>;
	skos:exactMatch medtop:20000237;
	skos:broader	subj:04004000.

subj:04004005
	rdf:type skos:Concept;
	skos:prefLabel	"land price"@en-GB;
	skos:definition	"The price of land in specific zoned areas such as commercial, residential arable as provided by a responsible body "@en-GB;
	skos:historyNote	"In Japan, government publishes lists of standard land prices every year as an economic barometer and Newspapers take up with a lot of space. "@en-GB;
	skos:inScheme <http://cv.iptc.org/newscodes/subjectcode/>;
	skos:exactMatch medtop:20000240;
	skos:broader	subj:04004000.

subj:04004006
	rdf:type skos:Concept;
	skos:prefLabel	"renovation"@en-GB;
	skos:definition	"Restoring properties/structures to a former better state by cleaning, repairing or rebuilding. "@en-GB;
	skos:inScheme <http://cv.iptc.org/newscodes/subjectcode/>;
	skos:exactMatch medtop:20000242;
	skos:broader	subj:04004000.

subj:04004007
	rdf:type skos:Concept;
	skos:prefLabel	"design and engineering"@en-GB;
	skos:definition	"Design and planning by Engineers, Architects etc. of roads, offices, factories, dams , offshore structures, "@en-GB;
	skos:inScheme <http://cv.iptc.org/newscodes/subjectcode/>;
	skos:exactMatch medtop:20000236;
	skos:broader	subj:04004000.

subj:04005000
	rdf:type skos:Concept;
	skos:prefLabel	"energy and resource"@en-GB;
	skos:definition	"Production of electrical power, and the water, air, sunlight, and fuels used to produce them "@en-GB;
	skos:inScheme <http://cv.iptc.org/newscodes/subjectcode/>;
	skos:exactMatch medtop:20000256;
	skos:broader	subj:04000000;
	skos:narrower	subj:04005001;
	skos:narrower	subj:04005002;
	skos:narrower	subj:04005003;
	skos:narrower	subj:04005004;
	skos:narrower	subj:04005005;
	skos:narrower	subj:04005006;
	skos:narrower	subj:04005007;
	skos:narrower	subj:04005008;
	skos:narrower	subj:04005009;
	skos:narrower	subj:04005010;
	skos:narrower	subj:04005011;
	skos:narrower	subj:04005012;
	skos:narrower	subj:04005013;
	skos:narrower	subj:04005014.

subj:04005001
	rdf:type skos:Concept;
	skos:prefLabel	"alternative energy"@en-GB;
	skos:definition	"Alternative energy business "@en-GB;
	skos:inScheme <http://cv.iptc.org/newscodes/subjectcode/>;
	skos:exactMatch medtop:20000257;
	skos:broader	subj:04005000.

subj:04005002
	rdf:type skos:Concept;
	skos:prefLabel	"coal"@en-GB;
	skos:definition	"Production and mining of anthracite and bituminous products for use in power production "@en-GB;
	skos:inScheme <http://cv.iptc.org/newscodes/subjectcode/>;
	skos:exactMatch medtop:20000258;
	skos:broader	subj:04005000.

subj:04005003
	rdf:type skos:Concept;
	skos:prefLabel	"oil and gas - downstream activities"@en-GB;
	skos:definition	"All matters concerning oil and gas, typically refining and distribution activities "@en-GB;
	skos:inScheme <http://cv.iptc.org/newscodes/subjectcode/>;
	skos:exactMatch medtop:20000266;
	skos:broader	subj:04005000.

subj:04005004
	rdf:type skos:Concept;
	skos:prefLabel	"oil and gas - upstream activities"@en-GB;
	skos:definition	"All matters concerning oil and gas, typically supply chain activities from the reservoir to the refinery gate "@en-GB;
	skos:inScheme <http://cv.iptc.org/newscodes/subjectcode/>;
	skos:exactMatch medtop:20000267;
	skos:broader	subj:04005000.

subj:04005005
	rdf:type skos:Concept;
	skos:prefLabel	"nuclear power"@en-GB;
	skos:definition	"Use of radioactive materials for power production "@en-GB;
	skos:inScheme <http://cv.iptc.org/newscodes/subjectcode/>;
	skos:exactMatch medtop:20000265;
	skos:broader	subj:04005000.

subj:04005006
	rdf:type skos:Concept;
	skos:prefLabel	"electricity production and distribution"@en-GB;
	skos:definition	"Primarily concerning the power line distribution system, but also the sale of electrical power at wholesale and retail levels "@en-GB;
	skos:inScheme <http://cv.iptc.org/newscodes/subjectcode/>;
	skos:exactMatch medtop:20000260;
	skos:broader	subj:04005000.

subj:04005007
	rdf:type skos:Concept;
	skos:prefLabel	"waste management and pollution control"@en-GB;
	skos:definition	"The business of waste management and pollution control "@en-GB;
	skos:inScheme <http://cv.iptc.org/newscodes/subjectcode/>;
	skos:exactMatch medtop:20000269;
	skos:broader	subj:04005000.

subj:04005008
	rdf:type skos:Concept;
	skos:prefLabel	"water supply"@en-GB;
	skos:definition	"The business of providing water for human use "@en-GB;
	skos:inScheme <http://cv.iptc.org/newscodes/subjectcode/>;
	skos:exactMatch medtop:20000270;
	skos:broader	subj:04005000.

subj:04005009
	rdf:type skos:Concept;
	skos:prefLabel	"natural resources (general)"@en-GB;
	skos:definition	"The general use of natural resources for business purposes, not focused on specific resources such as coal, oil, gas or water "@en-GB;
	skos:inScheme <http://cv.iptc.org/newscodes/subjectcode/>;
	skos:broadMatch medtop:20000256;
	skos:broader	subj:04005000.

subj:04005010
	rdf:type skos:Concept;
	skos:prefLabel	"energy (general)"@en-GB;
	skos:definition	"Energy industry, not focused on any specific sector "@en-GB;
	skos:inScheme <http://cv.iptc.org/newscodes/subjectcode/>;
	skos:broadMatch medtop:20000256;
	skos:broader	subj:04005000.

subj:04005011
	rdf:type skos:Concept;
	skos:prefLabel	"natural gas"@en-GB;
	skos:definition	"A natural resource, mainly methane in an flammable gaseous state, from the ground "@en-GB;
	skos:inScheme <http://cv.iptc.org/newscodes/subjectcode/>;
	skos:exactMatch medtop:20000263;
	skos:broader	subj:04005000.

subj:04005012
	rdf:type skos:Concept;
	skos:prefLabel	"petrol"@en-GB;
	skos:definition	"Distilled petroleum product used for automotive fuel, with or without additives "@en-GB;
	skos:inScheme <http://cv.iptc.org/newscodes/subjectcode/>;
	skos:exactMatch medtop:20000268;
	skos:broader	subj:04005000.

subj:04005013
	rdf:type skos:Concept;
	skos:prefLabel	"diesel fuel"@en-GB;
	skos:definition	"A distilled petroleum product heavier than gasoline used not only for trucks, marine engines, but in certain forms for home heating "@en-GB;
	skos:inScheme <http://cv.iptc.org/newscodes/subjectcode/>;
	skos:exactMatch medtop:20000259;
	skos:broader	subj:04005000.

subj:04005014
	rdf:type skos:Concept;
	skos:prefLabel	"kerosene/paraffin"@en-GB;
	skos:definition	"A light petroleum distillate used for cooking fuel, aircraft jet engines, lamps, heating and cleaning "@en-GB;
	skos:inScheme <http://cv.iptc.org/newscodes/subjectcode/>;
	skos:exactMatch medtop:20000262;
	skos:broader	subj:04005000.

subj:04006000
	rdf:type skos:Concept;
	skos:prefLabel	"financial and business service"@en-GB;
	skos:definition	"Services that transmit, safeguard, keep track of money or provide backup to commercial enterprises "@en-GB;
	skos:inScheme <http://cv.iptc.org/newscodes/subjectcode/>;
	skos:exactMatch medtop:20000271;
	skos:broader	subj:04000000;
	skos:narrower	subj:04006001;
	skos:narrower	subj:04006002;
	skos:narrower	subj:04006003;
	skos:narrower	subj:04006004;
	skos:narrower	subj:04006005;
	skos:narrower	subj:04006006;
	skos:narrower	subj:04006007;
	skos:narrower	subj:04006008;
	skos:narrower	subj:04006009;
	skos:narrower	subj:04006010;
	skos:narrower	subj:04006011;
	skos:narrower	subj:04006012;
	skos:narrower	subj:04006013;
	skos:narrower	subj:04006014;
	skos:narrower	subj:04006015;
	skos:narrower	subj:04006016;
	skos:narrower	subj:04006017;
	skos:narrower	subj:04006018;
	skos:narrower	subj:04006019;
	skos:narrower	subj:04006020;
	skos:narrower	subj:04006021;
	skos:narrower	subj:04006022.

subj:04006001
	rdf:type skos:Concept;
	skos:prefLabel	"accountancy and auditing"@en-GB;
	skos:definition	"Services provide balance sheet, budgets reconciliation and examine accuracy of financial statements "@en-GB;
	skos:inScheme <http://cv.iptc.org/newscodes/subjectcode/>;
	skos:exactMatch medtop:20000272;
	skos:broader	subj:04006000.

subj:04006002
	rdf:type skos:Concept;
	skos:prefLabel	"banking"@en-GB;
	skos:definition	"Services for storing, transmitting, receiving and delivery of cash moneys "@en-GB;
	skos:inScheme <http://cv.iptc.org/newscodes/subjectcode/>;
	skos:exactMatch medtop:20000274;
	skos:broader	subj:04006000.

subj:04006003
	rdf:type skos:Concept;
	skos:prefLabel	"consultancy service"@en-GB;
	skos:definition	"Providers of expert knowledge in a wide range of fields usually on a temporary, contract basis "@en-GB;
	skos:inScheme <http://cv.iptc.org/newscodes/subjectcode/>;
	skos:exactMatch medtop:20000275;
	skos:broader	subj:04006000.

subj:04006004
	rdf:type skos:Concept;
	skos:prefLabel	"employment agency"@en-GB;
	skos:definition	"A service helping people find jobs, and companies to find workers "@en-GB;
	skos:inScheme <http://cv.iptc.org/newscodes/subjectcode/>;
	skos:exactMatch medtop:20000276;
	skos:broader	subj:04006000.

subj:04006005
	rdf:type skos:Concept;
	skos:prefLabel	"healthcare provider"@en-GB;
	skos:definition	"Providers of medical services at all levels, including doctors, hospitals etc "@en-GB;
	skos:inScheme <http://cv.iptc.org/newscodes/subjectcode/>;
	skos:exactMatch medtop:20000278;
	skos:broader	subj:04006000.

subj:04006006
	rdf:type skos:Concept;
	skos:prefLabel	"insurance"@en-GB;
	skos:definition	"A risk taking venture that allows individuals to pay small amounts periodically to guard financially against unexpected events "@en-GB;
	skos:inScheme <http://cv.iptc.org/newscodes/subjectcode/>;
	skos:exactMatch medtop:20000279;
	skos:broader	subj:04006000.

subj:04006007
	rdf:type skos:Concept;
	skos:prefLabel	"legal service"@en-GB;
	skos:definition	"Lawyers and others who help companies and individuals deal with state, federal and local laws "@en-GB;
	skos:inScheme <http://cv.iptc.org/newscodes/subjectcode/>;
	skos:exactMatch medtop:20000282;
	skos:broader	subj:04006000.

subj:04006008
	rdf:type skos:Concept;
	skos:prefLabel	"market research"@en-GB;
	skos:definition	"A service that tries to determine what people want to buy "@en-GB;
	skos:inScheme <http://cv.iptc.org/newscodes/subjectcode/>;
	skos:exactMatch medtop:20000283;
	skos:broader	subj:04006000.

subj:04006009
	rdf:type skos:Concept;
	skos:prefLabel	"stock broking"@en-GB;
	skos:definition	"The buying and selling of company shares on behalf of individuals or other entities "@en-GB;
	skos:inScheme <http://cv.iptc.org/newscodes/subjectcode/>;
	skos:exactMatch medtop:20000292;
	skos:broader	subj:04006000.

subj:04006010
	rdf:type skos:Concept;
	skos:prefLabel	"personal investing"@en-GB;
	skos:definition	"Personal finance and investment "@en-GB;
	skos:inScheme <http://cv.iptc.org/newscodes/subjectcode/>;
	skos:exactMatch medtop:20000287;
	skos:broader	subj:04006000.

subj:04006011
	rdf:type skos:Concept;
	skos:prefLabel	"market trend"@en-GB;
	skos:definition	"Statistically significant consumer behaviour. "@en-GB;
	skos:inScheme <http://cv.iptc.org/newscodes/subjectcode/>;
	skos:exactMatch medtop:20000284;
	skos:broader	subj:04006000.

subj:04006012
	rdf:type skos:Concept;
	skos:prefLabel	"shipping service"@en-GB;
	skos:definition	"Companies that prepare and transport packages and documents for individuals or companies by any means, including postal services. "@en-GB;
	skos:inScheme <http://cv.iptc.org/newscodes/subjectcode/>;
	skos:exactMatch medtop:20000291;
	skos:broader	subj:04006000.

subj:04006013
	rdf:type skos:Concept;
	skos:prefLabel	"personal service"@en-GB;
	skos:definition	"Consumer service that is intangible e.g. beauty care as in hairdressing "@en-GB;
	skos:inScheme <http://cv.iptc.org/newscodes/subjectcode/>;
	skos:exactMatch medtop:20000288;
	skos:broader	subj:04006000.

subj:04006014
	rdf:type skos:Concept;
	skos:prefLabel	"janitorial service"@en-GB;
	skos:definition	"Companies that provide cleaning and similar services for homes and businesses. "@en-GB;
	skos:inScheme <http://cv.iptc.org/newscodes/subjectcode/>;
	skos:exactMatch medtop:20000281;
	skos:broader	subj:04006000.

subj:04006015
	rdf:type skos:Concept;
	skos:prefLabel	"funeral parlour and crematorium"@en-GB;
	skos:definition	"Companies that provide services for disposal of the dead "@en-GB;
	skos:inScheme <http://cv.iptc.org/newscodes/subjectcode/>;
	skos:exactMatch medtop:20000277;
	skos:broader	subj:04006000.

subj:04006016
	rdf:type skos:Concept;
	skos:prefLabel	"rental service"@en-GB;
	skos:definition	"Companies which provide rentals, including motor vehicles, tuxedos, tools, heavy equipment, and other supplies "@en-GB;
	skos:inScheme <http://cv.iptc.org/newscodes/subjectcode/>;
	skos:exactMatch medtop:20000290;
	skos:broader	subj:04006000.

subj:04006017
	rdf:type skos:Concept;
	skos:prefLabel	"wedding service"@en-GB;
	skos:definition	"Services and products related to the wedding industry "@en-GB;
	skos:inScheme <http://cv.iptc.org/newscodes/subjectcode/>;
	skos:exactMatch medtop:20000293;
	skos:broader	subj:04006000.

subj:04006018
	rdf:type skos:Concept;
	skos:prefLabel	"personal finance"@en-GB;
	skos:definition	"An individual's income and expenses "@en-GB;
	skos:inScheme <http://cv.iptc.org/newscodes/subjectcode/>;
	skos:exactMatch medtop:20000285;
	skos:broader	subj:04006000.

subj:04006019
	rdf:type skos:Concept;
	skos:prefLabel	"personal income"@en-GB;
	skos:definition	"Money that a person earns and is his/hers to keep or spend "@en-GB;
	skos:inScheme <http://cv.iptc.org/newscodes/subjectcode/>;
	skos:exactMatch medtop:20000286;
	skos:broader	subj:04006000.

subj:04006020
	rdf:type skos:Concept;
	skos:prefLabel	"auction service"@en-GB;
	skos:definition	"Sales by bidding "@en-GB;
	skos:inScheme <http://cv.iptc.org/newscodes/subjectcode/>;
	skos:exactMatch medtop:20000273;
	skos:broader	subj:04006000.

subj:04006021
	rdf:type skos:Concept;
	skos:prefLabel	"printing/promotional service"@en-GB;
	skos:definition	"Production of printed matter such as flyers, ads, signs etc "@en-GB;
	skos:inScheme <http://cv.iptc.org/newscodes/subjectcode/>;
	skos:exactMatch medtop:20000289;
	skos:broader	subj:04006000.

subj:04006022
	rdf:type skos:Concept;
	skos:prefLabel	"investment service"@en-GB;
	skos:definition	"Financial advisers, as opposed to stock dealers or consultants "@en-GB;
	skos:inScheme <http://cv.iptc.org/newscodes/subjectcode/>;
	skos:exactMatch medtop:20000280;
	skos:broader	subj:04006000.

subj:04007000
	rdf:type skos:Concept;
	skos:prefLabel	"consumer goods"@en-GB;
	skos:definition	"Items produced for and sold to individuals "@en-GB;
	skos:inScheme <http://cv.iptc.org/newscodes/subjectcode/>;
	skos:exactMatch medtop:20000243;
	skos:broader	subj:04000000;
	skos:narrower	subj:04007001;
	skos:narrower	subj:04007002;
	skos:narrower	subj:04007003;
	skos:narrower	subj:04007004;
	skos:narrower	subj:04007005;
	skos:narrower	subj:04007006;
	skos:narrower	subj:04007007;
	skos:narrower	subj:04007008;
	skos:narrower	subj:04007009;
	skos:narrower	subj:04007010;
	skos:narrower	subj:04007011;
	skos:narrower	subj:04007012.

subj:04007001
	rdf:type skos:Concept;
	skos:prefLabel	"clothing"@en-GB;
	skos:definition	"Items of apparel to wear "@en-GB;
	skos:inScheme <http://cv.iptc.org/newscodes/subjectcode/>;
	skos:exactMatch medtop:20000245;
	skos:broader	subj:04007000.

subj:04007002
	rdf:type skos:Concept;
	skos:prefLabel	"department store"@en-GB;
	skos:definition	"Stores largely devoted to the sale of clothing to individuals "@en-GB;
	skos:inScheme <http://cv.iptc.org/newscodes/subjectcode/>;
	skos:exactMatch medtop:20000246;
	skos:broader	subj:04007000.

subj:04007003
	rdf:type skos:Concept;
	skos:prefLabel	"food"@en-GB;
	skos:definition	"Fruits, vegetables, breads, meats for human consumption "@en-GB;
	skos:inScheme <http://cv.iptc.org/newscodes/subjectcode/>;
	skos:exactMatch medtop:20000248;
	skos:broader	subj:04007000.

subj:04007004
	rdf:type skos:Concept;
	skos:prefLabel	"mail order"@en-GB;
	skos:definition	"Items sold through and delivered by mail "@en-GB;
	skos:inScheme <http://cv.iptc.org/newscodes/subjectcode/>;
	skos:exactMatch medtop:20000250;
	skos:broader	subj:04007000.

subj:04007005
	rdf:type skos:Concept;
	skos:prefLabel	"retail"@en-GB;
	skos:definition	"The last stage in the sales chain "@en-GB;
	skos:inScheme <http://cv.iptc.org/newscodes/subjectcode/>;
	skos:exactMatch medtop:20000252;
	skos:broader	subj:04007000.

subj:04007006
	rdf:type skos:Concept;
	skos:prefLabel	"speciality store"@en-GB;
	skos:definition	"Retail outlets that specialize in categories such as shoes, coats, power tools, etc "@en-GB;
	skos:inScheme <http://cv.iptc.org/newscodes/subjectcode/>;
	skos:exactMatch medtop:20000253;
	skos:broader	subj:04007000.

subj:04007007
	rdf:type skos:Concept;
	skos:prefLabel	"wholesale"@en-GB;
	skos:definition	"The first link in the sales chain after production "@en-GB;
	skos:inScheme <http://cv.iptc.org/newscodes/subjectcode/>;
	skos:exactMatch medtop:20000255;
	skos:broader	subj:04007000.

subj:04007008
	rdf:type skos:Concept;
	skos:prefLabel	"beverage"@en-GB;
	skos:definition	"Liquid consumables, both alcoholic and non-alcoholic "@en-GB;
	skos:inScheme <http://cv.iptc.org/newscodes/subjectcode/>;
	skos:exactMatch medtop:20000244;
	skos:broader	subj:04007000.

subj:04007009
	rdf:type skos:Concept;
	skos:prefLabel	"electronic commerce"@en-GB;
	skos:definition	"Buying and selling items through the Internet "@en-GB;
	skos:inScheme <http://cv.iptc.org/newscodes/subjectcode/>;
	skos:exactMatch medtop:20000247;
	skos:broader	subj:04007000.

subj:04007010
	rdf:type skos:Concept;
	skos:prefLabel	"luxury good"@en-GB;
	skos:definition	"Leather bags, jewellery, haute couture, accessories etc "@en-GB;
	skos:inScheme <http://cv.iptc.org/newscodes/subjectcode/>;
	skos:exactMatch medtop:20000249;
	skos:broader	subj:04007000.

subj:04007011
	rdf:type skos:Concept;
	skos:prefLabel	"non-durable good"@en-GB;
	skos:definition	"Lighters, pens and stationery, tableware, watches, glasses etc "@en-GB;
	skos:inScheme <http://cv.iptc.org/newscodes/subjectcode/>;
	skos:exactMatch medtop:20000251;
	skos:broader	subj:04007000.

subj:04007012
	rdf:type skos:Concept;
	skos:prefLabel	"toy"@en-GB;
	skos:definition	"Children's plaything "@en-GB;
	skos:inScheme <http://cv.iptc.org/newscodes/subjectcode/>;
	skos:exactMatch medtop:20000254;
	skos:broader	subj:04007000.

subj:04008000
	rdf:type skos:Concept;
	skos:prefLabel	"macro economics"@en-GB;
	skos:definition	"Broad scale economics and the world or national level "@en-GB;
	skos:inScheme <http://cv.iptc.org/newscodes/subjectcode/>;
	skos:exactMatch medtop:20000346;
	skos:broader	subj:04000000;
	skos:narrower	subj:04008001;
	skos:narrower	subj:04008002;
	skos:narrower	subj:04008003;
	skos:narrower	subj:04008004;
	skos:narrower	subj:04008005;
	skos:narrower	subj:04008006;
	skos:narrower	subj:04008007;
	skos:narrower	subj:04008008;
	skos:narrower	subj:04008009;
	skos:narrower	subj:04008010;
	skos:narrower	subj:04008011;
	skos:narrower	subj:04008012;
	skos:narrower	subj:04008013;
	skos:narrower	subj:04008014;
	skos:narrower	subj:04008015;
	skos:narrower	subj:04008016;
	skos:narrower	subj:04008017;
	skos:narrower	subj:04008018;
	skos:narrower	subj:04008019;
	skos:narrower	subj:04008020;
	skos:narrower	subj:04008021;
	skos:narrower	subj:04008022;
	skos:narrower	subj:04008023;
	skos:narrower	subj:04008024;
	skos:narrower	subj:04008025;
	skos:narrower	subj:04008026;
	skos:narrower	subj:04008027;
	skos:narrower	subj:04008028;
	skos:narrower	subj:04008029;
	skos:narrower	subj:04008030;
	skos:narrower	subj:04008031;
	skos:narrower	subj:04008032;
	skos:narrower	subj:04008033;
	skos:narrower	subj:04008034;
	skos:narrower	subj:04008035;
	skos:narrower	subj:04008036.

subj:04008001
	rdf:type skos:Concept;
	skos:prefLabel	"central bank"@en-GB;
	skos:definition	"A country's major bank that sets interest rates, and provides transfer of funds between commercial banks "@en-GB;
	skos:inScheme <http://cv.iptc.org/newscodes/subjectcode/>;
	skos:exactMatch medtop:20000350;
	skos:broader	subj:04008000.

subj:04008002
	rdf:type skos:Concept;
	skos:prefLabel	"consumer issue"@en-GB;
	skos:definition	"Those issues, such as prices, inflation/deflation, quality of goods, at the retail sales level "@en-GB;
	skos:inScheme <http://cv.iptc.org/newscodes/subjectcode/>;
	skos:exactMatch medtop:20000353;
	skos:broader	subj:04008000.

subj:04008003
	rdf:type skos:Concept;
	skos:prefLabel	"debt market"@en-GB;
	skos:definition	"Market for trading debt instruments such as bonds, CDs, bankers acceptances, T bills, notes, IOUs etc "@en-GB;
	skos:inScheme <http://cv.iptc.org/newscodes/subjectcode/>;
	skos:exactMatch medtop:20000390;
	skos:broader	subj:04008000.

subj:04008004
	rdf:type skos:Concept;
	skos:prefLabel	"economic indicator"@en-GB;
	skos:definition	"Certain indexes, such as company inventories, the movement of prices that show whether the economy is improving or declining "@en-GB;
	skos:inScheme <http://cv.iptc.org/newscodes/subjectcode/>;
	skos:exactMatch medtop:20000358;
	skos:broader	subj:04008000.

subj:04008005
	rdf:type skos:Concept;
	skos:prefLabel	"emerging market"@en-GB;
	skos:definition	"Those markets that are struggling to enter the world economies and those requiring financial help from international lenders "@en-GB;
	skos:inScheme <http://cv.iptc.org/newscodes/subjectcode/>;
	skos:exactMatch medtop:20000364;
	skos:broader	subj:04008000.

subj:04008006
	rdf:type skos:Concept;
	skos:prefLabel	"foreign exchange market"@en-GB;
	skos:definition	"The trading of shekels, dinars, euros dollars etc around the world through regulated markets "@en-GB;
	skos:inScheme <http://cv.iptc.org/newscodes/subjectcode/>;
	skos:exactMatch medtop:20000391;
	skos:broader	subj:04008000.

subj:04008007
	rdf:type skos:Concept;
	skos:prefLabel	"government aid"@en-GB;
	skos:definition	"Supply of financial and other help by one government, usually to another "@en-GB;
	skos:inScheme <http://cv.iptc.org/newscodes/subjectcode/>;
	skos:exactMatch medtop:20000367;
	skos:broader	subj:04008000.

subj:04008008
	rdf:type skos:Concept;
	skos:prefLabel	"government debt"@en-GB;
	skos:definition	"The amount a government owes on bonds, services and for goods and services for which it has no ready cash "@en-GB;
	skos:inScheme <http://cv.iptc.org/newscodes/subjectcode/>;
	skos:exactMatch medtop:20000368;
	skos:broader	subj:04008000.

subj:04008009
	rdf:type skos:Concept;
	skos:prefLabel	"interest rate"@en-GB;
	skos:definition	"The amount of money one must pay to borrow money "@en-GB;
	skos:inScheme <http://cv.iptc.org/newscodes/subjectcode/>;
	skos:exactMatch medtop:20000371;
	skos:broader	subj:04008000.

subj:04008010
	rdf:type skos:Concept;
	skos:prefLabel	"international economic institution"@en-GB;
	skos:definition	"Entities such as UNIDO, World Bank, World Trade Organization, the Import-Expert Bank etc that deals at a world level "@en-GB;
	skos:inScheme <http://cv.iptc.org/newscodes/subjectcode/>;
	skos:exactMatch medtop:20000372;
	skos:broader	subj:04008000.

subj:04008011
	rdf:type skos:Concept;
	skos:prefLabel	"international (foreign) trade"@en-GB;
	skos:definition	"Trade of goods and services between nations "@en-GB;
	skos:inScheme <http://cv.iptc.org/newscodes/subjectcode/>;
	skos:exactMatch medtop:20000373;
	skos:broader	subj:04008000.

subj:04008012
	rdf:type skos:Concept;
	skos:prefLabel	"loan market"@en-GB;
	skos:definition	"The market where money is available to borrow, at certain rates of interest "@en-GB;
	skos:inScheme <http://cv.iptc.org/newscodes/subjectcode/>;
	skos:exactMatch medtop:20000392;
	skos:broader	subj:04008000.

subj:04008013
	rdf:type skos:Concept;
	skos:prefLabel	"economic organization"@en-GB;
	skos:definition	"Business, industrial and trade associations, societies and other private-sector groups. "@en-GB;
	skos:inScheme <http://cv.iptc.org/newscodes/subjectcode/>;
	skos:exactMatch medtop:20000363;
	skos:broader	subj:04008000.

subj:04008014
	rdf:type skos:Concept;
	skos:prefLabel	"consumer confidence"@en-GB;
	skos:definition	"Reports on consumer confidence in the economy. "@en-GB;
	skos:inScheme <http://cv.iptc.org/newscodes/subjectcode/>;
	skos:exactMatch medtop:20000352;
	skos:broader	subj:04008000.

subj:04008015
	rdf:type skos:Concept;
	skos:prefLabel	"trade dispute"@en-GB;
	skos:definition	"International dispute over trade barriers, cartels, dumping etc. "@en-GB;
	skos:inScheme <http://cv.iptc.org/newscodes/subjectcode/>;
	skos:exactMatch medtop:20000376;
	skos:broader	subj:04008000.

subj:04008016
	rdf:type skos:Concept;
	skos:prefLabel	"inflation and deflation"@en-GB;
	skos:definition	"An increase in the amount of money in circulation and thereby a rise in prices; deflation, tighter monetary policy causing lower prices "@en-GB;
	skos:inScheme <http://cv.iptc.org/newscodes/subjectcode/>;
	skos:broader	subj:04008000.

subj:04008017
	rdf:type skos:Concept;
	skos:prefLabel	"prices"@en-GB;
	skos:definition	"The monetary value of goods, services or stocks and bonds "@en-GB;
	skos:inScheme <http://cv.iptc.org/newscodes/subjectcode/>;
	skos:exactMatch medtop:20000382;
	skos:broader	subj:04008000.

subj:04008018
	rdf:type skos:Concept;
	skos:prefLabel	"currency values"@en-GB;
	skos:definition	"The value of one currency as measured against another "@en-GB;
	skos:inScheme <http://cv.iptc.org/newscodes/subjectcode/>;
	skos:exactMatch medtop:20000355;
	skos:broader	subj:04008000.

subj:04008019
	rdf:type skos:Concept;
	skos:prefLabel	"budgets and budgeting"@en-GB;
	skos:definition	"A method of balancing revenues against expenses "@en-GB;
	skos:inScheme <http://cv.iptc.org/newscodes/subjectcode/>;
	skos:exactMatch medtop:20000348;
	skos:broader	subj:04008000.

subj:04008020
	rdf:type skos:Concept;
	skos:prefLabel	"credit and debt"@en-GB;
	skos:definition	"Credit: the amount of money available to you, often by loan. Debt, the amount you owe. "@en-GB;
	skos:inScheme <http://cv.iptc.org/newscodes/subjectcode/>;
	skos:exactMatch medtop:20000354;
	skos:broader	subj:04008000.

subj:04008021
	rdf:type skos:Concept;
	skos:prefLabel	"loans"@en-GB;
	skos:definition	"An agreement by one individual or institution to temporarily disperse money to another, with an agreed rate and time for its return "@en-GB;
	skos:inScheme <http://cv.iptc.org/newscodes/subjectcode/>;
	skos:exactMatch medtop:20000393;
	skos:broader	subj:04008000.

subj:04008022
	rdf:type skos:Concept;
	skos:prefLabel	"mortgages"@en-GB;
	skos:definition	"The loan of money for the purpose of purchasing a property, whether land or building. Or, for homeowners to repair or maintain properties, often based on owner equity in a property "@en-GB;
	skos:inScheme <http://cv.iptc.org/newscodes/subjectcode/>;
	skos:exactMatch medtop:20000380;
	skos:broader	subj:04008000.

subj:04008023
	rdf:type skos:Concept;
	skos:prefLabel	"financial markets"@en-GB;
	skos:definition	"Institutions set up to trade the shares or other financial paper of companies or other organizations, can also include currency trading "@en-GB;
	skos:inScheme <http://cv.iptc.org/newscodes/subjectcode/>;
	skos:closeMatch medtop:20000385;
	skos:broader	subj:04008000.

subj:04008024
	rdf:type skos:Concept;
	skos:prefLabel	"commodity markets"@en-GB;
	skos:definition	"The bartering or trading of goods such as cotton, oil, coal, metals, etc "@en-GB;
	skos:inScheme <http://cv.iptc.org/newscodes/subjectcode/>;
	skos:exactMatch medtop:20000386;
	skos:broader	subj:04008000.

subj:04008025
	rdf:type skos:Concept;
	skos:prefLabel	"investments"@en-GB;
	skos:definition	"Speculative purchases of corporate instruments, of commodities, currencies, or parts thereof "@en-GB;
	skos:inScheme <http://cv.iptc.org/newscodes/subjectcode/>;
	skos:exactMatch medtop:20000378;
	skos:broader	subj:04008000.

subj:04008026
	rdf:type skos:Concept;
	skos:prefLabel	"stocks"@en-GB;
	skos:definition	"Corporate paper that gives an individual an ownership right to a part of a company's earnings "@en-GB;
	skos:inScheme <http://cv.iptc.org/newscodes/subjectcode/>;
	skos:exactMatch medtop:20000396;
	skos:broader	subj:04008000.

subj:04008027
	rdf:type skos:Concept;
	skos:prefLabel	"bonds"@en-GB;
	skos:definition	"Corporate or governmental paper representing the loan of money at a fixed rate and for a fixed time to that company or government "@en-GB;
	skos:inScheme <http://cv.iptc.org/newscodes/subjectcode/>;
	skos:exactMatch medtop:20000347;
	skos:broader	subj:04008000.

subj:04008028
	rdf:type skos:Concept;
	skos:prefLabel	"mutual funds"@en-GB;
	skos:definition	"Pools of shares or bonds for sale often grouped by investment intention, such as growth, income or security "@en-GB;
	skos:inScheme <http://cv.iptc.org/newscodes/subjectcode/>;
	skos:exactMatch medtop:20000381;
	skos:broader	subj:04008000.

subj:04008029
	rdf:type skos:Concept;
	skos:prefLabel	"derivative securities"@en-GB;
	skos:definition	"Financial instruments such as futures, swaps and options, used for risk management, whose characteristics and value depend upon the characteristics and value of an underlying instrument, such as a commodity, bond, equity or currency. "@en-GB;
	skos:inScheme <http://cv.iptc.org/newscodes/subjectcode/>;
	skos:exactMatch medtop:20000395;
	skos:broader	subj:04008000.

subj:04008030
	rdf:type skos:Concept;
	skos:prefLabel	"imports"@en-GB;
	skos:definition	"What is bought abroad and brought into a country for resale "@en-GB;
	skos:inScheme <http://cv.iptc.org/newscodes/subjectcode/>;
	skos:exactMatch medtop:20000369;
	skos:broader	subj:04008000.

subj:04008031
	rdf:type skos:Concept;
	skos:prefLabel	"exports"@en-GB;
	skos:definition	"What is produced or manufactured in your country and sent and sold elsewhere "@en-GB;
	skos:inScheme <http://cv.iptc.org/newscodes/subjectcode/>;
	skos:exactMatch medtop:20000366;
	skos:broader	subj:04008000.

subj:04008032
	rdf:type skos:Concept;
	skos:prefLabel	"trade agreements"@en-GB;
	skos:definition	"Government level agreements between countries for the sale and purchase of goods and services "@en-GB;
	skos:inScheme <http://cv.iptc.org/newscodes/subjectcode/>;
	skos:exactMatch medtop:20000374;
	skos:broader	subj:04008000.

subj:04008033
	rdf:type skos:Concept;
	skos:prefLabel	"trade policy"@en-GB;
	skos:definition	"Governmental decisions on tariffs, shipping, embargoes, and the types or kinds of goods and services to be imported and exported "@en-GB;
	skos:inScheme <http://cv.iptc.org/newscodes/subjectcode/>;
	skos:exactMatch medtop:20000377;
	skos:broader	subj:04008000.

subj:04008034
	rdf:type skos:Concept;
	skos:prefLabel	"business enterprises"@en-GB;
	skos:definition	"Organizations set up usually for profit-making purposes by creating and selling a product or service "@en-GB;
	skos:inScheme <http://cv.iptc.org/newscodes/subjectcode/>;
	skos:exactMatch medtop:20000349;
	skos:broader	subj:04008000.

subj:04008035
	rdf:type skos:Concept;
	skos:prefLabel	"tariff"@en-GB;
	skos:definition	"Fees placed on goods imported or exported, often punitive "@en-GB;
	skos:inScheme <http://cv.iptc.org/newscodes/subjectcode/>;
	skos:exactMatch medtop:20000384;
	skos:broader	subj:04008000.

subj:04008036
	rdf:type skos:Concept;
	skos:prefLabel	"trade balance"@en-GB;
	skos:definition	"The difference between the financial value of imports and exports "@en-GB;
	skos:inScheme <http://cv.iptc.org/newscodes/subjectcode/>;
	skos:exactMatch medtop:20000375;
	skos:broader	subj:04008000.

subj:04009000
	rdf:type skos:Concept;
	skos:prefLabel	"market and exchange"@en-GB;
	skos:definition	"Organized entities for buying and selling stocks, currencies, commodities and other goods "@en-GB;
	skos:inScheme <http://cv.iptc.org/newscodes/subjectcode/>;
	skos:exactMatch medtop:20000385;
	skos:broader	subj:04000000;
	skos:narrower	subj:04009001;
	skos:narrower	subj:04009002;
	skos:narrower	subj:04009003;
	skos:narrower	subj:04009004.

subj:04009001
	rdf:type skos:Concept;
	skos:prefLabel	"energy"@en-GB;
	skos:definition	"Stories related to energy trading and markets "@en-GB;
	skos:inScheme <http://cv.iptc.org/newscodes/subjectcode/>;
	skos:exactMatch medtop:20000387;
	skos:broader	subj:04009000.

subj:04009002
	rdf:type skos:Concept;
	skos:prefLabel	"metal"@en-GB;
	skos:definition	"Markets for trading base metals such as copper, aluminium, steel, zinc etc "@en-GB;
	skos:inScheme <http://cv.iptc.org/newscodes/subjectcode/>;
	skos:exactMatch medtop:20000388;
	skos:broader	subj:04009000.

subj:04009003
	rdf:type skos:Concept;
	skos:prefLabel	"securities"@en-GB;
	skos:definition	"Markets for trading types of company paper such as stocks and bonds "@en-GB;
	skos:inScheme <http://cv.iptc.org/newscodes/subjectcode/>;
	skos:exactMatch medtop:20000394;
	skos:broader	subj:04009000.

subj:04009004
	rdf:type skos:Concept;
	skos:prefLabel	"soft commodity"@en-GB;
	skos:definition	"Trading in commodities such as cotton, sugar, sorghum, soybeans etc. "@en-GB;
	skos:inScheme <http://cv.iptc.org/newscodes/subjectcode/>;
	skos:exactMatch medtop:20000389;
	skos:broader	subj:04009000.

subj:04010000
	rdf:type skos:Concept;
	skos:prefLabel	"media"@en-GB;
	skos:definition	"The various means of disseminating news and information to the public "@en-GB;
	skos:inScheme <http://cv.iptc.org/newscodes/subjectcode/>;
	skos:exactMatch medtop:20000304;
	skos:broader	subj:04000000;
	skos:narrower	subj:04010001;
	skos:narrower	subj:04010002;
	skos:narrower	subj:04010003;
	skos:narrower	subj:04010004;
	skos:narrower	subj:04010005;
	skos:narrower	subj:04010006;
	skos:narrower	subj:04010007;
	skos:narrower	subj:04010008;
	skos:narrower	subj:04010009;
	skos:narrower	subj:04010010;
	skos:narrower	subj:04010011.

subj:04010001
	rdf:type skos:Concept;
	skos:prefLabel	"advertising"@en-GB;
	skos:definition	"Methods of promoting goods and service to consumers through video, graphics, print text etc "@en-GB;
	skos:inScheme <http://cv.iptc.org/newscodes/subjectcode/>;
	skos:exactMatch medtop:20000305;
	skos:broader	subj:04010000.

subj:04010002
	rdf:type skos:Concept;
	skos:prefLabel	"book"@en-GB;
	skos:definition	"The business of producing and selling bound media, whether fiction or non-fiction "@en-GB;
	skos:inScheme <http://cv.iptc.org/newscodes/subjectcode/>;
	skos:exactMatch medtop:20000306;
	skos:broader	subj:04010000.

subj:04010003
	rdf:type skos:Concept;
	skos:prefLabel	"cinema industry"@en-GB;
	skos:definition	"The business of cinema "@en-GB;
	skos:inScheme <http://cv.iptc.org/newscodes/subjectcode/>;
	skos:exactMatch medtop:20000307;
	skos:broader	subj:04010000.

subj:04010004
	rdf:type skos:Concept;
	skos:prefLabel	"news agency"@en-GB;
	skos:definition	"Commercial agencies for production and distribution of newsworthy events through print, broadcast, video or electronic media "@en-GB;
	skos:inScheme <http://cv.iptc.org/newscodes/subjectcode/>;
	skos:exactMatch medtop:20000309;
	skos:broader	subj:04010000.

subj:04010005
	rdf:type skos:Concept;
	skos:prefLabel	"newspaper and magazine"@en-GB;
	skos:definition	"The business of producing bound and unbound printed paper products for periodic distribution of news items "@en-GB;
	skos:inScheme <http://cv.iptc.org/newscodes/subjectcode/>;
	skos:exactMatch medtop:20000310;
	skos:broader	subj:04010000.

subj:04010006
	rdf:type skos:Concept;
	skos:prefLabel	"online"@en-GB;
	skos:definition	"The business of distributing news and information through computer networks for public consumption "@en-GB;
	skos:inScheme <http://cv.iptc.org/newscodes/subjectcode/>;
	skos:exactMatch medtop:20000311;
	skos:broader	subj:04010000.

subj:04010007
	rdf:type skos:Concept;
	skos:prefLabel	"public relation"@en-GB;
	skos:definition	"The job of promoting products and services through advertising campaigns and/or through person-to-person contact or through news releases "@en-GB;
	skos:inScheme <http://cv.iptc.org/newscodes/subjectcode/>;
	skos:exactMatch medtop:20000312;
	skos:broader	subj:04010000.

subj:04010008
	rdf:type skos:Concept;
	skos:prefLabel	"radio industry"@en-GB;
	skos:definition	"Business of radio "@en-GB;
	skos:inScheme <http://cv.iptc.org/newscodes/subjectcode/>;
	skos:exactMatch medtop:20000313;
	skos:broader	subj:04010000.

subj:04010009
	rdf:type skos:Concept;
	skos:prefLabel	"satellite and cable service"@en-GB;
	skos:definition	"The business of transmitting of news, entertainment and information via satellite or cable television services "@en-GB;
	skos:inScheme <http://cv.iptc.org/newscodes/subjectcode/>;
	skos:exactMatch medtop:20000314;
	skos:broader	subj:04010000.

subj:04010010
	rdf:type skos:Concept;
	skos:prefLabel	"television industry"@en-GB;
	skos:definition	"Business of television "@en-GB;
	skos:inScheme <http://cv.iptc.org/newscodes/subjectcode/>;
	skos:exactMatch medtop:20000315;
	skos:broader	subj:04010000.

subj:04010011
	rdf:type skos:Concept;
	skos:prefLabel	"music industry"@en-GB;
	skos:definition	"Recording, production, marketing of music "@en-GB;
	skos:inScheme <http://cv.iptc.org/newscodes/subjectcode/>;
	skos:exactMatch medtop:20000308;
	skos:broader	subj:04010000.

subj:04011000
	rdf:type skos:Concept;
	skos:prefLabel	"manufacturing and engineering"@en-GB;
	skos:definition	"Manufacturers of electrical, electronic and mechanical equipment but does not cover civil engineering. "@en-GB;
	skos:historyNote	"Name changed, Explanation added in V 15 "@en-GB;
	skos:inScheme <http://cv.iptc.org/newscodes/subjectcode/>;
	skos:exactMatch medtop:20000294;
	skos:broader	subj:04000000;
	skos:narrower	subj:04011001;
	skos:narrower	subj:04011002;
	skos:narrower	subj:04011003;
	skos:narrower	subj:04011004;
	skos:narrower	subj:04011005;
	skos:narrower	subj:04011006;
	skos:narrower	subj:04011007;
	skos:narrower	subj:04011008;
	skos:narrower	subj:04011009.

subj:04011001
	rdf:type skos:Concept;
	skos:prefLabel	"aerospace"@en-GB;
	skos:definition	"Companies that assemble or manufacture components for airplanes and space ships. "@en-GB;
	skos:historyNote	"Explanation added in V 15 "@en-GB;
	skos:inScheme <http://cv.iptc.org/newscodes/subjectcode/>;
	skos:exactMatch medtop:20000295;
	skos:broader	subj:04011000.

subj:04011002
	rdf:type skos:Concept;
	skos:prefLabel	"automotive equipment"@en-GB;
	skos:definition	"Companies that produce components for automobiles "@en-GB;
	skos:historyNote	"Explanation added in V 15 "@en-GB;
	skos:inScheme <http://cv.iptc.org/newscodes/subjectcode/>;
	skos:exactMatch medtop:20000296;
	skos:broader	subj:04011000.

subj:04011003
	rdf:type skos:Concept;
	skos:prefLabel	"defence equipment"@en-GB;
	skos:definition	"Manufacturers of guns, tanks, cannons, ships etc for the military and non-military protection services "@en-GB;
	skos:historyNote	"Explanation added in V 15 "@en-GB;
	skos:inScheme <http://cv.iptc.org/newscodes/subjectcode/>;
	skos:exactMatch medtop:20000297;
	skos:broader	subj:04011000.

subj:04011004
	rdf:type skos:Concept;
	skos:prefLabel	"electrical appliance"@en-GB;
	skos:definition	"Makers of large and small electrical goods for use in homes or business "@en-GB;
	skos:historyNote	"Explanation added in V 15 "@en-GB;
	skos:inScheme <http://cv.iptc.org/newscodes/subjectcode/>;
	skos:exactMatch medtop:20000298;
	skos:broader	subj:04011000.

subj:04011005
	rdf:type skos:Concept;
	skos:prefLabel	"heavy engineering"@en-GB;
	skos:definition	"Manufacturers of cranes, bulldozers and the like for use in major construction projects "@en-GB;
	skos:historyNote	"Explanation added in V 15 "@en-GB;
	skos:inScheme <http://cv.iptc.org/newscodes/subjectcode/>;
	skos:exactMatch medtop:20000299;
	skos:broader	subj:04011000.

subj:04011006
	rdf:type skos:Concept;
	skos:prefLabel	"industrial component"@en-GB;
	skos:definition	"Manufacturers of mechanical, electrical, electronic items needed in the manufacture of other items "@en-GB;
	skos:historyNote	"Explanation added in V 15 "@en-GB;
	skos:inScheme <http://cv.iptc.org/newscodes/subjectcode/>;
	skos:exactMatch medtop:20000300;
	skos:broader	subj:04011000.

subj:04011007
	rdf:type skos:Concept;
	skos:prefLabel	"instrument engineering"@en-GB;
	skos:definition	"Manufacturers of instruments for calibration, measurement of things like speed, pressure, distance "@en-GB;
	skos:historyNote	"Explanation added in V 15 "@en-GB;
	skos:inScheme <http://cv.iptc.org/newscodes/subjectcode/>;
	skos:exactMatch medtop:20000301;
	skos:broader	subj:04011000.

subj:04011008
	rdf:type skos:Concept;
	skos:prefLabel	"shipbuilding"@en-GB;
	skos:definition	"Manufacturers of ships, submarines, barges. "@en-GB;
	skos:historyNote	"Explanation added in V 15 "@en-GB;
	skos:inScheme <http://cv.iptc.org/newscodes/subjectcode/>;
	skos:exactMatch medtop:20000303;
	skos:broader	subj:04011000.

subj:04011009
	rdf:type skos:Concept;
	skos:prefLabel	"machine manufacturing"@en-GB;
	skos:definition	"Manufacturers of turbines, engines, fans , pumps , motors and components for powered equipment. "@en-GB;
	skos:historyNote	"Explanation added in V 15 "@en-GB;
	skos:inScheme <http://cv.iptc.org/newscodes/subjectcode/>;
	skos:exactMatch medtop:20000302;
	skos:broader	subj:04011000.

subj:04012000
	rdf:type skos:Concept;
	skos:prefLabel	"metal and mineral"@en-GB;
	skos:definition	"Production and refining of ores into metals "@en-GB;
	skos:inScheme <http://cv.iptc.org/newscodes/subjectcode/>;
	skos:exactMatch medtop:20000316;
	skos:broader	subj:04000000;
	skos:narrower	subj:04012001;
	skos:narrower	subj:04012002;
	skos:narrower	subj:04012003;
	skos:narrower	subj:04012004;
	skos:narrower	subj:04012005.

subj:04012001
	rdf:type skos:Concept;
	skos:prefLabel	"building material"@en-GB;
	skos:definition	"Manufacture of materials like wallboard, lumber wiring for the building industry "@en-GB;
	skos:inScheme <http://cv.iptc.org/newscodes/subjectcode/>;
	skos:exactMatch medtop:20000317;
	skos:broader	subj:04012000.

subj:04012002
	rdf:type skos:Concept;
	skos:prefLabel	"gold and precious material"@en-GB;
	skos:definition	"Mining, refining and sales of gold and other precious metals "@en-GB;
	skos:inScheme <http://cv.iptc.org/newscodes/subjectcode/>;
	skos:exactMatch medtop:20000318;
	skos:broader	subj:04012000.

subj:04012003
	rdf:type skos:Concept;
	skos:prefLabel	"iron and steel"@en-GB;
	skos:definition	"Mining, refining and sales of iron-based metals "@en-GB;
	skos:inScheme <http://cv.iptc.org/newscodes/subjectcode/>;
	skos:exactMatch medtop:20000319;
	skos:broader	subj:04012000.

subj:04012004
	rdf:type skos:Concept;
	skos:prefLabel	"non ferrous metal"@en-GB;
	skos:definition	"Mining, refining and sales of copper, zinc, aluminium, and other metals not based on iron "@en-GB;
	skos:inScheme <http://cv.iptc.org/newscodes/subjectcode/>;
	skos:exactMatch medtop:20000321;
	skos:broader	subj:04012000.

subj:04012005
	rdf:type skos:Concept;
	skos:prefLabel	"mining"@en-GB;
	skos:definition	"The industry of digging for metals, raw materials such as coal, or precious gems such as diamonds "@en-GB;
	skos:inScheme <http://cv.iptc.org/newscodes/subjectcode/>;
	skos:exactMatch medtop:20000320;
	skos:broader	subj:04012000.

subj:04013000
	rdf:type skos:Concept;
	skos:prefLabel	"process industry"@en-GB;
	skos:definition	"The business of turning raw materials into useable products "@en-GB;
	skos:inScheme <http://cv.iptc.org/newscodes/subjectcode/>;
	skos:exactMatch medtop:20000322;
	skos:broader	subj:04000000;
	skos:narrower	subj:04013001;
	skos:narrower	subj:04013002;
	skos:narrower	subj:04013003;
	skos:narrower	subj:04013004;
	skos:narrower	subj:04013005;
	skos:narrower	subj:04013006;
	skos:narrower	subj:04013007;
	skos:narrower	subj:04013008.

subj:04013001
	rdf:type skos:Concept;
	skos:prefLabel	"distiller and brewer"@en-GB;
	skos:definition	"Manufacture of alcoholic beverages "@en-GB;
	skos:inScheme <http://cv.iptc.org/newscodes/subjectcode/>;
	skos:exactMatch medtop:20000323;
	skos:broader	subj:04013000.

subj:04013002
	rdf:type skos:Concept;
	skos:prefLabel	"food"@en-GB;
	skos:definition	"The business of processing, distributing and selling for basic human consumption "@en-GB;
	skos:inScheme <http://cv.iptc.org/newscodes/subjectcode/>;
	skos:exactMatch medtop:20000324;
	skos:broader	subj:04013000.

subj:04013003
	rdf:type skos:Concept;
	skos:prefLabel	"furnishings and furniture"@en-GB;
	skos:definition	"Manufacture of furniture, wallpaper, paints and fabrics for interior decoration "@en-GB;
	skos:inScheme <http://cv.iptc.org/newscodes/subjectcode/>;
	skos:exactMatch medtop:20000325;
	skos:broader	subj:04013000.

subj:04013004
	rdf:type skos:Concept;
	skos:prefLabel	"paper and packaging product"@en-GB;
	skos:definition	"Production of paper material for writing, wrapping, printing, or packaging "@en-GB;
	skos:inScheme <http://cv.iptc.org/newscodes/subjectcode/>;
	skos:exactMatch medtop:20000326;
	skos:broader	subj:04013000.

subj:04013005
	rdf:type skos:Concept;
	skos:prefLabel	"rubber product"@en-GB;
	skos:definition	"Production of rubber based materials for gloves, protective coatings, hoses and the like "@en-GB;
	skos:inScheme <http://cv.iptc.org/newscodes/subjectcode/>;
	skos:exactMatch medtop:20000327;
	skos:broader	subj:04013000.

subj:04013006
	rdf:type skos:Concept;
	skos:prefLabel	"soft drinks"@en-GB;
	skos:definition	"Production of non-alcoholic drinks "@en-GB;
	skos:inScheme <http://cv.iptc.org/newscodes/subjectcode/>;
	skos:exactMatch medtop:20000328;
	skos:broader	subj:04013000.

subj:04013007
	rdf:type skos:Concept;
	skos:prefLabel	"textile and clothing"@en-GB;
	skos:definition	"Production of fabrics for furnishings and fixtures, and for clothing of various types "@en-GB;
	skos:inScheme <http://cv.iptc.org/newscodes/subjectcode/>;
	skos:exactMatch medtop:20000329;
	skos:broader	subj:04013000.

subj:04013008
	rdf:type skos:Concept;
	skos:prefLabel	"tobacco"@en-GB;
	skos:definition	"Growing, producing and sale of tobacco products "@en-GB;
	skos:inScheme <http://cv.iptc.org/newscodes/subjectcode/>;
	skos:exactMatch medtop:20000330;
	skos:broader	subj:04013000.

subj:04014000
	rdf:type skos:Concept;
	skos:prefLabel	"tourism and leisure"@en-GB;
	skos:definition	"Tourism and leisure industries "@en-GB;
	skos:inScheme <http://cv.iptc.org/newscodes/subjectcode/>;
	skos:exactMatch medtop:20000332;
	skos:broader	subj:04000000;
	skos:narrower	subj:04014001;
	skos:narrower	subj:04014002;
	skos:narrower	subj:04014003;
	skos:narrower	subj:04014004;
	skos:narrower	subj:04014005.

subj:04014001
	rdf:type skos:Concept;
	skos:prefLabel	"casino and gambling"@en-GB;
	skos:definition	"The business of providing outlets for various games of chance using cards, dice, spinning wheels to betting on animal races "@en-GB;
	skos:inScheme <http://cv.iptc.org/newscodes/subjectcode/>;
	skos:exactMatch medtop:20000332;
	skos:broader	subj:04014000.

subj:04014002
	rdf:type skos:Concept;
	skos:prefLabel	"hotel and accommodation"@en-GB;
	skos:definition	"The business of providing food and shelter to travellers "@en-GB;
	skos:inScheme <http://cv.iptc.org/newscodes/subjectcode/>;
	skos:exactMatch medtop:20000333;
	skos:broader	subj:04014000.

subj:04014003
	rdf:type skos:Concept;
	skos:prefLabel	"recreational and sporting goods"@en-GB;
	skos:definition	"Manufacture of goods for leisure activities "@en-GB;
	skos:inScheme <http://cv.iptc.org/newscodes/subjectcode/>;
	skos:exactMatch medtop:20000334;
	skos:broader	subj:04014000.

subj:04014004
	rdf:type skos:Concept;
	skos:prefLabel	"restaurant and catering"@en-GB;
	skos:definition	"The business of providing prepared foods for customers in groups large and small "@en-GB;
	skos:inScheme <http://cv.iptc.org/newscodes/subjectcode/>;
	skos:exactMatch medtop:20000335;
	skos:broader	subj:04014000.

subj:04014005
	rdf:type skos:Concept;
	skos:prefLabel	"tour operator"@en-GB;
	skos:definition	"Operators of trips either locally, as around town, or to other countries "@en-GB;
	skos:inScheme <http://cv.iptc.org/newscodes/subjectcode/>;
	skos:exactMatch medtop:20000336;
	skos:broader	subj:04014000.

subj:04015000
	rdf:type skos:Concept;
	skos:prefLabel	"transport"@en-GB;
	skos:definition	"The means of getting from one place to the other without walking "@en-GB;
	skos:inScheme <http://cv.iptc.org/newscodes/subjectcode/>;
	skos:exactMatch medtop:20000337;
	skos:broader	subj:04000000;
	skos:narrower	subj:04015001;
	skos:narrower	subj:04015002;
	skos:narrower	subj:04015003;
	skos:narrower	subj:04015004.

subj:04015001
	rdf:type skos:Concept;
	skos:prefLabel	"air transport"@en-GB;
	skos:definition	"Airplane and airport operations "@en-GB;
	skos:inScheme <http://cv.iptc.org/newscodes/subjectcode/>;
	skos:exactMatch medtop:20000338;
	skos:broader	subj:04015000.

subj:04015002
	rdf:type skos:Concept;
	skos:prefLabel	"railway"@en-GB;
	skos:definition	"The business of transporting people or cargo by rail "@en-GB;
	skos:inScheme <http://cv.iptc.org/newscodes/subjectcode/>;
	skos:exactMatch medtop:20000340;
	skos:broader	subj:04015000.

subj:04015003
	rdf:type skos:Concept;
	skos:prefLabel	"road transport"@en-GB;
	skos:definition	"The business of transport goods by trucks and highways "@en-GB;
	skos:inScheme <http://cv.iptc.org/newscodes/subjectcode/>;
	skos:exactMatch medtop:20000341;
	skos:broader	subj:04015000.

subj:04015004
	rdf:type skos:Concept;
	skos:prefLabel	"waterway and maritime transport"@en-GB;
	skos:definition	"Commercial movement of people or goods via boats, ships and water "@en-GB;
	skos:inScheme <http://cv.iptc.org/newscodes/subjectcode/>;
	skos:exactMatch medtop:20000343;
	skos:broader	subj:04015000.

subj:04016000
	rdf:type skos:Concept;
	skos:prefLabel	"company information"@en-GB;
	skos:definition	"Information about individual companies or business entities "@en-GB;
	skos:inScheme <http://cv.iptc.org/newscodes/subjectcode/>;
	skos:exactMatch medtop:20000170;
	skos:broader	subj:04000000;
	skos:narrower	subj:04016001;
	skos:narrower	subj:04016002;
	skos:narrower	subj:04016003;
	skos:narrower	subj:04016004;
	skos:narrower	subj:04016005;
	skos:narrower	subj:04016006;
	skos:narrower	subj:04016007;
	skos:narrower	subj:04016008;
	skos:narrower	subj:04016009;
	skos:narrower	subj:04016010;
	skos:narrower	subj:04016011;
	skos:narrower	subj:04016012;
	skos:narrower	subj:04016013;
	skos:narrower	subj:04016014;
	skos:narrower	subj:04016015;
	skos:narrower	subj:04016016;
	skos:narrower	subj:04016017;
	skos:narrower	subj:04016018;
	skos:narrower	subj:04016019;
	skos:narrower	subj:04016020;
	skos:narrower	subj:04016021;
	skos:narrower	subj:04016022;
	skos:narrower	subj:04016023;
	skos:narrower	subj:04016024;
	skos:narrower	subj:04016025;
	skos:narrower	subj:04016026;
	skos:narrower	subj:04016027;
	skos:narrower	subj:04016028;
	skos:narrower	subj:04016029;
	skos:narrower	subj:04016030;
	skos:narrower	subj:04016031;
	skos:narrower	subj:04016032;
	skos:narrower	subj:04016033;
	skos:narrower	subj:04016034;
	skos:narrower	subj:04016035;
	skos:narrower	subj:04016036;
	skos:narrower	subj:04016037;
	skos:narrower	subj:04016038;
	skos:narrower	subj:04016039;
	skos:narrower	subj:04016040;
	skos:narrower	subj:04016041;
	skos:narrower	subj:04016042;
	skos:narrower	subj:04016043;
	skos:narrower	subj:04016044;
	skos:narrower	subj:04016045;
	skos:narrower	subj:04016046;
	skos:narrower	subj:04016047;
	skos:narrower	subj:04016048;
	skos:narrower	subj:04016049;
	skos:narrower	subj:04016050;
	skos:narrower	subj:04016051;
	skos:narrower	subj:04016052;
	skos:narrower	subj:04016053;
	skos:narrower	subj:04016054;
	skos:narrower	subj:04016055;
	skos:narrower	subj:04016056;
	skos:narrower	subj:04016057.

subj:04016001
	rdf:type skos:Concept;
	skos:prefLabel	"accounting and audit"@en-GB;
	skos:definition	"Changes in choice of auditing firm. Reports on impact of changes in GAAP. "@en-GB;
	skos:inScheme <http://cv.iptc.org/newscodes/subjectcode/>;
	skos:exactMatch medtop:20000172;
	skos:broader	subj:04016000.

subj:04016002
	rdf:type skos:Concept;
	skos:prefLabel	"annual and special corporate meeting"@en-GB;
	skos:definition	"Announcements of upcoming meetings. Reports on meetings. "@en-GB;
	skos:inScheme <http://cv.iptc.org/newscodes/subjectcode/>;
	skos:exactMatch medtop:20000193;
	skos:broader	subj:04016000.

subj:04016003
	rdf:type skos:Concept;
	skos:prefLabel	"annual report"@en-GB;
	skos:definition	"Availability or contents of annual company reports. "@en-GB;
	skos:inScheme <http://cv.iptc.org/newscodes/subjectcode/>;
	skos:exactMatch medtop:20000194;
	skos:broader	subj:04016000.

subj:04016004
	rdf:type skos:Concept;
	skos:prefLabel	"antitrust issue"@en-GB;
	skos:definition	"Antitrust activities, monopoly regulation, etc. "@en-GB;
	skos:inScheme <http://cv.iptc.org/newscodes/subjectcode/>;
	skos:exactMatch medtop:20000123;
	skos:broader	subj:04016000.

subj:04016005
	rdf:type skos:Concept;
	skos:prefLabel	"merger, acquisition and takeover"@en-GB;
	skos:definition	"News on mergers, takeovers or acquisitions. "@en-GB;
	skos:inScheme <http://cv.iptc.org/newscodes/subjectcode/>;
	skos:exactMatch medtop:20000204;
	skos:broader	subj:04016000.

subj:04016006
	rdf:type skos:Concept;
	skos:prefLabel	"analysts' comment"@en-GB;
	skos:definition	"Stock analyst comments, analysis and recommendations. "@en-GB;
	skos:inScheme <http://cv.iptc.org/newscodes/subjectcode/>;
	skos:exactMatch medtop:20000173;
	skos:broader	subj:04016000.

subj:04016007
	rdf:type skos:Concept;
	skos:prefLabel	"bankruptcy"@en-GB;
	skos:definition	"Actual bankruptcy filings. "@en-GB;
	skos:inScheme <http://cv.iptc.org/newscodes/subjectcode/>;
	skos:exactMatch medtop:20000174;
	skos:broader	subj:04016000.

subj:04016008
	rdf:type skos:Concept;
	skos:prefLabel	"board of directors (appointment and change)"@en-GB;
	skos:definition	"Appointments to or changes in the board of directors for a company. "@en-GB;
	skos:inScheme <http://cv.iptc.org/newscodes/subjectcode/>;
	skos:exactMatch medtop:20000195;
	skos:broader	subj:04016000.

subj:04016009
	rdf:type skos:Concept;
	skos:prefLabel	"buyback"@en-GB;
	skos:definition	"Stock buyback programs. This should be kept distinct from Stock Activity (see below). "@en-GB;
	skos:inScheme <http://cv.iptc.org/newscodes/subjectcode/>;
	skos:exactMatch medtop:20000175;
	skos:broader	subj:04016000.

subj:04016010
	rdf:type skos:Concept;
	skos:prefLabel	"C.E.O. interview"@en-GB;
	skos:definition	"Interviews with Chief Executive Officers. "@en-GB;
	skos:inScheme <http://cv.iptc.org/newscodes/subjectcode/>;
	skos:broadMatch medtop:20000170;
	skos:broader	subj:04016000.

subj:04016011
	rdf:type skos:Concept;
	skos:prefLabel	"corporate officer"@en-GB;
	skos:definition	"Appointments or changes in corporate officers. "@en-GB;
	skos:inScheme <http://cv.iptc.org/newscodes/subjectcode/>;
	skos:broadMatch medtop:20000190;
	skos:broader	subj:04016000.

subj:04016012
	rdf:type skos:Concept;
	skos:prefLabel	"corporate profile"@en-GB;
	skos:definition	"Descriptive profiles of companies. "@en-GB;
	skos:inScheme <http://cv.iptc.org/newscodes/subjectcode/>;
	skos:broadMatch medtop:20000170;
	skos:broader	subj:04016000.

subj:04016013
	rdf:type skos:Concept;
	skos:prefLabel	"contract"@en-GB;
	skos:definition	"Commercial contracts. "@en-GB;
	skos:inScheme <http://cv.iptc.org/newscodes/subjectcode/>;
	skos:exactMatch medtop:20000196;
	skos:broader	subj:04016000.

subj:04016014
	rdf:type skos:Concept;
	skos:prefLabel	"defence contract"@en-GB;
	skos:definition	"The award of government contracts for defence related activity. "@en-GB;
	skos:inScheme <http://cv.iptc.org/newscodes/subjectcode/>;
	skos:broadMatch medtop:20000196;
	skos:broader	subj:04016000.

subj:04016015
	rdf:type skos:Concept;
	skos:prefLabel	"dividend announcement"@en-GB;
	skos:definition	"Announcements regarding the disbursement of dividends. "@en-GB;
	skos:inScheme <http://cv.iptc.org/newscodes/subjectcode/>;
	skos:exactMatch medtop:20000177;
	skos:broader	subj:04016000.

subj:04016016
	rdf:type skos:Concept;
	skos:prefLabel	"earnings forecast"@en-GB;
	skos:definition	"Analyst prediction of company earnings. "@en-GB;
	skos:inScheme <http://cv.iptc.org/newscodes/subjectcode/>;
	skos:exactMatch medtop:20000179;
	skos:broader	subj:04016000.

subj:04016017
	rdf:type skos:Concept;
	skos:prefLabel	"financially distressed company"@en-GB;
	skos:definition	"Aa company is financially distressed - not yet having filed for bankruptcy. "@en-GB;
	skos:inScheme <http://cv.iptc.org/newscodes/subjectcode/>;
	skos:exactMatch medtop:20000182;
	skos:broader	subj:04016000.

subj:04016018
	rdf:type skos:Concept;
	skos:prefLabel	"earnings"@en-GB;
	skos:definition	"Any increase of earnings results. "@en-GB;
	skos:inScheme <http://cv.iptc.org/newscodes/subjectcode/>;
	skos:exactMatch medtop:20000178;
	skos:broader	subj:04016000.

subj:04016019
	rdf:type skos:Concept;
	skos:prefLabel	"financing and stock offering"@en-GB;
	skos:definition	"New offerings of equity including initial public offerings. "@en-GB;
	skos:inScheme <http://cv.iptc.org/newscodes/subjectcode/>;
	skos:exactMatch medtop:20000183;
	skos:broader	subj:04016000.

subj:04016020
	rdf:type skos:Concept;
	skos:prefLabel	"government contract"@en-GB;
	skos:definition	"The award of government contracts not related to defence activity "@en-GB;
	skos:inScheme <http://cv.iptc.org/newscodes/subjectcode/>;
	skos:broadMatch medtop:20000196;
	skos:broader	subj:04016000.

subj:04016021
	rdf:type skos:Concept;
	skos:prefLabel	"global expansion"@en-GB;
	skos:definition	"Planned or actual openings of offices in countries for the first time. "@en-GB;
	skos:inScheme <http://cv.iptc.org/newscodes/subjectcode/>;
	skos:broadMatch medtop:20000170;
	skos:broader	subj:04016000.

subj:04016022
	rdf:type skos:Concept;
	skos:prefLabel	"insider trading"@en-GB;
	skos:definition	"The purchase or sales of stock by corporate officers or board members. "@en-GB;
	skos:inScheme <http://cv.iptc.org/newscodes/subjectcode/>;
	skos:exactMatch medtop:20000091;
	skos:broader	subj:04016000.

subj:04016023
	rdf:type skos:Concept;
	skos:prefLabel	"joint venture"@en-GB;
	skos:definition	"Joint ventures between companies. (Not marketing related - see Marketing.) "@en-GB;
	skos:inScheme <http://cv.iptc.org/newscodes/subjectcode/>;
	skos:exactMatch medtop:20000200;
	skos:broader	subj:04016000.

subj:04016024
	rdf:type skos:Concept;
	skos:prefLabel	"leveraged buyout"@en-GB;
	skos:definition	"Leveraged buyouts. "@en-GB;
	skos:inScheme <http://cv.iptc.org/newscodes/subjectcode/>;
	skos:exactMatch medtop:20000201;
	skos:broader	subj:04016000.

subj:04016025
	rdf:type skos:Concept;
	skos:prefLabel	"layoffs and downsizing"@en-GB;
	skos:definition	"Planned or actual reductions in the labour force. "@en-GB;
	skos:inScheme <http://cv.iptc.org/newscodes/subjectcode/>;
	skos:exactMatch medtop:20000189;
	skos:broader	subj:04016000.

subj:04016026
	rdf:type skos:Concept;
	skos:prefLabel	"licensing agreement"@en-GB;
	skos:definition	"Licensing agreements between companies. "@en-GB;
	skos:inScheme <http://cv.iptc.org/newscodes/subjectcode/>;
	skos:exactMatch medtop:20000202;
	skos:broader	subj:04016000.

subj:04016027
	rdf:type skos:Concept;
	skos:prefLabel	"litigation and regulation"@en-GB;
	skos:definition	"Corporate law including litigation and regulations. "@en-GB;
	skos:inScheme <http://cv.iptc.org/newscodes/subjectcode/>;
	skos:closeMatch medtop:20000199;
	skos:broader	subj:04016000.

subj:04016028
	rdf:type skos:Concept;
	skos:prefLabel	"management change"@en-GB;
	skos:definition	"Major appointments or changes in management below the level of corporate officer. "@en-GB;
	skos:inScheme <http://cv.iptc.org/newscodes/subjectcode/>;
	skos:closeMatch medtop:20000190;
	skos:broader	subj:04016000.

subj:04016029
	rdf:type skos:Concept;
	skos:prefLabel	"marketing"@en-GB;
	skos:definition	"Includes news regarding joint marketing agreements between companies, adoption of new product marketing strategies, etc. "@en-GB;
	skos:inScheme <http://cv.iptc.org/newscodes/subjectcode/>;
	skos:closeMatch medtop:20000192;
	skos:broader	subj:04016000.

subj:04016030
	rdf:type skos:Concept;
	skos:prefLabel	"new product"@en-GB;
	skos:definition	"Announcements of new products. "@en-GB;
	skos:inScheme <http://cv.iptc.org/newscodes/subjectcode/>;
	skos:closeMatch medtop:20000205;
	skos:broader	subj:04016000.

subj:04016031
	rdf:type skos:Concept;
	skos:prefLabel	"patent, copyright and trademark"@en-GB;
	skos:definition	"News related to patents, copyright and trademarks. "@en-GB;
	skos:inScheme <http://cv.iptc.org/newscodes/subjectcode/>;
	skos:exactMatch medtop:20000206;
	skos:broader	subj:04016000.

subj:04016032
	rdf:type skos:Concept;
	skos:prefLabel	"plant closing"@en-GB;
	skos:definition	"Announcements of planned or actual plant closings. "@en-GB;
	skos:inScheme <http://cv.iptc.org/newscodes/subjectcode/>;
	skos:broadMatch medtop:20000170;
	skos:broader	subj:04016000.

subj:04016033
	rdf:type skos:Concept;
	skos:prefLabel	"plant opening"@en-GB;
	skos:definition	"Announcements of planned or actual plant openings. "@en-GB;
	skos:inScheme <http://cv.iptc.org/newscodes/subjectcode/>;
	skos:broadMatch medtop:20000170;
	skos:broader	subj:04016000.

subj:04016034
	rdf:type skos:Concept;
	skos:prefLabel	"privatisation"@en-GB;
	skos:definition	"Privatisation (privatisation) of state run companies. "@en-GB;
	skos:inScheme <http://cv.iptc.org/newscodes/subjectcode/>;
	skos:exactMatch medtop:20000624;
	skos:broader	subj:04016000.

subj:04016035
	rdf:type skos:Concept;
	skos:prefLabel	"proxy filing"@en-GB;
	skos:definition	"Filings with regulatory agencies of proxy statements for upcoming shareholder votes. "@en-GB;
	skos:inScheme <http://cv.iptc.org/newscodes/subjectcode/>;
	skos:exactMatch medtop:20000181;
	skos:broader	subj:04016000.

subj:04016036
	rdf:type skos:Concept;
	skos:prefLabel	"rating"@en-GB;
	skos:definition	"Corporate and sovereign debt and credit ratings (e.g. SandP or Moody's) "@en-GB;
	skos:inScheme <http://cv.iptc.org/newscodes/subjectcode/>;
	skos:exactMatch medtop:20000176;
	skos:broader	subj:04016000.

subj:04016037
	rdf:type skos:Concept;
	skos:prefLabel	"research and development"@en-GB;
	skos:definition	"Research and expenditure on new product development. "@en-GB;
	skos:inScheme <http://cv.iptc.org/newscodes/subjectcode/>;
	skos:exactMatch medtop:20000208;
	skos:broader	subj:04016000.

subj:04016038
	rdf:type skos:Concept;
	skos:prefLabel	"quarterly or semiannual financial statement"@en-GB;
	skos:definition	"Availability or contents of quarterly or semi-annual corporate reports. "@en-GB;
	skos:inScheme <http://cv.iptc.org/newscodes/subjectcode/>;
	skos:exactMatch medtop:20000180;
	skos:broader	subj:04016000.

subj:04016039
	rdf:type skos:Concept;
	skos:prefLabel	"restructuring and recapitalisation"@en-GB;
	skos:definition	"Sale of company units, splits of existing companies into units under a holding company, etc. "@en-GB;
	skos:inScheme <http://cv.iptc.org/newscodes/subjectcode/>;
	skos:exactMatch medtop:20000184;
	skos:broader	subj:04016000.

subj:04016040
	rdf:type skos:Concept;
	skos:prefLabel	"spin-off"@en-GB;
	skos:definition	"Creation of new companies being spun off from existing companies. "@en-GB;
	skos:inScheme <http://cv.iptc.org/newscodes/subjectcode/>;
	skos:exactMatch medtop:20000197;
	skos:broader	subj:04016000.

subj:04016041
	rdf:type skos:Concept;
	skos:prefLabel	"stock activity"@en-GB;
	skos:definition	"Announcements of major stock events: splits, block trades, new highs or lows, etc. "@en-GB;
	skos:inScheme <http://cv.iptc.org/newscodes/subjectcode/>;
	skos:exactMatch medtop:20000186;
	skos:broader	subj:04016000.

subj:04016042
	rdf:type skos:Concept;
	skos:prefLabel	"industrial production"@en-GB;
	skos:definition	"Manufacture of durable and non-durable goods "@en-GB;
	skos:inScheme <http://cv.iptc.org/newscodes/subjectcode/>;
	skos:exactMatch medtop:20000360;
	skos:broader	subj:04016000.

subj:04016043
	rdf:type skos:Concept;
	skos:prefLabel	"productivity"@en-GB;
	skos:definition	"The cost of labour to produce an item of value, often measured as output per hour per person "@en-GB;
	skos:inScheme <http://cv.iptc.org/newscodes/subjectcode/>;
	skos:exactMatch medtop:20000362;
	skos:broader	subj:04016000.

subj:04016044
	rdf:type skos:Concept;
	skos:prefLabel	"inventories"@en-GB;
	skos:definition	"Goods not sold and held by the producer, wholesaler or retailer "@en-GB;
	skos:inScheme <http://cv.iptc.org/newscodes/subjectcode/>;
	skos:exactMatch medtop:20000361;
	skos:broader	subj:04016000.

subj:04016045
	rdf:type skos:Concept;
	skos:prefLabel	"sales"@en-GB;
	skos:definition	"Either the exchange of goods for money, or the practice of discounting prices to increase the amount of goods sold, or to get rid of outdated merchandise "@en-GB;
	skos:inScheme <http://cv.iptc.org/newscodes/subjectcode/>;
	skos:closeMatch medtop:20000243;
	skos:broader	subj:04016000.

subj:04016046
	rdf:type skos:Concept;
	skos:prefLabel	"corporations"@en-GB;
	skos:definition	"Business enterprises formally licensed with boards of directors and hierarchical structures of governance "@en-GB;
	skos:inScheme <http://cv.iptc.org/newscodes/subjectcode/>;
	skos:broader	subj:04016000.

subj:04016047
	rdf:type skos:Concept;
	skos:prefLabel	"shareholders"@en-GB;
	skos:definition	"Anyone holding a piece of paper issued by a company which changes in value and entitles them to dividends depending on the performance of the company "@en-GB;
	skos:inScheme <http://cv.iptc.org/newscodes/subjectcode/>;
	skos:exactMatch medtop:20000185;
	skos:broader	subj:04016000.

subj:04016048
	rdf:type skos:Concept;
	skos:prefLabel	"corporate performance"@en-GB;
	skos:definition	"How well a company performs, measured by its net earnings, its dividends its earnings per share and price/earnings ratio "@en-GB;
	skos:inScheme <http://cv.iptc.org/newscodes/subjectcode/>;
	skos:broadMatch medtop:20000170;
	skos:broader	subj:04016000.

subj:04016049
	rdf:type skos:Concept;
	skos:prefLabel	"losses"@en-GB;
	skos:definition	"When expenses exceed revenue "@en-GB;
	skos:inScheme <http://cv.iptc.org/newscodes/subjectcode/>;
	skos:broadMatch medtop:20000170;
	skos:broader	subj:04016000.

subj:04016050
	rdf:type skos:Concept;
	skos:prefLabel	"credit ratings"@en-GB;
	skos:definition	"Formal statements by certain rating agencies such as Standard and Poor's on the investment risk of a company, a country or enterprise "@en-GB;
	skos:inScheme <http://cv.iptc.org/newscodes/subjectcode/>;
	skos:exactMatch medtop:20000176;
	skos:broader	subj:04016000.

subj:04016051
	rdf:type skos:Concept;
	skos:prefLabel	"stock splits"@en-GB;
	skos:definition	"Issuing multiple shares for one share of stock. Usually occurs when the price of a stock has increased so much that its purchase price is not attractive. A reverse split is when one share is issued for multiple shares, to raise the per share value. "@en-GB;
	skos:inScheme <http://cv.iptc.org/newscodes/subjectcode/>;
	skos:broader	subj:04016000.

subj:04016052
	rdf:type skos:Concept;
	skos:prefLabel	"stock options"@en-GB;
	skos:definition	"An agreement to either buy or sell a stock when it meets a certain price "@en-GB;
	skos:inScheme <http://cv.iptc.org/newscodes/subjectcode/>;
	skos:exactMatch medtop:20000191;
	skos:broader	subj:04016000.

subj:04016053
	rdf:type skos:Concept;
	skos:prefLabel	"recalls (products)"@en-GB;
	skos:definition	"A decision by a company to take back or repair a defective product "@en-GB;
	skos:inScheme <http://cv.iptc.org/newscodes/subjectcode/>;
	skos:exactMatch medtop:20000207;
	skos:broader	subj:04016000.

subj:04016054
	rdf:type skos:Concept;
	skos:prefLabel	"globalization"@en-GB;
	skos:definition	"Doing business around the world "@en-GB;
	skos:inScheme <http://cv.iptc.org/newscodes/subjectcode/>;
	skos:exactMatch medtop:20000198;
	skos:broader	subj:04016000.

subj:04016055
	rdf:type skos:Concept;
	skos:prefLabel	"consumers"@en-GB;
	skos:definition	"Buyers of goods and services "@en-GB;
	skos:inScheme <http://cv.iptc.org/newscodes/subjectcode/>;
	skos:exactMatch medtop:20000351;
	skos:broader	subj:04016000.

subj:04016056
	rdf:type skos:Concept;
	skos:prefLabel	"purchase"@en-GB;
	skos:definition	"Items that companies buy, such as raw materials, office supplies etc. "@en-GB;
	skos:inScheme <http://cv.iptc.org/newscodes/subjectcode/>;
	skos:closeMatch medtop:20000243;
	skos:broader	subj:04016000.

subj:04016057
	rdf:type skos:Concept;
	skos:prefLabel	"new service"@en-GB;
	skos:definition	"New services added by a company, such as new flight routes, etc. "@en-GB;
	skos:inScheme <http://cv.iptc.org/newscodes/subjectcode/>;
	skos:closeMatch medtop:20000205;
	skos:broader	subj:04016000.

subj:04017000
	rdf:type skos:Concept;
	skos:prefLabel	"economy (general)"@en-GB;
	skos:definition	"Content of a general nature about trade and the economy "@en-GB;
	skos:inScheme <http://cv.iptc.org/newscodes/subjectcode/>;
	skos:exactMatch medtop:20000344;
	skos:broader	subj:04000000;
	skos:narrower	subj:04017001.

subj:04017001
	rdf:type skos:Concept;
	skos:prefLabel	"economic policy"@en-GB;
	skos:definition	"Government directed policy on production, taxes, tariffs and things that affect the direction and health of the economy "@en-GB;
	skos:inScheme <http://cv.iptc.org/newscodes/subjectcode/>;
	skos:exactMatch medtop:20000345;
	skos:broader	subj:04017000.

subj:04018000
	rdf:type skos:Concept;
	skos:prefLabel	"business (general)"@en-GB;
	skos:definition	"Content of a general nature about business "@en-GB;
	skos:inScheme <http://cv.iptc.org/newscodes/subjectcode/>;
	skos:broadMatch medtop:04000000;
	skos:broader	subj:04000000;
	skos:narrower	subj:04018001.

subj:04018001
	rdf:type skos:Concept;
	skos:prefLabel	"institution"@en-GB;
	skos:definition	"Either an established law, practice or system or an organization having a social, religious, educational or similar purpose such as hospital, school, prison "@en-GB;
	skos:historyNote	"code changed, was 01018001 "@en-GB;
	skos:inScheme <http://cv.iptc.org/newscodes/subjectcode/>;
	skos:broadMatch medtop:04000000;
	skos:broader	subj:04018000.

subj:04019000
	rdf:type skos:Concept;
	skos:prefLabel	"finance (general)"@en-GB;
	skos:definition	"Content of a general nature about finance "@en-GB;
	skos:inScheme <http://cv.iptc.org/newscodes/subjectcode/>;
	skos:broadMatch medtop:04000000;
	skos:broader	subj:04000000;
	skos:narrower	subj:04019001.

subj:04019001
	rdf:type skos:Concept;
	skos:prefLabel	"money and monetary policy"@en-GB;
	skos:definition	"Government bank directed policy on the amount of money in circulation and the rate at which it can be loaned "@en-GB;
	skos:inScheme <http://cv.iptc.org/newscodes/subjectcode/>;
	skos:exactMatch medtop:20000379;
	skos:broader	subj:04019000.

subj:05000000
	rdf:type skos:Concept;
	skos:prefLabel	"education"@en-GB;
	skos:definition	"All aspects of furthering knowledge of human individuals from birth to death. "@en-GB;
	skos:inScheme <http://cv.iptc.org/newscodes/subjectcode/>;
	skos:exactMatch medtop:05000000;
	skos:narrower	subj:05001000;
	skos:narrower	subj:05002000;
	skos:narrower	subj:05003000;
	skos:narrower	subj:05004000;
	skos:narrower	subj:05005000;
	skos:narrower	subj:05006000;
	skos:narrower	subj:05007000;
	skos:narrower	subj:05008000;
	skos:narrower	subj:05009000;
	skos:narrower	subj:05010000;
	skos:narrower	subj:05011000.

subj:05001000
	rdf:type skos:Concept;
	skos:prefLabel	"adult education"@en-GB;
	skos:definition	"Education provided for older students outside the usual age groups of 5-25 "@en-GB;
	skos:inScheme <http://cv.iptc.org/newscodes/subjectcode/>;
	skos:exactMatch medtop:20000403;
	skos:broader	subj:05000000.

subj:05002000
	rdf:type skos:Concept;
	skos:prefLabel	"further education"@en-GB;
	skos:definition	"Any form of education beyond basic education of several levels "@en-GB;
	skos:inScheme <http://cv.iptc.org/newscodes/subjectcode/>;
	skos:exactMatch medtop:20000402;
	skos:broader	subj:05000000.

subj:05003000
	rdf:type skos:Concept;
	skos:prefLabel	"parent organisation"@en-GB;
	skos:definition	"Groups of parents set up to support schools "@en-GB;
	skos:inScheme <http://cv.iptc.org/newscodes/subjectcode/>;
	skos:exactMatch medtop:20000398;
	skos:broader	subj:05000000.

subj:05004000
	rdf:type skos:Concept;
	skos:prefLabel	"preschool"@en-GB;
	skos:definition	"Education for children under the national compulsory education age "@en-GB;
	skos:inScheme <http://cv.iptc.org/newscodes/subjectcode/>;
	skos:exactMatch medtop:20000409;
	skos:broader	subj:05000000.

subj:05005000
	rdf:type skos:Concept;
	skos:prefLabel	"school"@en-GB;
	skos:definition	"A building or institution in which education of various sorts is provided "@en-GB;
	skos:inScheme <http://cv.iptc.org/newscodes/subjectcode/>;
	skos:exactMatch medtop:20000400;
	skos:broader	subj:05000000;
	skos:narrower	subj:05005001;
	skos:narrower	subj:05005002;
	skos:narrower	subj:05005003.

subj:05005001
	rdf:type skos:Concept;
	skos:prefLabel	"elementary schools"@en-GB;
	skos:definition	"Schools usually of a level from kindergarten through 11 or 12 years of age "@en-GB;
	skos:inScheme <http://cv.iptc.org/newscodes/subjectcode/>;
	skos:exactMatch medtop:20000401;
	skos:broader	subj:05005000.

subj:05005002
	rdf:type skos:Concept;
	skos:prefLabel	"middle schools"@en-GB;
	skos:definition	"Transitional school between elementary and high school, 12 through 13 years of age "@en-GB;
	skos:inScheme <http://cv.iptc.org/newscodes/subjectcode/>;
	skos:exactMatch medtop:20000408;
	skos:broader	subj:05005000.

subj:05005003
	rdf:type skos:Concept;
	skos:prefLabel	"high schools"@en-GB;
	skos:definition	"Pre-college/ university level education, 14 to 17 or 18 years of age, called freshman, sophomore, junior and senior "@en-GB;
	skos:inScheme <http://cv.iptc.org/newscodes/subjectcode/>;
	skos:exactMatch medtop:20000404;
	skos:broader	subj:05005000.

subj:05006000
	rdf:type skos:Concept;
	skos:prefLabel	"teachers union"@en-GB;
	skos:definition	"Organization of teachers for collective bargaining and other purposes "@en-GB;
	skos:inScheme <http://cv.iptc.org/newscodes/subjectcode/>;
	skos:broadMatch medtop:20000536;
	skos:broader	subj:05000000.

subj:05007000
	rdf:type skos:Concept;
	skos:prefLabel	"university"@en-GB;
	skos:definition	"Institutions of higher learning capable of providing doctorate degrees "@en-GB;
	skos:inScheme <http://cv.iptc.org/newscodes/subjectcode/>;
	skos:exactMatch medtop:20000407;
	skos:broader	subj:05000000.

subj:05008000
	rdf:type skos:Concept;
	skos:prefLabel	"upbringing"@en-GB;
	skos:definition	"Lessons learned from parents and others as one grows up "@en-GB;
	skos:inScheme <http://cv.iptc.org/newscodes/subjectcode/>;
	skos:closeMatch medtop:20000410;
	skos:broader	subj:05000000.

subj:05009000
	rdf:type skos:Concept;
	skos:prefLabel	"entrance examination"@en-GB;
	skos:definition	"Exams for entering colleges, universities, junior and senior high schools, and all other higher and lower education institutes, including cram schools, which help students prepare for exams for entry to prestigious schools. "@en-GB;
	skos:inScheme <http://cv.iptc.org/newscodes/subjectcode/>;
	skos:exactMatch medtop:20000414;
	skos:broader	subj:05000000.

subj:05010000
	rdf:type skos:Concept;
	skos:prefLabel	"teaching and learning"@en-GB;
	skos:definition	"Either end of the education equation "@en-GB;
	skos:inScheme <http://cv.iptc.org/newscodes/subjectcode/>;
	skos:exactMatch medtop:20000411;
	skos:broader	subj:05000000;
	skos:narrower	subj:05010001;
	skos:narrower	subj:05010002;
	skos:narrower	subj:05010003;
	skos:narrower	subj:05010004.

subj:05010001
	rdf:type skos:Concept;
	skos:prefLabel	"students"@en-GB;
	skos:definition	"People of any age in a structured environment, not necessarily a classroom, in order to learn something "@en-GB;
	skos:inScheme <http://cv.iptc.org/newscodes/subjectcode/>;
	skos:exactMatch medtop:20000415;
	skos:broader	subj:05010000.

subj:05010002
	rdf:type skos:Concept;
	skos:prefLabel	"teachers"@en-GB;
	skos:definition	"People with knowledge who can impart that knowledge to others "@en-GB;
	skos:inScheme <http://cv.iptc.org/newscodes/subjectcode/>;
	skos:exactMatch medtop:20000416;
	skos:broader	subj:05010000.

subj:05010003
	rdf:type skos:Concept;
	skos:prefLabel	"curriculum"@en-GB;
	skos:definition	"The courses offered by a learning institution and the regulation of those courses "@en-GB;
	skos:inScheme <http://cv.iptc.org/newscodes/subjectcode/>;
	skos:exactMatch medtop:20000412;
	skos:broader	subj:05010000.

subj:05010004
	rdf:type skos:Concept;
	skos:prefLabel	"test/examination"@en-GB;
	skos:definition	"A measurement of student accomplishment "@en-GB;
	skos:inScheme <http://cv.iptc.org/newscodes/subjectcode/>;
	skos:closeMatch medtop:20000413;
	skos:broader	subj:05010000.

subj:05011000
	rdf:type skos:Concept;
	skos:prefLabel	"religious education"@en-GB;
	skos:definition	"Instruction by any faith, in that faith or about other faiths, usually, but not always, conducted in schools run by religious bodies "@en-GB;
	skos:inScheme <http://cv.iptc.org/newscodes/subjectcode/>;
	skos:exactMatch medtop:20000399;
	skos:broader	subj:05000000;
	skos:narrower	subj:05011001;
	skos:narrower	subj:05011002;
	skos:narrower	subj:05011003;
	skos:narrower	subj:05011004.

subj:05011001
	rdf:type skos:Concept;
	skos:prefLabel	"parochial school"@en-GB;
	skos:definition	"A school run by the Roman Catholic faith "@en-GB;
	skos:inScheme <http://cv.iptc.org/newscodes/subjectcode/>;
	skos:broadMatch medtop:20000399;
	skos:broader	subj:05011000.

subj:05011002
	rdf:type skos:Concept;
	skos:prefLabel	"seminary"@en-GB;
	skos:definition	"A school of any faith specifically designed to train ministers "@en-GB;
	skos:inScheme <http://cv.iptc.org/newscodes/subjectcode/>;
	skos:broadMatch medtop:20000399;
	skos:broader	subj:05011000.

subj:05011003
	rdf:type skos:Concept;
	skos:prefLabel	"yeshiva"@en-GB;
	skos:definition	"A school for training rabbis "@en-GB;
	skos:inScheme <http://cv.iptc.org/newscodes/subjectcode/>;
	skos:broadMatch medtop:20000399;
	skos:broader	subj:05011000.

subj:05011004
	rdf:type skos:Concept;
	skos:prefLabel	"madrasa"@en-GB;
	skos:definition	"A school for teaching Islam "@en-GB;
	skos:inScheme <http://cv.iptc.org/newscodes/subjectcode/>;
	skos:broadMatch medtop:20000399;
	skos:broader	subj:05011000.

subj:06000000
	rdf:type skos:Concept;
	skos:prefLabel	"environmental issue"@en-GB;
	skos:definition	"All aspects of protection, damage, and condition of the ecosystem of the planet earth and its surroundings. "@en-GB;
	skos:inScheme <http://cv.iptc.org/newscodes/subjectcode/>;
	skos:exactMatch medtop:06000000;
	skos:narrower	subj:06001000;
	skos:narrower	subj:06002000;
	skos:narrower	subj:06003000;
	skos:narrower	subj:06004000;
	skos:narrower	subj:06005000;
	skos:narrower	subj:06006000;
	skos:narrower	subj:06007000;
	skos:narrower	subj:06008000;
	skos:narrower	subj:06009000;
	skos:narrower	subj:06010000;
	skos:narrower	subj:06011000;
	skos:narrower	subj:06012000;
	skos:narrower	subj:06013000.

subj:06001000
	rdf:type skos:Concept;
	skos:prefLabel	"renewable energy"@en-GB;
	skos:definition	"Environmental impact of renewable energy, including solar, wind, hydro, biomass and geothermal "@en-GB;
	skos:inScheme <http://cv.iptc.org/newscodes/subjectcode/>;
	skos:exactMatch medtop:20000436;
	skos:broader	subj:06000000.

subj:06002000
	rdf:type skos:Concept;
	skos:prefLabel	"conservation"@en-GB;
	skos:definition	"Preservation of wilderness areas, flora and fauna, including species extinction "@en-GB;
	skos:inScheme <http://cv.iptc.org/newscodes/subjectcode/>;
	skos:exactMatch medtop:20000420;
	skos:broader	subj:06000000;
	skos:narrower	subj:06002001;
	skos:narrower	subj:06002002.

subj:06002001
	rdf:type skos:Concept;
	skos:prefLabel	"endangered species"@en-GB;
	skos:definition	"Those species of wildlife in danger of disappearing, largely because of changes in environment, hunting, or weather "@en-GB;
	skos:inScheme <http://cv.iptc.org/newscodes/subjectcode/>;
	skos:exactMatch medtop:20000443;
	skos:broader	subj:06002000.

subj:06002002
	rdf:type skos:Concept;
	skos:prefLabel	"ecosystem"@en-GB;
	skos:definition	"A system of plants, animals and bacteria interrelated in its physical/chemical environment "@en-GB;
	skos:inScheme <http://cv.iptc.org/newscodes/subjectcode/>;
	skos:exactMatch medtop:20000442;
	skos:broader	subj:06002000.

subj:06003000
	rdf:type skos:Concept;
	skos:prefLabel	"energy saving"@en-GB;
	skos:definition	"Conservation of electrical, and other power sources "@en-GB;
	skos:inScheme <http://cv.iptc.org/newscodes/subjectcode/>;
	skos:exactMatch medtop:20000421;
	skos:broader	subj:06000000.

subj:06004000
	rdf:type skos:Concept;
	skos:prefLabel	"environmental politics"@en-GB;
	skos:definition	"The debate on environmental policy "@en-GB;
	skos:inScheme <http://cv.iptc.org/newscodes/subjectcode/>;
	skos:exactMatch medtop:20000423;
	skos:broader	subj:06000000.

subj:06005000
	rdf:type skos:Concept;
	skos:prefLabel	"environmental pollution"@en-GB;
	skos:definition	"Corruption of air, water, land etc. by harmful substances "@en-GB;
	skos:inScheme <http://cv.iptc.org/newscodes/subjectcode/>;
	skos:exactMatch medtop:20000424;
	skos:broader	subj:06000000;
	skos:narrower	subj:06005001;
	skos:narrower	subj:06005002.

subj:06005001
	rdf:type skos:Concept;
	skos:prefLabel	"air pollution"@en-GB;
	skos:definition	"Solid or gaseous matter affecting the quality of air that we breathe "@en-GB;
	skos:inScheme <http://cv.iptc.org/newscodes/subjectcode/>;
	skos:exactMatch medtop:20000425;
	skos:broader	subj:06005000.

subj:06005002
	rdf:type skos:Concept;
	skos:prefLabel	"water pollution"@en-GB;
	skos:definition	"Solids or liquids that corrupt the quality of water that could be used for drinking or irrigation "@en-GB;
	skos:inScheme <http://cv.iptc.org/newscodes/subjectcode/>;
	skos:exactMatch medtop:20000429;
	skos:broader	subj:06005000.

subj:06006000
	rdf:type skos:Concept;
	skos:prefLabel	"natural resources"@en-GB;
	skos:definition	"Stories about the environmental issues related to the exploitation of natural resources for human use "@en-GB;
	skos:inScheme <http://cv.iptc.org/newscodes/subjectcode/>;
	skos:exactMatch medtop:20000430;
	skos:broader	subj:06000000;
	skos:narrower	subj:06006001;
	skos:narrower	subj:06006002;
	skos:narrower	subj:06006003;
	skos:narrower	subj:06006004;
	skos:narrower	subj:06006005;
	skos:narrower	subj:06006006;
	skos:narrower	subj:06006007;
	skos:narrower	subj:06006008;
	skos:narrower	subj:06006009.

subj:06006001
	rdf:type skos:Concept;
	skos:prefLabel	"land resources"@en-GB;
	skos:definition	"That portion of a nation or state that is above water and available for development either for profit or for the general good of the public "@en-GB;
	skos:inScheme <http://cv.iptc.org/newscodes/subjectcode/>;
	skos:exactMatch medtop:20000432;
	skos:broader	subj:06006000.

subj:06006002
	rdf:type skos:Concept;
	skos:prefLabel	"parks"@en-GB;
	skos:definition	"Areas set aside and developed for public enjoyment and recreation, including commercial development such as theme parks "@en-GB;
	skos:inScheme <http://cv.iptc.org/newscodes/subjectcode/>;
	skos:closeMatch medtop:20000422;
	skos:broader	subj:06006000.

subj:06006003
	rdf:type skos:Concept;
	skos:prefLabel	"forests"@en-GB;
	skos:definition	"Open areas of trees either available for public enjoyment, or for commercial purposes "@en-GB;
	skos:inScheme <http://cv.iptc.org/newscodes/subjectcode/>;
	skos:exactMatch medtop:20000433;
	skos:broader	subj:06006000.

subj:06006004
	rdf:type skos:Concept;
	skos:prefLabel	"wetlands"@en-GB;
	skos:definition	"Areas generally marshy and not either under water or dry land. Often related to aquifers for water quality and/or wildlife "@en-GB;
	skos:inScheme <http://cv.iptc.org/newscodes/subjectcode/>;
	skos:exactMatch medtop:20000440;
	skos:broader	subj:06006000.

subj:06006005
	rdf:type skos:Concept;
	skos:prefLabel	"mountains"@en-GB;
	skos:definition	"Elevated land masses formed over the ages either by erosion, volcanic eruption, or movement of massive geographical formations called plates "@en-GB;
	skos:inScheme <http://cv.iptc.org/newscodes/subjectcode/>;
	skos:exactMatch medtop:20000434;
	skos:broader	subj:06006000.

subj:06006006
	rdf:type skos:Concept;
	skos:prefLabel	"rivers"@en-GB;
	skos:definition	"Moving water areas bounded by land that extend from earth sources and meander through land areas to join with other water areas. In smaller forms they are creeks, rivulets, streams etc "@en-GB;
	skos:inScheme <http://cv.iptc.org/newscodes/subjectcode/>;
	skos:exactMatch medtop:20000439;
	skos:broader	subj:06006000.

subj:06006007
	rdf:type skos:Concept;
	skos:prefLabel	"oceans"@en-GB;
	skos:definition	"Salt water masses separating continents or other major geographical masses. smaller forms are seas or lakes or ponds "@en-GB;
	skos:inScheme <http://cv.iptc.org/newscodes/subjectcode/>;
	skos:exactMatch medtop:20000438;
	skos:broader	subj:06006000.

subj:06006008
	rdf:type skos:Concept;
	skos:prefLabel	"wildlife"@en-GB;
	skos:definition	"All forms of animal life that have not been domesticated "@en-GB;
	skos:inScheme <http://cv.iptc.org/newscodes/subjectcode/>;
	skos:closeMatch medtop:20000441;
	skos:broader	subj:06006000.

subj:06006009
	rdf:type skos:Concept;
	skos:prefLabel	"energy resources"@en-GB;
	skos:definition	"Such resources as coal, gas, wind, sunlight etc., used to generate heat, electricity and power "@en-GB;
	skos:inScheme <http://cv.iptc.org/newscodes/subjectcode/>;
	skos:exactMatch medtop:20000431;
	skos:broader	subj:06006000.

subj:06007000
	rdf:type skos:Concept;
	skos:prefLabel	"nature"@en-GB;
	skos:definition	"Taken as a whole the natural environment of flora and fauna "@en-GB;
	skos:inScheme <http://cv.iptc.org/newscodes/subjectcode/>;
	skos:closeMatch medtop:20000441;
	skos:broader	subj:06000000;
	skos:narrower	subj:06007001.

subj:06007001
	rdf:type skos:Concept;
	skos:prefLabel	"invasive species"@en-GB;
	skos:definition	"Non-native plants, animals and other organisms that tend to take over native species "@en-GB;
	skos:inScheme <http://cv.iptc.org/newscodes/subjectcode/>;
	skos:exactMatch medtop:20000444;
	skos:broader	subj:06007000.

subj:06008000
	rdf:type skos:Concept;
	skos:prefLabel	"population"@en-GB;
	skos:definition	"People and their growth and development within a natural setting "@en-GB;
	skos:inScheme <http://cv.iptc.org/newscodes/subjectcode/>;
	skos:exactMatch medtop:20000435;
	skos:broader	subj:06000000.

subj:06009000
	rdf:type skos:Concept;
	skos:prefLabel	"waste"@en-GB;
	skos:definition	"Environmental impact of waste, including recycling efforts "@en-GB;
	skos:inScheme <http://cv.iptc.org/newscodes/subjectcode/>;
	skos:exactMatch medtop:20000428;
	skos:broader	subj:06000000.

subj:06010000
	rdf:type skos:Concept;
	skos:prefLabel	"water"@en-GB;
	skos:definition	"Environmental issues about bodies of water, including oceans, lakes, streams and reservoirs, as well as ice, glaciers and forms of precipitation "@en-GB;
	skos:inScheme <http://cv.iptc.org/newscodes/subjectcode/>;
	skos:exactMatch medtop:20000437;
	skos:broader	subj:06000000.

subj:06011000
	rdf:type skos:Concept;
	skos:prefLabel	"global warming"@en-GB;
	skos:definition	"All issues relating to global warming including temperature research, remote sensing on temperature trends, debate on global warming, ways to reduce emissions and carbon trading. "@en-GB;
	skos:inScheme <http://cv.iptc.org/newscodes/subjectcode/>;
	skos:exactMatch medtop:20000419;
	skos:broader	subj:06000000.

subj:06012000
	rdf:type skos:Concept;
	skos:prefLabel	"hazardous materials"@en-GB;
	skos:definition	"Materials that are harmful to humans or animals if they are exposed to them. Includes radiation, poison gases, chemicals, heavy metals, PCBs, and certain plant products "@en-GB;
	skos:inScheme <http://cv.iptc.org/newscodes/subjectcode/>;
	skos:exactMatch medtop:20000427;
	skos:broader	subj:06000000.

subj:06013000
	rdf:type skos:Concept;
	skos:prefLabel	"environmental cleanup"@en-GB;
	skos:definition	"Processes whereby contaminated areas are cleaned of hazardous materials so they can be inhabited again by either people or animals. "@en-GB;
	skos:inScheme <http://cv.iptc.org/newscodes/subjectcode/>;
	skos:exactMatch medtop:20000426;
	skos:broader	subj:06000000.

subj:07000000
	rdf:type skos:Concept;
	skos:prefLabel	"health"@en-GB;
	skos:definition	"All aspects pertaining to the physical and mental welfare of human beings. "@en-GB;
	skos:inScheme <http://cv.iptc.org/newscodes/subjectcode/>;
	skos:exactMatch medtop:07000000;
	skos:narrower	subj:07001000;
	skos:narrower	subj:07002000;
	skos:narrower	subj:07003000;
	skos:narrower	subj:07004000;
	skos:narrower	subj:07005000;
	skos:narrower	subj:07006000;
	skos:narrower	subj:07007000;
	skos:narrower	subj:07008000;
	skos:narrower	subj:07009000;
	skos:narrower	subj:07010000;
	skos:narrower	subj:07011000;
	skos:narrower	subj:07012000;
	skos:narrower	subj:07013000;
	skos:narrower	subj:07014000;
	skos:narrower	subj:07015000;
	skos:narrower	subj:07016000;
	skos:narrower	subj:07017000;
	skos:narrower	subj:07018000;
	skos:narrower	subj:07019000.

subj:07001000
	rdf:type skos:Concept;
	skos:prefLabel	"disease"@en-GB;
	skos:definition	"Any harmful or destructive condition "@en-GB;
	skos:inScheme <http://cv.iptc.org/newscodes/subjectcode/>;
	skos:exactMatch medtop:20000455;
	skos:broader	subj:07000000;
	skos:narrower	subj:07001001;
	skos:narrower	subj:07001002;
	skos:narrower	subj:07001003;
	skos:narrower	subj:07001004;
	skos:narrower	subj:07001005;
	skos:narrower	subj:07001006;
	skos:narrower	subj:07001007;
	skos:narrower	subj:07001008;
	skos:narrower	subj:07001009.

subj:07001001
	rdf:type skos:Concept;
	skos:prefLabel	"communicable diseases"@en-GB;
	skos:definition	"Diseases that can be transmitted from one person or animal to another "@en-GB;
	skos:inScheme <http://cv.iptc.org/newscodes/subjectcode/>;
	skos:exactMatch medtop:20000448;
	skos:broader	subj:07001000.

subj:07001002
	rdf:type skos:Concept;
	skos:prefLabel	"virus diseases"@en-GB;
	skos:definition	"Diseases caused by infection within cells by viruses "@en-GB;
	skos:inScheme <http://cv.iptc.org/newscodes/subjectcode/>;
	skos:exactMatch medtop:20000451;
	skos:broader	subj:07001000.

subj:07001003
	rdf:type skos:Concept;
	skos:prefLabel	"AIDS"@en-GB;
	skos:definition	"Acquired Immunity Deficiency Syndrome, an incurable disease caused by the human immunodeficiency virus "@en-GB;
	skos:inScheme <http://cv.iptc.org/newscodes/subjectcode/>;
	skos:exactMatch medtop:20000452;
	skos:broader	subj:07001000.

subj:07001004
	rdf:type skos:Concept;
	skos:prefLabel	"cancer"@en-GB;
	skos:definition	"A serious and often fatal disease caused when normal cells mutate into tumours "@en-GB;
	skos:inScheme <http://cv.iptc.org/newscodes/subjectcode/>;
	skos:exactMatch medtop:20000447;
	skos:broader	subj:07001000.

subj:07001005
	rdf:type skos:Concept;
	skos:prefLabel	"heart disease"@en-GB;
	skos:definition	"A degenerative and serious disease caused by narrowing of the arteries feeding the heart "@en-GB;
	skos:inScheme <http://cv.iptc.org/newscodes/subjectcode/>;
	skos:exactMatch medtop:20000454;
	skos:broader	subj:07001000.

subj:07001006
	rdf:type skos:Concept;
	skos:prefLabel	"alzheimer's disease"@en-GB;
	skos:definition	"A disorder of the brain leading to dementia "@en-GB;
	skos:inScheme <http://cv.iptc.org/newscodes/subjectcode/>;
	skos:broadMatch medtop:20000446;
	skos:broader	subj:07001000.

subj:07001007
	rdf:type skos:Concept;
	skos:prefLabel	"animal diseases"@en-GB;
	skos:definition	"Disorders affecting animals that do not necessarily endanger humans "@en-GB;
	skos:inScheme <http://cv.iptc.org/newscodes/subjectcode/>;
	skos:exactMatch medtop:20000494;
	skos:broader	subj:07001000.

subj:07001008
	rdf:type skos:Concept;
	skos:prefLabel	"plant diseases"@en-GB;
	skos:definition	"Disorders affecting plants caused either by parasites or environmental factors "@en-GB;
	skos:inScheme <http://cv.iptc.org/newscodes/subjectcode/>;
	skos:exactMatch medtop:20000495;
	skos:broader	subj:07001000.

subj:07001009
	rdf:type skos:Concept;
	skos:prefLabel	"retrovirus"@en-GB;
	skos:definition	"A family of RNA viruses such as those causing leukaemia and AIDS "@en-GB;
	skos:historyNote	"typo fixed in Explanation "@en-GB;
	skos:inScheme <http://cv.iptc.org/newscodes/subjectcode/>;
	skos:exactMatch medtop:20000453;
	skos:broader	subj:07001000.

subj:07002000
	rdf:type skos:Concept;
	skos:prefLabel	"epidemic and plague"@en-GB;
	skos:definition	"An epidemic is a rapidly spreading condition in a community and a plague is usually a deadly disease of epidemic proportions "@en-GB;
	skos:inScheme <http://cv.iptc.org/newscodes/subjectcode/>;
	skos:closeMatch medtop:20000449;
	skos:broader	subj:07000000.

subj:07003000
	rdf:type skos:Concept;
	skos:prefLabel	"health treatment"@en-GB;
	skos:definition	"In general treatment of diseases and other conditions to produce wellness "@en-GB;
	skos:inScheme <http://cv.iptc.org/newscodes/subjectcode/>;
	skos:exactMatch medtop:20000464;
	skos:broader	subj:07000000;
	skos:narrower	subj:07003001;
	skos:narrower	subj:07003002;
	skos:narrower	subj:07003003;
	skos:narrower	subj:07003004;
	skos:narrower	subj:07003005.

subj:07003001
	rdf:type skos:Concept;
	skos:prefLabel	"prescription drugs"@en-GB;
	skos:definition	"Drugs that can be purchased only with a doctor's authorization "@en-GB;
	skos:inScheme <http://cv.iptc.org/newscodes/subjectcode/>;
	skos:exactMatch medtop:20000468;
	skos:broader	subj:07003000.

subj:07003002
	rdf:type skos:Concept;
	skos:prefLabel	"dietary supplements"@en-GB;
	skos:definition	"Nutrients taken in addition to food to bolster health "@en-GB;
	skos:inScheme <http://cv.iptc.org/newscodes/subjectcode/>;
	skos:exactMatch medtop:20000466;
	skos:broader	subj:07003000.

subj:07003003
	rdf:type skos:Concept;
	skos:prefLabel	"diet"@en-GB;
	skos:definition	"Controlled food consumption "@en-GB;
	skos:inScheme <http://cv.iptc.org/newscodes/subjectcode/>;
	skos:exactMatch medtop:20000465;
	skos:broader	subj:07003000.

subj:07003004
	rdf:type skos:Concept;
	skos:prefLabel	"medical procedure/test"@en-GB;
	skos:definition	"Any of a variety of treatments such as stress tests, catheterization, blood tests, computerised axial tomography scan or magnetic resonance imaging "@en-GB;
	skos:historyNote	"typo fixed in Explanation "@en-GB;
	skos:inScheme <http://cv.iptc.org/newscodes/subjectcode/>;
	skos:exactMatch medtop:20000469;
	skos:broader	subj:07003000.

subj:07003005
	rdf:type skos:Concept;
	skos:prefLabel	"therapy"@en-GB;
	skos:definition	"Treatment of physical, mental or medical conditions by non-surgical means "@en-GB;
	skos:historyNote	"typo fixed in Explanation "@en-GB;
	skos:inScheme <http://cv.iptc.org/newscodes/subjectcode/>;
	skos:exactMatch medtop:20000478;
	skos:broader	subj:07003000.

subj:07004000
	rdf:type skos:Concept;
	skos:prefLabel	"health organisations"@en-GB;
	skos:definition	"Includes stories about specific health organizations, including professional associations, non-profits and international groups "@en-GB;
	skos:inScheme <http://cv.iptc.org/newscodes/subjectcode/>;
	skos:exactMatch medtop:20000463;
	skos:broader	subj:07000000.

subj:07005000
	rdf:type skos:Concept;
	skos:prefLabel	"medical research"@en-GB;
	skos:definition	"Investigation into the causes and cures of diseases "@en-GB;
	skos:inScheme <http://cv.iptc.org/newscodes/subjectcode/>;
	skos:exactMatch medtop:20000737;
	skos:broader	subj:07000000.

subj:07006000
	rdf:type skos:Concept;
	skos:prefLabel	"medical staff"@en-GB;
	skos:definition	"Doctors, nurses, interns and others in a medical facility "@en-GB;
	skos:inScheme <http://cv.iptc.org/newscodes/subjectcode/>;
	skos:exactMatch medtop:20000492;
	skos:broader	subj:07000000;
	skos:narrower	subj:07006001;
	skos:narrower	subj:07006002.

subj:07006001
	rdf:type skos:Concept;
	skos:prefLabel	"primary care physician"@en-GB;
	skos:definition	"Patient's basic health care doctor - first point of call for all health related problems "@en-GB;
	skos:inScheme <http://cv.iptc.org/newscodes/subjectcode/>;
	skos:broadMatch medtop:20000485;
	skos:broader	subj:07006000.

subj:07006002
	rdf:type skos:Concept;
	skos:prefLabel	"health-workers union"@en-GB;
	skos:definition	"Issues involving industry groups for doctors, nurses, health workers etc. "@en-GB;
	skos:inScheme <http://cv.iptc.org/newscodes/subjectcode/>;
	skos:broadMatch medtop:20000536;
	skos:broader	subj:07006000.

subj:07007000
	rdf:type skos:Concept;
	skos:prefLabel	"medicine"@en-GB;
	skos:definition	"A substance used with the expectation that it will eliminate disease or illness "@en-GB;
	skos:inScheme <http://cv.iptc.org/newscodes/subjectcode/>;
	skos:exactMatch medtop:20000470;
	skos:broader	subj:07000000;
	skos:narrower	subj:07007001;
	skos:narrower	subj:07007002;
	skos:narrower	subj:07007003;
	skos:narrower	subj:07007004.

subj:07007001
	rdf:type skos:Concept;
	skos:prefLabel	"herbal"@en-GB;
	skos:definition	"Treatment based on the use of herbs and other plants to cure or alleviate disease symptoms "@en-GB;
	skos:inScheme <http://cv.iptc.org/newscodes/subjectcode/>;
	skos:exactMatch medtop:20000471;
	skos:broader	subj:07007000.

subj:07007002
	rdf:type skos:Concept;
	skos:prefLabel	"holistic"@en-GB;
	skos:definition	"Treatment of the whole person including mental and social factors rather than just the symptoms of the disease. "@en-GB;
	skos:inScheme <http://cv.iptc.org/newscodes/subjectcode/>;
	skos:exactMatch medtop:20000472;
	skos:broader	subj:07007000.

subj:07007003
	rdf:type skos:Concept;
	skos:prefLabel	"western"@en-GB;
	skos:definition	"The practice of diagnosis, treatment and prevention of disease based on modern scientific research in the western hemisphere. "@en-GB;
	skos:inScheme <http://cv.iptc.org/newscodes/subjectcode/>;
	skos:exactMatch medtop:20000474;
	skos:broader	subj:07007000.

subj:07007004
	rdf:type skos:Concept;
	skos:prefLabel	"traditional Chinese"@en-GB;
	skos:definition	"The practice of diagnosis, treatment and prevention of disease based on traditional methods developed in the orient. "@en-GB;
	skos:inScheme <http://cv.iptc.org/newscodes/subjectcode/>;
	skos:exactMatch medtop:20000473;
	skos:broader	subj:07007000.

subj:07008000
	rdf:type skos:Concept;
	skos:prefLabel	"preventative medicine"@en-GB;
	skos:definition	"Substances used to prevent diseases or illnesses "@en-GB;
	skos:inScheme <http://cv.iptc.org/newscodes/subjectcode/>;
	skos:exactMatch medtop:20000476;
	skos:broader	subj:07000000;
	skos:narrower	subj:07008001.

subj:07008001
	rdf:type skos:Concept;
	skos:prefLabel	"vaccines"@en-GB;
	skos:definition	"Medications designed to create immunity to diseases "@en-GB;
	skos:inScheme <http://cv.iptc.org/newscodes/subjectcode/>;
	skos:exactMatch medtop:20000477;
	skos:broader	subj:07008000.

subj:07009000
	rdf:type skos:Concept;
	skos:prefLabel	"injury"@en-GB;
	skos:definition	"A traumatic condition of the human body caused usually by outside forces "@en-GB;
	skos:inScheme <http://cv.iptc.org/newscodes/subjectcode/>;
	skos:exactMatch medtop:20000456;
	skos:broader	subj:07000000.

subj:07010000
	rdf:type skos:Concept;
	skos:prefLabel	"hospital and clinic"@en-GB;
	skos:definition	"Medical facilities for the treatment of illnesses and injury "@en-GB;
	skos:inScheme <http://cv.iptc.org/newscodes/subjectcode/>;
	skos:exactMatch medtop:20000482;
	skos:broader	subj:07000000.

subj:07011000
	rdf:type skos:Concept;
	skos:prefLabel	"government health care"@en-GB;
	skos:definition	"Health care provided by national governments "@en-GB;
	skos:inScheme <http://cv.iptc.org/newscodes/subjectcode/>;
	skos:exactMatch medtop:20000480;
	skos:broader	subj:07000000;
	skos:narrower	subj:07011001;
	skos:narrower	subj:07011002.

subj:07011001
	rdf:type skos:Concept;
	skos:prefLabel	"medicare"@en-GB;
	skos:definition	"A program of the U.S. government to provide health care to senior citizens "@en-GB;
	skos:inScheme <http://cv.iptc.org/newscodes/subjectcode/>;
	skos:broadMatch medtop:20000480;
	skos:broader	subj:07011000.

subj:07011002
	rdf:type skos:Concept;
	skos:prefLabel	"medicaid"@en-GB;
	skos:definition	"A program of the U.S. government to provide health care to needy citizens of all ages "@en-GB;
	skos:inScheme <http://cv.iptc.org/newscodes/subjectcode/>;
	skos:broadMatch medtop:20000480;
	skos:broader	subj:07011000.

subj:07012000
	rdf:type skos:Concept;
	skos:prefLabel	"private health care"@en-GB;
	skos:definition	"Health care provided by privately funded or insured organizations "@en-GB;
	skos:inScheme <http://cv.iptc.org/newscodes/subjectcode/>;
	skos:exactMatch medtop:20000484;
	skos:broader	subj:07000000.

subj:07013000
	rdf:type skos:Concept;
	skos:prefLabel	"healthcare policy"@en-GB;
	skos:definition	"Health-related policy decisions including what different countries are doing regarding prescription drug policies, AIDS, psychiatric care, health care funding and related topics. "@en-GB;
	skos:inScheme <http://cv.iptc.org/newscodes/subjectcode/>;
	skos:exactMatch medtop:20000479;
	skos:broader	subj:07000000;
	skos:narrower	subj:07013001.

subj:07013001
	rdf:type skos:Concept;
	skos:prefLabel	"food safety"@en-GB;
	skos:definition	"Issues relating to food cleanliness and contamination "@en-GB;
	skos:inScheme <http://cv.iptc.org/newscodes/subjectcode/>;
	skos:closeMatch medtop:20000637;
	skos:broader	subj:07013000.

subj:07014000
	rdf:type skos:Concept;
	skos:prefLabel	"medical specialisation"@en-GB;
	skos:definition	"The different medical specialist areas. "@en-GB;
	skos:inScheme <http://cv.iptc.org/newscodes/subjectcode/>;
	skos:exactMatch medtop:20000487;
	skos:broader	subj:07000000;
	skos:narrower	subj:07014001;
	skos:narrower	subj:07014002;
	skos:narrower	subj:07014003;
	skos:narrower	subj:07014004;
	skos:narrower	subj:07014005.

subj:07014001
	rdf:type skos:Concept;
	skos:prefLabel	"geriatric"@en-GB;
	skos:definition	"Research into aging and age-related issues including age-related illnesses, medical research, trends, geriatric medicine and related topics like age discrimination and health insurance for an ageing population. "@en-GB;
	skos:inScheme <http://cv.iptc.org/newscodes/subjectcode/>;
	skos:exactMatch medtop:20000488;
	skos:broader	subj:07014000.

subj:07014002
	rdf:type skos:Concept;
	skos:prefLabel	"pediatrics"@en-GB;
	skos:definition	"Research and medicine specifically for the young - includes premature babies, infant care, childhood disease and treatment - also teen-related health and behaviour problems. "@en-GB;
	skos:inScheme <http://cv.iptc.org/newscodes/subjectcode/>;
	skos:exactMatch medtop:20000490;
	skos:broader	subj:07014000.

subj:07014003
	rdf:type skos:Concept;
	skos:prefLabel	"reproduction"@en-GB;
	skos:definition	"Reproductive technologies like invitro fertilization and cloning as well as related debates. Sexual development matters and sexually transmitted diseases would also fall under this category. "@en-GB;
	skos:inScheme <http://cv.iptc.org/newscodes/subjectcode/>;
	skos:closeMatch medtop:20000491;
	skos:broader	subj:07014000.

subj:07014004
	rdf:type skos:Concept;
	skos:prefLabel	"genetics"@en-GB;
	skos:definition	"The science and research into genetic-base disease and cures for disease. This would include proteomics (the study of what proteins are produced by which genes and what those proteins do), general genetics and stem-cell research. "@en-GB;
	skos:inScheme <http://cv.iptc.org/newscodes/subjectcode/>;
	skos:exactMatch medtop:20000721;
	skos:broader	subj:07014000.

subj:07014005
	rdf:type skos:Concept;
	skos:prefLabel	"obstetrics/gynecology"@en-GB;
	skos:definition	"Specialty of female reproductive organs "@en-GB;
	skos:inScheme <http://cv.iptc.org/newscodes/subjectcode/>;
	skos:exactMatch medtop:20000489;
	skos:broader	subj:07014000.

subj:07015000
	rdf:type skos:Concept;
	skos:prefLabel	"medical service"@en-GB;
	skos:definition	"Medical support for doctors, including blood tests and other medical tests on individuals, X-rays CAT scans MRIs etc. "@en-GB;
	skos:inScheme <http://cv.iptc.org/newscodes/subjectcode/>;
	skos:exactMatch medtop:20000486;
	skos:broader	subj:07000000.

subj:07016000
	rdf:type skos:Concept;
	skos:prefLabel	"physical fitness"@en-GB;
	skos:definition	"The condition of a person's cardio-vascular and muscular health. "@en-GB;
	skos:inScheme <http://cv.iptc.org/newscodes/subjectcode/>;
	skos:exactMatch medtop:20000475;
	skos:broader	subj:07000000.

subj:07017000
	rdf:type skos:Concept;
	skos:prefLabel	"illness"@en-GB;
	skos:definition	"Non-specific maladies such as stomach aches, headaches, flat feet, lumbago "@en-GB;
	skos:inScheme <http://cv.iptc.org/newscodes/subjectcode/>;
	skos:exactMatch medtop:20000455;
	skos:broader	subj:07000000;
	skos:narrower	subj:07017001;
	skos:narrower	subj:07017002;
	skos:narrower	subj:07017003.

subj:07017001
	rdf:type skos:Concept;
	skos:prefLabel	"mental illness"@en-GB;
	skos:definition	"Those illnesses affecting the mind "@en-GB;
	skos:inScheme <http://cv.iptc.org/newscodes/subjectcode/>;
	skos:closeMatch medtop:20000458;
	skos:broader	subj:07017000.

subj:07017002
	rdf:type skos:Concept;
	skos:prefLabel	"eating disorder"@en-GB;
	skos:definition	"Anorexia, bulimia, overeating and similar illnesses "@en-GB;
	skos:inScheme <http://cv.iptc.org/newscodes/subjectcode/>;
	skos:exactMatch medtop:20000459;
	skos:broader	subj:07017000.

subj:07017003
	rdf:type skos:Concept;
	skos:prefLabel	"obesity"@en-GB;
	skos:definition	"A condition of body weight generally considered 20 percent above the norm for gender, age, height and bone structure "@en-GB;
	skos:inScheme <http://cv.iptc.org/newscodes/subjectcode/>;
	skos:exactMatch medtop:20000460;
	skos:broader	subj:07017000.

subj:07018000
	rdf:type skos:Concept;
	skos:prefLabel	"medical conditions"@en-GB;
	skos:definition	"Various stages of disease, illness or injury "@en-GB;
	skos:inScheme <http://cv.iptc.org/newscodes/subjectcode/>;
	skos:exactMatch medtop:20000457;
	skos:broader	subj:07000000.

subj:07019000
	rdf:type skos:Concept;
	skos:prefLabel	"patient"@en-GB;
	skos:definition	"Issues which affect population in general as attendees at hospitals or doctors' surgeries. "@en-GB;
	skos:inScheme <http://cv.iptc.org/newscodes/subjectcode/>;
	skos:broadMatch medtop:07000000;
	skos:broader	subj:07000000.

subj:08000000
	rdf:type skos:Concept;
	skos:prefLabel	"human interest"@en-GB;
	skos:definition	"Lighter items about individuals, groups, animals or objects. "@en-GB;
	skos:inScheme <http://cv.iptc.org/newscodes/subjectcode/>;
	skos:closeMatch medtop:08000000;
	skos:narrower	subj:08001000;
	skos:narrower	subj:08002000;
	skos:narrower	subj:08003000;
	skos:narrower	subj:08004000;
	skos:narrower	subj:08005000;
	skos:narrower	subj:08006000;
	skos:narrower	subj:08007000;
	skos:narrower	subj:08008000.

subj:08001000
	rdf:type skos:Concept;
	skos:prefLabel	"animal"@en-GB;
	skos:definition	"Animals of all types "@en-GB;
	skos:inScheme <http://cv.iptc.org/newscodes/subjectcode/>;
	skos:closeMatch medtop:20000500;
	skos:broader	subj:08000000.

subj:08002000
	rdf:type skos:Concept;
	skos:prefLabel	"curiosity"@en-GB;
	skos:definition	"Content of an unusual nature that can raise questions or amuse "@en-GB;
	skos:inScheme <http://cv.iptc.org/newscodes/subjectcode/>;
	skos:broadMatch medtop:08000000;
	skos:broader	subj:08000000.

subj:08003000
	rdf:type skos:Concept;
	skos:prefLabel	"people"@en-GB;
	skos:definition	"Unusual content about people of all levels "@en-GB;
	skos:inScheme <http://cv.iptc.org/newscodes/subjectcode/>;
	skos:closeMatch medtop:20000502;
	skos:broader	subj:08000000;
	skos:narrower	subj:08003001;
	skos:narrower	subj:08003002;
	skos:narrower	subj:08003003;
	skos:narrower	subj:08003004;
	skos:narrower	subj:08003005.

subj:08003001
	rdf:type skos:Concept;
	skos:prefLabel	"advice"@en-GB;
	skos:definition	"Letters and answers about personal problems that are publishable "@en-GB;
	skos:inScheme <http://cv.iptc.org/newscodes/subjectcode/>;
	skos:broadMatch medtop:08000000;
	skos:broader	subj:08003000.

subj:08003002
	rdf:type skos:Concept;
	skos:prefLabel	"celebrity"@en-GB;
	skos:definition	"Celebrity news, i.e. Madonna has a baby, Elton John sues his accountants etc. "@en-GB;
	skos:inScheme <http://cv.iptc.org/newscodes/subjectcode/>;
	skos:closeMatch medtop:20000505;
	skos:broader	subj:08003000.

subj:08003003
	rdf:type skos:Concept;
	skos:prefLabel	"accomplishment"@en-GB;
	skos:definition	"Achievements by individuals or groups, such as charitable fundraising, winning a competitive contest etc "@en-GB;
	skos:inScheme <http://cv.iptc.org/newscodes/subjectcode/>;
	skos:closeMatch medtop:20000497;
	skos:broader	subj:08003000.

subj:08003004
	rdf:type skos:Concept;
	skos:prefLabel	"human mishap"@en-GB;
	skos:definition	"Stories arising from silly/stupid human errors e.g. like forgetting to tie one end of a bungee cord "@en-GB;
	skos:inScheme <http://cv.iptc.org/newscodes/subjectcode/>;
	skos:closeMatch medtop:20000503;
	skos:broader	subj:08003000.

subj:08003005
	rdf:type skos:Concept;
	skos:prefLabel	"fortune-telling"@en-GB;
	skos:definition	"The forecasting of future events or the delineation of character by methods not ordinarily considered to have a rational basis "@en-GB;
	skos:inScheme <http://cv.iptc.org/newscodes/subjectcode/>;
	skos:broadMatch medtop:08000000;
	skos:broader	subj:08003000.

subj:08004000
	rdf:type skos:Concept;
	skos:prefLabel	"mystery"@en-GB;
	skos:definition	"Something unexplained or unknown "@en-GB;
	skos:inScheme <http://cv.iptc.org/newscodes/subjectcode/>;
	skos:broadMatch medtop:08000000;
	skos:broader	subj:08000000.

subj:08005000
	rdf:type skos:Concept;
	skos:prefLabel	"society"@en-GB;
	skos:definition	"Stories of well-known people "@en-GB;
	skos:inScheme <http://cv.iptc.org/newscodes/subjectcode/>;
	skos:closeMatch medtop:20000504;
	skos:broader	subj:08000000;
	skos:narrower	subj:08005001;
	skos:narrower	subj:08005002;
	skos:narrower	subj:08005003;
	skos:narrower	subj:08005004;
	skos:narrower	subj:08005005.

subj:08005001
	rdf:type skos:Concept;
	skos:prefLabel	"ceremony"@en-GB;
	skos:definition	"Rituals of a non-religious nature such as dedications, wreath layings, ship launchings etc "@en-GB;
	skos:inScheme <http://cv.iptc.org/newscodes/subjectcode/>;
	skos:exactMatch medtop:20000501;
	skos:broader	subj:08005000.

subj:08005002
	rdf:type skos:Concept;
	skos:prefLabel	"death"@en-GB;
	skos:definition	"The human interest aspects of the demise of a person "@en-GB;
	skos:inScheme <http://cv.iptc.org/newscodes/subjectcode/>;
	skos:broadMatch medtop:08000000;
	skos:broader	subj:08005000.

subj:08005003
	rdf:type skos:Concept;
	skos:prefLabel	"funeral"@en-GB;
	skos:definition	"The ceremony to intern the remains of a person "@en-GB;
	skos:inScheme <http://cv.iptc.org/newscodes/subjectcode/>;
	skos:broadMatch medtop:08000000;
	skos:broader	subj:08005000.

subj:08005004
	rdf:type skos:Concept;
	skos:prefLabel	"estate bestowal"@en-GB;
	skos:definition	"The distribution of the estate of a person according to their will and any disagreements between the heirs "@en-GB;
	skos:inScheme <http://cv.iptc.org/newscodes/subjectcode/>;
	skos:broadMatch medtop:08000000;
	skos:broader	subj:08005000.

subj:08005005
	rdf:type skos:Concept;
	skos:prefLabel	"memorial"@en-GB;
	skos:definition	"Commemorative ceremony or object - plaque, statue etc - in remembrance of a person. "@en-GB;
	skos:inScheme <http://cv.iptc.org/newscodes/subjectcode/>;
	skos:broadMatch medtop:08000000;
	skos:broader	subj:08005000.

subj:08006000
	rdf:type skos:Concept;
	skos:prefLabel	"award and prize"@en-GB;
	skos:definition	"Decorations, awards and prizes, including those given by the government. "@en-GB;
	skos:inScheme <http://cv.iptc.org/newscodes/subjectcode/>;
	skos:exactMatch medtop:20000498;
	skos:broader	subj:08000000;
	skos:narrower	subj:08006001.

subj:08006001
	rdf:type skos:Concept;
	skos:prefLabel	"record"@en-GB;
	skos:definition	"Non-sport achievement by an individual or group that sets a new record, such as most books read, holding your breath longest "@en-GB;
	skos:inScheme <http://cv.iptc.org/newscodes/subjectcode/>;
	skos:exactMatch medtop:20000499;
	skos:broader	subj:08006000.

subj:08007000
	rdf:type skos:Concept;
	skos:prefLabel	"imperial and royal matters"@en-GB;
	skos:definition	"Imperial and royal family members, including matters on legal systems. "@en-GB;
	skos:inScheme <http://cv.iptc.org/newscodes/subjectcode/>;
	skos:exactMatch medtop:20000506;
	skos:broader	subj:08000000.

subj:08008000
	rdf:type skos:Concept;
	skos:prefLabel	"plant"@en-GB;
	skos:definition	"An organism of the kind exemplified by trees, shrubs, grasses, ferns, and mosses, typically growing in a permanent site "@en-GB;
	skos:inScheme <http://cv.iptc.org/newscodes/subjectcode/>;
	skos:closeMatch medtop:20000507;
	skos:broader	subj:08000000.

subj:09000000
	rdf:type skos:Concept;
	skos:prefLabel	"labour"@en-GB;
	skos:definition	"Social aspects, organizations, rules and conditions affecting the employment of human effort for the generation of wealth or provision of services and the economic support of the unemployed. "@en-GB;
	skos:inScheme <http://cv.iptc.org/newscodes/subjectcode/>;
	skos:exactMatch medtop:09000000;
	skos:narrower	subj:09001000;
	skos:narrower	subj:09002000;
	skos:narrower	subj:09003000;
	skos:narrower	subj:09004000;
	skos:narrower	subj:09005000;
	skos:narrower	subj:09006000;
	skos:narrower	subj:09007000;
	skos:narrower	subj:09008000;
	skos:narrower	subj:09009000;
	skos:narrower	subj:09010000;
	skos:narrower	subj:09011000;
	skos:narrower	subj:09012000;
	skos:narrower	subj:09013000;
	skos:narrower	subj:09014000;
	skos:narrower	subj:09015000;
	skos:narrower	subj:09016000.

subj:09001000
	rdf:type skos:Concept;
	skos:prefLabel	"apprentices"@en-GB;
	skos:definition	"People who are in the work force at a learning level, serving under a master "@en-GB;
	skos:inScheme <http://cv.iptc.org/newscodes/subjectcode/>;
	skos:exactMatch medtop:20000510;
	skos:broader	subj:09000000.

subj:09002000
	rdf:type skos:Concept;
	skos:prefLabel	"collective contract"@en-GB;
	skos:definition	"Usually written contracts covering a specific class of worker "@en-GB;
	skos:inScheme <http://cv.iptc.org/newscodes/subjectcode/>;
	skos:exactMatch medtop:20000525;
	skos:broader	subj:09000000;
	skos:narrower	subj:09002001;
	skos:narrower	subj:09002002;
	skos:narrower	subj:09002003.

subj:09002001
	rdf:type skos:Concept;
	skos:prefLabel	"contract issue-wages"@en-GB;
	skos:definition	"Element of contracts and contract discussions centring on remuneration "@en-GB;
	skos:inScheme <http://cv.iptc.org/newscodes/subjectcode/>;
	skos:exactMatch medtop:20000527;
	skos:broader	subj:09002000.

subj:09002002
	rdf:type skos:Concept;
	skos:prefLabel	"contract issue-healthcare"@en-GB;
	skos:definition	"Element of contracts and contract discussions centring on health care issues "@en-GB;
	skos:inScheme <http://cv.iptc.org/newscodes/subjectcode/>;
	skos:exactMatch medtop:20000526;
	skos:broader	subj:09002000.

subj:09002003
	rdf:type skos:Concept;
	skos:prefLabel	"contract issue-work rules"@en-GB;
	skos:definition	"Element of contracts and contract discussions centring on rules affecting issues such as lunch and other breaks, work shifts, vacation scheduling, seniority, sick leave etc. "@en-GB;
	skos:inScheme <http://cv.iptc.org/newscodes/subjectcode/>;
	skos:exactMatch medtop:20000528;
	skos:broader	subj:09002000.

subj:09003000
	rdf:type skos:Concept;
	skos:prefLabel	"employment"@en-GB;
	skos:definition	"Paid labour "@en-GB;
	skos:inScheme <http://cv.iptc.org/newscodes/subjectcode/>;
	skos:closeMatch medtop:20000509;
	skos:broader	subj:09000000;
	skos:narrower	subj:09003001;
	skos:narrower	subj:09003002;
	skos:narrower	subj:09003003;
	skos:narrower	subj:09003004.

subj:09003001
	rdf:type skos:Concept;
	skos:prefLabel	"labor market"@en-GB;
	skos:definition	"A pool of people who are working or are seeking work "@en-GB;
	skos:inScheme <http://cv.iptc.org/newscodes/subjectcode/>;
	skos:exactMatch medtop:20000523;
	skos:broader	subj:09003000.

subj:09003002
	rdf:type skos:Concept;
	skos:prefLabel	"job layoffs"@en-GB;
	skos:definition	"The reduction of a company's work force through dismissal because of changing economic factors "@en-GB;
	skos:inScheme <http://cv.iptc.org/newscodes/subjectcode/>;
	skos:exactMatch medtop:20000534;
	skos:broader	subj:09003000.

subj:09003003
	rdf:type skos:Concept;
	skos:prefLabel	"child labor"@en-GB;
	skos:definition	"Employment of children, usually under the age of 18 "@en-GB;
	skos:inScheme <http://cv.iptc.org/newscodes/subjectcode/>;
	skos:exactMatch medtop:20000511;
	skos:broader	subj:09003000.

subj:09003004
	rdf:type skos:Concept;
	skos:prefLabel	"occupations"@en-GB;
	skos:definition	"Generally one's trade, profession or business although professions are usually such things as lawyers and doctors, and occupations are such as clerks or truckers "@en-GB;
	skos:inScheme <http://cv.iptc.org/newscodes/subjectcode/>;
	skos:exactMatch medtop:20000517;
	skos:broader	subj:09003000.

subj:09004000
	rdf:type skos:Concept;
	skos:prefLabel	"labour dispute"@en-GB;
	skos:definition	"Differences of opinion about work conditions, pay, etc "@en-GB;
	skos:inScheme <http://cv.iptc.org/newscodes/subjectcode/>;
	skos:exactMatch medtop:20000529;
	skos:broader	subj:09000000.

subj:09005000
	rdf:type skos:Concept;
	skos:prefLabel	"labour legislation"@en-GB;
	skos:definition	"Laws governing work and labour "@en-GB;
	skos:inScheme <http://cv.iptc.org/newscodes/subjectcode/>;
	skos:closeMatch medtop:20000521;
	skos:broader	subj:09000000.

subj:09006000
	rdf:type skos:Concept;
	skos:prefLabel	"retirement"@en-GB;
	skos:definition	"The years after work "@en-GB;
	skos:inScheme <http://cv.iptc.org/newscodes/subjectcode/>;
	skos:exactMatch medtop:20000531;
	skos:broader	subj:09000000.

subj:09007000
	rdf:type skos:Concept;
	skos:prefLabel	"retraining"@en-GB;
	skos:definition	"Providing a worker training in new skills when his old skills are no longer applicable "@en-GB;
	skos:inScheme <http://cv.iptc.org/newscodes/subjectcode/>;
	skos:exactMatch medtop:20000516;
	skos:broader	subj:09000000.

subj:09008000
	rdf:type skos:Concept;
	skos:prefLabel	"strike"@en-GB;
	skos:definition	"A job action involving cessation of work "@en-GB;
	skos:inScheme <http://cv.iptc.org/newscodes/subjectcode/>;
	skos:exactMatch medtop:20000530;
	skos:broader	subj:09000000.

subj:09009000
	rdf:type skos:Concept;
	skos:prefLabel	"unemployment"@en-GB;
	skos:definition	"Lack of paid work "@en-GB;
	skos:inScheme <http://cv.iptc.org/newscodes/subjectcode/>;
	skos:closeMatch medtop:20000533;
	skos:broader	subj:09000000.

subj:09010000
	rdf:type skos:Concept;
	skos:prefLabel	"unions"@en-GB;
	skos:definition	"Groups established to represent bodies of workers "@en-GB;
	skos:inScheme <http://cv.iptc.org/newscodes/subjectcode/>;
	skos:exactMatch medtop:20000536;
	skos:broader	subj:09000000.

subj:09011000
	rdf:type skos:Concept;
	skos:prefLabel	"wage and pension"@en-GB;
	skos:definition	"Parts of a salary divided for current income and future income "@en-GB;
	skos:inScheme <http://cv.iptc.org/newscodes/subjectcode/>;
	skos:closeMatch medtop:20000518;
	skos:broader	subj:09000000;
	skos:narrower	subj:09011001;
	skos:narrower	subj:09011002.

subj:09011001
	rdf:type skos:Concept;
	skos:prefLabel	"employee benefits"@en-GB;
	skos:definition	"Either benefits provided to an employee by a company, such as pensions, health insurance; or monetary compensation paid by a government to the jobless usually called unemployment benefits "@en-GB;
	skos:inScheme <http://cv.iptc.org/newscodes/subjectcode/>;
	skos:closeMatch medtop:20000519;
	skos:broader	subj:09011000.

subj:09011002
	rdf:type skos:Concept;
	skos:prefLabel	"social security"@en-GB;
	skos:definition	"FICA. Money paid by individual and companies into a government account to be paid out when that individual reaches a certain age "@en-GB;
	skos:inScheme <http://cv.iptc.org/newscodes/subjectcode/>;
	skos:exactMatch medtop:20000520;
	skos:broader	subj:09011000.

subj:09012000
	rdf:type skos:Concept;
	skos:prefLabel	"work relations"@en-GB;
	skos:definition	"The give and take between management and labour "@en-GB;
	skos:inScheme <http://cv.iptc.org/newscodes/subjectcode/>;
	skos:closeMatch medtop:20000524;
	skos:broader	subj:09000000.

subj:09013000
	rdf:type skos:Concept;
	skos:prefLabel	"health and safety at work"@en-GB;
	skos:definition	"Rules and procedures for guaranteeing the health of workers "@en-GB;
	skos:inScheme <http://cv.iptc.org/newscodes/subjectcode/>;
	skos:exactMatch medtop:20000522;
	skos:broader	subj:09000000.

subj:09014000
	rdf:type skos:Concept;
	skos:prefLabel	"advanced training"@en-GB;
	skos:definition	"Additional training to enhance current skills "@en-GB;
	skos:inScheme <http://cv.iptc.org/newscodes/subjectcode/>;
	skos:exactMatch medtop:20000515;
	skos:broader	subj:09000000.

subj:09015000
	rdf:type skos:Concept;
	skos:prefLabel	"employer"@en-GB;
	skos:definition	"The person who employs workers and pays the salaries and other benefits to workers "@en-GB;
	skos:inScheme <http://cv.iptc.org/newscodes/subjectcode/>;
	skos:exactMatch medtop:20000513;
	skos:broader	subj:09000000.

subj:09016000
	rdf:type skos:Concept;
	skos:prefLabel	"employee"@en-GB;
	skos:definition	"A person who trades his time and talent for money and other benefits "@en-GB;
	skos:inScheme <http://cv.iptc.org/newscodes/subjectcode/>;
	skos:exactMatch medtop:20000512;
	skos:broader	subj:09000000.

subj:10000000
	rdf:type skos:Concept;
	skos:prefLabel	"lifestyle and leisure"@en-GB;
	skos:definition	"Activities undertaken for pleasure, relaxation or recreation outside paid employment, including eating and travel. "@en-GB;
	skos:inScheme <http://cv.iptc.org/newscodes/subjectcode/>;
	skos:exactMatch medtop:10000000;
	skos:narrower	subj:10001000;
	skos:narrower	subj:10002000;
	skos:narrower	subj:10003000;
	skos:narrower	subj:10004000;
	skos:narrower	subj:10005000;
	skos:narrower	subj:10006000;
	skos:narrower	subj:10007000;
	skos:narrower	subj:10008000;
	skos:narrower	subj:10009000;
	skos:narrower	subj:10010000;
	skos:narrower	subj:10011000;
	skos:narrower	subj:10012000;
	skos:narrower	subj:10013000;
	skos:narrower	subj:10014000;
	skos:narrower	subj:10015000;
	skos:narrower	subj:10016000;
	skos:narrower	subj:10017000;
	skos:narrower	subj:10018000.

subj:10001000
	rdf:type skos:Concept;
	skos:prefLabel	"game"@en-GB;
	skos:definition	"Contests generally for ones amusement "@en-GB;
	skos:inScheme <http://cv.iptc.org/newscodes/subjectcode/>;
	skos:exactMatch medtop:20000540;
	skos:broader	subj:10000000;
	skos:narrower	subj:10001001;
	skos:narrower	subj:10001002;
	skos:narrower	subj:10001003;
	skos:narrower	subj:10001004.

subj:10001001
	rdf:type skos:Concept;
	skos:prefLabel	"Go"@en-GB;
	skos:definition	"A strategic, deterministic Chinese board game played by alternately placing stones on a grid "@en-GB;
	skos:historyNote	"Explanation changed in V17 "@en-GB;
	skos:inScheme <http://cv.iptc.org/newscodes/subjectcode/>;
	skos:broadMatch medtop:20000547;
	skos:broader	subj:10001000.

subj:10001002
	rdf:type skos:Concept;
	skos:prefLabel	"chess"@en-GB;
	skos:definition	"A game played on a chequered board with 16 pieces to each side with specific ranges of movement depending on their identity "@en-GB;
	skos:historyNote	"typo fixed in Explanation "@en-GB;
	skos:inScheme <http://cv.iptc.org/newscodes/subjectcode/>;
	skos:broadMatch medtop:20000541;
	skos:broader	subj:10001000.

subj:10001003
	rdf:type skos:Concept;
	skos:prefLabel	"bridge"@en-GB;
	skos:definition	"A card game of four players who bet on the hands of each other, developed from Russian whist "@en-GB;
	skos:inScheme <http://cv.iptc.org/newscodes/subjectcode/>;
	skos:broadMatch medtop:20000542;
	skos:broader	subj:10001000.

subj:10001004
	rdf:type skos:Concept;
	skos:prefLabel	"shogi"@en-GB;
	skos:definition	"A strategic board games which is native to Japan and is often called Japanese chess "@en-GB;
	skos:inScheme <http://cv.iptc.org/newscodes/subjectcode/>;
	skos:broadMatch medtop:20000541;
	skos:broader	subj:10001000.

subj:10002000
	rdf:type skos:Concept;
	skos:prefLabel	"gaming and lottery"@en-GB;
	skos:definition	"Gambling, often involving selection of sets of numbers one expects to come up "@en-GB;
	skos:inScheme <http://cv.iptc.org/newscodes/subjectcode/>;
	skos:exactMatch medtop:20000549;
	skos:broader	subj:10000000.

subj:10003000
	rdf:type skos:Concept;
	skos:prefLabel	"gastronomy"@en-GB;
	skos:definition	"The art of good eating "@en-GB;
	skos:inScheme <http://cv.iptc.org/newscodes/subjectcode/>;
	skos:closeMatch medtop:20000568;
	skos:broader	subj:10000000;
	skos:narrower	subj:10003001.

subj:10003001
	rdf:type skos:Concept;
	skos:prefLabel	"organic foods"@en-GB;
	skos:definition	"Food which is grown using no artificial fertilizers or chemical compounds "@en-GB;
	skos:inScheme <http://cv.iptc.org/newscodes/subjectcode/>;
	skos:exactMatch medtop:20000569;
	skos:broader	subj:10003000.

subj:10004000
	rdf:type skos:Concept;
	skos:prefLabel	"hobby"@en-GB;
	skos:definition	"Various types of activities for amusement, such as collecting stamps, building models, quilting, crafts "@en-GB;
	skos:inScheme <http://cv.iptc.org/newscodes/subjectcode/>;
	skos:exactMatch medtop:20000550;
	skos:broader	subj:10000000;
	skos:narrower	subj:10004001;
	skos:narrower	subj:10004002;
	skos:narrower	subj:10004003.

subj:10004001
	rdf:type skos:Concept;
	skos:prefLabel	"DIY"@en-GB;
	skos:definition	"DIY - do it yourself. Normally the construction, repair or maintenance of residential property by an amateur "@en-GB;
	skos:inScheme <http://cv.iptc.org/newscodes/subjectcode/>;
	skos:broadMatch medtop:20000570;
	skos:broader	subj:10004000.

subj:10004002
	rdf:type skos:Concept;
	skos:prefLabel	"shopping"@en-GB;
	skos:definition	"Consumer purchasing and related trends, but not the business aspects of retailing "@en-GB;
	skos:inScheme <http://cv.iptc.org/newscodes/subjectcode/>;
	skos:broadMatch medtop:10000000;
	skos:broader	subj:10004000.

subj:10004003
	rdf:type skos:Concept;
	skos:prefLabel	"gardening"@en-GB;
	skos:definition	"The non-commercial aspects of landscaping, growing plants, trees and other vegetation that gives pleasure to the gardener and others "@en-GB;
	skos:inScheme <http://cv.iptc.org/newscodes/subjectcode/>;
	skos:broadMatch medtop:20000550;
	skos:broader	subj:10004000.

subj:10005000
	rdf:type skos:Concept;
	skos:prefLabel	"holiday or vacation"@en-GB;
	skos:definition	"Leisure travel to a single location and/or country over a short period of time "@en-GB;
	skos:inScheme <http://cv.iptc.org/newscodes/subjectcode/>;
	skos:closeMatch medtop:20000551;
	skos:broader	subj:10000000.

subj:10006000
	rdf:type skos:Concept;
	skos:prefLabel	"tourism"@en-GB;
	skos:definition	"Leisure travel involving visits to a number of locations and/or countries over an extended period of time, often as part of an organized group "@en-GB;
	skos:inScheme <http://cv.iptc.org/newscodes/subjectcode/>;
	skos:closeMatch medtop:20000564;
	skos:broader	subj:10000000.

subj:10007000
	rdf:type skos:Concept;
	skos:prefLabel	"travel and commuting"@en-GB;
	skos:definition	"Transport options, travel networks, commuting, car pooling and business travel "@en-GB;
	skos:inScheme <http://cv.iptc.org/newscodes/subjectcode/>;
	skos:closeMatch medtop:20000339;
	skos:broader	subj:10000000;
	skos:narrower	subj:10007001.

subj:10007001
	rdf:type skos:Concept;
	skos:prefLabel	"traffic"@en-GB;
	skos:definition	"Traffic reports and/or warnings "@en-GB;
	skos:inScheme <http://cv.iptc.org/newscodes/subjectcode/>;
	skos:exactMatch medtop:20000342;
	skos:broader	subj:10007000.

subj:10008000
	rdf:type skos:Concept;
	skos:prefLabel	"club and association"@en-GB;
	skos:definition	"Organizations joined by individuals because of similar interests "@en-GB;
	skos:inScheme <http://cv.iptc.org/newscodes/subjectcode/>;
	skos:exactMatch medtop:20000539;
	skos:broader	subj:10000000.

subj:10009000
	rdf:type skos:Concept;
	skos:prefLabel	"lifestyle (house and home)"@en-GB;
	skos:definition	"Unique culture of ones own home "@en-GB;
	skos:inScheme <http://cv.iptc.org/newscodes/subjectcode/>;
	skos:closeMatch medtop:20000570;
	skos:broader	subj:10000000.

subj:10010000
	rdf:type skos:Concept;
	skos:prefLabel	"leisure (general)"@en-GB;
	skos:definition	"Activities carried out in ones' spare time "@en-GB;
	skos:inScheme <http://cv.iptc.org/newscodes/subjectcode/>;
	skos:closeMatch medtop:20000538;
	skos:broader	subj:10000000.

subj:10011000
	rdf:type skos:Concept;
	skos:prefLabel	"public holiday"@en-GB;
	skos:definition	"A day or days set off for celebration "@en-GB;
	skos:inScheme <http://cv.iptc.org/newscodes/subjectcode/>;
	skos:closeMatch medtop:20000552;
	skos:broader	subj:10000000.

subj:10012000
	rdf:type skos:Concept;
	skos:prefLabel	"hunting"@en-GB;
	skos:definition	"An activity involving the use of weapons or traps for the capturing of animals "@en-GB;
	skos:inScheme <http://cv.iptc.org/newscodes/subjectcode/>;
	skos:exactMatch medtop:20000562;
	skos:broader	subj:10000000.

subj:10013000
	rdf:type skos:Concept;
	skos:prefLabel	"fishing"@en-GB;
	skos:definition	"An activity involving the use of baits, lures, weapons and traps for the capture of aquatic species "@en-GB;
	skos:inScheme <http://cv.iptc.org/newscodes/subjectcode/>;
	skos:exactMatch medtop:20000561;
	skos:broader	subj:10000000.

subj:10014000
	rdf:type skos:Concept;
	skos:prefLabel	"auto trends"@en-GB;
	skos:definition	"The evolution of the automobile "@en-GB;
	skos:inScheme <http://cv.iptc.org/newscodes/subjectcode/>;
	skos:closeMatch medtop:20000566;
	skos:broader	subj:10000000.

subj:10015000
	rdf:type skos:Concept;
	skos:prefLabel	"adventure"@en-GB;
	skos:definition	"Expeditions, daring feats, exploration, record-breaking, risk-associated events "@en-GB;
	skos:inScheme <http://cv.iptc.org/newscodes/subjectcode/>;
	skos:broadMatch medtop:10000000;
	skos:broader	subj:10000000.

subj:10016000
	rdf:type skos:Concept;
	skos:prefLabel	"beauty"@en-GB;
	skos:definition	"Issues relating to improving one's appearance and attractiveness, including reviews of beauty products "@en-GB;
	skos:inScheme <http://cv.iptc.org/newscodes/subjectcode/>;
	skos:closeMatch medtop:20000220;
	skos:broader	subj:10000000.

subj:10017000
	rdf:type skos:Concept;
	skos:prefLabel	"consumer issue"@en-GB;
	skos:definition	"Shopping, products for the home, relevant surveys, product recalls "@en-GB;
	skos:inScheme <http://cv.iptc.org/newscodes/subjectcode/>;
	skos:closeMatch medtop:20000353;
	skos:broader	subj:10000000.

subj:10018000
	rdf:type skos:Concept;
	skos:prefLabel	"wedding"@en-GB;
	skos:definition	"The marriage ceremony and the events that surround it - showers, rehearsal, parties, honeymoon, etc. "@en-GB;
	skos:inScheme <http://cv.iptc.org/newscodes/subjectcode/>;
	skos:closeMatch medtop:20000293;
	skos:broader	subj:10000000.

subj:11000000
	rdf:type skos:Concept;
	skos:prefLabel	"politics"@en-GB;
	skos:definition	"Local, regional, national and international exercise of power, or struggle for power, and the relationships between governing bodies and states. "@en-GB;
	skos:inScheme <http://cv.iptc.org/newscodes/subjectcode/>;
	skos:exactMatch medtop:11000000;
	skos:narrower	subj:11001000;
	skos:narrower	subj:11002000;
	skos:narrower	subj:11003000;
	skos:narrower	subj:11004000;
	skos:narrower	subj:11005000;
	skos:narrower	subj:11006000;
	skos:narrower	subj:11007000;
	skos:narrower	subj:11008000;
	skos:narrower	subj:11009000;
	skos:narrower	subj:11010000;
	skos:narrower	subj:11011000;
	skos:narrower	subj:11012000;
	skos:narrower	subj:11013000;
	skos:narrower	subj:11014000;
	skos:narrower	subj:11015000;
	skos:narrower	subj:11016000;
	skos:narrower	subj:11017000;
	skos:narrower	subj:11018000;
	skos:narrower	subj:11019000;
	skos:narrower	subj:11020000;
	skos:narrower	subj:11021000;
	skos:narrower	subj:11022000;
	skos:narrower	subj:11023000;
	skos:narrower	subj:11024000;
	skos:narrower	subj:11025000;
	skos:narrower	subj:11026000;
	skos:narrower	subj:11027000;
	skos:narrower	subj:11028000.

subj:11001000
	rdf:type skos:Concept;
	skos:prefLabel	"defence"@en-GB;
	skos:definition	"Anything involving the defence of one's own country "@en-GB;
	skos:inScheme <http://cv.iptc.org/newscodes/subjectcode/>;
	skos:exactMatch medtop:20000598;
	skos:broader	subj:11000000;
	skos:narrower	subj:11001001;
	skos:narrower	subj:11001002;
	skos:narrower	subj:11001003;
	skos:narrower	subj:11001004;
	skos:narrower	subj:11001005;
	skos:narrower	subj:11001006;
	skos:narrower	subj:11001007;
	skos:narrower	subj:11001008;
	skos:narrower	subj:11001009.

subj:11001001
	rdf:type skos:Concept;
	skos:prefLabel	"veterans affairs"@en-GB;
	skos:definition	"Care and provision for those who served in the military "@en-GB;
	skos:inScheme <http://cv.iptc.org/newscodes/subjectcode/>;
	skos:exactMatch medtop:20000600;
	skos:broader	subj:11001000.

subj:11001002
	rdf:type skos:Concept;
	skos:prefLabel	"national security"@en-GB;
	skos:definition	"The philosophy of securing a nation and its borders, as well as the well being of its citizens "@en-GB;
	skos:inScheme <http://cv.iptc.org/newscodes/subjectcode/>;
	skos:exactMatch medtop:20000604;
	skos:broader	subj:11001000.

subj:11001003
	rdf:type skos:Concept;
	skos:prefLabel	"security measures"@en-GB;
	skos:definition	"Means of making a nation, a state, a building or a person secure from harm and outside interference. "@en-GB;
	skos:inScheme <http://cv.iptc.org/newscodes/subjectcode/>;
	skos:exactMatch medtop:20000603;
	skos:broader	subj:11001000.

subj:11001004
	rdf:type skos:Concept;
	skos:prefLabel	"armed Forces"@en-GB;
	skos:definition	"Those employed by a government to conduct war, or to enforce the security of a nation "@en-GB;
	skos:inScheme <http://cv.iptc.org/newscodes/subjectcode/>;
	skos:exactMatch medtop:20000599;
	skos:broader	subj:11001000.

subj:11001005
	rdf:type skos:Concept;
	skos:prefLabel	"military equipment"@en-GB;
	skos:definition	"Equipment issued to members of the armed forces "@en-GB;
	skos:inScheme <http://cv.iptc.org/newscodes/subjectcode/>;
	skos:exactMatch medtop:20000601;
	skos:broader	subj:11001000.

subj:11001006
	rdf:type skos:Concept;
	skos:prefLabel	"firearms"@en-GB;
	skos:definition	"Anything that uses an explosive in a directed manner to propel an object that can maim or kill "@en-GB;
	skos:inScheme <http://cv.iptc.org/newscodes/subjectcode/>;
	skos:broadMatch medtop:20000602;
	skos:broader	subj:11001000.

subj:11001007
	rdf:type skos:Concept;
	skos:prefLabel	"biological and chemical weapons"@en-GB;
	skos:definition	"Devices using biological agents, or chemical mixtures to disable, maim or kill an opponent "@en-GB;
	skos:inScheme <http://cv.iptc.org/newscodes/subjectcode/>;
	skos:broadMatch medtop:20000602;
	skos:broader	subj:11001000.

subj:11001008
	rdf:type skos:Concept;
	skos:prefLabel	"missile systems"@en-GB;
	skos:definition	"Anything that propels an inert, explosive, biological or chemical object through the air with the aim of disabling, maiming or killing an opponent. "@en-GB;
	skos:inScheme <http://cv.iptc.org/newscodes/subjectcode/>;
	skos:broadMatch medtop:20000602;
	skos:broader	subj:11001000.

subj:11001009
	rdf:type skos:Concept;
	skos:prefLabel	"nuclear weapons"@en-GB;
	skos:definition	"Weapons that use controlled radioactivity from the decay of certain elements to disable, maim or kill an opponent "@en-GB;
	skos:inScheme <http://cv.iptc.org/newscodes/subjectcode/>;
	skos:broadMatch medtop:20000602;
	skos:broader	subj:11001000.

subj:11002000
	rdf:type skos:Concept;
	skos:prefLabel	"diplomacy"@en-GB;
	skos:definition	"The use of verbal and written skills for persuading others to your point of view "@en-GB;
	skos:inScheme <http://cv.iptc.org/newscodes/subjectcode/>;
	skos:exactMatch medtop:20000639;
	skos:broader	subj:11000000;
	skos:narrower	subj:11002001;
	skos:narrower	subj:11002002;
	skos:narrower	subj:11002003;
	skos:narrower	subj:11002004.

subj:11002001
	rdf:type skos:Concept;
	skos:prefLabel	"summit"@en-GB;
	skos:definition	"Includes meetings of leaders, foreign and finance ministers from the Group of Eight major nations and Group of Seven industrialized nations. "@en-GB;
	skos:inScheme <http://cv.iptc.org/newscodes/subjectcode/>;
	skos:exactMatch medtop:20000640;
	skos:broader	subj:11002000.

subj:11002002
	rdf:type skos:Concept;
	skos:prefLabel	"international relations"@en-GB;
	skos:definition	"Non-violent relations between nations through negotiation, treaty, or personal meetings "@en-GB;
	skos:historyNote	"FormalName error fixed "@en-GB;
	skos:inScheme <http://cv.iptc.org/newscodes/subjectcode/>;
	skos:exactMatch medtop:20000638;
	skos:broader	subj:11002000.

subj:11002003
	rdf:type skos:Concept;
	skos:prefLabel	"peace negotiations"@en-GB;
	skos:definition	"Negotiations intended to bring an end to a conflict "@en-GB;
	skos:historyNote	"FormalName error fixed "@en-GB;
	skos:inScheme <http://cv.iptc.org/newscodes/subjectcode/>;
	skos:closeMatch medtop:20000073;
	skos:broader	subj:11002000.

subj:11002004
	rdf:type skos:Concept;
	skos:prefLabel	"alliances"@en-GB;
	skos:definition	"Coalitions of like-minded groups formed to present a stronger force against any challenges "@en-GB;
	skos:historyNote	"FormalName error fixed "@en-GB;
	skos:inScheme <http://cv.iptc.org/newscodes/subjectcode/>;
	skos:broadMatch medtop:20000639;
	skos:broader	subj:11002000.

subj:11003000
	rdf:type skos:Concept;
	skos:prefLabel	"election"@en-GB;
	skos:definition	"The selection of representatives by the casting of votes "@en-GB;
	skos:inScheme <http://cv.iptc.org/newscodes/subjectcode/>;
	skos:exactMatch medtop:20000574;
	skos:broader	subj:11000000;
	skos:narrower	subj:11003001;
	skos:narrower	subj:11003002;
	skos:narrower	subj:11003003;
	skos:narrower	subj:11003004;
	skos:narrower	subj:11003005;
	skos:narrower	subj:11003006;
	skos:narrower	subj:11003007;
	skos:narrower	subj:11003008;
	skos:narrower	subj:11003009;
	skos:narrower	subj:11003010.

subj:11003001
	rdf:type skos:Concept;
	skos:prefLabel	"political candidates"@en-GB;
	skos:definition	"Individuals who are chosen to stand for office "@en-GB;
	skos:inScheme <http://cv.iptc.org/newscodes/subjectcode/>;
	skos:exactMatch medtop:20000582;
	skos:broader	subj:11003000.

subj:11003002
	rdf:type skos:Concept;
	skos:prefLabel	"political campaigns"@en-GB;
	skos:definition	"Campaigns for public office "@en-GB;
	skos:inScheme <http://cv.iptc.org/newscodes/subjectcode/>;
	skos:exactMatch medtop:20000580;
	skos:broader	subj:11003000.

subj:11003003
	rdf:type skos:Concept;
	skos:prefLabel	"campaign finance"@en-GB;
	skos:definition	"The money that makes campaigns for public office possible "@en-GB;
	skos:inScheme <http://cv.iptc.org/newscodes/subjectcode/>;
	skos:exactMatch medtop:20000581;
	skos:broader	subj:11003000.

subj:11003004
	rdf:type skos:Concept;
	skos:prefLabel	"national elections"@en-GB;
	skos:definition	"Choosing individuals for government at a national level "@en-GB;
	skos:inScheme <http://cv.iptc.org/newscodes/subjectcode/>;
	skos:exactMatch medtop:20000579;
	skos:broader	subj:11003000.

subj:11003005
	rdf:type skos:Concept;
	skos:prefLabel	"regional elections"@en-GB;
	skos:definition	"Choosing individuals for government at a regional level "@en-GB;
	skos:inScheme <http://cv.iptc.org/newscodes/subjectcode/>;
	skos:exactMatch medtop:20000585;
	skos:broader	subj:11003000.

subj:11003006
	rdf:type skos:Concept;
	skos:prefLabel	"local elections"@en-GB;
	skos:definition	"Choosing individuals for government at the basic level, whether city, village or county "@en-GB;
	skos:inScheme <http://cv.iptc.org/newscodes/subjectcode/>;
	skos:exactMatch medtop:20000578;
	skos:broader	subj:11003000.

subj:11003007
	rdf:type skos:Concept;
	skos:prefLabel	"voting"@en-GB;
	skos:definition	"The act of selecting an individual you would like to represent your interests in government "@en-GB;
	skos:inScheme <http://cv.iptc.org/newscodes/subjectcode/>;
	skos:exactMatch medtop:20000586;
	skos:broader	subj:11003000.

subj:11003008
	rdf:type skos:Concept;
	skos:prefLabel	"poll"@en-GB;
	skos:definition	"Periodic measurement of a political candidate's standing with the public "@en-GB;
	skos:inScheme <http://cv.iptc.org/newscodes/subjectcode/>;
	skos:broadMatch medtop:20000574;
	skos:broader	subj:11003000.

subj:11003009
	rdf:type skos:Concept;
	skos:prefLabel	"european elections"@en-GB;
	skos:definition	"Choosing individuals for a body which is at a higher level than national government, e.g. European parliament "@en-GB;
	skos:inScheme <http://cv.iptc.org/newscodes/subjectcode/>;
	skos:closeMatch medtop:20000577;
	skos:broader	subj:11003000.

subj:11003010
	rdf:type skos:Concept;
	skos:prefLabel	"primary"@en-GB;
	skos:definition	"Preliminary elections on a local or regional basis leading up to a regional or national election "@en-GB;
	skos:inScheme <http://cv.iptc.org/newscodes/subjectcode/>;
	skos:exactMatch medtop:20000583;
	skos:broader	subj:11003000.

subj:11004000
	rdf:type skos:Concept;
	skos:prefLabel	"espionage and intelligence"@en-GB;
	skos:definition	"Covert collection of information "@en-GB;
	skos:inScheme <http://cv.iptc.org/newscodes/subjectcode/>;
	skos:exactMatch medtop:20000605;
	skos:broader	subj:11000000.

subj:11005000
	rdf:type skos:Concept;
	skos:prefLabel	"foreign aid"@en-GB;
	skos:definition	"Help provided by one nation to another "@en-GB;
	skos:inScheme <http://cv.iptc.org/newscodes/subjectcode/>;
	skos:exactMatch medtop:20000643;
	skos:broader	subj:11000000;
	skos:narrower	subj:11005001.

subj:11005001
	rdf:type skos:Concept;
	skos:prefLabel	"economic sanction"@en-GB;
	skos:definition	"Punitive actions taken by one country against another including trade restrictions, embargoes etc. "@en-GB;
	skos:inScheme <http://cv.iptc.org/newscodes/subjectcode/>;
	skos:exactMatch medtop:20000642;
	skos:broader	subj:11005000.

subj:11006000
	rdf:type skos:Concept;
	skos:prefLabel	"government"@en-GB;
	skos:definition	"The system for ruling a country "@en-GB;
	skos:inScheme <http://cv.iptc.org/newscodes/subjectcode/>;
	skos:exactMatch medtop:20000593;
	skos:broader	subj:11000000;
	skos:narrower	subj:11006001;
	skos:narrower	subj:11006002;
	skos:narrower	subj:11006003;
	skos:narrower	subj:11006004;
	skos:narrower	subj:11006005;
	skos:narrower	subj:11006006;
	skos:narrower	subj:11006007;
	skos:narrower	subj:11006008;
	skos:narrower	subj:11006009;
	skos:narrower	subj:11006010;
	skos:narrower	subj:11006011;
	skos:narrower	subj:11006012;
	skos:narrower	subj:11006013.

subj:11006001
	rdf:type skos:Concept;
	skos:prefLabel	"civil and public service"@en-GB;
	skos:definition	"The paid service by civilians for the government, and the often non-paid service of individuals for the benefit of others (public service) "@en-GB;
	skos:inScheme <http://cv.iptc.org/newscodes/subjectcode/>;
	skos:exactMatch medtop:20000594;
	skos:broader	subj:11006000.

subj:11006002
	rdf:type skos:Concept;
	skos:prefLabel	"safety of citizens"@en-GB;
	skos:definition	"Government policies to protect the well being of its citizens "@en-GB;
	skos:inScheme <http://cv.iptc.org/newscodes/subjectcode/>;
	skos:exactMatch medtop:20000619;
	skos:broader	subj:11006000.

subj:11006003
	rdf:type skos:Concept;
	skos:prefLabel	"think tank"@en-GB;
	skos:definition	"Group that undertakes political research and issue position papers, recommendations etc "@en-GB;
	skos:inScheme <http://cv.iptc.org/newscodes/subjectcode/>;
	skos:broadMatch medtop:20000593;
	skos:broader	subj:11006000.

subj:11006004
	rdf:type skos:Concept;
	skos:prefLabel	"national government"@en-GB;
	skos:definition	"The ruling body of a nation "@en-GB;
	skos:inScheme <http://cv.iptc.org/newscodes/subjectcode/>;
	skos:exactMatch medtop:20000614;
	skos:broader	subj:11006000.

subj:11006005
	rdf:type skos:Concept;
	skos:prefLabel	"executive (government)"@en-GB;
	skos:definition	"That portion of a ruling body involving the overall operation of government "@en-GB;
	skos:inScheme <http://cv.iptc.org/newscodes/subjectcode/>;
	skos:exactMatch medtop:20000606;
	skos:broader	subj:11006000.

subj:11006006
	rdf:type skos:Concept;
	skos:prefLabel	"heads of state"@en-GB;
	skos:definition	"Symbolic or actual chief representative of a nation, such as royalty, or president or emir, for example "@en-GB;
	skos:inScheme <http://cv.iptc.org/newscodes/subjectcode/>;
	skos:exactMatch medtop:20000610;
	skos:broader	subj:11006000.

subj:11006007
	rdf:type skos:Concept;
	skos:prefLabel	"government departments"@en-GB;
	skos:definition	"Divisions of a government that concentrate on specific areas such as health, welfare, economy or war "@en-GB;
	skos:inScheme <http://cv.iptc.org/newscodes/subjectcode/>;
	skos:exactMatch medtop:20000609;
	skos:broader	subj:11006000.

subj:11006008
	rdf:type skos:Concept;
	skos:prefLabel	"public officials"@en-GB;
	skos:definition	"Individuals, usually elected, who are in public service or commonly in the public eye. "@en-GB;
	skos:inScheme <http://cv.iptc.org/newscodes/subjectcode/>;
	skos:exactMatch medtop:20000596;
	skos:broader	subj:11006000.

subj:11006009
	rdf:type skos:Concept;
	skos:prefLabel	"ministers (government)"@en-GB;
	skos:definition	"Heads of various government departments at one level, also known as secretaries. At another level they form a legislative body. The chief minister is either prime minister or premier. "@en-GB;
	skos:inScheme <http://cv.iptc.org/newscodes/subjectcode/>;
	skos:exactMatch medtop:20000613;
	skos:broader	subj:11006000.

subj:11006010
	rdf:type skos:Concept;
	skos:prefLabel	"public employees"@en-GB;
	skos:definition	"People employed by a government at all levels "@en-GB;
	skos:inScheme <http://cv.iptc.org/newscodes/subjectcode/>;
	skos:exactMatch medtop:20000595;
	skos:broader	subj:11006000.

subj:11006011
	rdf:type skos:Concept;
	skos:prefLabel	"privatisation"@en-GB;
	skos:definition	"The privatisation of state-owned companies or property "@en-GB;
	skos:inScheme <http://cv.iptc.org/newscodes/subjectcode/>;
	skos:exactMatch medtop:20000624;
	skos:broader	subj:11006000.

subj:11006012
	rdf:type skos:Concept;
	skos:prefLabel	"nationalisation"@en-GB;
	skos:definition	"State takeover of private companies or property "@en-GB;
	skos:inScheme <http://cv.iptc.org/newscodes/subjectcode/>;
	skos:exactMatch medtop:20000623;
	skos:broader	subj:11006000.

subj:11006013
	rdf:type skos:Concept;
	skos:prefLabel	"impeachment"@en-GB;
	skos:definition	"The process of bringing a public official before a tribunal to answer charges of wrongdoing "@en-GB;
	skos:inScheme <http://cv.iptc.org/newscodes/subjectcode/>;
	skos:exactMatch medtop:20000611;
	skos:broader	subj:11006000.

subj:11007000
	rdf:type skos:Concept;
	skos:prefLabel	"human rights"@en-GB;
	skos:definition	"Rights entitled to be enjoyed by all citizens universally "@en-GB;
	skos:inScheme <http://cv.iptc.org/newscodes/subjectcode/>;
	skos:exactMatch medtop:20000592;
	skos:broader	subj:11000000.

subj:11008000
	rdf:type skos:Concept;
	skos:prefLabel	"local authority"@en-GB;
	skos:definition	"Authorities at city, county state or borough level "@en-GB;
	skos:inScheme <http://cv.iptc.org/newscodes/subjectcode/>;
	skos:exactMatch medtop:20000612;
	skos:broader	subj:11000000.

subj:11009000
	rdf:type skos:Concept;
	skos:prefLabel	"parliament"@en-GB;
	skos:definition	"The collective body of elected officials representing the people "@en-GB;
	skos:inScheme <http://cv.iptc.org/newscodes/subjectcode/>;
	skos:exactMatch medtop:20000615;
	skos:broader	subj:11000000;
	skos:narrower	subj:11009001;
	skos:narrower	subj:11009002.

subj:11009001
	rdf:type skos:Concept;
	skos:prefLabel	"upper house"@en-GB;
	skos:definition	"Senior chamber of a legislative body "@en-GB;
	skos:inScheme <http://cv.iptc.org/newscodes/subjectcode/>;
	skos:exactMatch medtop:20000617;
	skos:broader	subj:11009000.

subj:11009002
	rdf:type skos:Concept;
	skos:prefLabel	"lower house"@en-GB;
	skos:definition	"The lower chamber of a legislative body "@en-GB;
	skos:inScheme <http://cv.iptc.org/newscodes/subjectcode/>;
	skos:exactMatch medtop:20000616;
	skos:broader	subj:11009000.

subj:11010000
	rdf:type skos:Concept;
	skos:prefLabel	"parties and movements"@en-GB;
	skos:definition	"Covers both formally recognized and informal political associations "@en-GB;
	skos:inScheme <http://cv.iptc.org/newscodes/subjectcode/>;
	skos:exactMatch medtop:20000651;
	skos:broader	subj:11000000;
	skos:narrower	subj:11010001.

subj:11010001
	rdf:type skos:Concept;
	skos:prefLabel	"non government organizations (NGO)"@en-GB;
	skos:definition	"Groups officially outside of government that lobby, demonstrate or campaign on a wide range of issues such as economics, environment healthcare etc. "@en-GB;
	skos:inScheme <http://cv.iptc.org/newscodes/subjectcode/>;
	skos:exactMatch medtop:20000646;
	skos:broader	subj:11010000.

subj:11011000
	rdf:type skos:Concept;
	skos:prefLabel	"refugee"@en-GB;
	skos:definition	"A person seeking shelter in another country because of some fear of persecution in his own country "@en-GB;
	skos:inScheme <http://cv.iptc.org/newscodes/subjectcode/>;
	skos:exactMatch medtop:20000645;
	skos:broader	subj:11000000.

subj:11012000
	rdf:type skos:Concept;
	skos:prefLabel	"regional authority"@en-GB;
	skos:definition	"Government bodies at levels encompassing more than one jurisdiction, e.g. the Delaware River Basin Commission "@en-GB;
	skos:inScheme <http://cv.iptc.org/newscodes/subjectcode/>;
	skos:closeMatch medtop:20000618;
	skos:broader	subj:11000000.

subj:11013000
	rdf:type skos:Concept;
	skos:prefLabel	"state budget and tax"@en-GB;
	skos:definition	"The national budget as promulgated by the government "@en-GB;
	skos:inScheme <http://cv.iptc.org/newscodes/subjectcode/>;
	skos:closeMatch medtop:20000607;
	skos:broader	subj:11000000;
	skos:narrower	subj:11013001.

subj:11013001
	rdf:type skos:Concept;
	skos:prefLabel	"public finance"@en-GB;
	skos:definition	"The money of government used for paying for public programs and services and public debt "@en-GB;
	skos:inScheme <http://cv.iptc.org/newscodes/subjectcode/>;
	skos:exactMatch medtop:20000608;
	skos:broader	subj:11013000.

subj:11014000
	rdf:type skos:Concept;
	skos:prefLabel	"treaty and international organisation-DEPRECATED"@en-GB;
	skos:definition	"NA"@en-GB;
	skos:historyNote	"DEPRECATED in V 16, split to SubjectMatters 11027 and 11028 "@en-GB;
	skos:inScheme <http://cv.iptc.org/newscodes/subjectcode/>;
	skos:broadMatch medtop:20000638;
	skos:broader	subj:11000000;
	skos:narrower	subj:11014001;
	skos:narrower	subj:11014002;
	skos:narrower	subj:11014003.

subj:11014001
	rdf:type skos:Concept;
	skos:prefLabel	"international relations-DEPRECATED"@en-GB;
	skos:definition	"NA"@en-GB;
	skos:historyNote	"moved to SubjectMatter 11002 in V16 "@en-GB;
	skos:inScheme <http://cv.iptc.org/newscodes/subjectcode/>;
	skos:broadMatch medtop:20000639;
	skos:broader	subj:11014000.

subj:11014002
	rdf:type skos:Concept;
	skos:prefLabel	"peace negotiations-DEPRECATED"@en-GB;
	skos:definition	"NA"@en-GB;
	skos:historyNote	"moved to SubjectMatter 11002 in V16 "@en-GB;
	skos:inScheme <http://cv.iptc.org/newscodes/subjectcode/>;
	skos:broadMatch medtop:20000639;
	skos:broader	subj:11014000.

subj:11014003
	rdf:type skos:Concept;
	skos:prefLabel	"alliances-DEPRECATED"@en-GB;
	skos:definition	"NA"@en-GB;
	skos:historyNote	"moved to SubjectMatter 11002 in V16 "@en-GB;
	skos:inScheme <http://cv.iptc.org/newscodes/subjectcode/>;
	skos:broadMatch medtop:20000639;
	skos:broader	subj:11014000.

subj:11015000
	rdf:type skos:Concept;
	skos:prefLabel	"constitution"@en-GB;
	skos:definition	"Usually a written document setting forth the operations of a government and the rights of the citizens therein "@en-GB;
	skos:inScheme <http://cv.iptc.org/newscodes/subjectcode/>;
	skos:exactMatch medtop:20000597;
	skos:broader	subj:11000000.

subj:11016000
	rdf:type skos:Concept;
	skos:prefLabel	"interior policy"@en-GB;
	skos:definition	"Government policies affecting internal affairs of a country "@en-GB;
	skos:inScheme <http://cv.iptc.org/newscodes/subjectcode/>;
	skos:closeMatch medtop:20000626;
	skos:broader	subj:11000000;
	skos:narrower	subj:11016001;
	skos:narrower	subj:11016002;
	skos:narrower	subj:11016003;
	skos:narrower	subj:11016004;
	skos:narrower	subj:11016005;
	skos:narrower	subj:11016006;
	skos:narrower	subj:11016007.

subj:11016001
	rdf:type skos:Concept;
	skos:prefLabel	"data protection"@en-GB;
	skos:definition	"Efforts to protect personal information in either written, oral or electronic form "@en-GB;
	skos:inScheme <http://cv.iptc.org/newscodes/subjectcode/>;
	skos:exactMatch medtop:20000627;
	skos:broader	subj:11016000.

subj:11016002
	rdf:type skos:Concept;
	skos:prefLabel	"housing and urban planning"@en-GB;
	skos:definition	"Systematic planning of urban and suburban areas and the housing within those areas "@en-GB;
	skos:inScheme <http://cv.iptc.org/newscodes/subjectcode/>;
	skos:exactMatch medtop:20000628;
	skos:broader	subj:11016000.

subj:11016003
	rdf:type skos:Concept;
	skos:prefLabel	"pension and welfare"@en-GB;
	skos:definition	"Government policies affecting the well being of its citizens through unemployment benefits, state pensions and other similar payments "@en-GB;
	skos:inScheme <http://cv.iptc.org/newscodes/subjectcode/>;
	skos:exactMatch medtop:20000630;
	skos:broader	subj:11016000.

subj:11016004
	rdf:type skos:Concept;
	skos:prefLabel	"personal weapon control"@en-GB;
	skos:definition	"Government control of personal ownership of firearms and other offensive weapons, including control of weapons used for sports through licenses and other means "@en-GB;
	skos:inScheme <http://cv.iptc.org/newscodes/subjectcode/>;
	skos:exactMatch medtop:20000632;
	skos:broader	subj:11016000.

subj:11016005
	rdf:type skos:Concept;
	skos:prefLabel	"indigenous people"@en-GB;
	skos:definition	"Government policies toward indigenous peoples "@en-GB;
	skos:inScheme <http://cv.iptc.org/newscodes/subjectcode/>;
	skos:exactMatch medtop:20000629;
	skos:broader	subj:11016000.

subj:11016006
	rdf:type skos:Concept;
	skos:prefLabel	"personal data collection"@en-GB;
	skos:definition	"The collection, by government or other entities of information on individuals "@en-GB;
	skos:inScheme <http://cv.iptc.org/newscodes/subjectcode/>;
	skos:exactMatch medtop:20000631;
	skos:broader	subj:11016000.

subj:11016007
	rdf:type skos:Concept;
	skos:prefLabel	"planning inquiries"@en-GB;
	skos:definition	"Public hearings or planning inquiries on proposed constructions, e.g. Construction of water driven power station in a National Park. "@en-GB;
	skos:inScheme <http://cv.iptc.org/newscodes/subjectcode/>;
	skos:exactMatch medtop:20000633;
	skos:broader	subj:11016000.

subj:11017000
	rdf:type skos:Concept;
	skos:prefLabel	"migration"@en-GB;
	skos:definition	"Movement of one body of persons from one place to another "@en-GB;
	skos:inScheme <http://cv.iptc.org/newscodes/subjectcode/>;
	skos:exactMatch medtop:20000634;
	skos:broader	subj:11000000.

subj:11018000
	rdf:type skos:Concept;
	skos:prefLabel	"citizens initiative and recall"@en-GB;
	skos:definition	"Political suggestions by non-government officials for corrective action, or for changes in existing rules and regulations "@en-GB;
	skos:inScheme <http://cv.iptc.org/newscodes/subjectcode/>;
	skos:exactMatch medtop:20000575;
	skos:broader	subj:11000000.

subj:11019000
	rdf:type skos:Concept;
	skos:prefLabel	"referenda"@en-GB;
	skos:definition	"Political proposals, laws and actions suggested by non-government officials to be voted on by the entire voting body "@en-GB;
	skos:inScheme <http://cv.iptc.org/newscodes/subjectcode/>;
	skos:exactMatch medtop:20000584;
	skos:broader	subj:11000000.

subj:11020000
	rdf:type skos:Concept;
	skos:prefLabel	"nuclear policy"@en-GB;
	skos:definition	"Government policies as regards to use of nuclear fuels for power production or weapons "@en-GB;
	skos:inScheme <http://cv.iptc.org/newscodes/subjectcode/>;
	skos:exactMatch medtop:20000635;
	skos:broader	subj:11000000.

subj:11021000
	rdf:type skos:Concept;
	skos:prefLabel	"lobbying"@en-GB;
	skos:definition	"The attempt by non-government bodies and individual to affect the outcome of legislation through verbal, or other, persuasion "@en-GB;
	skos:inScheme <http://cv.iptc.org/newscodes/subjectcode/>;
	skos:exactMatch medtop:20000650;
	skos:broader	subj:11000000.

subj:11022000
	rdf:type skos:Concept;
	skos:prefLabel	"regulatory policy and organisation"@en-GB;
	skos:definition	"The rules and bodies, both national and international, that govern conflict of interest and good practice regulations. "@en-GB;
	skos:inScheme <http://cv.iptc.org/newscodes/subjectcode/>;
	skos:exactMatch medtop:20000636;
	skos:broader	subj:11000000.

subj:11023000
	rdf:type skos:Concept;
	skos:prefLabel	"censorship"@en-GB;
	skos:definition	"Attempts by any group to control freedoms of speech, religion, and ideas distributed in print, graphics, cyberspace and other ways. Does not include official standards such as cinema ratings, advertising and broadcast standards. "@en-GB;
	skos:historyNote	"replaced by "freedom of press" in V 12, reintroduced in V13 "@en-GB;
	skos:inScheme <http://cv.iptc.org/newscodes/subjectcode/>;
	skos:exactMatch medtop:20000588;
	skos:broader	subj:11000000.

subj:11024000
	rdf:type skos:Concept;
	skos:prefLabel	"politics (general)"@en-GB;
	skos:definition	"The art or science of participating in the affairs of government, a state of political party "@en-GB;
	skos:inScheme <http://cv.iptc.org/newscodes/subjectcode/>;
	skos:exactMatch medtop:20000649;
	skos:broader	subj:11000000;
	skos:narrower	subj:11024001;
	skos:narrower	subj:11024002;
	skos:narrower	subj:11024003.

subj:11024001
	rdf:type skos:Concept;
	skos:prefLabel	"political systems"@en-GB;
	skos:definition	"Systems designed to provide order to government "@en-GB;
	skos:inScheme <http://cv.iptc.org/newscodes/subjectcode/>;
	skos:exactMatch medtop:20000653;
	skos:broader	subj:11024000.

subj:11024002
	rdf:type skos:Concept;
	skos:prefLabel	"democracy"@en-GB;
	skos:definition	"Government in which the people hold the power either directly, or through elected officials. "@en-GB;
	skos:inScheme <http://cv.iptc.org/newscodes/subjectcode/>;
	skos:exactMatch medtop:20000654;
	skos:broader	subj:11024000.

subj:11024003
	rdf:type skos:Concept;
	skos:prefLabel	"political development"@en-GB;
	skos:definition	"The creation and rise of political systems and the history of the people and nations that are associated with those systems. "@en-GB;
	skos:inScheme <http://cv.iptc.org/newscodes/subjectcode/>;
	skos:exactMatch medtop:20000652;
	skos:broader	subj:11024000.

subj:11025000
	rdf:type skos:Concept;
	skos:prefLabel	"freedom of the press"@en-GB;
	skos:definition	"Mass media rights and freedoms, pressure and intimidation of the journalists, censorship in mass media, activities of government bodies, journalistic associations and/or organizations and other NGOs in regards to press freedom "@en-GB;
	skos:historyNote	"replaced "censorship" in V12, added as new Topic in V13 "@en-GB;
	skos:inScheme <http://cv.iptc.org/newscodes/subjectcode/>;
	skos:exactMatch medtop:20000591;
	skos:broader	subj:11000000.

subj:11026000
	rdf:type skos:Concept;
	skos:prefLabel	"freedom of religion"@en-GB;
	skos:definition	"Religious rights and freedoms, pressure and intimidation of the believers, censorship in mass media, activities of government bodies, journalistic associations and/or organizations and other NGOs in regards to freedom of belief and practice "@en-GB;
	skos:inScheme <http://cv.iptc.org/newscodes/subjectcode/>;
	skos:exactMatch medtop:20000590;
	skos:broader	subj:11000000.

subj:11027000
	rdf:type skos:Concept;
	skos:prefLabel	"treaty"@en-GB;
	skos:definition	"A treaty (as defined by the Vienna Convention on the Law of Treaties) is a written agreement between international entities that is binding under international law. "@en-GB;
	skos:inScheme <http://cv.iptc.org/newscodes/subjectcode/>;
	skos:exactMatch medtop:20000641;
	skos:broader	subj:11000000.

subj:11028000
	rdf:type skos:Concept;
	skos:prefLabel	"international organisation"@en-GB;
	skos:definition	"Includes organisations with members and functions that cross international borders, and may include intergovernmental organisations of sovereign nations. "@en-GB;
	skos:inScheme <http://cv.iptc.org/newscodes/subjectcode/>;
	skos:exactMatch medtop:20000644;
	skos:broader	subj:11000000.

subj:12000000
	rdf:type skos:Concept;
	skos:prefLabel	"religion and belief"@en-GB;
	skos:definition	"All aspects of human existence involving theology, philosophy, ethics and spirituality. "@en-GB;
	skos:inScheme <http://cv.iptc.org/newscodes/subjectcode/>;
	skos:exactMatch medtop:12000000;
	skos:narrower	subj:12001000;
	skos:narrower	subj:12002000;
	skos:narrower	subj:12003000;
	skos:narrower	subj:12004000;
	skos:narrower	subj:12005000;
	skos:narrower	subj:12006000;
	skos:narrower	subj:12007000;
	skos:narrower	subj:12008000;
	skos:narrower	subj:12009000;
	skos:narrower	subj:12010000;
	skos:narrower	subj:12011000;
	skos:narrower	subj:12012000;
	skos:narrower	subj:12013000;
	skos:narrower	subj:12014000;
	skos:narrower	subj:12015000;
	skos:narrower	subj:12016000;
	skos:narrower	subj:12017000;
	skos:narrower	subj:12018000;
	skos:narrower	subj:12019000;
	skos:narrower	subj:12020000;
	skos:narrower	subj:12021000;
	skos:narrower	subj:12022000;
	skos:narrower	subj:12023000;
	skos:narrower	subj:12024000;
	skos:narrower	subj:12025000;
	skos:narrower	subj:12026000;
	skos:narrower	subj:12027000.

subj:12001000
	rdf:type skos:Concept;
	skos:prefLabel	"cult and sect"@en-GB;
	skos:definition	"Offshoots of established religious bodies, or small narrow-focused group promulgated by one or two individuals "@en-GB;
	skos:inScheme <http://cv.iptc.org/newscodes/subjectcode/>;
	skos:exactMatch medtop:20000674;
	skos:broader	subj:12000000.

subj:12002000
	rdf:type skos:Concept;
	skos:prefLabel	"belief (faith)"@en-GB;
	skos:definition	"The established beliefs of an individuals religion "@en-GB;
	skos:inScheme <http://cv.iptc.org/newscodes/subjectcode/>;
	skos:exactMatch medtop:20000657;
	skos:broader	subj:12000000;
	skos:narrower	subj:12002001;
	skos:narrower	subj:12002002.

subj:12002001
	rdf:type skos:Concept;
	skos:prefLabel	"unificationism"@en-GB;
	skos:definition	"The belief system of members of the Unification Church established by the Rev. Sun Myung Moon. "@en-GB;
	skos:inScheme <http://cv.iptc.org/newscodes/subjectcode/>;
	skos:exactMatch medtop:20000686;
	skos:broader	subj:12002000.

subj:12002002
	rdf:type skos:Concept;
	skos:prefLabel	"scientology"@en-GB;
	skos:definition	"Believe that man is a spiritual being endowed with abilities well beyond those which he normally envisages; he's able to solve his own problems, accomplish his goals and gain lasting happiness. "@en-GB;
	skos:inScheme <http://cv.iptc.org/newscodes/subjectcode/>;
	skos:exactMatch medtop:20000682;
	skos:broader	subj:12002000.

subj:12003000
	rdf:type skos:Concept;
	skos:prefLabel	"freemasonry"@en-GB;
	skos:definition	"A secret international society based on the principles of brotherhood, charity and mutual aid "@en-GB;
	skos:inScheme <http://cv.iptc.org/newscodes/subjectcode/>;
	skos:exactMatch medtop:20000675;
	skos:broader	subj:12000000.

subj:12004000
	rdf:type skos:Concept;
	skos:prefLabel	"religion-DEPRECATED"@en-GB;
	skos:definition	"NA"@en-GB;
	skos:historyNote	"SubjectMatter deprecated, SubjectDetails moved to other SubjectMatter "@en-GB;
	skos:inScheme <http://cv.iptc.org/newscodes/subjectcode/>;
	skos:closeMatch medtop:12000000;
	skos:broader	subj:12000000;
	skos:narrower	subj:12004001;
	skos:narrower	subj:12004002;
	skos:narrower	subj:12004003;
	skos:narrower	subj:12004004;
	skos:narrower	subj:12004005.

subj:12004001
	rdf:type skos:Concept;
	skos:prefLabel	"christianity-DEPRECATED"@en-GB;
	skos:definition	"NA"@en-GB;
	skos:historyNote	"moved to 12009000 "@en-GB;
	skos:inScheme <http://cv.iptc.org/newscodes/subjectcode/>;
	skos:exactMatch medtop:20000659;
	skos:broader	subj:12004000.

subj:12004002
	rdf:type skos:Concept;
	skos:prefLabel	"islam-DEPRECATED"@en-GB;
	skos:definition	"NA"@en-GB;
	skos:historyNote	"moved to 12010000 "@en-GB;
	skos:inScheme <http://cv.iptc.org/newscodes/subjectcode/>;
	skos:exactMatch medtop:20000677;
	skos:broader	subj:12004000.

subj:12004003
	rdf:type skos:Concept;
	skos:prefLabel	"judaism-DEPRECATED"@en-GB;
	skos:definition	"NA"@en-GB;
	skos:historyNote	"moved to 12011000 "@en-GB;
	skos:inScheme <http://cv.iptc.org/newscodes/subjectcode/>;
	skos:exactMatch medtop:20000679;
	skos:broader	subj:12004000.

subj:12004004
	rdf:type skos:Concept;
	skos:prefLabel	"buddhism-DEPRECATED"@en-GB;
	skos:definition	"NA"@en-GB;
	skos:historyNote	"moved to 12012000 "@en-GB;
	skos:inScheme <http://cv.iptc.org/newscodes/subjectcode/>;
	skos:exactMatch medtop:20000658;
	skos:broader	subj:12004000.

subj:12004005
	rdf:type skos:Concept;
	skos:prefLabel	"hinduism-DEPRECATED"@en-GB;
	skos:definition	"NA"@en-GB;
	skos:historyNote	"moved to 12013000 "@en-GB;
	skos:inScheme <http://cv.iptc.org/newscodes/subjectcode/>;
	skos:exactMatch medtop:20000676;
	skos:broader	subj:12004000.

subj:12005000
	rdf:type skos:Concept;
	skos:prefLabel	"church (organisation)-DEPRECATED"@en-GB;
	skos:definition	"NA"@en-GB;
	skos:historyNote	"moved to 12000001/SubjectQualifier "@en-GB;
	skos:inScheme <http://cv.iptc.org/newscodes/subjectcode/>;
	skos:exactMatch medtop:20000698;
	skos:broader	subj:12000000;
	skos:narrower	subj:12005001.

subj:12005001
	rdf:type skos:Concept;
	skos:prefLabel	"religious facilities-DEPRECATED"@en-GB;
	skos:definition	"NA"@en-GB;
	skos:historyNote	"moved to 12000002/SubjectQualifier "@en-GB;
	skos:inScheme <http://cv.iptc.org/newscodes/subjectcode/>;
	skos:exactMatch medtop:20000697;
	skos:broader	subj:12005000.

subj:12006000
	rdf:type skos:Concept;
	skos:prefLabel	"values"@en-GB;
	skos:definition	"Personal levels of social behaviour "@en-GB;
	skos:inScheme <http://cv.iptc.org/newscodes/subjectcode/>;
	skos:exactMatch medtop:20000808;
	skos:broader	subj:12000000;
	skos:narrower	subj:12006001;
	skos:narrower	subj:12006002.

subj:12006001
	rdf:type skos:Concept;
	skos:prefLabel	"ethics"@en-GB;
	skos:definition	"A system of beliefs about acceptable behaviour "@en-GB;
	skos:inScheme <http://cv.iptc.org/newscodes/subjectcode/>;
	skos:exactMatch medtop:20000814;
	skos:broader	subj:12006000.

subj:12006002
	rdf:type skos:Concept;
	skos:prefLabel	"corrupt practices"@en-GB;
	skos:definition	"Any action which is harmful to others "@en-GB;
	skos:inScheme <http://cv.iptc.org/newscodes/subjectcode/>;
	skos:exactMatch medtop:20000809;
	skos:broader	subj:12006000.

subj:12007000
	rdf:type skos:Concept;
	skos:prefLabel	"church and state relations"@en-GB;
	skos:definition	"The legal and social division between religious institutions and the affairs of state "@en-GB;
	skos:inScheme <http://cv.iptc.org/newscodes/subjectcode/>;
	skos:exactMatch medtop:20000702;
	skos:broader	subj:12000000.

subj:12008000
	rdf:type skos:Concept;
	skos:prefLabel	"philosophy"@en-GB;
	skos:definition	"Different thoughts about the way the world works "@en-GB;
	skos:inScheme <http://cv.iptc.org/newscodes/subjectcode/>;
	skos:closeMatch medtop:20000751;
	skos:broader	subj:12000000.

subj:12009000
	rdf:type skos:Concept;
	skos:prefLabel	"christianity"@en-GB;
	skos:definition	"Those that use Jesus Christ and his teachings as their centre of belief "@en-GB;
	skos:historyNote	"moved from 12004001 "@en-GB;
	skos:inScheme <http://cv.iptc.org/newscodes/subjectcode/>;
	skos:exactMatch medtop:20000659;
	skos:broader	subj:12000000;
	skos:narrower	subj:12009001;
	skos:narrower	subj:12009002;
	skos:narrower	subj:12009003;
	skos:narrower	subj:12009004;
	skos:narrower	subj:12009005;
	skos:narrower	subj:12009006;
	skos:narrower	subj:12009007;
	skos:narrower	subj:12009009;
	skos:narrower	subj:12009010;
	skos:narrower	subj:12009011;
	skos:narrower	subj:12009012;
	skos:narrower	subj:12009013.

subj:12009001
	rdf:type skos:Concept;
	skos:prefLabel	"protestant"@en-GB;
	skos:definition	"General term for christian churches and religious communities which developed through the reformation in the 16th century "@en-GB;
	skos:inScheme <http://cv.iptc.org/newscodes/subjectcode/>;
	skos:exactMatch medtop:20000664;
	skos:broader	subj:12009000.

subj:12009002
	rdf:type skos:Concept;
	skos:prefLabel	"lutheran"@en-GB;
	skos:definition	"Christians who follow the teaching of reformer Martin Luther "@en-GB;
	skos:inScheme <http://cv.iptc.org/newscodes/subjectcode/>;
	skos:exactMatch medtop:20000667;
	skos:broader	subj:12009000.

subj:12009003
	rdf:type skos:Concept;
	skos:prefLabel	"reformed"@en-GB;
	skos:definition	"Christians who follow the teaching of reformers Johannes Calvin and Ulrich Zwingli "@en-GB;
	skos:inScheme <http://cv.iptc.org/newscodes/subjectcode/>;
	skos:exactMatch medtop:20000670;
	skos:broader	subj:12009000.

subj:12009004
	rdf:type skos:Concept;
	skos:prefLabel	"anglican"@en-GB;
	skos:definition	"Members of the worldwide anglican communion which started in the 16th century in England as a breakaway church from the roman catholic church "@en-GB;
	skos:inScheme <http://cv.iptc.org/newscodes/subjectcode/>;
	skos:exactMatch medtop:20000665;
	skos:broader	subj:12009000.

subj:12009005
	rdf:type skos:Concept;
	skos:prefLabel	"methodist"@en-GB;
	skos:definition	"Followers of John and Charles Wesley who tried to reform the Church of England in the 18th century and turned into a separate church "@en-GB;
	skos:inScheme <http://cv.iptc.org/newscodes/subjectcode/>;
	skos:exactMatch medtop:20000669;
	skos:broader	subj:12009000.

subj:12009006
	rdf:type skos:Concept;
	skos:prefLabel	"baptist"@en-GB;
	skos:definition	"Members of a christian church which only baptises adults who truly believe in Christ "@en-GB;
	skos:inScheme <http://cv.iptc.org/newscodes/subjectcode/>;
	skos:exactMatch medtop:20000666;
	skos:broader	subj:12009000.

subj:12009007
	rdf:type skos:Concept;
	skos:prefLabel	"mennonite"@en-GB;
	skos:definition	"Members of a 16th century christian church which is against military service and baptising infants "@en-GB;
	skos:inScheme <http://cv.iptc.org/newscodes/subjectcode/>;
	skos:exactMatch medtop:20000668;
	skos:broader	subj:12009000.

subj:12009009
	rdf:type skos:Concept;
	skos:prefLabel	"mormon"@en-GB;
	skos:definition	"Members of a religious community which believes in the ´Book of Mormon´ and the revelations of founder M.J. Smith "@en-GB;
	skos:inScheme <http://cv.iptc.org/newscodes/subjectcode/>;
	skos:exactMatch medtop:20000661;
	skos:broader	subj:12009000.

subj:12009010
	rdf:type skos:Concept;
	skos:prefLabel	"roman catholic"@en-GB;
	skos:definition	"Biggest christian church worldwide tracing its origins back to Jesus Christ "@en-GB;
	skos:inScheme <http://cv.iptc.org/newscodes/subjectcode/>;
	skos:exactMatch medtop:20000671;
	skos:broader	subj:12009000.

subj:12009011
	rdf:type skos:Concept;
	skos:prefLabel	"old catholic"@en-GB;
	skos:definition	"Members of a catholic church which started in 1870 and denies the dogma of the infallibility of the pope "@en-GB;
	skos:inScheme <http://cv.iptc.org/newscodes/subjectcode/>;
	skos:exactMatch medtop:20000662;
	skos:broader	subj:12009000.

subj:12009012
	rdf:type skos:Concept;
	skos:prefLabel	"orthodoxy"@en-GB;
	skos:definition	"Eastern rite churches which are characterised by their continuity with the apostolic church, their liturgy and their territorial churches, mainly in eastern and south-eastern Europe and the Middle East "@en-GB;
	skos:inScheme <http://cv.iptc.org/newscodes/subjectcode/>;
	skos:exactMatch medtop:20000663;
	skos:broader	subj:12009000.

subj:12009013
	rdf:type skos:Concept;
	skos:prefLabel	"salvation army"@en-GB;
	skos:definition	"Christian community organised in a military fashion which does missionary and social work "@en-GB;
	skos:inScheme <http://cv.iptc.org/newscodes/subjectcode/>;
	skos:broadMatch medtop:20000659;
	skos:broader	subj:12009000.

subj:12010000
	rdf:type skos:Concept;
	skos:prefLabel	"islam"@en-GB;
	skos:definition	"Those who use Allah and his teachings as their centre of belief "@en-GB;
	skos:historyNote	"moved from 12004002 "@en-GB;
	skos:inScheme <http://cv.iptc.org/newscodes/subjectcode/>;
	skos:exactMatch medtop:20000677;
	skos:broader	subj:12000000.

subj:12011000
	rdf:type skos:Concept;
	skos:prefLabel	"judaism"@en-GB;
	skos:definition	"A group believing in one god, basing their beliefs on written scriptures and the Talmud, including the first coming of the Messiah "@en-GB;
	skos:historyNote	"moved from 12004003 "@en-GB;
	skos:inScheme <http://cv.iptc.org/newscodes/subjectcode/>;
	skos:exactMatch medtop:20000679;
	skos:broader	subj:12000000.

subj:12012000
	rdf:type skos:Concept;
	skos:prefLabel	"buddhism"@en-GB;
	skos:definition	"A major Asian religion founded by Buddha in the 6th century BC in India and preaching that right thinking and self denial will lead to a divine state without desire "@en-GB;
	skos:historyNote	"moved from 12004004 "@en-GB;
	skos:inScheme <http://cv.iptc.org/newscodes/subjectcode/>;
	skos:exactMatch medtop:20000658;
	skos:broader	subj:12000000.

subj:12013000
	rdf:type skos:Concept;
	skos:prefLabel	"hinduism"@en-GB;
	skos:definition	"A religious and social system, believing in a caste system with the Brahmans the highest and untouchables the lowest. "@en-GB;
	skos:historyNote	"moved from 12004005 "@en-GB;
	skos:inScheme <http://cv.iptc.org/newscodes/subjectcode/>;
	skos:exactMatch medtop:20000676;
	skos:broader	subj:12000000.

subj:12014000
	rdf:type skos:Concept;
	skos:prefLabel	"religious festival or holiday"@en-GB;
	skos:definition	"Holy day or day of observance in a religion which sometimes is a public holiday as well "@en-GB;
	skos:inScheme <http://cv.iptc.org/newscodes/subjectcode/>;
	skos:exactMatch medtop:20000690;
	skos:broader	subj:12000000;
	skos:narrower	subj:12014001;
	skos:narrower	subj:12014002;
	skos:narrower	subj:12014003;
	skos:narrower	subj:12014004;
	skos:narrower	subj:12014005.

subj:12014001
	rdf:type skos:Concept;
	skos:prefLabel	"christmas"@en-GB;
	skos:definition	"Christian festival in commemorating the birth of Jesus Christ "@en-GB;
	skos:inScheme <http://cv.iptc.org/newscodes/subjectcode/>;
	skos:exactMatch medtop:20000691;
	skos:broader	subj:12014000.

subj:12014002
	rdf:type skos:Concept;
	skos:prefLabel	"easter"@en-GB;
	skos:definition	"Christian festival in commemorating the resurrection of Jesus Christ "@en-GB;
	skos:inScheme <http://cv.iptc.org/newscodes/subjectcode/>;
	skos:exactMatch medtop:20000692;
	skos:broader	subj:12014000.

subj:12014003
	rdf:type skos:Concept;
	skos:prefLabel	"pentecost"@en-GB;
	skos:definition	"Christian festival, celebrated on the 50th day after Easter commemorating the descent of the Holy Spirit "@en-GB;
	skos:inScheme <http://cv.iptc.org/newscodes/subjectcode/>;
	skos:exactMatch medtop:20000693;
	skos:broader	subj:12014000.

subj:12014004
	rdf:type skos:Concept;
	skos:prefLabel	"ramadan"@en-GB;
	skos:definition	"Holy month of fasting in Islam "@en-GB;
	skos:inScheme <http://cv.iptc.org/newscodes/subjectcode/>;
	skos:exactMatch medtop:20000694;
	skos:broader	subj:12014000.

subj:12014005
	rdf:type skos:Concept;
	skos:prefLabel	"yom kippur"@en-GB;
	skos:definition	"Most solemn of Jewish religious holidays, observed on the 10th day of the lunar month of tishri (in the course of September and October, when Jews seek reconciliation with god "@en-GB;
	skos:inScheme <http://cv.iptc.org/newscodes/subjectcode/>;
	skos:exactMatch medtop:20000695;
	skos:broader	subj:12014000.

subj:12015000
	rdf:type skos:Concept;
	skos:prefLabel	"religious leader"@en-GB;
	skos:definition	"Person or persons who have a ritual, juridical or otherwise leading role in their respective church or religion "@en-GB;
	skos:inScheme <http://cv.iptc.org/newscodes/subjectcode/>;
	skos:exactMatch medtop:20000703;
	skos:broader	subj:12000000;
	skos:narrower	subj:12015001.

subj:12015001
	rdf:type skos:Concept;
	skos:prefLabel	"pope"@en-GB;
	skos:definition	"Head of the roman catholic church worldwide "@en-GB;
	skos:inScheme <http://cv.iptc.org/newscodes/subjectcode/>;
	skos:exactMatch medtop:20000704;
	skos:broader	subj:12015000.

subj:12016000
	rdf:type skos:Concept;
	skos:prefLabel	"nature religion"@en-GB;
	skos:definition	"Worship of natural elements like fire, water, trees, mountains "@en-GB;
	skos:inScheme <http://cv.iptc.org/newscodes/subjectcode/>;
	skos:exactMatch medtop:20000680;
	skos:broader	subj:12000000.

subj:12017000
	rdf:type skos:Concept;
	skos:prefLabel	"taoism"@en-GB;
	skos:definition	"Indigenous religio-philosophical tradition that has shaped Chinese life for more than 2000 years "@en-GB;
	skos:inScheme <http://cv.iptc.org/newscodes/subjectcode/>;
	skos:exactMatch medtop:20000685;
	skos:broader	subj:12000000.

subj:12018000
	rdf:type skos:Concept;
	skos:prefLabel	"shintoism"@en-GB;
	skos:definition	"Indigenous religious beliefs and practices of Japan. The word Shinto came into use in order to distinguish indigenous Japanese beliefs from Buddhism. "@en-GB;
	skos:inScheme <http://cv.iptc.org/newscodes/subjectcode/>;
	skos:exactMatch medtop:20000683;
	skos:broader	subj:12000000.

subj:12019000
	rdf:type skos:Concept;
	skos:prefLabel	"sikhism"@en-GB;
	skos:definition	"The religion of an Indian group, combining Hindu and Islamic elements, founded in the Punjab (or Panjab) in the late 15th century AD by Guru Nanak. "@en-GB;
	skos:inScheme <http://cv.iptc.org/newscodes/subjectcode/>;
	skos:exactMatch medtop:20000684;
	skos:broader	subj:12000000.

subj:12020000
	rdf:type skos:Concept;
	skos:prefLabel	"jainism"@en-GB;
	skos:definition	"A religion of India that teaches a path to spiritual purity and enlightenment through a disciplined mode of life founded upon the tradition of ahimsa, non-violence to all living creatures. It began in the 7th-5th century BC. "@en-GB;
	skos:inScheme <http://cv.iptc.org/newscodes/subjectcode/>;
	skos:exactMatch medtop:20000678;
	skos:broader	subj:12000000.

subj:12021000
	rdf:type skos:Concept;
	skos:prefLabel	"parsasm"@en-GB;
	skos:definition	"A religion in India following the Iranian prophet Zoroaster, mainly in Bombay, but also in Karachi (Pakistan). "@en-GB;
	skos:inScheme <http://cv.iptc.org/newscodes/subjectcode/>;
	skos:exactMatch medtop:20000681;
	skos:broader	subj:12000000.

subj:12022000
	rdf:type skos:Concept;
	skos:prefLabel	"confucianism"@en-GB;
	skos:definition	"The way of life propagated by Confucius in the 6th-5th century BC and followed by the Chinese people for more than 2000 years. Its influence has extended to Korea, Japan, and Vietnam. "@en-GB;
	skos:inScheme <http://cv.iptc.org/newscodes/subjectcode/>;
	skos:exactMatch medtop:20000673;
	skos:broader	subj:12000000.

subj:12023000
	rdf:type skos:Concept;
	skos:prefLabel	"religious text"@en-GB;
	skos:definition	"Scriptures holy or important for a church or religion "@en-GB;
	skos:inScheme <http://cv.iptc.org/newscodes/subjectcode/>;
	skos:exactMatch medtop:20000705;
	skos:broader	subj:12000000;
	skos:narrower	subj:12023001;
	skos:narrower	subj:12023002;
	skos:narrower	subj:12023003.

subj:12023001
	rdf:type skos:Concept;
	skos:prefLabel	"bible"@en-GB;
	skos:definition	"Sacred scriptures of Christianity consisting of the old and new testament "@en-GB;
	skos:inScheme <http://cv.iptc.org/newscodes/subjectcode/>;
	skos:exactMatch medtop:20000706;
	skos:broader	subj:12023000.

subj:12023002
	rdf:type skos:Concept;
	skos:prefLabel	"qur'an"@en-GB;
	skos:definition	"Holy book of Islam "@en-GB;
	skos:inScheme <http://cv.iptc.org/newscodes/subjectcode/>;
	skos:exactMatch medtop:20000707;
	skos:broader	subj:12023000.

subj:12023003
	rdf:type skos:Concept;
	skos:prefLabel	"torah"@en-GB;
	skos:definition	"Holy scriptures of Judaism "@en-GB;
	skos:inScheme <http://cv.iptc.org/newscodes/subjectcode/>;
	skos:exactMatch medtop:20000708;
	skos:broader	subj:12023000.

subj:12024000
	rdf:type skos:Concept;
	skos:prefLabel	"interreligious dialogue"@en-GB;
	skos:definition	"Any form of communication between religions "@en-GB;
	skos:inScheme <http://cv.iptc.org/newscodes/subjectcode/>;
	skos:exactMatch medtop:20000687;
	skos:broader	subj:12000000.

subj:12025000
	rdf:type skos:Concept;
	skos:prefLabel	"religious event"@en-GB;
	skos:definition	"News regarding a religious event but not a festival or holiday "@en-GB;
	skos:inScheme <http://cv.iptc.org/newscodes/subjectcode/>;
	skos:exactMatch medtop:20000689;
	skos:broader	subj:12000000;
	skos:narrower	subj:12025001;
	skos:narrower	subj:12025002;
	skos:narrower	subj:12025004.

subj:12025001
	rdf:type skos:Concept;
	skos:prefLabel	"catholic convention"@en-GB;
	skos:definition	"A catholic convention "@en-GB;
	skos:inScheme <http://cv.iptc.org/newscodes/subjectcode/>;
	skos:broadMatch medtop:20000689;
	skos:broader	subj:12025000.

subj:12025002
	rdf:type skos:Concept;
	skos:prefLabel	"protestant convention"@en-GB;
	skos:definition	"A protestant convention "@en-GB;
	skos:inScheme <http://cv.iptc.org/newscodes/subjectcode/>;
	skos:broadMatch medtop:20000689;
	skos:broader	subj:12025000.

subj:12025004
	rdf:type skos:Concept;
	skos:prefLabel	"ritual"@en-GB;
	skos:definition	"Established religious rituals such as mass, baptism, prayer meetings "@en-GB;
	skos:inScheme <http://cv.iptc.org/newscodes/subjectcode/>;
	skos:exactMatch medtop:20000696;
	skos:broader	subj:12025000.

subj:12026000
	rdf:type skos:Concept;
	skos:prefLabel	"concordat"@en-GB;
	skos:definition	"Treaty between the Holy See and another country for the regulation of ecclesiastical affairs in the territory of the latter "@en-GB;
	skos:inScheme <http://cv.iptc.org/newscodes/subjectcode/>;
	skos:exactMatch medtop:20000672;
	skos:broader	subj:12000000.

subj:12027000
	rdf:type skos:Concept;
	skos:prefLabel	"ecumenism"@en-GB;
	skos:definition	"Relations between christian churches "@en-GB;
	skos:inScheme <http://cv.iptc.org/newscodes/subjectcode/>;
	skos:exactMatch medtop:20000660;
	skos:broader	subj:12000000.

subj:13000000
	rdf:type skos:Concept;
	skos:prefLabel	"science and technology"@en-GB;
	skos:definition	"All aspects pertaining to human understanding of nature and the physical world and the development and application of this knowledge "@en-GB;
	skos:inScheme <http://cv.iptc.org/newscodes/subjectcode/>;
	skos:exactMatch medtop:13000000;
	skos:narrower	subj:13001000;
	skos:narrower	subj:13002000;
	skos:narrower	subj:13003000;
	skos:narrower	subj:13004000;
	skos:narrower	subj:13005000;
	skos:narrower	subj:13006000;
	skos:narrower	subj:13007000;
	skos:narrower	subj:13008000;
	skos:narrower	subj:13009000;
	skos:narrower	subj:13010000;
	skos:narrower	subj:13011000;
	skos:narrower	subj:13012000;
	skos:narrower	subj:13013000;
	skos:narrower	subj:13014000;
	skos:narrower	subj:13015000;
	skos:narrower	subj:13016000;
	skos:narrower	subj:13017000;
	skos:narrower	subj:13018000;
	skos:narrower	subj:13019000;
	skos:narrower	subj:13020000;
	skos:narrower	subj:13021000;
	skos:narrower	subj:13022000;
	skos:narrower	subj:13023000.

subj:13001000
	rdf:type skos:Concept;
	skos:prefLabel	"applied science"@en-GB;
	skos:definition	"Stories about putting scientific knowledge to practical uses in the fields of the medical sciences, agriculture, domestic sciences as well as trades and crafts "@en-GB;
	skos:inScheme <http://cv.iptc.org/newscodes/subjectcode/>;
	skos:broadMatch medtop:13000000;
	skos:broader	subj:13000000;
	skos:narrower	subj:13001001;
	skos:narrower	subj:13001002;
	skos:narrower	subj:13001003;
	skos:narrower	subj:13001004.

subj:13001001
	rdf:type skos:Concept;
	skos:prefLabel	"physics"@en-GB;
	skos:definition	"The study of the properties and changes of matter "@en-GB;
	skos:inScheme <http://cv.iptc.org/newscodes/subjectcode/>;
	skos:exactMatch medtop:20000731;
	skos:broader	subj:13001000.

subj:13001002
	rdf:type skos:Concept;
	skos:prefLabel	"chemistry"@en-GB;
	skos:definition	"The study of the composition and reaction of substances "@en-GB;
	skos:inScheme <http://cv.iptc.org/newscodes/subjectcode/>;
	skos:exactMatch medtop:20000725;
	skos:broader	subj:13001000.

subj:13001003
	rdf:type skos:Concept;
	skos:prefLabel	"cosmology"@en-GB;
	skos:definition	"Study of the organization and structure of the universe "@en-GB;
	skos:inScheme <http://cv.iptc.org/newscodes/subjectcode/>;
	skos:exactMatch medtop:20000726;
	skos:broader	subj:13001000.

subj:13001004
	rdf:type skos:Concept;
	skos:prefLabel	"particle physics"@en-GB;
	skos:definition	"The study of elementary particles and atomic nuclei through the use of high-energy particles "@en-GB;
	skos:inScheme <http://cv.iptc.org/newscodes/subjectcode/>;
	skos:exactMatch medtop:20000734;
	skos:broader	subj:13001000.

subj:13002000
	rdf:type skos:Concept;
	skos:prefLabel	"engineering"@en-GB;
	skos:definition	"Stories about putting scientific knowledge to practical uses in the fields of civil, electrical, mechanical and chemical engineering "@en-GB;
	skos:inScheme <http://cv.iptc.org/newscodes/subjectcode/>;
	skos:broadMatch medtop:20000756;
	skos:broader	subj:13000000;
	skos:narrower	subj:13002001.

subj:13002001
	rdf:type skos:Concept;
	skos:prefLabel	"material science"@en-GB;
	skos:definition	"The study of materials used in manufacturing "@en-GB;
	skos:inScheme <http://cv.iptc.org/newscodes/subjectcode/>;
	skos:exactMatch medtop:20000764;
	skos:broader	subj:13002000.

subj:13003000
	rdf:type skos:Concept;
	skos:prefLabel	"human science"@en-GB;
	skos:definition	"Sociology, psychology, anthropology and political science "@en-GB;
	skos:inScheme <http://cv.iptc.org/newscodes/subjectcode/>;
	skos:closeMatch medtop:20000742;
	skos:broader	subj:13000000;
	skos:narrower	subj:13003001;
	skos:narrower	subj:13003002;
	skos:narrower	subj:13003003;
	skos:narrower	subj:13003004;
	skos:narrower	subj:13003005.

subj:13003001
	rdf:type skos:Concept;
	skos:prefLabel	"social sciences"@en-GB;
	skos:definition	"The study of people living in groups, as families, tribes and communities "@en-GB;
	skos:inScheme <http://cv.iptc.org/newscodes/subjectcode/>;
	skos:exactMatch medtop:20000742;
	skos:broader	subj:13003000.

subj:13003002
	rdf:type skos:Concept;
	skos:prefLabel	"history"@en-GB;
	skos:definition	"The study of human events of the past "@en-GB;
	skos:inScheme <http://cv.iptc.org/newscodes/subjectcode/>;
	skos:exactMatch medtop:20000747;
	skos:broader	subj:13003000.

subj:13003003
	rdf:type skos:Concept;
	skos:prefLabel	"psychology"@en-GB;
	skos:definition	"The study of the human mind and mental and emotional processes "@en-GB;
	skos:inScheme <http://cv.iptc.org/newscodes/subjectcode/>;
	skos:exactMatch medtop:20000753;
	skos:broader	subj:13003000.

subj:13003004
	rdf:type skos:Concept;
	skos:prefLabel	"sociology"@en-GB;
	skos:definition	"The study of human social relations, organization and change "@en-GB;
	skos:inScheme <http://cv.iptc.org/newscodes/subjectcode/>;
	skos:exactMatch medtop:20000754;
	skos:broader	subj:13003000.

subj:13003005
	rdf:type skos:Concept;
	skos:prefLabel	"anthropology"@en-GB;
	skos:definition	"The study of human beings in groups or societies "@en-GB;
	skos:inScheme <http://cv.iptc.org/newscodes/subjectcode/>;
	skos:exactMatch medtop:20000743;
	skos:broader	subj:13003000.

subj:13004000
	rdf:type skos:Concept;
	skos:prefLabel	"natural science"@en-GB;
	skos:definition	"Astronomy, astrophysics, physics, chemistry, earth sciences, palaeontology, biological sciences, botany and zoology, as well as mathematics "@en-GB;
	skos:inScheme <http://cv.iptc.org/newscodes/subjectcode/>;
	skos:exactMatch medtop:20000717;
	skos:broader	subj:13000000;
	skos:narrower	subj:13004001;
	skos:narrower	subj:13004002;
	skos:narrower	subj:13004003;
	skos:narrower	subj:13004004;
	skos:narrower	subj:13004005;
	skos:narrower	subj:13004006;
	skos:narrower	subj:13004007;
	skos:narrower	subj:13004008.

subj:13004001
	rdf:type skos:Concept;
	skos:prefLabel	"geology"@en-GB;
	skos:definition	"The study of Earth's physical processes "@en-GB;
	skos:inScheme <http://cv.iptc.org/newscodes/subjectcode/>;
	skos:exactMatch medtop:20000727;
	skos:broader	subj:13004000.

subj:13004002
	rdf:type skos:Concept;
	skos:prefLabel	"paleontology"@en-GB;
	skos:definition	"The study of ancient animals "@en-GB;
	skos:inScheme <http://cv.iptc.org/newscodes/subjectcode/>;
	skos:exactMatch medtop:20000722;
	skos:broader	subj:13004000.

subj:13004003
	rdf:type skos:Concept;
	skos:prefLabel	"geography"@en-GB;
	skos:definition	"The study of the surface of Earth and its political divisions "@en-GB;
	skos:inScheme <http://cv.iptc.org/newscodes/subjectcode/>;
	skos:exactMatch medtop:20000746;
	skos:broader	subj:13004000.

subj:13004004
	rdf:type skos:Concept;
	skos:prefLabel	"botany"@en-GB;
	skos:definition	"The study of plants "@en-GB;
	skos:inScheme <http://cv.iptc.org/newscodes/subjectcode/>;
	skos:exactMatch medtop:20000720;
	skos:broader	subj:13004000.

subj:13004005
	rdf:type skos:Concept;
	skos:prefLabel	"zoology"@en-GB;
	skos:definition	"The study of animals "@en-GB;
	skos:inScheme <http://cv.iptc.org/newscodes/subjectcode/>;
	skos:exactMatch medtop:20000724;
	skos:broader	subj:13004000.

subj:13004006
	rdf:type skos:Concept;
	skos:prefLabel	"physiology"@en-GB;
	skos:definition	"The study of vital processes of living organisms "@en-GB;
	skos:inScheme <http://cv.iptc.org/newscodes/subjectcode/>;
	skos:exactMatch medtop:20000723;
	skos:broader	subj:13004000.

subj:13004007
	rdf:type skos:Concept;
	skos:prefLabel	"astronomy"@en-GB;
	skos:definition	"The study of the stars and planets "@en-GB;
	skos:inScheme <http://cv.iptc.org/newscodes/subjectcode/>;
	skos:exactMatch medtop:20000718;
	skos:broader	subj:13004000.

subj:13004008
	rdf:type skos:Concept;
	skos:prefLabel	"biology"@en-GB;
	skos:definition	"The study of living organisms "@en-GB;
	skos:inScheme <http://cv.iptc.org/newscodes/subjectcode/>;
	skos:exactMatch medtop:20000719;
	skos:broader	subj:13004000.

subj:13005000
	rdf:type skos:Concept;
	skos:prefLabel	"philosophical science"@en-GB;
	skos:definition	"Philosophy, logic and ethics, among others "@en-GB;
	skos:inScheme <http://cv.iptc.org/newscodes/subjectcode/>;
	skos:closeMatch medtop:20000751;
	skos:broader	subj:13000000.

subj:13006000
	rdf:type skos:Concept;
	skos:prefLabel	"research"@en-GB;
	skos:definition	"Methodical investigation of events, procedures etc to explain why they occur, or to find solutions for problems "@en-GB;
	skos:inScheme <http://cv.iptc.org/newscodes/subjectcode/>;
	skos:exactMatch medtop:20000735;
	skos:broader	subj:13000000;
	skos:narrower	subj:13006001.

subj:13006001
	rdf:type skos:Concept;
	skos:prefLabel	"survey"@en-GB;
	skos:definition	"Examination of public attitudes on various subjects or issues, such as the quality of goods, the value of services etc. "@en-GB;
	skos:inScheme <http://cv.iptc.org/newscodes/subjectcode/>;
	skos:closeMatch medtop:20000735;
	skos:broader	subj:13006000.

subj:13007000
	rdf:type skos:Concept;
	skos:prefLabel	"scientific exploration"@en-GB;
	skos:definition	"Methodical land, sea and space journeys to discover new information about them "@en-GB;
	skos:inScheme <http://cv.iptc.org/newscodes/subjectcode/>;
	skos:exactMatch medtop:20000738;
	skos:broader	subj:13000000.

subj:13008000
	rdf:type skos:Concept;
	skos:prefLabel	"space programme"@en-GB;
	skos:definition	"The government's organized effort for the exploration of outer space and the bodies therein "@en-GB;
	skos:inScheme <http://cv.iptc.org/newscodes/subjectcode/>;
	skos:exactMatch medtop:20000739;
	skos:broader	subj:13000000.

subj:13009000
	rdf:type skos:Concept;
	skos:prefLabel	"science (general)"@en-GB;
	skos:definition	"Establishing and systematizing information about nature and the physical world through observation, experimentation and hypothesis "@en-GB;
	skos:inScheme <http://cv.iptc.org/newscodes/subjectcode/>;
	skos:broadMatch medtop:13000000;
	skos:broader	subj:13000000.

subj:13010000
	rdf:type skos:Concept;
	skos:prefLabel	"technology (general)"@en-GB;
	skos:definition	"The study of the practical or industrial arts, and applied sciences such as physics, hydrodynamics and thermodynamics "@en-GB;
	skos:inScheme <http://cv.iptc.org/newscodes/subjectcode/>;
	skos:broadMatch medtop:20000756;
	skos:broader	subj:13000000;
	skos:narrower	subj:13010001;
	skos:narrower	subj:13010002.

subj:13010001
	rdf:type skos:Concept;
	skos:prefLabel	"rocketry"@en-GB;
	skos:definition	"The development of rockets "@en-GB;
	skos:inScheme <http://cv.iptc.org/newscodes/subjectcode/>;
	skos:exactMatch medtop:20000758;
	skos:broader	subj:13010000.

subj:13010002
	rdf:type skos:Concept;
	skos:prefLabel	"laser"@en-GB;
	skos:definition	"The development and use of light amplification by stimulated emission of radiation "@en-GB;
	skos:inScheme <http://cv.iptc.org/newscodes/subjectcode/>;
	skos:broadMatch medtop:13000000;
	skos:broader	subj:13010000.

subj:13011000
	rdf:type skos:Concept;
	skos:prefLabel	"standards"@en-GB;
	skos:definition	"The rules, national and international, that govern science and technology. These might include international standards setting for equipment and interference standards. "@en-GB;
	skos:inScheme <http://cv.iptc.org/newscodes/subjectcode/>;
	skos:exactMatch medtop:20000755;
	skos:broader	subj:13000000.

subj:13012000
	rdf:type skos:Concept;
	skos:prefLabel	"animal science"@en-GB;
	skos:definition	"Science involving animals "@en-GB;
	skos:inScheme <http://cv.iptc.org/newscodes/subjectcode/>;
	skos:exactMatch medtop:20000724;
	skos:broader	subj:13000000.

subj:13013000
	rdf:type skos:Concept;
	skos:prefLabel	"micro science"@en-GB;
	skos:definition	"The multi-disciplinary areas of nanotechnology and Micro-Electrical Mechanical Systems. "@en-GB;
	skos:inScheme <http://cv.iptc.org/newscodes/subjectcode/>;
	skos:exactMatch medtop:20000765;
	skos:broader	subj:13000000.

subj:13014000
	rdf:type skos:Concept;
	skos:prefLabel	"marine science"@en-GB;
	skos:definition	"The multi-disciplinary research areas involving the worlds' waterways and oceans. This could include hyper-spectral sensing of ice flows, fisheries studies and underwater research. "@en-GB;
	skos:inScheme <http://cv.iptc.org/newscodes/subjectcode/>;
	skos:exactMatch medtop:20000729;
	skos:broader	subj:13000000.

subj:13015000
	rdf:type skos:Concept;
	skos:prefLabel	"weather science"@en-GB;
	skos:definition	"All scientific aspects of the weather and climate. "@en-GB;
	skos:inScheme <http://cv.iptc.org/newscodes/subjectcode/>;
	skos:exactMatch medtop:20000730;
	skos:broader	subj:13000000.

subj:13016000
	rdf:type skos:Concept;
	skos:prefLabel	"electronics"@en-GB;
	skos:definition	"The branch of engineering or physics concerned with the controlled flow of electrons or other carriers of electric charges, especially in semiconductor devices, including the design, manufacture, and maintenance of electronic devices "@en-GB;
	skos:inScheme <http://cv.iptc.org/newscodes/subjectcode/>;
	skos:exactMatch medtop:20000761;
	skos:broader	subj:13000000.

subj:13017000
	rdf:type skos:Concept;
	skos:prefLabel	"identification technology"@en-GB;
	skos:definition	"Includes biometrics, new computer-based identification cards, retinal scans, face scanning and mobile augmented reality systems (MARS) and other ways technology can identify individuals. Also technology vs. the privacy of personal information. "@en-GB;
	skos:inScheme <http://cv.iptc.org/newscodes/subjectcode/>;
	skos:exactMatch medtop:20000762;
	skos:broader	subj:13000000.

subj:13018000
	rdf:type skos:Concept;
	skos:prefLabel	"mathematics"@en-GB;
	skos:definition	"The study of quantities and shapes and their symbolic relationships. "@en-GB;
	skos:inScheme <http://cv.iptc.org/newscodes/subjectcode/>;
	skos:exactMatch medtop:20000715;
	skos:broader	subj:13000000.

subj:13019000
	rdf:type skos:Concept;
	skos:prefLabel	"biotechnology"@en-GB;
	skos:definition	"Manipulating natural organisms for scientific, medical or agricultural purposes "@en-GB;
	skos:inScheme <http://cv.iptc.org/newscodes/subjectcode/>;
	skos:exactMatch medtop:20000711;
	skos:broader	subj:13000000.

subj:13020000
	rdf:type skos:Concept;
	skos:prefLabel	"agricultural research and technology"@en-GB;
	skos:definition	"Pertaining to the growing of crops and management of farm animals "@en-GB;
	skos:inScheme <http://cv.iptc.org/newscodes/subjectcode/>;
	skos:closeMatch medtop:20000759;
	skos:broader	subj:13000000.

subj:13021000
	rdf:type skos:Concept;
	skos:prefLabel	"nanotechnology"@en-GB;
	skos:definition	"Manipulating objects at the molecular scale "@en-GB;
	skos:inScheme <http://cv.iptc.org/newscodes/subjectcode/>;
	skos:exactMatch medtop:20000766;
	skos:broader	subj:13000000.

subj:13022000
	rdf:type skos:Concept;
	skos:prefLabel	"IT/computer sciences"@en-GB;
	skos:definition	"The study and design of computer systems and networks. "@en-GB;
	skos:inScheme <http://cv.iptc.org/newscodes/subjectcode/>;
	skos:exactMatch medtop:20000763;
	skos:broader	subj:13000000.

subj:13023000
	rdf:type skos:Concept;
	skos:prefLabel	"scientific institutions"@en-GB;
	skos:definition	"Institutions that carry out or govern scientific work (e.g. National Academy of Arts and Sciences ) "@en-GB;
	skos:inScheme <http://cv.iptc.org/newscodes/subjectcode/>;
	skos:exactMatch medtop:20000741;
	skos:broader	subj:13000000.

subj:14000000
	rdf:type skos:Concept;
	skos:prefLabel	"social issue"@en-GB;
	skos:definition	"Aspects of the behaviour of humans affecting the quality of life. "@en-GB;
	skos:inScheme <http://cv.iptc.org/newscodes/subjectcode/>;
	skos:closeMatch medtop:14000000;
	skos:narrower	subj:14001000;
	skos:narrower	subj:14002000;
	skos:narrower	subj:14003000;
	skos:narrower	subj:14004000;
	skos:narrower	subj:14005000;
	skos:narrower	subj:14006000;
	skos:narrower	subj:14007000;
	skos:narrower	subj:14008000;
	skos:narrower	subj:14009000;
	skos:narrower	subj:14010000;
	skos:narrower	subj:14011000;
	skos:narrower	subj:14012000;
	skos:narrower	subj:14013000;
	skos:narrower	subj:14014000;
	skos:narrower	subj:14015000;
	skos:narrower	subj:14016000;
	skos:narrower	subj:14017000;
	skos:narrower	subj:14018000;
	skos:narrower	subj:14019000;
	skos:narrower	subj:14020000;
	skos:narrower	subj:14021000;
	skos:narrower	subj:14022000;
	skos:narrower	subj:14023000;
	skos:narrower	subj:14024000;
	skos:narrower	subj:14025000;
	skos:narrower	subj:14026000;
	skos:narrower	subj:14027000.

subj:14001000
	rdf:type skos:Concept;
	skos:prefLabel	"addiction"@en-GB;
	skos:definition	"The habitual and often uncontrollable use of harmful substances such as alcohol, tobacco and pharmaceuticals or drugs "@en-GB;
	skos:inScheme <http://cv.iptc.org/newscodes/subjectcode/>;
	skos:exactMatch medtop:20000804;
	skos:broader	subj:14000000.

subj:14002000
	rdf:type skos:Concept;
	skos:prefLabel	"charity"@en-GB;
	skos:definition	"Philanthropic giving "@en-GB;
	skos:inScheme <http://cv.iptc.org/newscodes/subjectcode/>;
	skos:exactMatch medtop:20000818;
	skos:broader	subj:14000000.

subj:14003000
	rdf:type skos:Concept;
	skos:prefLabel	"demographics"@en-GB;
	skos:definition	"The study of people and here they live and how they interact "@en-GB;
	skos:inScheme <http://cv.iptc.org/newscodes/subjectcode/>;
	skos:exactMatch medtop:20000770;
	skos:broader	subj:14000000;
	skos:narrower	subj:14003001;
	skos:narrower	subj:14003002;
	skos:narrower	subj:14003003;
	skos:narrower	subj:14003004.

subj:14003001
	rdf:type skos:Concept;
	skos:prefLabel	"population and census"@en-GB;
	skos:definition	"Population is the number of people in a geographical region and census is the process of counting them "@en-GB;
	skos:inScheme <http://cv.iptc.org/newscodes/subjectcode/>;
	skos:exactMatch medtop:20000774;
	skos:broader	subj:14003000.

subj:14003002
	rdf:type skos:Concept;
	skos:prefLabel	"immigration"@en-GB;
	skos:definition	"Movement of individuals from one country to the other "@en-GB;
	skos:inScheme <http://cv.iptc.org/newscodes/subjectcode/>;
	skos:exactMatch medtop:20000771;
	skos:broader	subj:14003000.

subj:14003003
	rdf:type skos:Concept;
	skos:prefLabel	"illegal immigrants"@en-GB;
	skos:definition	"Movement of individuals from one country to the other by illicit means "@en-GB;
	skos:inScheme <http://cv.iptc.org/newscodes/subjectcode/>;
	skos:exactMatch medtop:20000773;
	skos:broader	subj:14003000.

subj:14003004
	rdf:type skos:Concept;
	skos:prefLabel	"emigrants"@en-GB;
	skos:definition	"People who leave their country of origin, their relationship with their country of origin and their association with fellow emigrants "@en-GB;
	skos:inScheme <http://cv.iptc.org/newscodes/subjectcode/>;
	skos:exactMatch medtop:20000772;
	skos:broader	subj:14003000.

subj:14004000
	rdf:type skos:Concept;
	skos:prefLabel	"disabled"@en-GB;
	skos:definition	"Being incapacitated either physically, emotionally or mentally "@en-GB;
	skos:inScheme <http://cv.iptc.org/newscodes/subjectcode/>;
	skos:exactMatch medtop:20000791;
	skos:broader	subj:14000000.

subj:14005000
	rdf:type skos:Concept;
	skos:prefLabel	"euthanasia (also includes assisted suicide)"@en-GB;
	skos:definition	"Voluntary death with the aid of another "@en-GB;
	skos:inScheme <http://cv.iptc.org/newscodes/subjectcode/>;
	skos:exactMatch medtop:20000811;
	skos:broader	subj:14000000;
	skos:narrower	subj:14005001.

subj:14005001
	rdf:type skos:Concept;
	skos:prefLabel	"suicide"@en-GB;
	skos:definition	"Death by one's own hand "@en-GB;
	skos:inScheme <http://cv.iptc.org/newscodes/subjectcode/>;
	skos:exactMatch medtop:20000813;
	skos:broader	subj:14005000.

subj:14006000
	rdf:type skos:Concept;
	skos:prefLabel	"family"@en-GB;
	skos:definition	"A group of individuals related by blood or marriage "@en-GB;
	skos:inScheme <http://cv.iptc.org/newscodes/subjectcode/>;
	skos:exactMatch medtop:20000780;
	skos:broader	subj:14000000;
	skos:narrower	subj:14006001;
	skos:narrower	subj:14006002;
	skos:narrower	subj:14006003;
	skos:narrower	subj:14006004;
	skos:narrower	subj:14006005;
	skos:narrower	subj:14006006.

subj:14006001
	rdf:type skos:Concept;
	skos:prefLabel	"parent and child"@en-GB;
	skos:definition	"Two or more individuals with a hierarchical familial relationship "@en-GB;
	skos:inScheme <http://cv.iptc.org/newscodes/subjectcode/>;
	skos:exactMatch medtop:20000787;
	skos:broader	subj:14006000.

subj:14006002
	rdf:type skos:Concept;
	skos:prefLabel	"adoption"@en-GB;
	skos:definition	"A legal process of bringing a child with no supporting parents into a supportive union "@en-GB;
	skos:inScheme <http://cv.iptc.org/newscodes/subjectcode/>;
	skos:exactMatch medtop:20000781;
	skos:broader	subj:14006000.

subj:14006003
	rdf:type skos:Concept;
	skos:prefLabel	"marriage"@en-GB;
	skos:definition	"The union of two individuals who pledge fidelity, respect and support for each other "@en-GB;
	skos:inScheme <http://cv.iptc.org/newscodes/subjectcode/>;
	skos:exactMatch medtop:20000786;
	skos:broader	subj:14006000.

subj:14006004
	rdf:type skos:Concept;
	skos:prefLabel	"divorce"@en-GB;
	skos:definition	"The process by which a marriage is dissolved "@en-GB;
	skos:inScheme <http://cv.iptc.org/newscodes/subjectcode/>;
	skos:exactMatch medtop:20000783;
	skos:broader	subj:14006000.

subj:14006005
	rdf:type skos:Concept;
	skos:prefLabel	"sex"@en-GB;
	skos:definition	"The classification of individuals as either male or female. Or conjugal relationship between two individuals. "@en-GB;
	skos:inScheme <http://cv.iptc.org/newscodes/subjectcode/>;
	skos:closeMatch medtop:20000816;
	skos:broader	subj:14006000.

subj:14006006
	rdf:type skos:Concept;
	skos:prefLabel	"courtship"@en-GB;
	skos:definition	"Preliminaries of wooing and winning a partner "@en-GB;
	skos:inScheme <http://cv.iptc.org/newscodes/subjectcode/>;
	skos:exactMatch medtop:20000782;
	skos:broader	subj:14006000.

subj:14007000
	rdf:type skos:Concept;
	skos:prefLabel	"family planning"@en-GB;
	skos:definition	"Conscious decisions and efforts involving reproduction "@en-GB;
	skos:inScheme <http://cv.iptc.org/newscodes/subjectcode/>;
	skos:exactMatch medtop:20000784;
	skos:broader	subj:14000000.

subj:14008000
	rdf:type skos:Concept;
	skos:prefLabel	"health insurance"@en-GB;
	skos:definition	"Insurance covering extraordinary medical costs "@en-GB;
	skos:inScheme <http://cv.iptc.org/newscodes/subjectcode/>;
	skos:exactMatch medtop:20000483;
	skos:broader	subj:14000000.

subj:14009000
	rdf:type skos:Concept;
	skos:prefLabel	"homelessness"@en-GB;
	skos:definition	"Lacking a fixed place of residence "@en-GB;
	skos:inScheme <http://cv.iptc.org/newscodes/subjectcode/>;
	skos:exactMatch medtop:20000800;
	skos:broader	subj:14000000.

subj:14010000
	rdf:type skos:Concept;
	skos:prefLabel	"minority group"@en-GB;
	skos:definition	"A group of people classified by race, language, religion or other characteristic numerically smaller than others of the same classification "@en-GB;
	skos:inScheme <http://cv.iptc.org/newscodes/subjectcode/>;
	skos:closeMatch medtop:20000795;
	skos:broader	subj:14000000;
	skos:narrower	subj:14010001;
	skos:narrower	subj:14010002.

subj:14010001
	rdf:type skos:Concept;
	skos:prefLabel	"gays and lesbians"@en-GB;
	skos:definition	"Those that consider themselves attracted to their same gender in an erotic or sensual or similar way. "@en-GB;
	skos:inScheme <http://cv.iptc.org/newscodes/subjectcode/>;
	skos:exactMatch medtop:20000792;
	skos:broader	subj:14010000.

subj:14010002
	rdf:type skos:Concept;
	skos:prefLabel	"national or ethnic minority"@en-GB;
	skos:definition	"Groups of people that form a minority on ethnic or national basis, their status, problems and relations to the majority "@en-GB;
	skos:inScheme <http://cv.iptc.org/newscodes/subjectcode/>;
	skos:exactMatch medtop:20000795;
	skos:broader	subj:14010000.

subj:14011000
	rdf:type skos:Concept;
	skos:prefLabel	"pornography"@en-GB;
	skos:definition	"Audio or visual depictions of various sex related acts considered outside accepted community standards "@en-GB;
	skos:inScheme <http://cv.iptc.org/newscodes/subjectcode/>;
	skos:exactMatch medtop:20000815;
	skos:broader	subj:14000000.

subj:14012000
	rdf:type skos:Concept;
	skos:prefLabel	"poverty"@en-GB;
	skos:definition	"Having insufficient resources to provide for basic services to oneself or family "@en-GB;
	skos:inScheme <http://cv.iptc.org/newscodes/subjectcode/>;
	skos:exactMatch medtop:20000801;
	skos:broader	subj:14000000.

subj:14013000
	rdf:type skos:Concept;
	skos:prefLabel	"prostitution"@en-GB;
	skos:definition	"Sex for sale, either male or female, and those who profit from it "@en-GB;
	skos:inScheme <http://cv.iptc.org/newscodes/subjectcode/>;
	skos:exactMatch medtop:20000806;
	skos:broader	subj:14000000.

subj:14014000
	rdf:type skos:Concept;
	skos:prefLabel	"racism"@en-GB;
	skos:definition	"Harmful attitudes toward another group based on racial differences "@en-GB;
	skos:inScheme <http://cv.iptc.org/newscodes/subjectcode/>;
	skos:exactMatch medtop:20000777;
	skos:broader	subj:14000000.

subj:14015000
	rdf:type skos:Concept;
	skos:prefLabel	"welfare"@en-GB;
	skos:definition	"Generally government help for those in need of food, housing health and other services "@en-GB;
	skos:inScheme <http://cv.iptc.org/newscodes/subjectcode/>;
	skos:exactMatch medtop:20000817;
	skos:broader	subj:14000000.

subj:14016000
	rdf:type skos:Concept;
	skos:prefLabel	"abortion"@en-GB;
	skos:definition	"Usually the planned disruption of the process of reproduction of human life "@en-GB;
	skos:inScheme <http://cv.iptc.org/newscodes/subjectcode/>;
	skos:exactMatch medtop:20000785;
	skos:broader	subj:14000000.

subj:14017000
	rdf:type skos:Concept;
	skos:prefLabel	"missing person"@en-GB;
	skos:definition	"A person who is not where they are expected to be for a period of time "@en-GB;
	skos:inScheme <http://cv.iptc.org/newscodes/subjectcode/>;
	skos:exactMatch medtop:20000132;
	skos:broader	subj:14000000;
	skos:narrower	subj:14017001.

subj:14017001
	rdf:type skos:Concept;
	skos:prefLabel	"missing due to hostilities"@en-GB;
	skos:definition	"People, both civilian and military, missing during or after hostilities "@en-GB;
	skos:inScheme <http://cv.iptc.org/newscodes/subjectcode/>;
	skos:exactMatch medtop:20000061;
	skos:broader	subj:14017000.

subj:14018000
	rdf:type skos:Concept;
	skos:prefLabel	"long term care"@en-GB;
	skos:definition	"Extensive health care because of serious illness or disability "@en-GB;
	skos:inScheme <http://cv.iptc.org/newscodes/subjectcode/>;
	skos:exactMatch medtop:20000819;
	skos:broader	subj:14000000.

subj:14019000
	rdf:type skos:Concept;
	skos:prefLabel	"juvenile delinquency"@en-GB;
	skos:definition	"Incidents involving perpetrators who are minors. "@en-GB;
	skos:inScheme <http://cv.iptc.org/newscodes/subjectcode/>;
	skos:exactMatch medtop:20000805;
	skos:broader	subj:14000000.

subj:14020000
	rdf:type skos:Concept;
	skos:prefLabel	"nuclear radiation victims"@en-GB;
	skos:definition	"Includes antinuclear movements and compensation for atomic blast victims. "@en-GB;
	skos:inScheme <http://cv.iptc.org/newscodes/subjectcode/>;
	skos:exactMatch medtop:20000796;
	skos:broader	subj:14000000.

subj:14021000
	rdf:type skos:Concept;
	skos:prefLabel	"slavery"@en-GB;
	skos:definition	"The involuntary servitude, outside of legal incarceration for statuary criminal offences, of men, women and children, including involuntary unpaid labour, coerced actions, child labour "@en-GB;
	skos:inScheme <http://cv.iptc.org/newscodes/subjectcode/>;
	skos:exactMatch medtop:20000807;
	skos:broader	subj:14000000.

subj:14022000
	rdf:type skos:Concept;
	skos:prefLabel	"abusive behaviour"@en-GB;
	skos:definition	"The maltreatment of one or more individuals by others through dehumanizing treatment including sexual or mental abuse, deprivation of sensory abilities, deprivation of physical needs, physical mistreatment including beatings, and other forms of torture "@en-GB;
	skos:inScheme <http://cv.iptc.org/newscodes/subjectcode/>;
	skos:exactMatch medtop:20000803;
	skos:broader	subj:14000000.

subj:14023000
	rdf:type skos:Concept;
	skos:prefLabel	"death and dying"@en-GB;
	skos:definition	"Dying is the route to death. Death is the state you are in when there are no signs that you can function as a human being either physically or mentally "@en-GB;
	skos:inScheme <http://cv.iptc.org/newscodes/subjectcode/>;
	skos:closeMatch medtop:20000810;
	skos:broader	subj:14000000.

subj:14024000
	rdf:type skos:Concept;
	skos:prefLabel	"people"@en-GB;
	skos:definition	"Individuals as a whole, sometimes broken down into various classes, such as indigenous people, people of class etc "@en-GB;
	skos:inScheme <http://cv.iptc.org/newscodes/subjectcode/>;
	skos:closeMatch medtop:20000788;
	skos:broader	subj:14000000;
	skos:narrower	subj:14024001;
	skos:narrower	subj:14024002;
	skos:narrower	subj:14024003;
	skos:narrower	subj:14024004;
	skos:narrower	subj:14024005.

subj:14024001
	rdf:type skos:Concept;
	skos:prefLabel	"children"@en-GB;
	skos:definition	"Immature people, usually up to the age of puberty "@en-GB;
	skos:inScheme <http://cv.iptc.org/newscodes/subjectcode/>;
	skos:exactMatch medtop:20000790;
	skos:broader	subj:14024000.

subj:14024002
	rdf:type skos:Concept;
	skos:prefLabel	"infants"@en-GB;
	skos:definition	"Those people from birth until ages of one or two, usually when they begin walking "@en-GB;
	skos:inScheme <http://cv.iptc.org/newscodes/subjectcode/>;
	skos:exactMatch medtop:20000794;
	skos:broader	subj:14024000.

subj:14024003
	rdf:type skos:Concept;
	skos:prefLabel	"teen-agers"@en-GB;
	skos:definition	"People aged 13 to 19 years of age "@en-GB;
	skos:inScheme <http://cv.iptc.org/newscodes/subjectcode/>;
	skos:exactMatch medtop:20000798;
	skos:broader	subj:14024000.

subj:14024004
	rdf:type skos:Concept;
	skos:prefLabel	"adults"@en-GB;
	skos:definition	"People aged 20 and above "@en-GB;
	skos:inScheme <http://cv.iptc.org/newscodes/subjectcode/>;
	skos:exactMatch medtop:20000789;
	skos:broader	subj:14024000.

subj:14024005
	rdf:type skos:Concept;
	skos:prefLabel	"senior citizens"@en-GB;
	skos:definition	"People aged 60 or 65 and older "@en-GB;
	skos:inScheme <http://cv.iptc.org/newscodes/subjectcode/>;
	skos:exactMatch medtop:20000797;
	skos:broader	subj:14024000.

subj:14025000
	rdf:type skos:Concept;
	skos:prefLabel	"social issues (general)"@en-GB;
	skos:definition	"Issues affecting a number of individuals in their daily lives like housing, food, education, personal relationships "@en-GB;
	skos:inScheme <http://cv.iptc.org/newscodes/subjectcode/>;
	skos:exactMatch medtop:14000000;
	skos:broader	subj:14000000;
	skos:narrower	subj:14025001;
	skos:narrower	subj:14025002;
	skos:narrower	subj:14025003;
	skos:narrower	subj:14025004;
	skos:narrower	subj:14025005.

subj:14025001
	rdf:type skos:Concept;
	skos:prefLabel	"social conditions"@en-GB;
	skos:definition	"Conditions under which people live in terms of housing, water supply, availability of education "@en-GB;
	skos:inScheme <http://cv.iptc.org/newscodes/subjectcode/>;
	skos:exactMatch medtop:20000799;
	skos:broader	subj:14025000.

subj:14025002
	rdf:type skos:Concept;
	skos:prefLabel	"social problems"@en-GB;
	skos:definition	"Issues affecting the lives of individuals such as housing, education nutrition, communication etc "@en-GB;
	skos:inScheme <http://cv.iptc.org/newscodes/subjectcode/>;
	skos:closeMatch medtop:20000802;
	skos:broader	subj:14025000.

subj:14025003
	rdf:type skos:Concept;
	skos:prefLabel	"discrimination"@en-GB;
	skos:definition	"Denial of services to one or more people because of race, colour, sexual identity, religion, political beliefs etc "@en-GB;
	skos:inScheme <http://cv.iptc.org/newscodes/subjectcode/>;
	skos:exactMatch medtop:20000775;
	skos:broader	subj:14025000.

subj:14025004
	rdf:type skos:Concept;
	skos:prefLabel	"social services"@en-GB;
	skos:definition	"Government supported programs to improve the well-being of individuals or groups of individuals "@en-GB;
	skos:inScheme <http://cv.iptc.org/newscodes/subjectcode/>;
	skos:closeMatch medtop:20000820;
	skos:broader	subj:14025000.

subj:14025005
	rdf:type skos:Concept;
	skos:prefLabel	"death penalty policies"@en-GB;
	skos:definition	"National or international polices regarding death sentences "@en-GB;
	skos:inScheme <http://cv.iptc.org/newscodes/subjectcode/>;
	skos:closeMatch medtop:20000135;
	skos:broader	subj:14025000.

subj:14026000
	rdf:type skos:Concept;
	skos:prefLabel	"ordnance clearance"@en-GB;
	skos:definition	"The removal or neutralization of ordnance such as landmines or cluster bombs, remaining after a war or armed conflict "@en-GB;
	skos:inScheme <http://cv.iptc.org/newscodes/subjectcode/>;
	skos:exactMatch medtop:20000079;
	skos:broader	subj:14000000.

subj:14027000
	rdf:type skos:Concept;
	skos:prefLabel	"reconstruction"@en-GB;
	skos:definition	"The reconstruction of economy, infrastructure and property, as well as life in general, after a war or natural disaster "@en-GB;
	skos:inScheme <http://cv.iptc.org/newscodes/subjectcode/>;
	skos:closeMatch medtop:20000077;
	skos:broader	subj:14000000.

subj:15000000
	rdf:type skos:Concept;
	skos:prefLabel	"sport"@en-GB;
	skos:definition	"Competitive exercise involving physical effort. Organizations and bodies involved in these activities. "@en-GB;
	skos:inScheme <http://cv.iptc.org/newscodes/subjectcode/>;
	skos:exactMatch medtop:15000000;
	skos:narrower	subj:15001000;
	skos:narrower	subj:15002000;
	skos:narrower	subj:15003000;
	skos:narrower	subj:15004000;
	skos:narrower	subj:15005000;
	skos:narrower	subj:15006000;
	skos:narrower	subj:15007000;
	skos:narrower	subj:15008000;
	skos:narrower	subj:15009000;
	skos:narrower	subj:15010000;
	skos:narrower	subj:15011000;
	skos:narrower	subj:15012000;
	skos:narrower	subj:15013000;
	skos:narrower	subj:15014000;
	skos:narrower	subj:15015000;
	skos:narrower	subj:15016000;
	skos:narrower	subj:15017000;
	skos:narrower	subj:15018000;
	skos:narrower	subj:15019000;
	skos:narrower	subj:15020000;
	skos:narrower	subj:15021000;
	skos:narrower	subj:15022000;
	skos:narrower	subj:15023000;
	skos:narrower	subj:15024000;
	skos:narrower	subj:15025000;
	skos:narrower	subj:15026000;
	skos:narrower	subj:15027000;
	skos:narrower	subj:15028000;
	skos:narrower	subj:15029000;
	skos:narrower	subj:15030000;
	skos:narrower	subj:15031000;
	skos:narrower	subj:15032000;
	skos:narrower	subj:15033000;
	skos:narrower	subj:15034000;
	skos:narrower	subj:15035000;
	skos:narrower	subj:15036000;
	skos:narrower	subj:15037000;
	skos:narrower	subj:15038000;
	skos:narrower	subj:15039000;
	skos:narrower	subj:15040000;
	skos:narrower	subj:15041000;
	skos:narrower	subj:15042000;
	skos:narrower	subj:15043000;
	skos:narrower	subj:15044000;
	skos:narrower	subj:15045000;
	skos:narrower	subj:15046000;
	skos:narrower	subj:15047000;
	skos:narrower	subj:15048000;
	skos:narrower	subj:15049000;
	skos:narrower	subj:15050000;
	skos:narrower	subj:15051000;
	skos:narrower	subj:15052000;
	skos:narrower	subj:15053000;
	skos:narrower	subj:15054000;
	skos:narrower	subj:15055000;
	skos:narrower	subj:15056000;
	skos:narrower	subj:15057000;
	skos:narrower	subj:15058000;
	skos:narrower	subj:15059000;
	skos:narrower	subj:15060000;
	skos:narrower	subj:15061000;
	skos:narrower	subj:15062000;
	skos:narrower	subj:15063000;
	skos:narrower	subj:15064000;
	skos:narrower	subj:15065000;
	skos:narrower	subj:15066000;
	skos:narrower	subj:15067000;
	skos:narrower	subj:15068000;
	skos:narrower	subj:15069000;
	skos:narrower	subj:15070000;
	skos:narrower	subj:15071000;
	skos:narrower	subj:15072000;
	skos:narrower	subj:15073000;
	skos:narrower	subj:15074000;
	skos:narrower	subj:15075000;
	skos:narrower	subj:15076000;
	skos:narrower	subj:15077000;
	skos:narrower	subj:15078000;
	skos:narrower	subj:15079000;
	skos:narrower	subj:15080000;
	skos:narrower	subj:15081000;
	skos:narrower	subj:15082000;
	skos:narrower	subj:15083000;
	skos:narrower	subj:15084000;
	skos:narrower	subj:15085000;
	skos:narrower	subj:15086000;
	skos:narrower	subj:15087000;
	skos:narrower	subj:15088000;
	skos:narrower	subj:15089000;
	skos:narrower	subj:15090000;
	skos:narrower	subj:15091000;
	skos:narrower	subj:15092000;
	skos:narrower	subj:15093000;
	skos:narrower	subj:15094000;
	skos:narrower	subj:15095000;
	skos:narrower	subj:15096000;
	skos:narrower	subj:15097000;
	skos:narrower	subj:15098000;
	skos:narrower	subj:15099000;
	skos:narrower	subj:15100000;
	skos:narrower	subj:15101000;
	skos:narrower	subj:15102000;
	skos:narrower	subj:15103000.

subj:15001000
	rdf:type skos:Concept;
	skos:prefLabel	"aero and aviation sport"@en-GB;
	skos:definition	"Parachuting, freefall (parapente, delta-plane), gliding, aerostat, motorised flight (airplane, ultra light craft, helicopter) "@en-GB;
	skos:inScheme <http://cv.iptc.org/newscodes/subjectcode/>;
	skos:broadMatch medtop:15000000;
	skos:broader	subj:15000000;
	skos:narrower	subj:15001001;
	skos:narrower	subj:15001002.

subj:15001001
	rdf:type skos:Concept;
	skos:prefLabel	"parachuting"@en-GB;
	skos:definition	"Parachuting competitions: precision landings, voltige, individual and team "@en-GB;
	skos:inScheme <http://cv.iptc.org/newscodes/subjectcode/>;
	skos:exactMatch medtop:20001013;
	skos:broader	subj:15001000.

subj:15001002
	rdf:type skos:Concept;
	skos:prefLabel	"sky diving"@en-GB;
	skos:definition	"Parachuting competitions involving sky-diving "@en-GB;
	skos:inScheme <http://cv.iptc.org/newscodes/subjectcode/>;
	skos:exactMatch medtop:20001062;
	skos:broader	subj:15001000.

subj:15002000
	rdf:type skos:Concept;
	skos:prefLabel	"alpine skiing"@en-GB;
	skos:definition	"Skiing downhill on snow-covered slopes as fast as possible. The slopes contain intermediate gates which are spaced according to the discipline involved "@en-GB;
	skos:inScheme <http://cv.iptc.org/newscodes/subjectcode/>;
	skos:exactMatch medtop:20001057;
	skos:broader	subj:15000000;
	skos:narrower	subj:15002001;
	skos:narrower	subj:15002002;
	skos:narrower	subj:15002003;
	skos:narrower	subj:15002004;
	skos:narrower	subj:15002005.

subj:15002001
	rdf:type skos:Concept;
	skos:prefLabel	"downhill"@en-GB;
	skos:definition	"Skiing at top speed down a steep slope with interspersed turns but no gates. The fastest wins. "@en-GB;
	skos:inScheme <http://cv.iptc.org/newscodes/subjectcode/>;
	skos:broadMatch medtop:20001057;
	skos:broader	subj:15002000.

subj:15002002
	rdf:type skos:Concept;
	skos:prefLabel	"giant slalom"@en-GB;
	skos:definition	"Skiing down a slope, but with more turns and bends than in super-G skiing. The fastest wins. "@en-GB;
	skos:historyNote	"typo fixed in Explanation "@en-GB;
	skos:inScheme <http://cv.iptc.org/newscodes/subjectcode/>;
	skos:broadMatch medtop:20001057;
	skos:broader	subj:15002000.

subj:15002003
	rdf:type skos:Concept;
	skos:prefLabel	"super G"@en-GB;
	skos:definition	"Skiing down a steep slope, but with more turns and bends than in the downhill. The fastest wins. "@en-GB;
	skos:inScheme <http://cv.iptc.org/newscodes/subjectcode/>;
	skos:broadMatch medtop:20001057;
	skos:broader	subj:15002000.

subj:15002004
	rdf:type skos:Concept;
	skos:prefLabel	"slalom"@en-GB;
	skos:definition	"Skiers must zig-zag their way down a slope with closely positioned gates which they must negotiate. It is run over two legs with the combined fastest winning. "@en-GB;
	skos:inScheme <http://cv.iptc.org/newscodes/subjectcode/>;
	skos:broadMatch medtop:20001057;
	skos:broader	subj:15002000.

subj:15002005
	rdf:type skos:Concept;
	skos:prefLabel	"combined"@en-GB;
	skos:definition	"Race, usually competed over two days that combines a downhill leg and a slalom leg rewarding the most complete skiers. Combined fastest time wins. "@en-GB;
	skos:inScheme <http://cv.iptc.org/newscodes/subjectcode/>;
	skos:broadMatch medtop:20001057;
	skos:broader	subj:15002000.

subj:15003000
	rdf:type skos:Concept;
	skos:prefLabel	"American football"@en-GB;
	skos:definition	"Team ball game that opposes two teams that have attack sections and defence sections. Each attack goes up against the other defence and attempts to move an oval-shaped ball down the field and into the end-zone to mark a touchdown and earn points. "@en-GB;
	skos:inScheme <http://cv.iptc.org/newscodes/subjectcode/>;
	skos:exactMatch medtop:20000823;
	skos:broader	subj:15000000;
	skos:narrower	subj:15003001;
	skos:narrower	subj:15003002;
	skos:narrower	subj:15003003.

subj:15003001
	rdf:type skos:Concept;
	skos:prefLabel	"(US) National Football League (NFL) (North American)"@en-GB;
	skos:definition	"The association of professional American football teams "@en-GB;
	skos:inScheme <http://cv.iptc.org/newscodes/subjectcode/>;
	skos:broadMatch medtop:20000823;
	skos:broader	subj:15003000.

subj:15003002
	rdf:type skos:Concept;
	skos:prefLabel	"CFL"@en-GB;
	skos:definition	"The Canadian Football League (CFL), also known as Ligue Canadienne de Football (LCF), is a professional league located entirely in Canada that plays Canadian football. "@en-GB;
	skos:historyNote	"re-added, with corresponding explanation "@en-GB;
	skos:inScheme <http://cv.iptc.org/newscodes/subjectcode/>;
	skos:broadMatch medtop:20000876;
	skos:broader	subj:15003000.

subj:15003003
	rdf:type skos:Concept;
	skos:prefLabel	"AFL-DEPRECATED"@en-GB;
	skos:definition	"The American Football League (AFL) was a professional league of American football that operated from 1960 to 1969. In 1970, the AFL merged with the National Football League. "@en-GB;
	skos:historyNote	"explanation fixed - and code deprecated "@en-GB;
	skos:inScheme <http://cv.iptc.org/newscodes/subjectcode/>;
	skos:broadMatch medtop:20000823;
	skos:broader	subj:15003000.

subj:15004000
	rdf:type skos:Concept;
	skos:prefLabel	"archery"@en-GB;
	skos:definition	"Archers use bows and arrows to aim at targets 1.22 metres in diameter which are on average 70 metres distant. "@en-GB;
	skos:historyNote	"typo fixed in Explanation "@en-GB;
	skos:inScheme <http://cv.iptc.org/newscodes/subjectcode/>;
	skos:exactMatch medtop:20000824;
	skos:broader	subj:15000000;
	skos:narrower	subj:15004001;
	skos:narrower	subj:15004002.

subj:15004001
	rdf:type skos:Concept;
	skos:prefLabel	"FITA / Outdoor target archery"@en-GB;
	skos:definition	"The competition is held outdoors on an open (flat) field, at various fixed distances. The archery competition in the Olympic Games is a part of the FITA outdoor target archery program. "@en-GB;
	skos:inScheme <http://cv.iptc.org/newscodes/subjectcode/>;
	skos:broadMatch medtop:20000824;
	skos:broader	subj:15004000.

subj:15004002
	rdf:type skos:Concept;
	skos:prefLabel	"crossbow shooting"@en-GB;
	skos:definition	"Shooting with crossbow on targets from different distances "@en-GB;
	skos:inScheme <http://cv.iptc.org/newscodes/subjectcode/>;
	skos:exactMatch medtop:20000825;
	skos:broader	subj:15004000.

subj:15005000
	rdf:type skos:Concept;
	skos:prefLabel	"athletics, track and field"@en-GB;
	skos:definition	"Competitions involving foot races, jumping and throwing which can be on a track inside a stadium or on outside roads "@en-GB;
	skos:inScheme <http://cv.iptc.org/newscodes/subjectcode/>;
	skos:exactMatch medtop:20000827;
	skos:broader	subj:15000000;
	skos:narrower	subj:15005001;
	skos:narrower	subj:15005002;
	skos:narrower	subj:15005003;
	skos:narrower	subj:15005004;
	skos:narrower	subj:15005005;
	skos:narrower	subj:15005006;
	skos:narrower	subj:15005007;
	skos:narrower	subj:15005008;
	skos:narrower	subj:15005009;
	skos:narrower	subj:15005010;
	skos:narrower	subj:15005011;
	skos:narrower	subj:15005012;
	skos:narrower	subj:15005013;
	skos:narrower	subj:15005014;
	skos:narrower	subj:15005015;
	skos:narrower	subj:15005016;
	skos:narrower	subj:15005017;
	skos:narrower	subj:15005018;
	skos:narrower	subj:15005019;
	skos:narrower	subj:15005020;
	skos:narrower	subj:15005021;
	skos:narrower	subj:15005022;
	skos:narrower	subj:15005023;
	skos:narrower	subj:15005024;
	skos:narrower	subj:15005025;
	skos:narrower	subj:15005026;
	skos:narrower	subj:15005027;
	skos:narrower	subj:15005028;
	skos:narrower	subj:15005029;
	skos:narrower	subj:15005030;
	skos:narrower	subj:15005031;
	skos:narrower	subj:15005032;
	skos:narrower	subj:15005033;
	skos:narrower	subj:15005034;
	skos:narrower	subj:15005035;
	skos:narrower	subj:15005036;
	skos:narrower	subj:15005037;
	skos:narrower	subj:15005038;
	skos:narrower	subj:15005039;
	skos:narrower	subj:15005040;
	skos:narrower	subj:15005041;
	skos:narrower	subj:15005042;
	skos:narrower	subj:15005043;
	skos:narrower	subj:15005044;
	skos:narrower	subj:15005045;
	skos:narrower	subj:15005046;
	skos:narrower	subj:15005047;
	skos:narrower	subj:15005048;
	skos:narrower	subj:15005049;
	skos:narrower	subj:15005050;
	skos:narrower	subj:15005051;
	skos:narrower	subj:15005052;
	skos:narrower	subj:15005053;
	skos:narrower	subj:15005054;
	skos:narrower	subj:15005055;
	skos:narrower	subj:15005056;
	skos:narrower	subj:15005057;
	skos:narrower	subj:15005058;
	skos:narrower	subj:15005059;
	skos:narrower	subj:15005060;
	skos:narrower	subj:15005061;
	skos:narrower	subj:15005062;
	skos:narrower	subj:15005063;
	skos:narrower	subj:15005064;
	skos:narrower	subj:15005065;
	skos:narrower	subj:15005066;
	skos:narrower	subj:15005067;
	skos:narrower	subj:15005068;
	skos:narrower	subj:15005069.

subj:15005001
	rdf:type skos:Concept;
	skos:prefLabel	"100 m"@en-GB;
	skos:definition	"Running over a distance of 100 metres with the fastest time winning "@en-GB;
	skos:inScheme <http://cv.iptc.org/newscodes/subjectcode/>;
	skos:broadMatch medtop:20000844;
	skos:broader	subj:15005000.

subj:15005002
	rdf:type skos:Concept;
	skos:prefLabel	"200 m"@en-GB;
	skos:definition	"Running over a distance of 200 metres with the fastest time winning "@en-GB;
	skos:inScheme <http://cv.iptc.org/newscodes/subjectcode/>;
	skos:broadMatch medtop:20000844;
	skos:broader	subj:15005000.

subj:15005003
	rdf:type skos:Concept;
	skos:prefLabel	"400 m"@en-GB;
	skos:definition	"Running over a distance of 400 metres with the fastest time winning "@en-GB;
	skos:inScheme <http://cv.iptc.org/newscodes/subjectcode/>;
	skos:broadMatch medtop:20000844;
	skos:broader	subj:15005000.

subj:15005004
	rdf:type skos:Concept;
	skos:prefLabel	"800 m"@en-GB;
	skos:definition	"Running over a distance of 800 metres with the fastest time winning "@en-GB;
	skos:inScheme <http://cv.iptc.org/newscodes/subjectcode/>;
	skos:broadMatch medtop:20000838;
	skos:broader	subj:15005000.

subj:15005005
	rdf:type skos:Concept;
	skos:prefLabel	"1000 m"@en-GB;
	skos:definition	"Running over a distance of 1000 metres with the fastest time winning "@en-GB;
	skos:inScheme <http://cv.iptc.org/newscodes/subjectcode/>;
	skos:broadMatch medtop:20000838;
	skos:broader	subj:15005000.

subj:15005006
	rdf:type skos:Concept;
	skos:prefLabel	"1500 m"@en-GB;
	skos:definition	"Running over a distance of 1000 metres with the fastest time winning "@en-GB;
	skos:inScheme <http://cv.iptc.org/newscodes/subjectcode/>;
	skos:broadMatch medtop:20000838;
	skos:broader	subj:15005000.

subj:15005007
	rdf:type skos:Concept;
	skos:prefLabel	"mile"@en-GB;
	skos:definition	"Running over a distance of one mile with the fastest time winning "@en-GB;
	skos:historyNote	"typo fixed in Explanation "@en-GB;
	skos:inScheme <http://cv.iptc.org/newscodes/subjectcode/>;
	skos:broadMatch medtop:20000836;
	skos:broader	subj:15005000.

subj:15005008
	rdf:type skos:Concept;
	skos:prefLabel	"2000 m"@en-GB;
	skos:definition	"Running over a distance of 2000 metres with the fastest time winning "@en-GB;
	skos:inScheme <http://cv.iptc.org/newscodes/subjectcode/>;
	skos:broadMatch medtop:20000836;
	skos:broader	subj:15005000.

subj:15005009
	rdf:type skos:Concept;
	skos:prefLabel	"3000 m"@en-GB;
	skos:definition	"Running over a distance of 3000 metres with the fastest time winning "@en-GB;
	skos:inScheme <http://cv.iptc.org/newscodes/subjectcode/>;
	skos:broadMatch medtop:20000836;
	skos:broader	subj:15005000.

subj:15005010
	rdf:type skos:Concept;
	skos:prefLabel	"5000 m"@en-GB;
	skos:definition	"Running over a distance of 5000 metres with the fastest time winning "@en-GB;
	skos:inScheme <http://cv.iptc.org/newscodes/subjectcode/>;
	skos:broadMatch medtop:20000836;
	skos:broader	subj:15005000.

subj:15005011
	rdf:type skos:Concept;
	skos:prefLabel	"10,000 m"@en-GB;
	skos:definition	"Running over a distance of 10,000 metres with the fastest time winning "@en-GB;
	skos:inScheme <http://cv.iptc.org/newscodes/subjectcode/>;
	skos:broadMatch medtop:20000836;
	skos:broader	subj:15005000.

subj:15005012
	rdf:type skos:Concept;
	skos:prefLabel	"20 km"@en-GB;
	skos:definition	"Walking over a distance of 20 km on public roads with the fastest time winning "@en-GB;
	skos:inScheme <http://cv.iptc.org/newscodes/subjectcode/>;
	skos:broadMatch medtop:20000841;
	skos:broader	subj:15005000.

subj:15005013
	rdf:type skos:Concept;
	skos:prefLabel	"one hour"@en-GB;
	skos:definition	"Walking as far as possible in the time of one hour "@en-GB;
	skos:inScheme <http://cv.iptc.org/newscodes/subjectcode/>;
	skos:broadMatch medtop:20000841;
	skos:broader	subj:15005000.

subj:15005014
	rdf:type skos:Concept;
	skos:prefLabel	"25000"@en-GB;
	skos:definition	"Walking over a distance of 25km with the fastest time winning "@en-GB;
	skos:inScheme <http://cv.iptc.org/newscodes/subjectcode/>;
	skos:broadMatch medtop:20000841;
	skos:broader	subj:15005000.

subj:15005015
	rdf:type skos:Concept;
	skos:prefLabel	"30000"@en-GB;
	skos:definition	"Walking over a distance of 30kms with the fastest time winning "@en-GB;
	skos:inScheme <http://cv.iptc.org/newscodes/subjectcode/>;
	skos:broadMatch medtop:20000841;
	skos:broader	subj:15005000.

subj:15005016
	rdf:type skos:Concept;
	skos:prefLabel	"110 m hurdles"@en-GB;
	skos:definition	"Race consisting of covering 110 metres as fast as possible while jumping over 10 hurdles placed on the track "@en-GB;
	skos:inScheme <http://cv.iptc.org/newscodes/subjectcode/>;
	skos:broadMatch medtop:20000834;
	skos:broader	subj:15005000.

subj:15005017
	rdf:type skos:Concept;
	skos:prefLabel	"400 m hurdles"@en-GB;
	skos:definition	"Race consisting of covering 400 metres as fast as possible while jumping over 10 hurdles placed on the track "@en-GB;
	skos:inScheme <http://cv.iptc.org/newscodes/subjectcode/>;
	skos:broadMatch medtop:20000834;
	skos:broader	subj:15005000.

subj:15005018
	rdf:type skos:Concept;
	skos:prefLabel	"3000 m steeplechase"@en-GB;
	skos:definition	"Race consisting of covering 3000 metres as fast as possible while jumping over 28 hurdles which are 91/4 centimetres high and seven water obstacles "@en-GB;
	skos:inScheme <http://cv.iptc.org/newscodes/subjectcode/>;
	skos:broadMatch medtop:20000827;
	skos:broader	subj:15005000.

subj:15005019
	rdf:type skos:Concept;
	skos:prefLabel	"high jump"@en-GB;
	skos:definition	"Competitors jump as high as possible over a bar which is raised each time they clear the height. The highest clearance wins. "@en-GB;
	skos:inScheme <http://cv.iptc.org/newscodes/subjectcode/>;
	skos:exactMatch medtop:20000833;
	skos:broader	subj:15005000.

subj:15005020
	rdf:type skos:Concept;
	skos:prefLabel	"pole vault"@en-GB;
	skos:definition	"Competitors use a flexible pole to propel themselves feet-first into the air and clear a bar which is raised higher at each round of jumps. "@en-GB;
	skos:historyNote	"typo fixed in Explanation "@en-GB;
	skos:inScheme <http://cv.iptc.org/newscodes/subjectcode/>;
	skos:exactMatch medtop:20000840;
	skos:broader	subj:15005000.

subj:15005021
	rdf:type skos:Concept;
	skos:prefLabel	"long jump"@en-GB;
	skos:definition	"Competitors build up speed over a short sprint and them attempt to jump as far forward as they can from a given point into sand trap. The longest jump wins. "@en-GB;
	skos:inScheme <http://cv.iptc.org/newscodes/subjectcode/>;
	skos:exactMatch medtop:20000837;
	skos:broader	subj:15005000.

subj:15005022
	rdf:type skos:Concept;
	skos:prefLabel	"triple jump"@en-GB;
	skos:definition	"Competitors build up speed over a short sprint and then attempt to jump as far forward as they can using a hop, skip and a jump technique. The longest jump wins. "@en-GB;
	skos:historyNote	"typo fixed in Explanation "@en-GB;
	skos:inScheme <http://cv.iptc.org/newscodes/subjectcode/>;
	skos:exactMatch medtop:20000845;
	skos:broader	subj:15005000.

subj:15005023
	rdf:type skos:Concept;
	skos:prefLabel	"shot put"@en-GB;
	skos:definition	"Competitors stand in a circle with a 2.13 metres diameter and attempt to throw a metal ball weighing 7.26 kg for men and 4kg for women as far as possible. The longest throw wins. "@en-GB;
	skos:inScheme <http://cv.iptc.org/newscodes/subjectcode/>;
	skos:exactMatch medtop:20000843;
	skos:broader	subj:15005000.

subj:15005024
	rdf:type skos:Concept;
	skos:prefLabel	"discus throw"@en-GB;
	skos:definition	"Competitors stand in a netted circle with a 2.50 metres diameter and with a turning motion attempt to throw a discus weighing 2kg for men and 1kg for women as far as possible. The longest throw wins. "@en-GB;
	skos:inScheme <http://cv.iptc.org/newscodes/subjectcode/>;
	skos:exactMatch medtop:20000830;
	skos:broader	subj:15005000.

subj:15005025
	rdf:type skos:Concept;
	skos:prefLabel	"hammer throw"@en-GB;
	skos:definition	"Competitors throw a hammer consisting of a metal ball, chain and handle as far as they can from a netted circle which is 2.13 metres in diameter. The hammer weighs 7.26 kg for men and 4 kg for women. "@en-GB;
	skos:inScheme <http://cv.iptc.org/newscodes/subjectcode/>;
	skos:exactMatch medtop:20000831;
	skos:broader	subj:15005000.

subj:15005026
	rdf:type skos:Concept;
	skos:prefLabel	"javelin throw"@en-GB;
	skos:definition	"Competitors in a specially-designated throwing area attempt to fling a spear-like javelin as far as possible. The javelin weighs 800 grammes for men and 600 grammes for women. "@en-GB;
	skos:inScheme <http://cv.iptc.org/newscodes/subjectcode/>;
	skos:exactMatch medtop:20000835;
	skos:broader	subj:15005000.

subj:15005027
	rdf:type skos:Concept;
	skos:prefLabel	"decathlon"@en-GB;
	skos:definition	"Individual men's competition which involves accumulating points in 10 different disciplines over two days: 1st day - 100m, long-jump, shot-putt, high-jump, 400m. 2nd day - 110m hurdles, discus, pole-vault, javelin and 1,500 metres. "@en-GB;
	skos:historyNote	"typo fixed in Explanation "@en-GB;
	skos:inScheme <http://cv.iptc.org/newscodes/subjectcode/>;
	skos:exactMatch medtop:20000829;
	skos:broader	subj:15005000.

subj:15005028
	rdf:type skos:Concept;
	skos:prefLabel	"4x100 m"@en-GB;
	skos:definition	"Team race involving four runners each covering 100 metres. "@en-GB;
	skos:inScheme <http://cv.iptc.org/newscodes/subjectcode/>;
	skos:broadMatch medtop:20000842;
	skos:broader	subj:15005000.

subj:15005029
	rdf:type skos:Concept;
	skos:prefLabel	"4x200 m"@en-GB;
	skos:definition	"Team race involving four runners each covering 200 metres. "@en-GB;
	skos:inScheme <http://cv.iptc.org/newscodes/subjectcode/>;
	skos:broadMatch medtop:20000842;
	skos:broader	subj:15005000.

subj:15005030
	rdf:type skos:Concept;
	skos:prefLabel	"4x400 m"@en-GB;
	skos:definition	"Team race involving four runners each covering 400 metres. "@en-GB;
	skos:inScheme <http://cv.iptc.org/newscodes/subjectcode/>;
	skos:broadMatch medtop:20000842;
	skos:broader	subj:15005000.

subj:15005031
	rdf:type skos:Concept;
	skos:prefLabel	"4x800 m"@en-GB;
	skos:definition	"Team race involving four runners each covering 800 metres. "@en-GB;
	skos:inScheme <http://cv.iptc.org/newscodes/subjectcode/>;
	skos:broadMatch medtop:20000842;
	skos:broader	subj:15005000.

subj:15005032
	rdf:type skos:Concept;
	skos:prefLabel	"4x1500 m"@en-GB;
	skos:definition	"Team race involving four runners each covering 1500 metres. "@en-GB;
	skos:inScheme <http://cv.iptc.org/newscodes/subjectcode/>;
	skos:broadMatch medtop:20000842;
	skos:broader	subj:15005000.

subj:15005033
	rdf:type skos:Concept;
	skos:prefLabel	"walk 1 h"@en-GB;
	skos:definition	"One-hour long race where competitors must maintain at least one foot in contact with the ground and are not allowed to run. "@en-GB;
	skos:inScheme <http://cv.iptc.org/newscodes/subjectcode/>;
	skos:broadMatch medtop:20000841;
	skos:broader	subj:15005000.

subj:15005034
	rdf:type skos:Concept;
	skos:prefLabel	"walk 2 h"@en-GB;
	skos:definition	"Two-hour long walking race where competitors must maintain at least one foot in contact with the ground and are not allowed to run. "@en-GB;
	skos:inScheme <http://cv.iptc.org/newscodes/subjectcode/>;
	skos:broadMatch medtop:20000841;
	skos:broader	subj:15005000.

subj:15005035
	rdf:type skos:Concept;
	skos:prefLabel	"10 km walk"@en-GB;
	skos:definition	"Walking race over 10 kilometres where competitors must maintain at least one foot in contact with the ground and are not allowed to run. "@en-GB;
	skos:inScheme <http://cv.iptc.org/newscodes/subjectcode/>;
	skos:broadMatch medtop:20000841;
	skos:broader	subj:15005000.

subj:15005036
	rdf:type skos:Concept;
	skos:prefLabel	"15 km walk"@en-GB;
	skos:definition	"Walking race over 15 kilometres where competitors must maintain at least one foot in contact with the ground and are not allowed to run. "@en-GB;
	skos:inScheme <http://cv.iptc.org/newscodes/subjectcode/>;
	skos:broadMatch medtop:20000841;
	skos:broader	subj:15005000.

subj:15005037
	rdf:type skos:Concept;
	skos:prefLabel	"20 km walk"@en-GB;
	skos:definition	"Walking race over 20 kilometres where competitors must maintain at least one foot in contact with the ground and are not allowed to run. "@en-GB;
	skos:historyNote	"typo fixed in Explanation "@en-GB;
	skos:inScheme <http://cv.iptc.org/newscodes/subjectcode/>;
	skos:broadMatch medtop:20000841;
	skos:broader	subj:15005000.

subj:15005038
	rdf:type skos:Concept;
	skos:prefLabel	"30 km walk"@en-GB;
	skos:definition	"Walking race over 30 kilometres where competitors must maintain at least one foot in contact with the ground and are not allowed to run. "@en-GB;
	skos:inScheme <http://cv.iptc.org/newscodes/subjectcode/>;
	skos:broadMatch medtop:20000841;
	skos:broader	subj:15005000.

subj:15005039
	rdf:type skos:Concept;
	skos:prefLabel	"50 km walk"@en-GB;
	skos:definition	"Walking race over 50 kilometres where competitors must maintain at least one foot in contact with the ground and are not allowed to run. "@en-GB;
	skos:inScheme <http://cv.iptc.org/newscodes/subjectcode/>;
	skos:broadMatch medtop:20000841;
	skos:broader	subj:15005000.

subj:15005040
	rdf:type skos:Concept;
	skos:prefLabel	"100 m hurdles"@en-GB;
	skos:definition	"Sprint over a distance of 100 metres with competitors having to clear 10 hurdles placed in their way. "@en-GB;
	skos:inScheme <http://cv.iptc.org/newscodes/subjectcode/>;
	skos:broadMatch medtop:20000834;
	skos:broader	subj:15005000.

subj:15005041
	rdf:type skos:Concept;
	skos:prefLabel	"5 km walk"@en-GB;
	skos:definition	"Walking race over 5 kilometres where competitors must maintain at least one foot in contact with the ground and are not allowed to run. "@en-GB;
	skos:inScheme <http://cv.iptc.org/newscodes/subjectcode/>;
	skos:broadMatch medtop:20000841;
	skos:broader	subj:15005000.

subj:15005042
	rdf:type skos:Concept;
	skos:prefLabel	"heptathlon"@en-GB;
	skos:definition	"Individual women's competition involving seven separate disciplines over two days. 1st day - 100m hurdles, high-jump, shot-putt, 200 metres. 2nd day - long-jump, javelin, 800 metres. "@en-GB;
	skos:historyNote	"typo fixed in Explanation "@en-GB;
	skos:inScheme <http://cv.iptc.org/newscodes/subjectcode/>;
	skos:exactMatch medtop:20000832;
	skos:broader	subj:15005000.

subj:15005043
	rdf:type skos:Concept;
	skos:prefLabel	"1500 m walk"@en-GB;
	skos:definition	"Walking race over 1500 metres where competitors must maintain at least one foot in contact with the ground and are not allowed to run. "@en-GB;
	skos:inScheme <http://cv.iptc.org/newscodes/subjectcode/>;
	skos:broadMatch medtop:20000841;
	skos:broader	subj:15005000.

subj:15005044
	rdf:type skos:Concept;
	skos:prefLabel	"2000 m walk"@en-GB;
	skos:definition	"Walking race over 2000 metres where competitors must maintain at least one foot in contact with the ground and are not allowed to run. "@en-GB;
	skos:inScheme <http://cv.iptc.org/newscodes/subjectcode/>;
	skos:broadMatch medtop:20000841;
	skos:broader	subj:15005000.

subj:15005045
	rdf:type skos:Concept;
	skos:prefLabel	"3000 m walk"@en-GB;
	skos:definition	"Walking race over 3000 metres where competitors must maintain at least one foot in contact with the ground and are not allowed to run. "@en-GB;
	skos:inScheme <http://cv.iptc.org/newscodes/subjectcode/>;
	skos:broadMatch medtop:20000841;
	skos:broader	subj:15005000.

subj:15005046
	rdf:type skos:Concept;
	skos:prefLabel	"50 m"@en-GB;
	skos:definition	"Short sprint race over 50 metres with the fastest time winning. "@en-GB;
	skos:inScheme <http://cv.iptc.org/newscodes/subjectcode/>;
	skos:broadMatch medtop:20000844;
	skos:broader	subj:15005000.

subj:15005047
	rdf:type skos:Concept;
	skos:prefLabel	"50 m hurdles"@en-GB;
	skos:definition	"Short sprint race over 50 metres interspersed with hurdles. "@en-GB;
	skos:inScheme <http://cv.iptc.org/newscodes/subjectcode/>;
	skos:broadMatch medtop:20000834;
	skos:broader	subj:15005000.

subj:15005048
	rdf:type skos:Concept;
	skos:prefLabel	"50 yards"@en-GB;
	skos:definition	"Short sprint race over 50 yards with the fastest time winning. "@en-GB;
	skos:inScheme <http://cv.iptc.org/newscodes/subjectcode/>;
	skos:broadMatch medtop:20000844;
	skos:broader	subj:15005000.

subj:15005049
	rdf:type skos:Concept;
	skos:prefLabel	"50 yard hurdles"@en-GB;
	skos:definition	"Short sprint race over 50 yards interspersed with hurdles. "@en-GB;
	skos:inScheme <http://cv.iptc.org/newscodes/subjectcode/>;
	skos:broadMatch medtop:20000834;
	skos:broader	subj:15005000.

subj:15005050
	rdf:type skos:Concept;
	skos:prefLabel	"60 m"@en-GB;
	skos:definition	"Short sprint race over 60 metres with the fastest time winning. "@en-GB;
	skos:inScheme <http://cv.iptc.org/newscodes/subjectcode/>;
	skos:broadMatch medtop:20000844;
	skos:broader	subj:15005000.

subj:15005051
	rdf:type skos:Concept;
	skos:prefLabel	"60 m hurdles"@en-GB;
	skos:definition	"Short sprint race over 60 metres interspersed with hurdles. "@en-GB;
	skos:inScheme <http://cv.iptc.org/newscodes/subjectcode/>;
	skos:broadMatch medtop:20000834;
	skos:broader	subj:15005000.

subj:15005052
	rdf:type skos:Concept;
	skos:prefLabel	"60 yards"@en-GB;
	skos:definition	"Short sprint race over 60 yards with the fastest time winning. "@en-GB;
	skos:inScheme <http://cv.iptc.org/newscodes/subjectcode/>;
	skos:broadMatch medtop:20000844;
	skos:broader	subj:15005000.

subj:15005053
	rdf:type skos:Concept;
	skos:prefLabel	"60 yard hurdles"@en-GB;
	skos:definition	"Short sprint race over 60 yards interspersed with hurdles. "@en-GB;
	skos:historyNote	"typo fixed in Explanation "@en-GB;
	skos:inScheme <http://cv.iptc.org/newscodes/subjectcode/>;
	skos:broadMatch medtop:20000834;
	skos:broader	subj:15005000.

subj:15005054
	rdf:type skos:Concept;
	skos:prefLabel	"100 yards"@en-GB;
	skos:definition	"Sprint race over 100 yards with the fastest time winning. "@en-GB;
	skos:inScheme <http://cv.iptc.org/newscodes/subjectcode/>;
	skos:broadMatch medtop:20000844;
	skos:broader	subj:15005000.

subj:15005055
	rdf:type skos:Concept;
	skos:prefLabel	"100 yard hurdles"@en-GB;
	skos:definition	"Sprint race over 100 yards interspersed with hurdles. "@en-GB;
	skos:inScheme <http://cv.iptc.org/newscodes/subjectcode/>;
	skos:broadMatch medtop:20000834;
	skos:broader	subj:15005000.

subj:15005056
	rdf:type skos:Concept;
	skos:prefLabel	"300 m"@en-GB;
	skos:definition	"Race over 300 metres with the fastest time winning. "@en-GB;
	skos:inScheme <http://cv.iptc.org/newscodes/subjectcode/>;
	skos:broadMatch medtop:20000844;
	skos:broader	subj:15005000.

subj:15005057
	rdf:type skos:Concept;
	skos:prefLabel	"300 yards"@en-GB;
	skos:definition	"Race over 300 yards with the fastest time winning. "@en-GB;
	skos:inScheme <http://cv.iptc.org/newscodes/subjectcode/>;
	skos:broadMatch medtop:20000844;
	skos:broader	subj:15005000.

subj:15005058
	rdf:type skos:Concept;
	skos:prefLabel	"440 yards"@en-GB;
	skos:definition	"Race over 440 yards with the fastest time winning. "@en-GB;
	skos:inScheme <http://cv.iptc.org/newscodes/subjectcode/>;
	skos:broadMatch medtop:20000838;
	skos:broader	subj:15005000.

subj:15005059
	rdf:type skos:Concept;
	skos:prefLabel	"500 m"@en-GB;
	skos:definition	"Race over 500 metres with the fastest time winning. "@en-GB;
	skos:inScheme <http://cv.iptc.org/newscodes/subjectcode/>;
	skos:broadMatch medtop:20000838;
	skos:broader	subj:15005000.

subj:15005060
	rdf:type skos:Concept;
	skos:prefLabel	"500 yards"@en-GB;
	skos:definition	"Race over 500 yards with the fastest time winning. "@en-GB;
	skos:inScheme <http://cv.iptc.org/newscodes/subjectcode/>;
	skos:broadMatch medtop:20000838;
	skos:broader	subj:15005000.

subj:15005061
	rdf:type skos:Concept;
	skos:prefLabel	"600 m"@en-GB;
	skos:definition	"Race over 600 metres with the fastest time winning. "@en-GB;
	skos:inScheme <http://cv.iptc.org/newscodes/subjectcode/>;
	skos:broadMatch medtop:20000838;
	skos:broader	subj:15005000.

subj:15005062
	rdf:type skos:Concept;
	skos:prefLabel	"600 yards"@en-GB;
	skos:definition	"Race over 600 yards with the fastest time winning. "@en-GB;
	skos:inScheme <http://cv.iptc.org/newscodes/subjectcode/>;
	skos:broadMatch medtop:20000838;
	skos:broader	subj:15005000.

subj:15005063
	rdf:type skos:Concept;
	skos:prefLabel	"880 yards"@en-GB;
	skos:definition	"Race over 880 yards with the fastest time winning. "@en-GB;
	skos:inScheme <http://cv.iptc.org/newscodes/subjectcode/>;
	skos:broadMatch medtop:20000838;
	skos:broader	subj:15005000.

subj:15005064
	rdf:type skos:Concept;
	skos:prefLabel	"1000 yards"@en-GB;
	skos:definition	"Race over 1000 yards with the fastest time winning. "@en-GB;
	skos:inScheme <http://cv.iptc.org/newscodes/subjectcode/>;
	skos:broadMatch medtop:20000838;
	skos:broader	subj:15005000.

subj:15005065
	rdf:type skos:Concept;
	skos:prefLabel	"2 miles"@en-GB;
	skos:definition	"Race over two miles with the fastest time winning. "@en-GB;
	skos:inScheme <http://cv.iptc.org/newscodes/subjectcode/>;
	skos:broadMatch medtop:20000836;
	skos:broader	subj:15005000.

subj:15005066
	rdf:type skos:Concept;
	skos:prefLabel	"3 miles"@en-GB;
	skos:definition	"Race over three miles with the fastest time winning. "@en-GB;
	skos:inScheme <http://cv.iptc.org/newscodes/subjectcode/>;
	skos:broadMatch medtop:20000836;
	skos:broader	subj:15005000.

subj:15005067
	rdf:type skos:Concept;
	skos:prefLabel	"6 miles"@en-GB;
	skos:definition	"Race over six miles with the fastest time winning. "@en-GB;
	skos:inScheme <http://cv.iptc.org/newscodes/subjectcode/>;
	skos:broadMatch medtop:20000836;
	skos:broader	subj:15005000.

subj:15005068
	rdf:type skos:Concept;
	skos:prefLabel	"4x1 mile"@en-GB;
	skos:definition	"Team Relay race with four runners on each team running for one mile. "@en-GB;
	skos:inScheme <http://cv.iptc.org/newscodes/subjectcode/>;
	skos:broadMatch medtop:20000842;
	skos:broader	subj:15005000.

subj:15005069
	rdf:type skos:Concept;
	skos:prefLabel	"pentathlon"@en-GB;
	skos:definition	"Only indoor, 60m hurdles, high jump, shot put, long jump, 800 m "@en-GB;
	skos:inScheme <http://cv.iptc.org/newscodes/subjectcode/>;
	skos:exactMatch medtop:20000839;
	skos:broader	subj:15005000.

subj:15006000
	rdf:type skos:Concept;
	skos:prefLabel	"badminton"@en-GB;
	skos:definition	"Two players or two teams of two compete by hitting a shuttlecock weighing approximately five grams over a high net. The aim for each player/team is to prevent the shuttlecock landing on their side of the court. "@en-GB;
	skos:historyNote	"typo fixed in Explanation "@en-GB;
	skos:inScheme <http://cv.iptc.org/newscodes/subjectcode/>;
	skos:exactMatch medtop:20000847;
	skos:broader	subj:15000000.

subj:15007000
	rdf:type skos:Concept;
	skos:prefLabel	"baseball"@en-GB;
	skos:definition	"A game between two teams of nine played on an enclosed ground. The team which scores the most points wins. A point is scored when a player runs around the ground marked out by four bases. "@en-GB;
	skos:historyNote	"Explanation shortened "@en-GB;
	skos:inScheme <http://cv.iptc.org/newscodes/subjectcode/>;
	skos:exactMatch medtop:20000849;
	skos:broader	subj:15000000;
	skos:narrower	subj:15007001;
	skos:narrower	subj:15007002;
	skos:narrower	subj:15007003;
	skos:narrower	subj:15007004;
	skos:narrower	subj:15007005;
	skos:narrower	subj:15007006.

subj:15007001
	rdf:type skos:Concept;
	skos:prefLabel	"Major League Baseball (North American Professional) - American League"@en-GB;
	skos:definition	"Baseball league comprising 14 teams. "@en-GB;
	skos:inScheme <http://cv.iptc.org/newscodes/subjectcode/>;
	skos:broadMatch medtop:20000849;
	skos:broader	subj:15007000.

subj:15007002
	rdf:type skos:Concept;
	skos:prefLabel	"Major League Baseball (North American Professional) - National League"@en-GB;
	skos:definition	"Baseball league comprising 16 teams. "@en-GB;
	skos:inScheme <http://cv.iptc.org/newscodes/subjectcode/>;
	skos:broadMatch medtop:20000849;
	skos:broader	subj:15007000.

subj:15007003
	rdf:type skos:Concept;
	skos:prefLabel	"Major League Baseball (North American Professional) - Special (e.g. All-Star, World Series)"@en-GB;
	skos:definition	"Baseball competition other than the World Series. "@en-GB;
	skos:inScheme <http://cv.iptc.org/newscodes/subjectcode/>;
	skos:broadMatch medtop:20000849;
	skos:broader	subj:15007000.

subj:15007004
	rdf:type skos:Concept;
	skos:prefLabel	"rubberball baseball"@en-GB;
	skos:definition	"Sometimes called ''soft baseball,'' the game is played with a rubber baseball of varying degrees of hardness depending upon the age and level of the players. "@en-GB;
	skos:inScheme <http://cv.iptc.org/newscodes/subjectcode/>;
	skos:exactMatch medtop:20000850;
	skos:broader	subj:15007000.

subj:15007005
	rdf:type skos:Concept;
	skos:prefLabel	"Major League Baseball Playoffs"@en-GB;
	skos:definition	"Consists of several rounds of play to determine representatives to the U.S.-based World Series "@en-GB;
	skos:inScheme <http://cv.iptc.org/newscodes/subjectcode/>;
	skos:broadMatch medtop:20000849;
	skos:broader	subj:15007000.

subj:15007006
	rdf:type skos:Concept;
	skos:prefLabel	"World Series"@en-GB;
	skos:definition	"U.S.-based annual series of games between the top two teams of Major League Baseball to determine the overall champion "@en-GB;
	skos:inScheme <http://cv.iptc.org/newscodes/subjectcode/>;
	skos:broadMatch medtop:20000849;
	skos:broader	subj:15007000.

subj:15008000
	rdf:type skos:Concept;
	skos:prefLabel	"basketball"@en-GB;
	skos:definition	"Game played between two teams of five - points are scored by placing the large inflated ball into a net fixed on a ring 3.05m above the ground. "@en-GB;
	skos:inScheme <http://cv.iptc.org/newscodes/subjectcode/>;
	skos:exactMatch medtop:20000851;
	skos:broader	subj:15000000;
	skos:narrower	subj:15008001;
	skos:narrower	subj:15008002;
	skos:narrower	subj:15008003;
	skos:narrower	subj:15008004;
	skos:narrower	subj:15008005.

subj:15008001
	rdf:type skos:Concept;
	skos:prefLabel	"National Basketball Association (North American Professional)"@en-GB;
	skos:definition	"The NBA is the umbrella organisation running professional basketball in the United States. The NBA is made up of two conferences (east and west), four divisions (Atlantic and Central for the East, and Midwest and Pacific for the west). "@en-GB;
	skos:historyNote	"typo fixed in Explanation "@en-GB;
	skos:inScheme <http://cv.iptc.org/newscodes/subjectcode/>;
	skos:broadMatch medtop:20000851;
	skos:broader	subj:15008000.

subj:15008002
	rdf:type skos:Concept;
	skos:prefLabel	"professional - Women general"@en-GB;
	skos:definition	"Women's professional league "@en-GB;
	skos:inScheme <http://cv.iptc.org/newscodes/subjectcode/>;
	skos:broadMatch medtop:20000851;
	skos:broader	subj:15008000.

subj:15008003
	rdf:type skos:Concept;
	skos:prefLabel	"Swiss netball"@en-GB;
	skos:definition	"Similar to Basketball. Basket without a board. Mainly executed by women "@en-GB;
	skos:inScheme <http://cv.iptc.org/newscodes/subjectcode/>;
	skos:broadMatch medtop:20001010;
	skos:broader	subj:15008000.

subj:15008004
	rdf:type skos:Concept;
	skos:prefLabel	"German netball"@en-GB;
	skos:definition	"Same as Swiss Netball, but with specific German rules "@en-GB;
	skos:inScheme <http://cv.iptc.org/newscodes/subjectcode/>;
	skos:broadMatch medtop:20001010;
	skos:broader	subj:15008000.

subj:15008005
	rdf:type skos:Concept;
	skos:prefLabel	"Dutch netball"@en-GB;
	skos:definition	"Same as Swiss Netball, but with specific Dutch rule "@en-GB;
	skos:inScheme <http://cv.iptc.org/newscodes/subjectcode/>;
	skos:broadMatch medtop:20001010;
	skos:broader	subj:15008000.

subj:15009000
	rdf:type skos:Concept;
	skos:prefLabel	"biathlon"@en-GB;
	skos:definition	"A combination of cross country skiing and target shooting in a pursuit format. "@en-GB;
	skos:inScheme <http://cv.iptc.org/newscodes/subjectcode/>;
	skos:exactMatch medtop:20000852;
	skos:broader	subj:15000000;
	skos:narrower	subj:15009001;
	skos:narrower	subj:15009002;
	skos:narrower	subj:15009003;
	skos:narrower	subj:15009004;
	skos:narrower	subj:15009005;
	skos:narrower	subj:15009006.

subj:15009001
	rdf:type skos:Concept;
	skos:prefLabel	"7.5 km"@en-GB;
	skos:definition	"Timed cross country skiing race. Competitors set off at 30sec intervals for three circuits totalling 7.5km. "@en-GB;
	skos:inScheme <http://cv.iptc.org/newscodes/subjectcode/>;
	skos:broadMatch medtop:20000852;
	skos:broader	subj:15009000.

subj:15009002
	rdf:type skos:Concept;
	skos:prefLabel	"10 km"@en-GB;
	skos:definition	"Sprint races for men, pursuit for women. "@en-GB;
	skos:inScheme <http://cv.iptc.org/newscodes/subjectcode/>;
	skos:broadMatch medtop:20000852;
	skos:broader	subj:15009000.

subj:15009003
	rdf:type skos:Concept;
	skos:prefLabel	"15 km"@en-GB;
	skos:definition	"Individual women's race in sprint format staged over three laps with competitors setting off at intervals of a minute. "@en-GB;
	skos:historyNote	"typo fixed in Explanation "@en-GB;
	skos:inScheme <http://cv.iptc.org/newscodes/subjectcode/>;
	skos:broadMatch medtop:20000852;
	skos:broader	subj:15009000.

subj:15009004
	rdf:type skos:Concept;
	skos:prefLabel	"20 km"@en-GB;
	skos:definition	"Individual men's race in sprint format staged over five laps with competitors setting off at intervals of a minute. "@en-GB;
	skos:inScheme <http://cv.iptc.org/newscodes/subjectcode/>;
	skos:broadMatch medtop:20000852;
	skos:broader	subj:15009000.

subj:15009005
	rdf:type skos:Concept;
	skos:prefLabel	"4x7.5 km relay"@en-GB;
	skos:definition	"Teams consisting of four biathletes with each team covering a distance of 7.5km with two rounds of target shooting. "@en-GB;
	skos:inScheme <http://cv.iptc.org/newscodes/subjectcode/>;
	skos:broadMatch medtop:20000852;
	skos:broader	subj:15009000.

subj:15009006
	rdf:type skos:Concept;
	skos:prefLabel	"12.5 km pursuit"@en-GB;
	skos:definition	"The start is determined by the results from the sprint. A race held over five laps with target shooting (standing or prone) "@en-GB;
	skos:inScheme <http://cv.iptc.org/newscodes/subjectcode/>;
	skos:broadMatch medtop:20000852;
	skos:broader	subj:15009000.

subj:15010000
	rdf:type skos:Concept;
	skos:prefLabel	"billiards, snooker and pool"@en-GB;
	skos:definition	"A game played on a flat table covered with a cloth (baize) where players hit balls according to specific rules using a wooden cue. "@en-GB;
	skos:inScheme <http://cv.iptc.org/newscodes/subjectcode/>;
	skos:closeMatch medtop:20001063;
	skos:closeMatch medtop:20000853;
	skos:closeMatch medtop:20001015;
	skos:broader	subj:15000000;
	skos:narrower	subj:15010001;
	skos:narrower	subj:15010002;
	skos:narrower	subj:15010003;
	skos:narrower	subj:15010004;
	skos:narrower	subj:15010005;
	skos:narrower	subj:15010006.

subj:15010001
	rdf:type skos:Concept;
	skos:prefLabel	"8 ball"@en-GB;
	skos:definition	"A game using 15 balls and a white. The first player aims to pot the balls numbered 1-7 (solids) with the second player potting balls 9-15 (stripes). After that the first player to pot the black wins. "@en-GB;
	skos:inScheme <http://cv.iptc.org/newscodes/subjectcode/>;
	skos:broadMatch medtop:20001015;
	skos:broader	subj:15010000.

subj:15010002
	rdf:type skos:Concept;
	skos:prefLabel	"9 ball"@en-GB;
	skos:definition	"A game played with nine balls numbered 1-9, and a white. On each turn the player must hit the lowest numbered ball. "@en-GB;
	skos:inScheme <http://cv.iptc.org/newscodes/subjectcode/>;
	skos:broadMatch medtop:20001015;
	skos:broader	subj:15010000.

subj:15010003
	rdf:type skos:Concept;
	skos:prefLabel	"14.1"@en-GB;
	skos:definition	"A player nominates the ball he is attempting to pot and into which pocket. He collects points for each successful hit. He continues until he makes a mistake. Before hitting the 15th ball, the 14 reds are set up again in the triangle. "@en-GB;
	skos:historyNote	"Explanation shortened "@en-GB;
	skos:inScheme <http://cv.iptc.org/newscodes/subjectcode/>;
	skos:broadMatch medtop:20001015;
	skos:broader	subj:15010000.

subj:15010004
	rdf:type skos:Concept;
	skos:prefLabel	"continuous-DEPRECATED"@en-GB;
	skos:definition	"NA "@en-GB;
	skos:historyNote	"DEPRECATED in V 16 "@en-GB;
	skos:inScheme <http://cv.iptc.org/newscodes/subjectcode/>;
	skos:broader	subj:15010000.

subj:15010005
	rdf:type skos:Concept;
	skos:prefLabel	"other-DEPRECATED"@en-GB;
	skos:definition	"NA "@en-GB;
	skos:historyNote	"DEPRECATED in V 16 "@en-GB;
	skos:inScheme <http://cv.iptc.org/newscodes/subjectcode/>;
	skos:broader	subj:15010000.

subj:15010006
	rdf:type skos:Concept;
	skos:prefLabel	"snooker"@en-GB;
	skos:definition	"Two players using a cue and a white ball to ´sink´ other coloured balls in a correct order on a baize table and to cause an opponent to miss-hit by positioning the white ball in an inappropriate place - snookering. "@en-GB;
	skos:inScheme <http://cv.iptc.org/newscodes/subjectcode/>;
	skos:exactMatch medtop:20001063;
	skos:broader	subj:15010000.

subj:15011000
	rdf:type skos:Concept;
	skos:prefLabel	"bobsleigh"@en-GB;
	skos:definition	"In bobsleigh two or four persons race down a course sitting in a sled that consists of a main hull, a frame, two axles and sets of runners. The total time of all heats in a competition is added together to determine the winner. "@en-GB;
	skos:inScheme <http://cv.iptc.org/newscodes/subjectcode/>;
	skos:exactMatch medtop:20000854;
	skos:broader	subj:15000000;
	skos:narrower	subj:15011001;
	skos:narrower	subj:15011002.

subj:15011001
	rdf:type skos:Concept;
	skos:prefLabel	"two-man sled"@en-GB;
	skos:definition	"race consisting of a team of two competitors "@en-GB;
	skos:inScheme <http://cv.iptc.org/newscodes/subjectcode/>;
	skos:broadMatch medtop:20000854;
	skos:broader	subj:15011000.

subj:15011002
	rdf:type skos:Concept;
	skos:prefLabel	"four-man sled"@en-GB;
	skos:definition	"race consisting of a team of four competitors "@en-GB;
	skos:inScheme <http://cv.iptc.org/newscodes/subjectcode/>;
	skos:broadMatch medtop:20000854;
	skos:broader	subj:15011000.

subj:15012000
	rdf:type skos:Concept;
	skos:prefLabel	"bowling"@en-GB;
	skos:definition	"A game in which a player scores points by trying to knock down ten 'pins' using a ball - if unsuccessful the player has a second attempt. A game consists of ten frames. "@en-GB;
	skos:inScheme <http://cv.iptc.org/newscodes/subjectcode/>;
	skos:exactMatch medtop:20001086;
	skos:broader	subj:15000000.

subj:15013000
	rdf:type skos:Concept;
	skos:prefLabel	"bowls and petanque"@en-GB;
	skos:definition	"A game in which players throw bowls at a target, the winner being the player who lands closest. "@en-GB;
	skos:inScheme <http://cv.iptc.org/newscodes/subjectcode/>;
	skos:exactMatch medtop:20000855;
	skos:broader	subj:15000000.

subj:15014000
	rdf:type skos:Concept;
	skos:prefLabel	"boxing"@en-GB;
	skos:definition	"Combat sport in which two men/women fight using only their fists covered by padded gloves in a square ring measuring 6m a side. The fight is usually split into 12 rounds of three minutes each. "@en-GB;
	skos:inScheme <http://cv.iptc.org/newscodes/subjectcode/>;
	skos:exactMatch medtop:20000856;
	skos:broader	subj:15000000;
	skos:narrower	subj:15014001;
	skos:narrower	subj:15014002;
	skos:narrower	subj:15014003;
	skos:narrower	subj:15014004;
	skos:narrower	subj:15014005;
	skos:narrower	subj:15014006;
	skos:narrower	subj:15014007;
	skos:narrower	subj:15014008;
	skos:narrower	subj:15014009;
	skos:narrower	subj:15014010;
	skos:narrower	subj:15014011;
	skos:narrower	subj:15014012;
	skos:narrower	subj:15014013;
	skos:narrower	subj:15014014;
	skos:narrower	subj:15014015;
	skos:narrower	subj:15014016;
	skos:narrower	subj:15014017;
	skos:narrower	subj:15014018;
	skos:narrower	subj:15014019;
	skos:narrower	subj:15014020;
	skos:narrower	subj:15014021;
	skos:narrower	subj:15014022;
	skos:narrower	subj:15014023;
	skos:narrower	subj:15014024.

subj:15014001
	rdf:type skos:Concept;
	skos:prefLabel	"super-heavyweight"@en-GB;
	skos:definition	"Weight category in boxing which varies according to the federation"@en-GB;
	skos:inScheme <http://cv.iptc.org/newscodes/subjectcode/>;
	skos:broadMatch medtop:20000856;
	skos:broader	subj:15014000.

subj:15014002
	rdf:type skos:Concept;
	skos:prefLabel	"heavyweight"@en-GB;
	skos:definition	"Weight category in boxing which varies according to the federation"@en-GB;
	skos:inScheme <http://cv.iptc.org/newscodes/subjectcode/>;
	skos:broadMatch medtop:20000856;
	skos:broader	subj:15014000.

subj:15014003
	rdf:type skos:Concept;
	skos:prefLabel	"cruiserweight"@en-GB;
	skos:definition	"Weight category in boxing which varies according to the federation"@en-GB;
	skos:inScheme <http://cv.iptc.org/newscodes/subjectcode/>;
	skos:broadMatch medtop:20000856;
	skos:broader	subj:15014000.

subj:15014004
	rdf:type skos:Concept;
	skos:prefLabel	"light-heavyweight"@en-GB;
	skos:definition	"Weight category in boxing which varies according to the federation"@en-GB;
	skos:inScheme <http://cv.iptc.org/newscodes/subjectcode/>;
	skos:broadMatch medtop:20000856;
	skos:broader	subj:15014000.

subj:15014005
	rdf:type skos:Concept;
	skos:prefLabel	"super-middleweight"@en-GB;
	skos:definition	"Weight category in boxing which varies according to the federation"@en-GB;
	skos:inScheme <http://cv.iptc.org/newscodes/subjectcode/>;
	skos:broadMatch medtop:20000856;
	skos:broader	subj:15014000.

subj:15014006
	rdf:type skos:Concept;
	skos:prefLabel	"middleweight"@en-GB;
	skos:definition	"Weight category in boxing which varies according to the federation"@en-GB;
	skos:inScheme <http://cv.iptc.org/newscodes/subjectcode/>;
	skos:broadMatch medtop:20000856;
	skos:broader	subj:15014000.

subj:15014007
	rdf:type skos:Concept;
	skos:prefLabel	"light-middleweight"@en-GB;
	skos:definition	"Weight category in boxing which varies according to the federation"@en-GB;
	skos:inScheme <http://cv.iptc.org/newscodes/subjectcode/>;
	skos:broadMatch medtop:20000856;
	skos:broader	subj:15014000.

subj:15014008
	rdf:type skos:Concept;
	skos:prefLabel	"welterweight"@en-GB;
	skos:definition	"Weight category in boxing which varies according to the federation"@en-GB;
	skos:inScheme <http://cv.iptc.org/newscodes/subjectcode/>;
	skos:broadMatch medtop:20000856;
	skos:broader	subj:15014000.

subj:15014009
	rdf:type skos:Concept;
	skos:prefLabel	"light-welterweight"@en-GB;
	skos:definition	"Weight category in boxing which varies according to the federation"@en-GB;
	skos:inScheme <http://cv.iptc.org/newscodes/subjectcode/>;
	skos:broadMatch medtop:20000856;
	skos:broader	subj:15014000.

subj:15014010
	rdf:type skos:Concept;
	skos:prefLabel	"lightweight"@en-GB;
	skos:definition	"Weight category in boxing which varies according to the federation"@en-GB;
	skos:inScheme <http://cv.iptc.org/newscodes/subjectcode/>;
	skos:broadMatch medtop:20000856;
	skos:broader	subj:15014000.

subj:15014011
	rdf:type skos:Concept;
	skos:prefLabel	"super-featherweight"@en-GB;
	skos:definition	"Weight category in boxing which varies according to the federation"@en-GB;
	skos:inScheme <http://cv.iptc.org/newscodes/subjectcode/>;
	skos:broadMatch medtop:20000856;
	skos:broader	subj:15014000.

subj:15014012
	rdf:type skos:Concept;
	skos:prefLabel	"featherweight"@en-GB;
	skos:definition	"Weight category in boxing which varies according to the federation"@en-GB;
	skos:inScheme <http://cv.iptc.org/newscodes/subjectcode/>;
	skos:broadMatch medtop:20000856;
	skos:broader	subj:15014000.

subj:15014013
	rdf:type skos:Concept;
	skos:prefLabel	"super-bantamweight"@en-GB;
	skos:definition	"Weight category in boxing which varies according to the federation"@en-GB;
	skos:inScheme <http://cv.iptc.org/newscodes/subjectcode/>;
	skos:broadMatch medtop:20000856;
	skos:broader	subj:15014000.

subj:15014014
	rdf:type skos:Concept;
	skos:prefLabel	"bantamweight"@en-GB;
	skos:definition	"Weight category in boxing which varies according to the federation"@en-GB;
	skos:inScheme <http://cv.iptc.org/newscodes/subjectcode/>;
	skos:broadMatch medtop:20000856;
	skos:broader	subj:15014000.

subj:15014015
	rdf:type skos:Concept;
	skos:prefLabel	"super-flyweight"@en-GB;
	skos:definition	"Weight category in boxing which varies according to the federation"@en-GB;
	skos:inScheme <http://cv.iptc.org/newscodes/subjectcode/>;
	skos:broadMatch medtop:20000856;
	skos:broader	subj:15014000.

subj:15014016
	rdf:type skos:Concept;
	skos:prefLabel	"flyweight"@en-GB;
	skos:definition	"Weight category in boxing which varies according to the federation"@en-GB;
	skos:inScheme <http://cv.iptc.org/newscodes/subjectcode/>;
	skos:broadMatch medtop:20000856;
	skos:broader	subj:15014000.

subj:15014017
	rdf:type skos:Concept;
	skos:prefLabel	"light flyweight"@en-GB;
	skos:definition	"Weight category in boxing which varies according to the federation"@en-GB;
	skos:inScheme <http://cv.iptc.org/newscodes/subjectcode/>;
	skos:broadMatch medtop:20000856;
	skos:broader	subj:15014000.

subj:15014018
	rdf:type skos:Concept;
	skos:prefLabel	"straw"@en-GB;
	skos:definition	"Weight category in boxing which varies according to the federation"@en-GB;
	skos:inScheme <http://cv.iptc.org/newscodes/subjectcode/>;
	skos:broadMatch medtop:20000856;
	skos:broader	subj:15014000.

subj:15014019
	rdf:type skos:Concept;
	skos:prefLabel	"IBF"@en-GB;
	skos:definition	"International boxing federation "@en-GB;
	skos:inScheme <http://cv.iptc.org/newscodes/subjectcode/>;
	skos:broadMatch medtop:20000856;
	skos:broader	subj:15014000.

subj:15014020
	rdf:type skos:Concept;
	skos:prefLabel	"WBA"@en-GB;
	skos:definition	"World boxing association "@en-GB;
	skos:inScheme <http://cv.iptc.org/newscodes/subjectcode/>;
	skos:broadMatch medtop:20000856;
	skos:broader	subj:15014000.

subj:15014021
	rdf:type skos:Concept;
	skos:prefLabel	"WBC"@en-GB;
	skos:definition	"World boxing council "@en-GB;
	skos:inScheme <http://cv.iptc.org/newscodes/subjectcode/>;
	skos:broadMatch medtop:20000856;
	skos:broader	subj:15014000.

subj:15014022
	rdf:type skos:Concept;
	skos:prefLabel	"WBO"@en-GB;
	skos:definition	"World boxing organisation "@en-GB;
	skos:inScheme <http://cv.iptc.org/newscodes/subjectcode/>;
	skos:broadMatch medtop:20000856;
	skos:broader	subj:15014000.

subj:15014023
	rdf:type skos:Concept;
	skos:prefLabel	"French boxing"@en-GB;
	skos:definition	"Combat sport in which kicking with all parts of the feet are permitted and punching with the front of the fist is also allowed "@en-GB;
	skos:inScheme <http://cv.iptc.org/newscodes/subjectcode/>;
	skos:broadMatch medtop:20000856;
	skos:broader	subj:15014000.

subj:15014024
	rdf:type skos:Concept;
	skos:prefLabel	"Thai boxing"@en-GB;
	skos:definition	"Form of boxing involving punches with fists, feet, knees, elbows and legs. "@en-GB;
	skos:inScheme <http://cv.iptc.org/newscodes/subjectcode/>;
	skos:broadMatch medtop:20000856;
	skos:broader	subj:15014000.

subj:15015000
	rdf:type skos:Concept;
	skos:prefLabel	"canoeing and kayaking"@en-GB;
	skos:definition	"races in either 'white' or 'dead' water "@en-GB;
	skos:inScheme <http://cv.iptc.org/newscodes/subjectcode/>;
	skos:closeMatch medtop:20000877;
	skos:closeMatch medtop:20000979;
	skos:broader	subj:15000000;
	skos:narrower	subj:15015001;
	skos:narrower	subj:15015002;
	skos:narrower	subj:15015003;
	skos:narrower	subj:15015004;
	skos:narrower	subj:15015005;
	skos:narrower	subj:15015006;
	skos:narrower	subj:15015007;
	skos:narrower	subj:15015008;
	skos:narrower	subj:15015009;
	skos:narrower	subj:15015010;
	skos:narrower	subj:15015011;
	skos:narrower	subj:15015012.

subj:15015001
	rdf:type skos:Concept;
	skos:prefLabel	"Slalom"@en-GB;
	skos:definition	"White water course set out with gates consisting of two poles suspended vertically over the water. Competitors must negotiate the gates or face penalties "@en-GB;
	skos:inScheme <http://cv.iptc.org/newscodes/subjectcode/>;
	skos:closeMatch medtop:20000979;
	skos:closeMatch medtop:20000877;
	skos:broader	subj:15015000.

subj:15015002
	rdf:type skos:Concept;
	skos:prefLabel	"200 m"@en-GB;
	skos:definition	"race held over 200m "@en-GB;
	skos:inScheme <http://cv.iptc.org/newscodes/subjectcode/>;
	skos:closeMatch medtop:20000877;
	skos:closeMatch medtop:20000979;
	skos:broader	subj:15015000.

subj:15015003
	rdf:type skos:Concept;
	skos:prefLabel	"500 m"@en-GB;
	skos:definition	"race held over 500m "@en-GB;
	skos:inScheme <http://cv.iptc.org/newscodes/subjectcode/>;
	skos:closeMatch medtop:20000877;
	skos:closeMatch medtop:20000979;
	skos:broader	subj:15015000.

subj:15015004
	rdf:type skos:Concept;
	skos:prefLabel	"1000 m"@en-GB;
	skos:definition	"race held over 1000m "@en-GB;
	skos:inScheme <http://cv.iptc.org/newscodes/subjectcode/>;
	skos:closeMatch medtop:20000979;
	skos:closeMatch medtop:20000877;
	skos:broader	subj:15015000.

subj:15015005
	rdf:type skos:Concept;
	skos:prefLabel	"K1"@en-GB;
	skos:definition	"an enclosed boat with the competitor sitting on a fixed seat for one person using a double bladed paddle "@en-GB;
	skos:inScheme <http://cv.iptc.org/newscodes/subjectcode/>;
	skos:broadMatch medtop:20000979;
	skos:broader	subj:15015000.

subj:15015006
	rdf:type skos:Concept;
	skos:prefLabel	"K2"@en-GB;
	skos:definition	"an enclosed boat with the competitor sitting on a fixed seat for two people using double bladed paddles. "@en-GB;
	skos:inScheme <http://cv.iptc.org/newscodes/subjectcode/>;
	skos:broadMatch medtop:20000979;
	skos:broader	subj:15015000.

subj:15015007
	rdf:type skos:Concept;
	skos:prefLabel	"K4"@en-GB;
	skos:definition	"an enclosed boat with the competitor sitting on a fixed seat for four people using double bladed paddles. "@en-GB;
	skos:inScheme <http://cv.iptc.org/newscodes/subjectcode/>;
	skos:broadMatch medtop:20000979;
	skos:broader	subj:15015000.

subj:15015008
	rdf:type skos:Concept;
	skos:prefLabel	"C1"@en-GB;
	skos:definition	"One-seater canoe (open boat with competitor using a single bladed paddle. "@en-GB;
	skos:inScheme <http://cv.iptc.org/newscodes/subjectcode/>;
	skos:broadMatch medtop:20000877;
	skos:broader	subj:15015000.

subj:15015009
	rdf:type skos:Concept;
	skos:prefLabel	"C2"@en-GB;
	skos:definition	"Two-seater canoe (open boat) - competitors use a single bladed paddle. "@en-GB;
	skos:inScheme <http://cv.iptc.org/newscodes/subjectcode/>;
	skos:broadMatch medtop:20000877;
	skos:broader	subj:15015000.

subj:15015010
	rdf:type skos:Concept;
	skos:prefLabel	"C4"@en-GB;
	skos:definition	"Four-seater canoe (open boat) with each competitor using a single bladed paddle. "@en-GB;
	skos:inScheme <http://cv.iptc.org/newscodes/subjectcode/>;
	skos:broadMatch medtop:20000877;
	skos:broader	subj:15015000.

subj:15015011
	rdf:type skos:Concept;
	skos:prefLabel	"canoe sailing"@en-GB;
	skos:definition	"A race involving a canoe equipped with a sail. "@en-GB;
	skos:inScheme <http://cv.iptc.org/newscodes/subjectcode/>;
	skos:exactMatch medtop:20000881;
	skos:broader	subj:15015000.

subj:15015012
	rdf:type skos:Concept;
	skos:prefLabel	"pontoniering"@en-GB;
	skos:definition	"Team sport, military tradition, similar to canoe regatta, in boats "@en-GB;
	skos:inScheme <http://cv.iptc.org/newscodes/subjectcode/>;
	skos:exactMatch medtop:20000882;
	skos:broader	subj:15015000.

subj:15016000
	rdf:type skos:Concept;
	skos:prefLabel	"climbing"@en-GB;
	skos:definition	"mountain sports "@en-GB;
	skos:inScheme <http://cv.iptc.org/newscodes/subjectcode/>;
	skos:exactMatch medtop:20000884;
	skos:broader	subj:15000000;
	skos:narrower	subj:15016001;
	skos:narrower	subj:15016002.

subj:15016001
	rdf:type skos:Concept;
	skos:prefLabel	"mountaineering"@en-GB;
	skos:definition	"Alpine climbing "@en-GB;
	skos:inScheme <http://cv.iptc.org/newscodes/subjectcode/>;
	skos:exactMatch medtop:20000886;
	skos:broader	subj:15016000.

subj:15016002
	rdf:type skos:Concept;
	skos:prefLabel	"sport climbing"@en-GB;
	skos:definition	"Sport climbing as a special category: individual competition, on an artificial wall with time measurement "@en-GB;
	skos:inScheme <http://cv.iptc.org/newscodes/subjectcode/>;
	skos:exactMatch medtop:20000887;
	skos:broader	subj:15016000.

subj:15017000
	rdf:type skos:Concept;
	skos:prefLabel	"cricket"@en-GB;
	skos:definition	"Ball sport involving two teams of 11 players, balls, bats and wickets. The aim is to score as many runs as possible, and to get the opposing team 'out'. A 'run' involves a player running between two wickets. The opposing team try to get their rivals 'out' "@en-GB;
	skos:inScheme <http://cv.iptc.org/newscodes/subjectcode/>;
	skos:exactMatch medtop:20000888;
	skos:broader	subj:15000000.

subj:15018000
	rdf:type skos:Concept;
	skos:prefLabel	"curling"@en-GB;
	skos:definition	"A game played on ice with large flat round stones. A player throws the stone, aiming at a target. Team mates of the player who has thrown the stone can sweep the ice in front of the stone to help smooth its path towards the target. "@en-GB;
	skos:inScheme <http://cv.iptc.org/newscodes/subjectcode/>;
	skos:exactMatch medtop:20000890;
	skos:broader	subj:15000000;
	skos:narrower	subj:15018001.

subj:15018001
	rdf:type skos:Concept;
	skos:prefLabel	"icestock sport"@en-GB;
	skos:definition	"Similar to curling, played on targets on ice, different stones with straight handle and different rules, played in alpine countries "@en-GB;
	skos:inScheme <http://cv.iptc.org/newscodes/subjectcode/>;
	skos:exactMatch medtop:20000891;
	skos:broader	subj:15018000.

subj:15019000
	rdf:type skos:Concept;
	skos:prefLabel	"cycling"@en-GB;
	skos:definition	"A race over a given distance on bicycles. "@en-GB;
	skos:inScheme <http://cv.iptc.org/newscodes/subjectcode/>;
	skos:exactMatch medtop:20000892;
	skos:broader	subj:15000000;
	skos:narrower	subj:15019001;
	skos:narrower	subj:15019002;
	skos:narrower	subj:15019003;
	skos:narrower	subj:15019004;
	skos:narrower	subj:15019005;
	skos:narrower	subj:15019006;
	skos:narrower	subj:15019007;
	skos:narrower	subj:15019008;
	skos:narrower	subj:15019009;
	skos:narrower	subj:15019010;
	skos:narrower	subj:15019011;
	skos:narrower	subj:15019012;
	skos:narrower	subj:15019013;
	skos:narrower	subj:15019014;
	skos:narrower	subj:15019015;
	skos:narrower	subj:15019016;
	skos:narrower	subj:15019017;
	skos:narrower	subj:15019018;
	skos:narrower	subj:15019019;
	skos:narrower	subj:15019020;
	skos:narrower	subj:15019021.

subj:15019001
	rdf:type skos:Concept;
	skos:prefLabel	"track"@en-GB;
	skos:definition	"A race staged on a track in a velodrome "@en-GB;
	skos:inScheme <http://cv.iptc.org/newscodes/subjectcode/>;
	skos:exactMatch medtop:20000910;
	skos:broader	subj:15019000.

subj:15019002
	rdf:type skos:Concept;
	skos:prefLabel	"pursuit"@en-GB;
	skos:definition	"Two cyclists or teams set off from midway down opposite straights and try to make up the gap between them. "@en-GB;
	skos:inScheme <http://cv.iptc.org/newscodes/subjectcode/>;
	skos:exactMatch medtop:20000899;
	skos:broader	subj:15019000.

subj:15019003
	rdf:type skos:Concept;
	skos:prefLabel	"Olympic sprint"@en-GB;
	skos:definition	"Qualifying race held over 200m. From the quarter-finals two cyclists go head-to-heads. By teams races consist of three cyclists from different countries. "@en-GB;
	skos:inScheme <http://cv.iptc.org/newscodes/subjectcode/>;
	skos:closeMatch medtop:20000897;
	skos:broader	subj:15019000.

subj:15019004
	rdf:type skos:Concept;
	skos:prefLabel	"sprint"@en-GB;
	skos:definition	"Races between two cyclists over two or three laps, with a timed sprint finish over the last 200m. "@en-GB;
	skos:historyNote	"typo fixed in Explanation "@en-GB;
	skos:inScheme <http://cv.iptc.org/newscodes/subjectcode/>;
	skos:exactMatch medtop:20000897;
	skos:broader	subj:15019000.

subj:15019005
	rdf:type skos:Concept;
	skos:prefLabel	"Keirin"@en-GB;
	skos:definition	"Sprint between six cyclists where a pacemaker on a moped gradually increases the pace over the first 1400m. When the pacemaker leaves the track the race develops into a sprint finish over the final 6-700m. "@en-GB;
	skos:inScheme <http://cv.iptc.org/newscodes/subjectcode/>;
	skos:exactMatch medtop:20000901;
	skos:broader	subj:15019000.

subj:15019006
	rdf:type skos:Concept;
	skos:prefLabel	"points race"@en-GB;
	skos:definition	"Cyclists aim to complete the highest number of laps. Bonus points are picked up in intermediate sprints held every 2500m. "@en-GB;
	skos:inScheme <http://cv.iptc.org/newscodes/subjectcode/>;
	skos:exactMatch medtop:20000904;
	skos:broader	subj:15019000.

subj:15019007
	rdf:type skos:Concept;
	skos:prefLabel	"Madison race"@en-GB;
	skos:definition	"A points race by teams comprising two cyclists in relay-format. "@en-GB;
	skos:inScheme <http://cv.iptc.org/newscodes/subjectcode/>;
	skos:exactMatch medtop:20000902;
	skos:broader	subj:15019000.

subj:15019008
	rdf:type skos:Concept;
	skos:prefLabel	"500 m time trial"@en-GB;
	skos:definition	"Individual race against the clock over 500m for women. "@en-GB;
	skos:inScheme <http://cv.iptc.org/newscodes/subjectcode/>;
	skos:broadMatch medtop:20000900;
	skos:broader	subj:15019000.

subj:15019009
	rdf:type skos:Concept;
	skos:prefLabel	"1 km time trial"@en-GB;
	skos:definition	"Individual race over 1000m against the clock for men. "@en-GB;
	skos:inScheme <http://cv.iptc.org/newscodes/subjectcode/>;
	skos:broadMatch medtop:20000900;
	skos:broader	subj:15019000.

subj:15019010
	rdf:type skos:Concept;
	skos:prefLabel	"one hour"@en-GB;
	skos:definition	"Competitors aim to complete as many kilometres as possible in one hour. "@en-GB;
	skos:inScheme <http://cv.iptc.org/newscodes/subjectcode/>;
	skos:broadMatch medtop:20000892;
	skos:broader	subj:15019000.

subj:15019011
	rdf:type skos:Concept;
	skos:prefLabel	"road race"@en-GB;
	skos:definition	"Road race with all the competitor starting en masse. "@en-GB;
	skos:inScheme <http://cv.iptc.org/newscodes/subjectcode/>;
	skos:exactMatch medtop:20000905;
	skos:broader	subj:15019000.

subj:15019012
	rdf:type skos:Concept;
	skos:prefLabel	"road time trial"@en-GB;
	skos:definition	"A race or stage against the clock with each cyclist setting off individually. "@en-GB;
	skos:inScheme <http://cv.iptc.org/newscodes/subjectcode/>;
	skos:exactMatch medtop:20000900;
	skos:broader	subj:15019000.

subj:15019013
	rdf:type skos:Concept;
	skos:prefLabel	"staging race"@en-GB;
	skos:definition	"A race disputed by teams with the classifications determined by the combined times over a day. "@en-GB;
	skos:inScheme <http://cv.iptc.org/newscodes/subjectcode/>;
	skos:exactMatch medtop:20000906;
	skos:broader	subj:15019000.

subj:15019014
	rdf:type skos:Concept;
	skos:prefLabel	"cyclo-cross"@en-GB;
	skos:definition	"Staged on various surfaces - earth, grass, sand or tarmac. "@en-GB;
	skos:inScheme <http://cv.iptc.org/newscodes/subjectcode/>;
	skos:exactMatch medtop:20000898;
	skos:broader	subj:15019000.

subj:15019015
	rdf:type skos:Concept;
	skos:prefLabel	"Vtt"@en-GB;
	skos:definition	"Mountain bikes "@en-GB;
	skos:inScheme <http://cv.iptc.org/newscodes/subjectcode/>;
	skos:closeMatch medtop:20000903;
	skos:broader	subj:15019000.

subj:15019016
	rdf:type skos:Concept;
	skos:prefLabel	"Vtt-cross"@en-GB;
	skos:definition	"An endurance race on mountain bikes around a 10km circuit over various terrain and with different degrees of slopes. Competitors are not allowed any exterior help. "@en-GB;
	skos:historyNote	"typo fixed in Explanation "@en-GB;
	skos:inScheme <http://cv.iptc.org/newscodes/subjectcode/>;
	skos:broadMatch medtop:20000903;
	skos:broader	subj:15019000.

subj:15019017
	rdf:type skos:Concept;
	skos:prefLabel	"Vtt-downhill"@en-GB;
	skos:definition	"Individual mountain bike race against the clock staged on a downhill circuit featuring obstacles. "@en-GB;
	skos:inScheme <http://cv.iptc.org/newscodes/subjectcode/>;
	skos:broadMatch medtop:20000903;
	skos:broader	subj:15019000.

subj:15019018
	rdf:type skos:Concept;
	skos:prefLabel	"bi-crossing"@en-GB;
	skos:definition	"A race where competitors have to cover a circuit with obstacles as quickly as possible. "@en-GB;
	skos:historyNote	"typo fixed in Explanation "@en-GB;
	skos:inScheme <http://cv.iptc.org/newscodes/subjectcode/>;
	skos:exactMatch medtop:20000894;
	skos:broader	subj:15019000.

subj:15019019
	rdf:type skos:Concept;
	skos:prefLabel	"trial"@en-GB;
	skos:definition	"A timed race in which competitors on mountain bikes must negotiate tricky terrain and obstacles without putting their feet down. "@en-GB;
	skos:historyNote	"typo fixed in Explanation "@en-GB;
	skos:inScheme <http://cv.iptc.org/newscodes/subjectcode/>;
	skos:broadMatch medtop:20000903;
	skos:broader	subj:15019000.

subj:15019020
	rdf:type skos:Concept;
	skos:prefLabel	"artistic cycling"@en-GB;
	skos:definition	"Individual or teams on one or two bicycles in an arena. Points are awarded by a jury. "@en-GB;
	skos:inScheme <http://cv.iptc.org/newscodes/subjectcode/>;
	skos:exactMatch medtop:20000893;
	skos:broader	subj:15019000.

subj:15019021
	rdf:type skos:Concept;
	skos:prefLabel	"cycle ball"@en-GB;
	skos:definition	"Competitive team sport using bicycles. One team against another with two persons per team. The aim is for competitors to move the ball using the front and rear wheels without letting their feet touch the ground. "@en-GB;
	skos:inScheme <http://cv.iptc.org/newscodes/subjectcode/>;
	skos:exactMatch medtop:20000896;
	skos:broader	subj:15019000.

subj:15020000
	rdf:type skos:Concept;
	skos:prefLabel	"dancing"@en-GB;
	skos:definition	"Dancing competition where couples are judged on technique and interpretation. "@en-GB;
	skos:inScheme <http://cv.iptc.org/newscodes/subjectcode/>;
	skos:exactMatch medtop:20000911;
	skos:broader	subj:15000000.

subj:15021000
	rdf:type skos:Concept;
	skos:prefLabel	"diving"@en-GB;
	skos:definition	"Competitors dive off a fixed or spring board and are assessed by seven judges giving marks up to ten for their acrobatic moves. "@en-GB;
	skos:inScheme <http://cv.iptc.org/newscodes/subjectcode/>;
	skos:exactMatch medtop:20000913;
	skos:broader	subj:15000000;
	skos:narrower	subj:15021001;
	skos:narrower	subj:15021002;
	skos:narrower	subj:15021003;
	skos:narrower	subj:15021004;
	skos:narrower	subj:15021005;
	skos:narrower	subj:15021006.

subj:15021001
	rdf:type skos:Concept;
	skos:prefLabel	"10 m platform"@en-GB;
	skos:definition	"Divers take off from a ten metre high platform. "@en-GB;
	skos:inScheme <http://cv.iptc.org/newscodes/subjectcode/>;
	skos:broadMatch medtop:20000914;
	skos:broader	subj:15021000.

subj:15021002
	rdf:type skos:Concept;
	skos:prefLabel	"10 m platform synchronised"@en-GB;
	skos:definition	"Two competitors from the same team dive off at the same time from separate platforms. As well as being judged on the standard criteria they are also awarded marks for synchronisation. "@en-GB;
	skos:inScheme <http://cv.iptc.org/newscodes/subjectcode/>;
	skos:broadMatch medtop:20000916;
	skos:broader	subj:15021000.

subj:15021003
	rdf:type skos:Concept;
	skos:prefLabel	"3 m springboard"@en-GB;
	skos:definition	"Divers dive from a three-metre high springboard. "@en-GB;
	skos:inScheme <http://cv.iptc.org/newscodes/subjectcode/>;
	skos:broadMatch medtop:20000915;
	skos:broader	subj:15021000.

subj:15021004
	rdf:type skos:Concept;
	skos:prefLabel	"3 m springboard synchronised"@en-GB;
	skos:definition	"Two competitors from the same team dive off at the same time from separate three-metre high springboards. As well as being judged on the standard criteria they are also awarded marks for synchronisation. "@en-GB;
	skos:inScheme <http://cv.iptc.org/newscodes/subjectcode/>;
	skos:broadMatch medtop:20000916;
	skos:broader	subj:15021000.

subj:15021005
	rdf:type skos:Concept;
	skos:prefLabel	"subaquatics"@en-GB;
	skos:definition	"Sports like hockey held under water "@en-GB;
	skos:historyNote	"typo fixed in Explanation "@en-GB;
	skos:inScheme <http://cv.iptc.org/newscodes/subjectcode/>;
	skos:exactMatch medtop:20000918;
	skos:broader	subj:15021000.

subj:15021006
	rdf:type skos:Concept;
	skos:prefLabel	"scuba diving"@en-GB;
	skos:definition	"Diving into different depths, with time measurement "@en-GB;
	skos:inScheme <http://cv.iptc.org/newscodes/subjectcode/>;
	skos:exactMatch medtop:20000917;
	skos:broader	subj:15021000.

subj:15022000
	rdf:type skos:Concept;
	skos:prefLabel	"equestrian"@en-GB;
	skos:definition	"Sport involving a horse and rider. "@en-GB;
	skos:inScheme <http://cv.iptc.org/newscodes/subjectcode/>;
	skos:exactMatch medtop:20000923;
	skos:broader	subj:15000000;
	skos:narrower	subj:15022001;
	skos:narrower	subj:15022002;
	skos:narrower	subj:15022003;
	skos:narrower	subj:15022004.

subj:15022001
	rdf:type skos:Concept;
	skos:prefLabel	"three-day event"@en-GB;
	skos:definition	"Equestrian event involving three disciplines - Dressage, cross-country and show jumping. "@en-GB;
	skos:inScheme <http://cv.iptc.org/newscodes/subjectcode/>;
	skos:exactMatch medtop:20000927;
	skos:broader	subj:15022000.

subj:15022002
	rdf:type skos:Concept;
	skos:prefLabel	"dressage"@en-GB;
	skos:definition	"A rider is judged on a series of moves at three different paces - walk, trot and gallop. "@en-GB;
	skos:inScheme <http://cv.iptc.org/newscodes/subjectcode/>;
	skos:exactMatch medtop:20000925;
	skos:broader	subj:15022000.

subj:15022003
	rdf:type skos:Concept;
	skos:prefLabel	"jumping"@en-GB;
	skos:definition	"A rider and horse attempt to jump a series of obstacles in an enclosed arena against the clock. "@en-GB;
	skos:inScheme <http://cv.iptc.org/newscodes/subjectcode/>;
	skos:exactMatch medtop:20000926;
	skos:broader	subj:15022000.

subj:15022004
	rdf:type skos:Concept;
	skos:prefLabel	"cross country"@en-GB;
	skos:definition	"Equestrian event held on a designated circuit in the countryside featuring artificial and natural obstacles. "@en-GB;
	skos:historyNote	"typo fixed in Explanation "@en-GB;
	skos:inScheme <http://cv.iptc.org/newscodes/subjectcode/>;
	skos:exactMatch medtop:20000924;
	skos:broader	subj:15022000.

subj:15023000
	rdf:type skos:Concept;
	skos:prefLabel	"fencing"@en-GB;
	skos:definition	"Combat sport using a sword or foil. "@en-GB;
	skos:inScheme <http://cv.iptc.org/newscodes/subjectcode/>;
	skos:exactMatch medtop:20000929;
	skos:broader	subj:15000000;
	skos:narrower	subj:15023001;
	skos:narrower	subj:15023002;
	skos:narrower	subj:15023003.

subj:15023001
	rdf:type skos:Concept;
	skos:prefLabel	"epee"@en-GB;
	skos:definition	"category of fencing using a weapon with a triangular cross-section blade and a large bell guard. "@en-GB;
	skos:inScheme <http://cv.iptc.org/newscodes/subjectcode/>;
	skos:exactMatch medtop:20000930;
	skos:broader	subj:15023000.

subj:15023002
	rdf:type skos:Concept;
	skos:prefLabel	"foil"@en-GB;
	skos:definition	"category of fencing using a weapon with a rectangular cross-section blade and a small bell guard. "@en-GB;
	skos:inScheme <http://cv.iptc.org/newscodes/subjectcode/>;
	skos:exactMatch medtop:20000931;
	skos:broader	subj:15023000.

subj:15023003
	rdf:type skos:Concept;
	skos:prefLabel	"sabre"@en-GB;
	skos:definition	"a fencing weapon with a flat blade and knuckle guard used with cutting or thrusting moves. "@en-GB;
	skos:inScheme <http://cv.iptc.org/newscodes/subjectcode/>;
	skos:exactMatch medtop:20000932;
	skos:broader	subj:15023000.

subj:15024000
	rdf:type skos:Concept;
	skos:prefLabel	"field Hockey"@en-GB;
	skos:definition	"A ball sport involving two teams of 11 players using curved sticks. The aim is to score as many goals as possible. "@en-GB;
	skos:inScheme <http://cv.iptc.org/newscodes/subjectcode/>;
	skos:exactMatch medtop:20000933;
	skos:broader	subj:15000000;
	skos:narrower	subj:15024001.

subj:15024001
	rdf:type skos:Concept;
	skos:prefLabel	"roll hockey"@en-GB;
	skos:definition	"Team sport similar to ice hockey, executed on 4 wheel roller skates with sticks and a ball "@en-GB;
	skos:inScheme <http://cv.iptc.org/newscodes/subjectcode/>;
	skos:exactMatch medtop:20001025;
	skos:broader	subj:15024000.

subj:15025000
	rdf:type skos:Concept;
	skos:prefLabel	"figure Skating"@en-GB;
	skos:definition	"To obtain the best marks possible from nine judges who award scores after two prepared sections - both skated to music - during which competitors must attempt to achieve the greatest possible harmony between artistic flair and technical precision. "@en-GB;
	skos:inScheme <http://cv.iptc.org/newscodes/subjectcode/>;
	skos:exactMatch medtop:20000934;
	skos:broader	subj:15000000;
	skos:narrower	subj:15025001;
	skos:narrower	subj:15025002;
	skos:narrower	subj:15025003.

subj:15025001
	rdf:type skos:Concept;
	skos:prefLabel	"singles"@en-GB;
	skos:definition	"The individual events comprise a short program which counts for 33.3% of the score, and the free skate which is worth 66.7%. "@en-GB;
	skos:inScheme <http://cv.iptc.org/newscodes/subjectcode/>;
	skos:broadMatch medtop:20000934;
	skos:broader	subj:15025000.

subj:15025002
	rdf:type skos:Concept;
	skos:prefLabel	"pairs"@en-GB;
	skos:definition	"The pairs event comprise a short program which counts for 33.3% of the score, and the free skate which is worth 66.7%. "@en-GB;
	skos:inScheme <http://cv.iptc.org/newscodes/subjectcode/>;
	skos:broadMatch medtop:20000934;
	skos:broader	subj:15025000.

subj:15025003
	rdf:type skos:Concept;
	skos:prefLabel	"ice dance"@en-GB;
	skos:definition	"Takes place over three days with, in order, two compulsory dances, the original dance (2min 30sec) and the free dance (4min). "@en-GB;
	skos:inScheme <http://cv.iptc.org/newscodes/subjectcode/>;
	skos:exactMatch medtop:20000935;
	skos:broader	subj:15025000.

subj:15026000
	rdf:type skos:Concept;
	skos:prefLabel	"freestyle Skiing"@en-GB;
	skos:definition	"Competitors perform a series of breathtaking acrobatic leaps from a prepared jump. Combined with moguls, jumps and ski ballet. "@en-GB;
	skos:inScheme <http://cv.iptc.org/newscodes/subjectcode/>;
	skos:exactMatch medtop:20001058;
	skos:broader	subj:15000000;
	skos:narrower	subj:15026001;
	skos:narrower	subj:15026002;
	skos:narrower	subj:15026003.

subj:15026001
	rdf:type skos:Concept;
	skos:prefLabel	"moguls"@en-GB;
	skos:definition	"Contestants attack a heavily moguled slope, performing technically challenging turns and jumps, while maintaining the most direct line from the top to the bottom of the hill. "@en-GB;
	skos:historyNote	"typo fixed in Explanation "@en-GB;
	skos:inScheme <http://cv.iptc.org/newscodes/subjectcode/>;
	skos:broadMatch medtop:20001058;
	skos:broader	subj:15026000.

subj:15026002
	rdf:type skos:Concept;
	skos:prefLabel	"aerials"@en-GB;
	skos:definition	"Competitors perform a series of aerial twists and turns from a prepared jump. "@en-GB;
	skos:inScheme <http://cv.iptc.org/newscodes/subjectcode/>;
	skos:broadMatch medtop:20001058;
	skos:broader	subj:15026000.

subj:15026003
	rdf:type skos:Concept;
	skos:prefLabel	"artistic skiing"@en-GB;
	skos:definition	"Competitors perform a series of artistic moves (jumps and twists) all set to music. The use of ski poles is permitted. "@en-GB;
	skos:inScheme <http://cv.iptc.org/newscodes/subjectcode/>;
	skos:broadMatch medtop:20001058;
	skos:broader	subj:15026000.

subj:15027000
	rdf:type skos:Concept;
	skos:prefLabel	"golf"@en-GB;
	skos:definition	"Competitors attempt to hit a small white ball with different clubs around a course of 18 holes varying in distance. The object is to make the fewest strokes possible. "@en-GB;
	skos:inScheme <http://cv.iptc.org/newscodes/subjectcode/>;
	skos:exactMatch medtop:20000940;
	skos:broader	subj:15000000.

subj:15028000
	rdf:type skos:Concept;
	skos:prefLabel	"gymnastics"@en-GB;
	skos:definition	"A sport consisting of a variety of disciplines in which gymnasts perform artistic and acrobatic moves on different apparatus. There are 6 disciplines for men and 4 for women. "@en-GB;
	skos:inScheme <http://cv.iptc.org/newscodes/subjectcode/>;
	skos:exactMatch medtop:20000942;
	skos:broader	subj:15000000;
	skos:narrower	subj:15028001;
	skos:narrower	subj:15028002;
	skos:narrower	subj:15028003;
	skos:narrower	subj:15028004;
	skos:narrower	subj:15028005;
	skos:narrower	subj:15028006;
	skos:narrower	subj:15028007;
	skos:narrower	subj:15028008;
	skos:narrower	subj:15028009;
	skos:narrower	subj:15028010;
	skos:narrower	subj:15028011;
	skos:narrower	subj:15028012;
	skos:narrower	subj:15028013;
	skos:narrower	subj:15028014;
	skos:narrower	subj:15028015.

subj:15028001
	rdf:type skos:Concept;
	skos:prefLabel	"floor exercise"@en-GB;
	skos:definition	"A gymnastics floor exercise on a 12m/sq matt. "@en-GB;
	skos:inScheme <http://cv.iptc.org/newscodes/subjectcode/>;
	skos:broadMatch medtop:20001152;
	skos:broader	subj:15028000.

subj:15028002
	rdf:type skos:Concept;
	skos:prefLabel	"vault"@en-GB;
	skos:definition	"gymnasts propel themselves by jumping on a trampoline after running quickly down a 25m lane "@en-GB;
	skos:inScheme <http://cv.iptc.org/newscodes/subjectcode/>;
	skos:broadMatch medtop:20001152;
	skos:broader	subj:15028000.

subj:15028003
	rdf:type skos:Concept;
	skos:prefLabel	"pommel horse"@en-GB;
	skos:definition	"Gymnasts perform an uninterrupted swing motion over a handled horse using balance and strength. "@en-GB;
	skos:inScheme <http://cv.iptc.org/newscodes/subjectcode/>;
	skos:broadMatch medtop:20001152;
	skos:broader	subj:15028000.

subj:15028004
	rdf:type skos:Concept;
	skos:prefLabel	"uneven bars"@en-GB;
	skos:definition	"Gymnasts run through an airborne routine swinging around and between the uneven bars. "@en-GB;
	skos:historyNote	"typo fixed in Explanation "@en-GB;
	skos:inScheme <http://cv.iptc.org/newscodes/subjectcode/>;
	skos:broadMatch medtop:20001152;
	skos:broader	subj:15028000.

subj:15028005
	rdf:type skos:Concept;
	skos:prefLabel	"parallel bars"@en-GB;
	skos:definition	"Gymnasts swing and turn with guile and grace around the parallel bars. "@en-GB;
	skos:inScheme <http://cv.iptc.org/newscodes/subjectcode/>;
	skos:broadMatch medtop:20001152;
	skos:broader	subj:15028000.

subj:15028006
	rdf:type skos:Concept;
	skos:prefLabel	"horizontal bar"@en-GB;
	skos:definition	"Gymnasts turn, spin and perform pirouettes around the horizontal bar. "@en-GB;
	skos:inScheme <http://cv.iptc.org/newscodes/subjectcode/>;
	skos:broadMatch medtop:20001152;
	skos:broader	subj:15028000.

subj:15028007
	rdf:type skos:Concept;
	skos:prefLabel	"rings"@en-GB;
	skos:definition	"Gymnasts perform feats of balance and strength from two suspended rings. "@en-GB;
	skos:inScheme <http://cv.iptc.org/newscodes/subjectcode/>;
	skos:broadMatch medtop:20001152;
	skos:broader	subj:15028000.

subj:15028008
	rdf:type skos:Concept;
	skos:prefLabel	"beam"@en-GB;
	skos:definition	"Gymnasts perform leaps and flips from the much feared balance beam just 10 cm wide. "@en-GB;
	skos:historyNote	"typo fixed in Explanation "@en-GB;
	skos:inScheme <http://cv.iptc.org/newscodes/subjectcode/>;
	skos:broadMatch medtop:20001152;
	skos:broader	subj:15028000.

subj:15028009
	rdf:type skos:Concept;
	skos:prefLabel	"rhythmic"@en-GB;
	skos:definition	"A mixture of dance and gymnastic moves. "@en-GB;
	skos:historyNote	"typo fixed in Name "@en-GB;
	skos:inScheme <http://cv.iptc.org/newscodes/subjectcode/>;
	skos:exactMatch medtop:20000951;
	skos:broader	subj:15028000.

subj:15028010
	rdf:type skos:Concept;
	skos:prefLabel	"clubs"@en-GB;
	skos:definition	"Dance and gymnastic moves whilst juggling clubs. "@en-GB;
	skos:inScheme <http://cv.iptc.org/newscodes/subjectcode/>;
	skos:broadMatch medtop:20000951;
	skos:broader	subj:15028000.

subj:15028011
	rdf:type skos:Concept;
	skos:prefLabel	"hoop"@en-GB;
	skos:definition	"A hoop is rolled and thrown whilst performing a dance routine. "@en-GB;
	skos:inScheme <http://cv.iptc.org/newscodes/subjectcode/>;
	skos:broadMatch medtop:20000951;
	skos:broader	subj:15028000.

subj:15028012
	rdf:type skos:Concept;
	skos:prefLabel	"ribbon"@en-GB;
	skos:definition	"Gymnasts work through a pre-arranged routine whilst manipulating a spectacular length of ribbon. "@en-GB;
	skos:historyNote	"typo fixed in Explanation "@en-GB;
	skos:inScheme <http://cv.iptc.org/newscodes/subjectcode/>;
	skos:broadMatch medtop:20000951;
	skos:broader	subj:15028000.

subj:15028013
	rdf:type skos:Concept;
	skos:prefLabel	"rope"@en-GB;
	skos:definition	"Jump and figure movements are performed while a rope is manipulated. "@en-GB;
	skos:inScheme <http://cv.iptc.org/newscodes/subjectcode/>;
	skos:broadMatch medtop:20000951;
	skos:broader	subj:15028000.

subj:15028014
	rdf:type skos:Concept;
	skos:prefLabel	"ball"@en-GB;
	skos:definition	"An exercise based on suppleness of the body using a ball. "@en-GB;
	skos:inScheme <http://cv.iptc.org/newscodes/subjectcode/>;
	skos:broadMatch medtop:20000951;
	skos:broader	subj:15028000.

subj:15028015
	rdf:type skos:Concept;
	skos:prefLabel	"trampoline"@en-GB;
	skos:definition	"Competitors perform complicated twists and turns whilst bouncing on the trampoline. "@en-GB;
	skos:inScheme <http://cv.iptc.org/newscodes/subjectcode/>;
	skos:exactMatch medtop:20000955;
	skos:broader	subj:15028000.

subj:15029000
	rdf:type skos:Concept;
	skos:prefLabel	"handball (team)"@en-GB;
	skos:definition	"A ball game using the hands contested by two teams of seven trying to throw the ball into the opponents goal. "@en-GB;
	skos:inScheme <http://cv.iptc.org/newscodes/subjectcode/>;
	skos:exactMatch medtop:20000958;
	skos:broader	subj:15000000.

subj:15030000
	rdf:type skos:Concept;
	skos:prefLabel	"horse racing, harness racing"@en-GB;
	skos:definition	"Mounted horse races. "@en-GB;
	skos:inScheme <http://cv.iptc.org/newscodes/subjectcode/>;
	skos:exactMatch medtop:20000960;
	skos:broader	subj:15000000;
	skos:narrower	subj:15030001;
	skos:narrower	subj:15030002;
	skos:narrower	subj:15030003;
	skos:narrower	subj:15030004.

subj:15030001
	rdf:type skos:Concept;
	skos:prefLabel	"flat racing"@en-GB;
	skos:definition	"A horse race over a flat course. "@en-GB;
	skos:inScheme <http://cv.iptc.org/newscodes/subjectcode/>;
	skos:exactMatch medtop:20000961;
	skos:broader	subj:15030000.

subj:15030002
	rdf:type skos:Concept;
	skos:prefLabel	"steeple chase"@en-GB;
	skos:definition	"A mounted horse race over at least eight classic obstacles, four of which must be different, such as the water jump, spruce fences, mud walls etc. "@en-GB;
	skos:inScheme <http://cv.iptc.org/newscodes/subjectcode/>;
	skos:exactMatch medtop:20000963;
	skos:broader	subj:15030000.

subj:15030003
	rdf:type skos:Concept;
	skos:prefLabel	"trotting"@en-GB;
	skos:definition	"Horses pitched to a jockeyed buggy race in a trot round a flat course. "@en-GB;
	skos:inScheme <http://cv.iptc.org/newscodes/subjectcode/>;
	skos:exactMatch medtop:20000962;
	skos:broader	subj:15030000.

subj:15030004
	rdf:type skos:Concept;
	skos:prefLabel	"cross country"@en-GB;
	skos:definition	"A long distance race including rustic obstacles such as real fences, streams and fallen trees. "@en-GB;
	skos:inScheme <http://cv.iptc.org/newscodes/subjectcode/>;
	skos:broadMatch medtop:20000960;
	skos:broader	subj:15030000.

subj:15031000
	rdf:type skos:Concept;
	skos:prefLabel	"ice hockey"@en-GB;
	skos:definition	"Two teams of six heavily padded skaters try and outscore each other by hitting a puck into the opponents goal. "@en-GB;
	skos:inScheme <http://cv.iptc.org/newscodes/subjectcode/>;
	skos:exactMatch medtop:20000965;
	skos:broader	subj:15000000;
	skos:narrower	subj:15031001;
	skos:narrower	subj:15031002.

subj:15031001
	rdf:type skos:Concept;
	skos:prefLabel	"National Hockey League (North American)"@en-GB;
	skos:definition	"Teams from the US and Canada make up the North American continents top league. "@en-GB;
	skos:inScheme <http://cv.iptc.org/newscodes/subjectcode/>;
	skos:broadMatch medtop:20000965;
	skos:broader	subj:15031000.

subj:15031002
	rdf:type skos:Concept;
	skos:prefLabel	"sledge hockey"@en-GB;
	skos:definition	"Like ice hockey but instead of skates small sledges are used. Competitors move by pushing with the arms "@en-GB;
	skos:inScheme <http://cv.iptc.org/newscodes/subjectcode/>;
	skos:exactMatch medtop:20000966;
	skos:broader	subj:15031000.

subj:15032000
	rdf:type skos:Concept;
	skos:prefLabel	"Jai Alai (Pelota)"@en-GB;
	skos:definition	"Because of the game organization, the proper identification of a specific game may require the combination of 2 subject details "@en-GB;
	skos:inScheme <http://cv.iptc.org/newscodes/subjectcode/>;
	skos:exactMatch medtop:20000968;
	skos:broader	subj:15000000;
	skos:narrower	subj:15032001;
	skos:narrower	subj:15032002;
	skos:narrower	subj:15032003;
	skos:narrower	subj:15032004;
	skos:narrower	subj:15032005;
	skos:narrower	subj:15032006;
	skos:narrower	subj:15032007;
	skos:narrower	subj:15032008;
	skos:narrower	subj:15032009;
	skos:narrower	subj:15032010;
	skos:narrower	subj:15032011;
	skos:narrower	subj:15032012.

subj:15032001
	rdf:type skos:Concept;
	skos:prefLabel	"fronton"@en-GB;
	skos:definition	"The ´fronton´ known as ´Fronton Place Libre´ consists of a rectangular outdoor court plus a large pink shaped wall at one end. The two sides and the other end are left opened. "@en-GB;
	skos:inScheme <http://cv.iptc.org/newscodes/subjectcode/>;
	skos:broadMatch medtop:20000968;
	skos:broader	subj:15032000.

subj:15032002
	rdf:type skos:Concept;
	skos:prefLabel	"jai-alai"@en-GB;
	skos:definition	"A ´Jaï-Alai´ is an indoor fronton with a 56 meters long court which is used exclusively to play ´chistera-ancha´. Three walls are used in the game: the front, the back and the left hand wall. "@en-GB;
	skos:inScheme <http://cv.iptc.org/newscodes/subjectcode/>;
	skos:broadMatch medtop:20000968;
	skos:broader	subj:15032000.

subj:15032003
	rdf:type skos:Concept;
	skos:prefLabel	"left wall"@en-GB;
	skos:definition	"A ´fronton with left hand wall´ is an indoor fronton with a 36 meters long court where Pala or Main Nue are played. Three walls are used in the game: the front, the back and the left hand wall. "@en-GB;
	skos:inScheme <http://cv.iptc.org/newscodes/subjectcode/>;
	skos:broadMatch medtop:20000968;
	skos:broader	subj:15032000.

subj:15032004
	rdf:type skos:Concept;
	skos:prefLabel	"trinquet"@en-GB;
	skos:definition	"A ´Trinquet´ is an indoor fronton with a 28.5 meters long court surrounded by four walls. The four walls are used in the game. "@en-GB;
	skos:inScheme <http://cv.iptc.org/newscodes/subjectcode/>;
	skos:broadMatch medtop:20000968;
	skos:broader	subj:15032000.

subj:15032005
	rdf:type skos:Concept;
	skos:prefLabel	"rebot"@en-GB;
	skos:definition	"The ´rebot´ is the game played in a fronton ´place libre´ with 5 players in each team. They use a ´chistera´ (56 cm long and 12 cm large) or bare hands. "@en-GB;
	skos:inScheme <http://cv.iptc.org/newscodes/subjectcode/>;
	skos:broadMatch medtop:20000968;
	skos:broader	subj:15032000.

subj:15032006
	rdf:type skos:Concept;
	skos:prefLabel	"chistera ancha"@en-GB;
	skos:definition	"The ´chistera-ancha´ also called the ´cesta punta´ is the game played in a ´jaï alai´ with 1 or 2 players in each team. The players use a long curved basket called the ´chistera´ (68 cm long and 13 cm wide). "@en-GB;
	skos:inScheme <http://cv.iptc.org/newscodes/subjectcode/>;
	skos:broadMatch medtop:20000968;
	skos:broader	subj:15032000.

subj:15032007
	rdf:type skos:Concept;
	skos:prefLabel	"chistera corta"@en-GB;
	skos:definition	"The ´chistera-corta´ is the game played in a fronton ´place libre´ with left hand wall and 3 players in each team. The players use a long curved basket called the ´chistera´ (56 cm long and 12 cm wide). "@en-GB;
	skos:inScheme <http://cv.iptc.org/newscodes/subjectcode/>;
	skos:broadMatch medtop:20000968;
	skos:broader	subj:15032000.

subj:15032008
	rdf:type skos:Concept;
	skos:prefLabel	"bare hand"@en-GB;
	skos:definition	"The ´Main Nue´ (bare hand) is the ancestor of all Basque sports. "@en-GB;
	skos:inScheme <http://cv.iptc.org/newscodes/subjectcode/>;
	skos:broadMatch medtop:20000968;
	skos:broader	subj:15032000.

subj:15032009
	rdf:type skos:Concept;
	skos:prefLabel	"pala-ancha"@en-GB;
	skos:definition	"The ´pala-ancha´ is the game played in a fronton ´place libre´ with 2 players in each team. The players use a heavy wooden bat ´the pala´ (50 cm long and 20 cm wide). "@en-GB;
	skos:inScheme <http://cv.iptc.org/newscodes/subjectcode/>;
	skos:broadMatch medtop:20000968;
	skos:broader	subj:15032000.

subj:15032010
	rdf:type skos:Concept;
	skos:prefLabel	"pala-corta"@en-GB;
	skos:definition	"The ´pala-corta´ is the game played in a fronton with left hand wall and 2 players in each team. The players use a heavy wooden bat the ´pala-corta´ (50 cm long and 10 cm wide). The ´pala´ is the name for a heavy wooden bat. "@en-GB;
	skos:historyNote	"Explanation shortened "@en-GB;
	skos:inScheme <http://cv.iptc.org/newscodes/subjectcode/>;
	skos:broadMatch medtop:20000968;
	skos:broader	subj:15032000.

subj:15032011
	rdf:type skos:Concept;
	skos:prefLabel	"pasaka"@en-GB;
	skos:definition	"The ´pasaka´ is the name of the game played in a trinquet by teams of 2 players facing each other on each side of a net where the pelota is hit between opponents. "@en-GB;
	skos:inScheme <http://cv.iptc.org/newscodes/subjectcode/>;
	skos:broadMatch medtop:20000968;
	skos:broader	subj:15032000.

subj:15032012
	rdf:type skos:Concept;
	skos:prefLabel	"xare"@en-GB;
	skos:definition	"The ´xare´, is the name of the game played in a trinquet by teams of 2 players. The players use a ´xare´ (or the Argentina bat) 55 cm long and 16 cm wide. "@en-GB;
	skos:inScheme <http://cv.iptc.org/newscodes/subjectcode/>;
	skos:broadMatch medtop:20000968;
	skos:broader	subj:15032000.

subj:15033000
	rdf:type skos:Concept;
	skos:prefLabel	"judo"@en-GB;
	skos:definition	"A defensive martial art. "@en-GB;
	skos:inScheme <http://cv.iptc.org/newscodes/subjectcode/>;
	skos:exactMatch medtop:20000969;
	skos:broader	subj:15000000;
	skos:narrower	subj:15033001;
	skos:narrower	subj:15033002;
	skos:narrower	subj:15033003;
	skos:narrower	subj:15033004;
	skos:narrower	subj:15033005;
	skos:narrower	subj:15033006;
	skos:narrower	subj:15033007.

subj:15033001
	rdf:type skos:Concept;
	skos:prefLabel	"heavyweight"@en-GB;
	skos:definition	"Weight categoriy in Judo: open but usually over 100kg for men and over 78kg for women "@en-GB;
	skos:inScheme <http://cv.iptc.org/newscodes/subjectcode/>;
	skos:broadMatch medtop:20000974;
	skos:broader	subj:15033000.

subj:15033002
	rdf:type skos:Concept;
	skos:prefLabel	"half-heavyweight"@en-GB;
	skos:definition	"Weight categoriy in Judo: up to 100kg for men and 78kg for women. "@en-GB;
	skos:inScheme <http://cv.iptc.org/newscodes/subjectcode/>;
	skos:broadMatch medtop:20000971;
	skos:broader	subj:15033000.

subj:15033003
	rdf:type skos:Concept;
	skos:prefLabel	"middleweight"@en-GB;
	skos:definition	"Weight categoriy in Judo: up to 90kg for men and 70kg for women. "@en-GB;
	skos:inScheme <http://cv.iptc.org/newscodes/subjectcode/>;
	skos:broadMatch medtop:20000976;
	skos:broader	subj:15033000.

subj:15033004
	rdf:type skos:Concept;
	skos:prefLabel	"half-middleweight"@en-GB;
	skos:definition	"Weight categoriy in Judo: up to 81kg for men and 63kg for women. "@en-GB;
	skos:inScheme <http://cv.iptc.org/newscodes/subjectcode/>;
	skos:broadMatch medtop:20000973;
	skos:broader	subj:15033000.

subj:15033005
	rdf:type skos:Concept;
	skos:prefLabel	"half-lightweight"@en-GB;
	skos:definition	"Weight categoriy in Judo: up to 73kg for men and 57kg for women. "@en-GB;
	skos:inScheme <http://cv.iptc.org/newscodes/subjectcode/>;
	skos:broadMatch medtop:20000972;
	skos:broader	subj:15033000.

subj:15033006
	rdf:type skos:Concept;
	skos:prefLabel	"lightweight"@en-GB;
	skos:definition	"Weight categoriy in Judo: up to 66kg for men and 52kg for women. "@en-GB;
	skos:inScheme <http://cv.iptc.org/newscodes/subjectcode/>;
	skos:broadMatch medtop:20000975;
	skos:broader	subj:15033000.

subj:15033007
	rdf:type skos:Concept;
	skos:prefLabel	"extra lightweight"@en-GB;
	skos:definition	"Weight categoriy in Judo: up to 60kg for men and 48kg for women. "@en-GB;
	skos:inScheme <http://cv.iptc.org/newscodes/subjectcode/>;
	skos:broadMatch medtop:20000970;
	skos:broader	subj:15033000.

subj:15034000
	rdf:type skos:Concept;
	skos:prefLabel	"karate"@en-GB;
	skos:definition	"A martial art where chops, punches, kicks and throws are used to defeat an opponent. "@en-GB;
	skos:inScheme <http://cv.iptc.org/newscodes/subjectcode/>;
	skos:exactMatch medtop:20000983;
	skos:broader	subj:15000000;
	skos:narrower	subj:15034001;
	skos:narrower	subj:15034002.

subj:15034001
	rdf:type skos:Concept;
	skos:prefLabel	"sparring"@en-GB;
	skos:definition	"Boxing without competition, with padded helmets "@en-GB;
	skos:inScheme <http://cv.iptc.org/newscodes/subjectcode/>;
	skos:broadMatch medtop:20000983;
	skos:broader	subj:15034000.

subj:15034002
	rdf:type skos:Concept;
	skos:prefLabel	"formal exercise-DEPRECATED"@en-GB;
	skos:definition	"NA "@en-GB;
	skos:historyNote	"DEPRECATED in V 16 "@en-GB;
	skos:inScheme <http://cv.iptc.org/newscodes/subjectcode/>;
	skos:broadMatch medtop:20000983;
	skos:broader	subj:15034000.

subj:15035000
	rdf:type skos:Concept;
	skos:prefLabel	"lacrosse"@en-GB;
	skos:definition	"Two teams of helmeted and padded players try and outscore each other using a netted stick and hard ball. "@en-GB;
	skos:inScheme <http://cv.iptc.org/newscodes/subjectcode/>;
	skos:exactMatch medtop:20000986;
	skos:broader	subj:15000000.

subj:15036000
	rdf:type skos:Concept;
	skos:prefLabel	"luge"@en-GB;
	skos:definition	"Luge (French word for sled) is competed in singles or doubles. The competitor(s) lay on their back(s) on an open sled and race down a course. The competitor(s) and the sled must be in contact when passing the finishing line. "@en-GB;
	skos:historyNote	"Explanation shortened "@en-GB;
	skos:inScheme <http://cv.iptc.org/newscodes/subjectcode/>;
	skos:exactMatch medtop:20000987;
	skos:broader	subj:15000000;
	skos:narrower	subj:15036001;
	skos:narrower	subj:15036002.

subj:15036001
	rdf:type skos:Concept;
	skos:prefLabel	"singles"@en-GB;
	skos:definition	"individual time trial event in a one seater luge "@en-GB;
	skos:inScheme <http://cv.iptc.org/newscodes/subjectcode/>;
	skos:broadMatch medtop:20000987;
	skos:broader	subj:15036000.

subj:15036002
	rdf:type skos:Concept;
	skos:prefLabel	"doubles"@en-GB;
	skos:definition	"time trial for a twin berth luge "@en-GB;
	skos:inScheme <http://cv.iptc.org/newscodes/subjectcode/>;
	skos:broadMatch medtop:20000987;
	skos:broader	subj:15036000.

subj:15037000
	rdf:type skos:Concept;
	skos:prefLabel	"marathon"@en-GB;
	skos:definition	"A road race where competitors run 42.195km, generally through city streets "@en-GB;
	skos:inScheme <http://cv.iptc.org/newscodes/subjectcode/>;
	skos:exactMatch medtop:20000988;
	skos:broader	subj:15000000.

subj:15038000
	rdf:type skos:Concept;
	skos:prefLabel	"modern pentathlon"@en-GB;
	skos:definition	"The Modern Pentathlon comprises five events run over a single day in the following order: shooting, fencing, swimming, horse riding and running. "@en-GB;
	skos:inScheme <http://cv.iptc.org/newscodes/subjectcode/>;
	skos:exactMatch medtop:20000989;
	skos:broader	subj:15000000;
	skos:narrower	subj:15038001;
	skos:narrower	subj:15038002;
	skos:narrower	subj:15038003;
	skos:narrower	subj:15038004;
	skos:narrower	subj:15038005.

subj:15038001
	rdf:type skos:Concept;
	skos:prefLabel	"running"@en-GB;
	skos:definition	"Pentathlon event "@en-GB;
	skos:inScheme <http://cv.iptc.org/newscodes/subjectcode/>;
	skos:broadMatch medtop:20000989;
	skos:broader	subj:15038000.

subj:15038002
	rdf:type skos:Concept;
	skos:prefLabel	"shooting"@en-GB;
	skos:definition	"Pentathlon event "@en-GB;
	skos:inScheme <http://cv.iptc.org/newscodes/subjectcode/>;
	skos:broadMatch medtop:20000989;
	skos:broader	subj:15038000.

subj:15038003
	rdf:type skos:Concept;
	skos:prefLabel	"swimming"@en-GB;
	skos:definition	"Pentathlon event "@en-GB;
	skos:inScheme <http://cv.iptc.org/newscodes/subjectcode/>;
	skos:broadMatch medtop:20000989;
	skos:broader	subj:15038000.

subj:15038004
	rdf:type skos:Concept;
	skos:prefLabel	"fencing"@en-GB;
	skos:definition	"Pentathlon event "@en-GB;
	skos:inScheme <http://cv.iptc.org/newscodes/subjectcode/>;
	skos:broadMatch medtop:20000989;
	skos:broader	subj:15038000.

subj:15038005
	rdf:type skos:Concept;
	skos:prefLabel	"showjumping"@en-GB;
	skos:definition	"Pentathlon event "@en-GB;
	skos:inScheme <http://cv.iptc.org/newscodes/subjectcode/>;
	skos:broadMatch medtop:20000989;
	skos:broader	subj:15038000.

subj:15039000
	rdf:type skos:Concept;
	skos:prefLabel	"motor racing"@en-GB;
	skos:definition	"Motor racing where speed and trusty mechanics are key "@en-GB;
	skos:inScheme <http://cv.iptc.org/newscodes/subjectcode/>;
	skos:exactMatch medtop:20000991;
	skos:broader	subj:15000000;
	skos:narrower	subj:15039001;
	skos:narrower	subj:15039002;
	skos:narrower	subj:15039003;
	skos:narrower	subj:15039004;
	skos:narrower	subj:15039005;
	skos:narrower	subj:15039006;
	skos:narrower	subj:15039007;
	skos:narrower	subj:15039008.

subj:15039001
	rdf:type skos:Concept;
	skos:prefLabel	"Formula One"@en-GB;
	skos:definition	"Single cockpit car racing where 20 or so competitors race head to head over varied circuits around the world to win Grand Prix points in an individual and constructors championship "@en-GB;
	skos:inScheme <http://cv.iptc.org/newscodes/subjectcode/>;
	skos:exactMatch medtop:20000994;
	skos:broader	subj:15039000.

subj:15039002
	rdf:type skos:Concept;
	skos:prefLabel	"F3000"@en-GB;
	skos:definition	"Using less powerful motors than the Formula One, designated construction teams race over varied circuits the world over in speed races for individual and team honours over a season. "@en-GB;
	skos:inScheme <http://cv.iptc.org/newscodes/subjectcode/>;
	skos:exactMatch medtop:20000993;
	skos:broader	subj:15039000.

subj:15039003
	rdf:type skos:Concept;
	skos:prefLabel	"endurance"@en-GB;
	skos:definition	"Endurance races for a driver and co-pilot using specially built cars. "@en-GB;
	skos:inScheme <http://cv.iptc.org/newscodes/subjectcode/>;
	skos:exactMatch medtop:20000992;
	skos:broader	subj:15039000.

subj:15039004
	rdf:type skos:Concept;
	skos:prefLabel	"Indy"@en-GB;
	skos:definition	"North American top range professional league speed racing over circuits. "@en-GB;
	skos:inScheme <http://cv.iptc.org/newscodes/subjectcode/>;
	skos:exactMatch medtop:20000995;
	skos:broader	subj:15039000.

subj:15039005
	rdf:type skos:Concept;
	skos:prefLabel	"CART"@en-GB;
	skos:definition	"North American professional league speed racing. "@en-GB;
	skos:inScheme <http://cv.iptc.org/newscodes/subjectcode/>;
	skos:broadMatch medtop:20000991;
	skos:broader	subj:15039000.

subj:15039006
	rdf:type skos:Concept;
	skos:prefLabel	"NHRA"@en-GB;
	skos:definition	"North American professional league speed racing. "@en-GB;
	skos:inScheme <http://cv.iptc.org/newscodes/subjectcode/>;
	skos:broadMatch medtop:20000991;
	skos:broader	subj:15039000.

subj:15039007
	rdf:type skos:Concept;
	skos:prefLabel	"NASCAR"@en-GB;
	skos:definition	"North American professional league speed racing. "@en-GB;
	skos:inScheme <http://cv.iptc.org/newscodes/subjectcode/>;
	skos:broadMatch medtop:20000991;
	skos:broader	subj:15039000.

subj:15039008
	rdf:type skos:Concept;
	skos:prefLabel	"TRUCKI"@en-GB;
	skos:definition	"North American professional league speed racing. "@en-GB;
	skos:inScheme <http://cv.iptc.org/newscodes/subjectcode/>;
	skos:broadMatch medtop:20000991;
	skos:broader	subj:15039000.

subj:15040000
	rdf:type skos:Concept;
	skos:prefLabel	"motor rallying"@en-GB;
	skos:definition	"A season of endurance races over closed circuits including dirt tracks, roads and even snowy conditions featuring specials using adapted road cars with a driver and co-pilot. "@en-GB;
	skos:inScheme <http://cv.iptc.org/newscodes/subjectcode/>;
	skos:exactMatch medtop:20000997;
	skos:broader	subj:15000000;
	skos:narrower	subj:15040001;
	skos:narrower	subj:15040002;
	skos:narrower	subj:15040003.

subj:15040001
	rdf:type skos:Concept;
	skos:prefLabel	"rallying"@en-GB;
	skos:definition	"Stage races "@en-GB;
	skos:inScheme <http://cv.iptc.org/newscodes/subjectcode/>;
	skos:broadMatch medtop:20000997;
	skos:broader	subj:15040000.

subj:15040002
	rdf:type skos:Concept;
	skos:prefLabel	"pursuit"@en-GB;
	skos:definition	"Cross-country race with mass start, first half of the distance in classic and the other half in free style. "@en-GB;
	skos:historyNote	"changed name and added explanation in V15 "@en-GB;
	skos:inScheme <http://cv.iptc.org/newscodes/subjectcode/>;
	skos:broadMatch medtop:20000997;
	skos:broader	subj:15040000.

subj:15040003
	rdf:type skos:Concept;
	skos:prefLabel	"rallycross"@en-GB;
	skos:definition	"Stage races over dirt tracks "@en-GB;
	skos:inScheme <http://cv.iptc.org/newscodes/subjectcode/>;
	skos:exactMatch medtop:20000996;
	skos:broader	subj:15040000.

subj:15041000
	rdf:type skos:Concept;
	skos:prefLabel	"motorcycling"@en-GB;
	skos:definition	"Races with 2, 3 or 4 wheels vehicles with a saddle and handlebars "@en-GB;
	skos:inScheme <http://cv.iptc.org/newscodes/subjectcode/>;
	skos:exactMatch medtop:20000998;
	skos:broader	subj:15000000;
	skos:narrower	subj:15041001;
	skos:narrower	subj:15041002;
	skos:narrower	subj:15041003;
	skos:narrower	subj:15041004;
	skos:narrower	subj:15041005;
	skos:narrower	subj:15041006;
	skos:narrower	subj:15041007;
	skos:narrower	subj:15041008;
	skos:narrower	subj:15041009;
	skos:narrower	subj:15041010;
	skos:narrower	subj:15041011;
	skos:narrower	subj:15041012;
	skos:narrower	subj:15041013;
	skos:narrower	subj:15041014.

subj:15041001
	rdf:type skos:Concept;
	skos:prefLabel	"speed-Grand-Prix"@en-GB;
	skos:definition	"A fast and furious race where every second counts "@en-GB;
	skos:inScheme <http://cv.iptc.org/newscodes/subjectcode/>;
	skos:broadMatch medtop:20000998;
	skos:broader	subj:15041000.

subj:15041002
	rdf:type skos:Concept;
	skos:prefLabel	"enduro"@en-GB;
	skos:definition	"A race of speed, endurance and regularity over varied surfaces such as through forests and on dirt tracks "@en-GB;
	skos:inScheme <http://cv.iptc.org/newscodes/subjectcode/>;
	skos:exactMatch medtop:20001000;
	skos:broader	subj:15041000.

subj:15041003
	rdf:type skos:Concept;
	skos:prefLabel	"grass-track"@en-GB;
	skos:definition	"A race competed on turf "@en-GB;
	skos:inScheme <http://cv.iptc.org/newscodes/subjectcode/>;
	skos:exactMatch medtop:20001001;
	skos:broader	subj:15041000.

subj:15041004
	rdf:type skos:Concept;
	skos:prefLabel	"moto-ball"@en-GB;
	skos:definition	"Team sport where drivers play a ball "@en-GB;
	skos:inScheme <http://cv.iptc.org/newscodes/subjectcode/>;
	skos:exactMatch medtop:20001002;
	skos:broader	subj:15041000.

subj:15041005
	rdf:type skos:Concept;
	skos:prefLabel	"moto-cross"@en-GB;
	skos:definition	"Raced over dirt tracks featuring severe mounds "@en-GB;
	skos:inScheme <http://cv.iptc.org/newscodes/subjectcode/>;
	skos:exactMatch medtop:20001003;
	skos:broader	subj:15041000.

subj:15041006
	rdf:type skos:Concept;
	skos:prefLabel	"rallying"@en-GB;
	skos:definition	"Races run over regular roads "@en-GB;
	skos:inScheme <http://cv.iptc.org/newscodes/subjectcode/>;
	skos:exactMatch medtop:20001005;
	skos:broader	subj:15041000.

subj:15041007
	rdf:type skos:Concept;
	skos:prefLabel	"trial"@en-GB;
	skos:definition	"A race of consistency and endurance over varied terrain "@en-GB;
	skos:inScheme <http://cv.iptc.org/newscodes/subjectcode/>;
	skos:exactMatch medtop:20001008;
	skos:broader	subj:15041000.

subj:15041008
	rdf:type skos:Concept;
	skos:prefLabel	"endurance"@en-GB;
	skos:definition	"A road race of consistency and endurance "@en-GB;
	skos:inScheme <http://cv.iptc.org/newscodes/subjectcode/>;
	skos:exactMatch medtop:20000999;
	skos:broader	subj:15041000.

subj:15041009
	rdf:type skos:Concept;
	skos:prefLabel	"superbike"@en-GB;
	skos:definition	"Engine size "@en-GB;
	skos:inScheme <http://cv.iptc.org/newscodes/subjectcode/>;
	skos:broadMatch medtop:20000998;
	skos:broader	subj:15041000.

subj:15041010
	rdf:type skos:Concept;
	skos:prefLabel	"125 cm3"@en-GB;
	skos:definition	"Engine size "@en-GB;
	skos:inScheme <http://cv.iptc.org/newscodes/subjectcode/>;
	skos:broadMatch medtop:20000998;
	skos:broader	subj:15041000.

subj:15041011
	rdf:type skos:Concept;
	skos:prefLabel	"250 cm3"@en-GB;
	skos:definition	"Engine size "@en-GB;
	skos:inScheme <http://cv.iptc.org/newscodes/subjectcode/>;
	skos:broadMatch medtop:20000998;
	skos:broader	subj:15041000.

subj:15041012
	rdf:type skos:Concept;
	skos:prefLabel	"500 cm3"@en-GB;
	skos:definition	"Engine size "@en-GB;
	skos:inScheme <http://cv.iptc.org/newscodes/subjectcode/>;
	skos:broadMatch medtop:20000998;
	skos:broader	subj:15041000.

subj:15041013
	rdf:type skos:Concept;
	skos:prefLabel	"side-cars"@en-GB;
	skos:definition	"Of different engine sizes but attached to a side car featuring a passenger "@en-GB;
	skos:inScheme <http://cv.iptc.org/newscodes/subjectcode/>;
	skos:exactMatch medtop:20001006;
	skos:broader	subj:15041000.

subj:15041014
	rdf:type skos:Concept;
	skos:prefLabel	"motoGP"@en-GB;
	skos:definition	"Capacity class 1000ccm "@en-GB;
	skos:inScheme <http://cv.iptc.org/newscodes/subjectcode/>;
	skos:exactMatch medtop:20001004;
	skos:broader	subj:15041000.

subj:15042000
	rdf:type skos:Concept;
	skos:prefLabel	"netball"@en-GB;
	skos:definition	"A woman's sport similar to basketball without a board behind the basket "@en-GB;
	skos:historyNote	"typo fixed in Explanation "@en-GB;
	skos:inScheme <http://cv.iptc.org/newscodes/subjectcode/>;
	skos:exactMatch medtop:20001010;
	skos:broader	subj:15000000.

subj:15043000
	rdf:type skos:Concept;
	skos:prefLabel	"nordic skiing"@en-GB;
	skos:definition	"Practiced in snowy countryside and based on power and endurance. There are classic and free style events with mass or staggered starts. "@en-GB;
	skos:inScheme <http://cv.iptc.org/newscodes/subjectcode/>;
	skos:exactMatch medtop:20001060;
	skos:broader	subj:15000000;
	skos:narrower	subj:15043001;
	skos:narrower	subj:15043002;
	skos:narrower	subj:15043003;
	skos:narrower	subj:15043004;
	skos:narrower	subj:15043005;
	skos:narrower	subj:15043006;
	skos:narrower	subj:15043007;
	skos:narrower	subj:15043008;
	skos:narrower	subj:15043009;
	skos:narrower	subj:15043010;
	skos:narrower	subj:15043011;
	skos:narrower	subj:15043012;
	skos:narrower	subj:15043013;
	skos:narrower	subj:15043014;
	skos:narrower	subj:15043015;
	skos:narrower	subj:15043016;
	skos:narrower	subj:15043017.

subj:15043001
	rdf:type skos:Concept;
	skos:prefLabel	"cross-country"@en-GB;
	skos:definition	"Nordic ski race "@en-GB;
	skos:inScheme <http://cv.iptc.org/newscodes/subjectcode/>;
	skos:exactMatch medtop:20001149;
	skos:broader	subj:15043000.

subj:15043002
	rdf:type skos:Concept;
	skos:prefLabel	"5 km classical time"@en-GB;
	skos:definition	"A 5km classic race in that the competitor keeps his skis parallel except on steep inclines where the scissor move is used "@en-GB;
	skos:inScheme <http://cv.iptc.org/newscodes/subjectcode/>;
	skos:broadMatch medtop:20001060;
	skos:broader	subj:15043000.

subj:15043003
	rdf:type skos:Concept;
	skos:prefLabel	"10 km classical style"@en-GB;
	skos:definition	"A 10km classic race in that the competitor keeps his skis parallel except on steep inclines where the scissor move is used "@en-GB;
	skos:inScheme <http://cv.iptc.org/newscodes/subjectcode/>;
	skos:broadMatch medtop:20001060;
	skos:broader	subj:15043000.

subj:15043004
	rdf:type skos:Concept;
	skos:prefLabel	"10 km pursuit free style"@en-GB;
	skos:definition	"Staggered start depending on positions with competitors using a skating like technique on skis "@en-GB;
	skos:inScheme <http://cv.iptc.org/newscodes/subjectcode/>;
	skos:broadMatch medtop:20001060;
	skos:broader	subj:15043000.

subj:15043005
	rdf:type skos:Concept;
	skos:prefLabel	"15 km classical style"@en-GB;
	skos:definition	"A 15km race using the classical style of keeping skies parallel "@en-GB;
	skos:inScheme <http://cv.iptc.org/newscodes/subjectcode/>;
	skos:broadMatch medtop:20001060;
	skos:broader	subj:15043000.

subj:15043006
	rdf:type skos:Concept;
	skos:prefLabel	"15 km pursuit free style"@en-GB;
	skos:definition	"15km race with staggered start using free style technique similar to a skating motion "@en-GB;
	skos:inScheme <http://cv.iptc.org/newscodes/subjectcode/>;
	skos:broadMatch medtop:20001060;
	skos:broader	subj:15043000.

subj:15043007
	rdf:type skos:Concept;
	skos:prefLabel	"10 km + 15 km combined"@en-GB;
	skos:definition	"10km classic followed by 15km free-style race "@en-GB;
	skos:inScheme <http://cv.iptc.org/newscodes/subjectcode/>;
	skos:broadMatch medtop:20001060;
	skos:broader	subj:15043000.

subj:15043008
	rdf:type skos:Concept;
	skos:prefLabel	"30 km classical style"@en-GB;
	skos:definition	"A 30km classic race in that the competitor keeps his skis parallel except on steep inclines where the scissor move is used "@en-GB;
	skos:inScheme <http://cv.iptc.org/newscodes/subjectcode/>;
	skos:broadMatch medtop:20001060;
	skos:broader	subj:15043000.

subj:15043009
	rdf:type skos:Concept;
	skos:prefLabel	"30km free style"@en-GB;
	skos:definition	"A 30km free-style race where the most common style is the skate style where competitors slide and the skis do not need to be parallel "@en-GB;
	skos:inScheme <http://cv.iptc.org/newscodes/subjectcode/>;
	skos:broadMatch medtop:20001060;
	skos:broader	subj:15043000.

subj:15043010
	rdf:type skos:Concept;
	skos:prefLabel	"50 km free style"@en-GB;
	skos:definition	"A 50km free style race where the most common style is the skate style where competitors slide and the skis do not need to be parallel "@en-GB;
	skos:inScheme <http://cv.iptc.org/newscodes/subjectcode/>;
	skos:broadMatch medtop:20001060;
	skos:broader	subj:15043000.

subj:15043011
	rdf:type skos:Concept;
	skos:prefLabel	"4x5 km relay"@en-GB;
	skos:definition	"Teams of four competitors ski 5km each in relay fashion "@en-GB;
	skos:inScheme <http://cv.iptc.org/newscodes/subjectcode/>;
	skos:broadMatch medtop:20001060;
	skos:broader	subj:15043000.

subj:15043012
	rdf:type skos:Concept;
	skos:prefLabel	"4x10 km relay"@en-GB;
	skos:definition	"Teams of four competitors ski 10km each in relay fashion "@en-GB;
	skos:historyNote	"typo fixed in Explanation "@en-GB;
	skos:inScheme <http://cv.iptc.org/newscodes/subjectcode/>;
	skos:broadMatch medtop:20001060;
	skos:broader	subj:15043000.

subj:15043013
	rdf:type skos:Concept;
	skos:prefLabel	"nordic combined"@en-GB;
	skos:definition	"A two day competition combining the ski jump and a cross-country race. "@en-GB;
	skos:historyNote	"typo fixed in Explanation "@en-GB;
	skos:inScheme <http://cv.iptc.org/newscodes/subjectcode/>;
	skos:exactMatch medtop:20001150;
	skos:broader	subj:15043000.

subj:15043014
	rdf:type skos:Concept;
	skos:prefLabel	"raid"@en-GB;
	skos:definition	"NA "@en-GB;
	skos:inScheme <http://cv.iptc.org/newscodes/subjectcode/>;
	skos:broadMatch medtop:20001060;
	skos:broader	subj:15043000.

subj:15043015
	rdf:type skos:Concept;
	skos:prefLabel	"5 km pursuit free style"@en-GB;
	skos:definition	"Cross-country skiing over a 5km course in a pursuit format "@en-GB;
	skos:inScheme <http://cv.iptc.org/newscodes/subjectcode/>;
	skos:broadMatch medtop:20001060;
	skos:broader	subj:15043000.

subj:15043016
	rdf:type skos:Concept;
	skos:prefLabel	"1.5 km sprint free"@en-GB;
	skos:definition	"Cross-country skiing over a 1.5km course in a sprint format "@en-GB;
	skos:inScheme <http://cv.iptc.org/newscodes/subjectcode/>;
	skos:broadMatch medtop:20001060;
	skos:broader	subj:15043000.

subj:15043017
	rdf:type skos:Concept;
	skos:prefLabel	"50 km classic style"@en-GB;
	skos:definition	"Cross-country skiing over a 50km course in a classic style format "@en-GB;
	skos:inScheme <http://cv.iptc.org/newscodes/subjectcode/>;
	skos:broadMatch medtop:20001060;
	skos:broader	subj:15043000.

subj:15044000
	rdf:type skos:Concept;
	skos:prefLabel	"orienteering"@en-GB;
	skos:definition	"An individual time-trial over a route marked out by beacons. The competitor has to search out and find in a specific order. The contestant makes his way with the help of a compass and map "@en-GB;
	skos:inScheme <http://cv.iptc.org/newscodes/subjectcode/>;
	skos:exactMatch medtop:20001011;
	skos:broader	subj:15000000;
	skos:narrower	subj:15044001.

subj:15044001
	rdf:type skos:Concept;
	skos:prefLabel	"ski orienteering"@en-GB;
	skos:definition	"An individual ski time-trial over a route marked out by beacons, that the competitor has to search out and find in a specific order. The contestant makes his way with the help of a compass and map "@en-GB;
	skos:inScheme <http://cv.iptc.org/newscodes/subjectcode/>;
	skos:exactMatch medtop:20001012;
	skos:broader	subj:15044000.

subj:15045000
	rdf:type skos:Concept;
	skos:prefLabel	"polo"@en-GB;
	skos:definition	"With the aid of a mallet two teams of four horsemen try and knock a bamboo ball into the opponents goal over a pitch 250m long and 150m wide. The game is divided into 4, 6, or 8 time periods of 7min 30sec called chukkas. "@en-GB;
	skos:inScheme <http://cv.iptc.org/newscodes/subjectcode/>;
	skos:exactMatch medtop:20001014;
	skos:broader	subj:15000000.

subj:15046000
	rdf:type skos:Concept;
	skos:prefLabel	"power boating"@en-GB;
	skos:definition	"Races between motor boats on rivers or lakes "@en-GB;
	skos:inScheme <http://cv.iptc.org/newscodes/subjectcode/>;
	skos:exactMatch medtop:20001016;
	skos:broader	subj:15000000;
	skos:narrower	subj:15046001;
	skos:narrower	subj:15046002.

subj:15046001
	rdf:type skos:Concept;
	skos:prefLabel	"F1"@en-GB;
	skos:definition	"Sprint race "@en-GB;
	skos:inScheme <http://cv.iptc.org/newscodes/subjectcode/>;
	skos:broadMatch medtop:20001016;
	skos:broader	subj:15046000.

subj:15046002
	rdf:type skos:Concept;
	skos:prefLabel	"F2"@en-GB;
	skos:definition	"Long distance race "@en-GB;
	skos:inScheme <http://cv.iptc.org/newscodes/subjectcode/>;
	skos:broadMatch medtop:20001016;
	skos:broader	subj:15046000.

subj:15047000
	rdf:type skos:Concept;
	skos:prefLabel	"rowing"@en-GB;
	skos:definition	"Boat racing usually on flat calm waters with boats for 1, 2, 4 or 8 rowers "@en-GB;
	skos:inScheme <http://cv.iptc.org/newscodes/subjectcode/>;
	skos:exactMatch medtop:20001026;
	skos:broader	subj:15000000;
	skos:narrower	subj:15047001;
	skos:narrower	subj:15047002;
	skos:narrower	subj:15047003;
	skos:narrower	subj:15047004;
	skos:narrower	subj:15047005;
	skos:narrower	subj:15047006;
	skos:narrower	subj:15047007.

subj:15047001
	rdf:type skos:Concept;
	skos:prefLabel	"single sculls"@en-GB;
	skos:definition	"Single person boats with two oars "@en-GB;
	skos:inScheme <http://cv.iptc.org/newscodes/subjectcode/>;
	skos:broadMatch medtop:20001026;
	skos:broader	subj:15047000.

subj:15047002
	rdf:type skos:Concept;
	skos:prefLabel	"double sculls"@en-GB;
	skos:definition	"Two person boats with two oars each "@en-GB;
	skos:inScheme <http://cv.iptc.org/newscodes/subjectcode/>;
	skos:broadMatch medtop:20001026;
	skos:broader	subj:15047000.

subj:15047003
	rdf:type skos:Concept;
	skos:prefLabel	"quadruple sculls"@en-GB;
	skos:definition	"Four person boats with two oars each and without a team mate to give directions "@en-GB;
	skos:inScheme <http://cv.iptc.org/newscodes/subjectcode/>;
	skos:broadMatch medtop:20001026;
	skos:broader	subj:15047000.

subj:15047004
	rdf:type skos:Concept;
	skos:prefLabel	"coxless pair"@en-GB;
	skos:definition	"Two person boats with just one oar each and without a team mate to give directions "@en-GB;
	skos:inScheme <http://cv.iptc.org/newscodes/subjectcode/>;
	skos:broadMatch medtop:20001026;
	skos:broader	subj:15047000.

subj:15047005
	rdf:type skos:Concept;
	skos:prefLabel	"coxless four"@en-GB;
	skos:definition	"Four person boats with just one oar each and without a team mate to give directions "@en-GB;
	skos:inScheme <http://cv.iptc.org/newscodes/subjectcode/>;
	skos:broadMatch medtop:20001026;
	skos:broader	subj:15047000.

subj:15047006
	rdf:type skos:Concept;
	skos:prefLabel	"eight"@en-GB;
	skos:definition	"Eight person boats with just one oar each and without a team mate to give directions "@en-GB;
	skos:inScheme <http://cv.iptc.org/newscodes/subjectcode/>;
	skos:broadMatch medtop:20001026;
	skos:broader	subj:15047000.

subj:15047007
	rdf:type skos:Concept;
	skos:prefLabel	"lightweight"@en-GB;
	skos:definition	"Where a weight category is imposed on competitors "@en-GB;
	skos:inScheme <http://cv.iptc.org/newscodes/subjectcode/>;
	skos:broadMatch medtop:20001026;
	skos:broader	subj:15047000.

subj:15048000
	rdf:type skos:Concept;
	skos:prefLabel	"rugby league"@en-GB;
	skos:definition	"Two teams of 13 compete on a pitch where they score tries and penalties by running with and passing an oval ball to be touched down behind the goal line or kicked between goal posts in a tough physical contest "@en-GB;
	skos:inScheme <http://cv.iptc.org/newscodes/subjectcode/>;
	skos:exactMatch medtop:20001035;
	skos:broader	subj:15000000.

subj:15049000
	rdf:type skos:Concept;
	skos:prefLabel	"rugby union"@en-GB;
	skos:definition	"Two teams of 15 compete on a pitch where they score tries and penalties by running with and passing an oval ball to be touched down behind the goal line or kicked between goal posts in a tough physical contest "@en-GB;
	skos:inScheme <http://cv.iptc.org/newscodes/subjectcode/>;
	skos:exactMatch medtop:20001036;
	skos:broader	subj:15000000;
	skos:narrower	subj:15049001.

subj:15049001
	rdf:type skos:Concept;
	skos:prefLabel	"rugby 7"@en-GB;
	skos:definition	"A more fun and exciting variety where two teams of 7 compete on a pitch where they score tries and penalties by running with and passing an oval ball to be touched down behind the goal line or kicked between goal posts in a tough physical contest "@en-GB;
	skos:inScheme <http://cv.iptc.org/newscodes/subjectcode/>;
	skos:exactMatch medtop:20001037;
	skos:broader	subj:15049000.

subj:15050000
	rdf:type skos:Concept;
	skos:prefLabel	"sailing"@en-GB;
	skos:definition	"Sail boat racing over a route marked by buoys. "@en-GB;
	skos:historyNote	"typo fixed in Explanation "@en-GB;
	skos:inScheme <http://cv.iptc.org/newscodes/subjectcode/>;
	skos:exactMatch medtop:20001038;
	skos:broader	subj:15000000;
	skos:narrower	subj:15050001;
	skos:narrower	subj:15050002;
	skos:narrower	subj:15050003;
	skos:narrower	subj:15050004;
	skos:narrower	subj:15050005;
	skos:narrower	subj:15050006;
	skos:narrower	subj:15050007;
	skos:narrower	subj:15050008;
	skos:narrower	subj:15050009;
	skos:narrower	subj:15050010;
	skos:narrower	subj:15050011;
	skos:narrower	subj:15050012;
	skos:narrower	subj:15050013;
	skos:narrower	subj:15050014;
	skos:narrower	subj:15050015;
	skos:narrower	subj:15050016.

subj:15050001
	rdf:type skos:Concept;
	skos:prefLabel	"Tornado"@en-GB;
	skos:definition	"Boat Category: two man catamaran (21m/sq mainsail) Olympic sport "@en-GB;
	skos:inScheme <http://cv.iptc.org/newscodes/subjectcode/>;
	skos:broadMatch medtop:20001039;
	skos:broader	subj:15050000.

subj:15050002
	rdf:type skos:Concept;
	skos:prefLabel	"soling"@en-GB;
	skos:definition	"Boat Category: three man keel boat "@en-GB;
	skos:inScheme <http://cv.iptc.org/newscodes/subjectcode/>;
	skos:broadMatch medtop:20001041;
	skos:broader	subj:15050000.

subj:15050003
	rdf:type skos:Concept;
	skos:prefLabel	"49er"@en-GB;
	skos:definition	"Boat Category: two man dinghy (8.23m/sq mainsail) Olympic sport "@en-GB;
	skos:inScheme <http://cv.iptc.org/newscodes/subjectcode/>;
	skos:broadMatch medtop:20001040;
	skos:broader	subj:15050000.

subj:15050004
	rdf:type skos:Concept;
	skos:prefLabel	"Europe"@en-GB;
	skos:definition	"Boat Category: one man dinghy (4.57m/sq mainsail) Olympic sport "@en-GB;
	skos:inScheme <http://cv.iptc.org/newscodes/subjectcode/>;
	skos:broadMatch medtop:20001040;
	skos:broader	subj:15050000.

subj:15050005
	rdf:type skos:Concept;
	skos:prefLabel	"Laser"@en-GB;
	skos:definition	"Boat Category: one man dinghy (4.6m/sq mainsail) Olympic sport "@en-GB;
	skos:inScheme <http://cv.iptc.org/newscodes/subjectcode/>;
	skos:broadMatch medtop:20001040;
	skos:broader	subj:15050000.

subj:15050006
	rdf:type skos:Concept;
	skos:prefLabel	"470"@en-GB;
	skos:definition	"Boat Category: two man dinghy (7.10m/sq mainsail) Olympic sport "@en-GB;
	skos:inScheme <http://cv.iptc.org/newscodes/subjectcode/>;
	skos:broadMatch medtop:20001040;
	skos:broader	subj:15050000.

subj:15050007
	rdf:type skos:Concept;
	skos:prefLabel	"Finn"@en-GB;
	skos:definition	"Boat Category: one man dinghy (10m/sq mainsail) Olympic sport "@en-GB;
	skos:inScheme <http://cv.iptc.org/newscodes/subjectcode/>;
	skos:broadMatch medtop:20001040;
	skos:broader	subj:15050000.

subj:15050008
	rdf:type skos:Concept;
	skos:prefLabel	"Star"@en-GB;
	skos:definition	"Boat Category: two man keel boat (7.10m/sq mainsail) Olympic sport "@en-GB;
	skos:inScheme <http://cv.iptc.org/newscodes/subjectcode/>;
	skos:broadMatch medtop:20001041;
	skos:broader	subj:15050000.

subj:15050009
	rdf:type skos:Concept;
	skos:prefLabel	"flying dutchmann"@en-GB;
	skos:definition	"Boat Category: two man dinghy "@en-GB;
	skos:inScheme <http://cv.iptc.org/newscodes/subjectcode/>;
	skos:broadMatch medtop:20001040;
	skos:broader	subj:15050000.

subj:15050010
	rdf:type skos:Concept;
	skos:prefLabel	"505"@en-GB;
	skos:definition	"Boat Category: two man dinghy "@en-GB;
	skos:inScheme <http://cv.iptc.org/newscodes/subjectcode/>;
	skos:broadMatch medtop:20001040;
	skos:broader	subj:15050000.

subj:15050011
	rdf:type skos:Concept;
	skos:prefLabel	"staging race"@en-GB;
	skos:definition	"Sea racing "@en-GB;
	skos:inScheme <http://cv.iptc.org/newscodes/subjectcode/>;
	skos:broadMatch medtop:20001038;
	skos:broader	subj:15050000.

subj:15050012
	rdf:type skos:Concept;
	skos:prefLabel	"around the world"@en-GB;
	skos:definition	"Open seas racing "@en-GB;
	skos:inScheme <http://cv.iptc.org/newscodes/subjectcode/>;
	skos:exactMatch medtop:20001044;
	skos:broader	subj:15050000.

subj:15050013
	rdf:type skos:Concept;
	skos:prefLabel	"monohull"@en-GB;
	skos:definition	"Single hull craft "@en-GB;
	skos:inScheme <http://cv.iptc.org/newscodes/subjectcode/>;
	skos:broadMatch medtop:20001038;
	skos:broader	subj:15050000.

subj:15050014
	rdf:type skos:Concept;
	skos:prefLabel	"multihulls"@en-GB;
	skos:definition	"Multi hull craft "@en-GB;
	skos:inScheme <http://cv.iptc.org/newscodes/subjectcode/>;
	skos:exactMatch medtop:20001039;
	skos:broader	subj:15050000.

subj:15050015
	rdf:type skos:Concept;
	skos:prefLabel	"yngling"@en-GB;
	skos:definition	"Olympic boat-class. A race around different courses in a boat of 6.35 metres (20ft 10in) long and 1.73 metres (5ft 8in) wide, crewed in Olympic competition only by women. The number of races and the length of the courses varies. "@en-GB;
	skos:inScheme <http://cv.iptc.org/newscodes/subjectcode/>;
	skos:broadMatch medtop:20001038;
	skos:broader	subj:15050000.

subj:15050016
	rdf:type skos:Concept;
	skos:prefLabel	"mistral"@en-GB;
	skos:definition	"Olympic boat class. A staged race using boats of the mistral type, which are 4.24 metres (13ft 11in) long and 1.3 metres (4ft 3in) wide. The number of races and the length of the courses varies. "@en-GB;
	skos:inScheme <http://cv.iptc.org/newscodes/subjectcode/>;
	skos:broadMatch medtop:20001038;
	skos:broader	subj:15050000.

subj:15051000
	rdf:type skos:Concept;
	skos:prefLabel	"shooting"@en-GB;
	skos:definition	"Precision sport using a hand gun, rifle or shotgun "@en-GB;
	skos:inScheme <http://cv.iptc.org/newscodes/subjectcode/>;
	skos:exactMatch medtop:20001049;
	skos:broader	subj:15000000;
	skos:narrower	subj:15051001;
	skos:narrower	subj:15051002;
	skos:narrower	subj:15051003;
	skos:narrower	subj:15051004;
	skos:narrower	subj:15051005;
	skos:narrower	subj:15051006;
	skos:narrower	subj:15051007;
	skos:narrower	subj:15051008;
	skos:narrower	subj:15051009;
	skos:narrower	subj:15051010;
	skos:narrower	subj:15051011;
	skos:narrower	subj:15051012.

subj:15051001
	rdf:type skos:Concept;
	skos:prefLabel	"10 m air rifle"@en-GB;
	skos:definition	"Shooting event "@en-GB;
	skos:inScheme <http://cv.iptc.org/newscodes/subjectcode/>;
	skos:broadMatch medtop:20001051;
	skos:broader	subj:15051000.

subj:15051002
	rdf:type skos:Concept;
	skos:prefLabel	"10 m air pistol"@en-GB;
	skos:definition	"Shooting event "@en-GB;
	skos:inScheme <http://cv.iptc.org/newscodes/subjectcode/>;
	skos:broadMatch medtop:20001050;
	skos:broader	subj:15051000.

subj:15051003
	rdf:type skos:Concept;
	skos:prefLabel	"10 m running target"@en-GB;
	skos:definition	"Shooting event "@en-GB;
	skos:inScheme <http://cv.iptc.org/newscodes/subjectcode/>;
	skos:broadMatch medtop:20001052;
	skos:broader	subj:15051000.

subj:15051004
	rdf:type skos:Concept;
	skos:prefLabel	"25 m rapid fire pistol"@en-GB;
	skos:definition	"Shooting event "@en-GB;
	skos:inScheme <http://cv.iptc.org/newscodes/subjectcode/>;
	skos:broadMatch medtop:20001050;
	skos:broader	subj:15051000.

subj:15051005
	rdf:type skos:Concept;
	skos:prefLabel	"25 m sport pistol"@en-GB;
	skos:definition	"Shooting event "@en-GB;
	skos:inScheme <http://cv.iptc.org/newscodes/subjectcode/>;
	skos:broadMatch medtop:20001050;
	skos:broader	subj:15051000.

subj:15051006
	rdf:type skos:Concept;
	skos:prefLabel	"50 m free pistol"@en-GB;
	skos:definition	"Shooting event "@en-GB;
	skos:inScheme <http://cv.iptc.org/newscodes/subjectcode/>;
	skos:broadMatch medtop:20001050;
	skos:broader	subj:15051000.

subj:15051007
	rdf:type skos:Concept;
	skos:prefLabel	"50 m free rifle prone"@en-GB;
	skos:definition	"Shooting event "@en-GB;
	skos:inScheme <http://cv.iptc.org/newscodes/subjectcode/>;
	skos:broadMatch medtop:20001051;
	skos:broader	subj:15051000.

subj:15051008
	rdf:type skos:Concept;
	skos:prefLabel	"50 m free rifle 3x40"@en-GB;
	skos:definition	"Shooting event "@en-GB;
	skos:inScheme <http://cv.iptc.org/newscodes/subjectcode/>;
	skos:broadMatch medtop:20001051;
	skos:broader	subj:15051000.

subj:15051009
	rdf:type skos:Concept;
	skos:prefLabel	"50 m sport rifle 3x20"@en-GB;
	skos:definition	"Shooting event "@en-GB;
	skos:inScheme <http://cv.iptc.org/newscodes/subjectcode/>;
	skos:broadMatch medtop:20001051;
	skos:broader	subj:15051000.

subj:15051010
	rdf:type skos:Concept;
	skos:prefLabel	"trap"@en-GB;
	skos:definition	"Shooting event with moving targets "@en-GB;
	skos:inScheme <http://cv.iptc.org/newscodes/subjectcode/>;
	skos:broadMatch medtop:20001054;
	skos:broader	subj:15051000.

subj:15051011
	rdf:type skos:Concept;
	skos:prefLabel	"double trap"@en-GB;
	skos:definition	"Shooting event with two moving targets launched at the same time "@en-GB;
	skos:inScheme <http://cv.iptc.org/newscodes/subjectcode/>;
	skos:broadMatch medtop:20001054;
	skos:broader	subj:15051000.

subj:15051012
	rdf:type skos:Concept;
	skos:prefLabel	"skeet"@en-GB;
	skos:definition	"Shooting event with moving targets, competitor shoots from a series of positions "@en-GB;
	skos:inScheme <http://cv.iptc.org/newscodes/subjectcode/>;
	skos:broadMatch medtop:20001054;
	skos:broader	subj:15051000.

subj:15052000
	rdf:type skos:Concept;
	skos:prefLabel	"ski jumping"@en-GB;
	skos:definition	"Competitors descend a snow covered elevated ramp on skis and try to fly off it as far as possible, receiving marks for distance, style of flight and landing "@en-GB;
	skos:historyNote	"typo fixed in Explanation "@en-GB;
	skos:inScheme <http://cv.iptc.org/newscodes/subjectcode/>;
	skos:exactMatch medtop:20001061;
	skos:broader	subj:15000000;
	skos:narrower	subj:15052001;
	skos:narrower	subj:15052002;
	skos:narrower	subj:15052003.

subj:15052001
	rdf:type skos:Concept;
	skos:prefLabel	"K90 jump"@en-GB;
	skos:definition	"Competitors jump from 70m and must clear 90m distance in their jump before scoring points for it "@en-GB;
	skos:historyNote	"typo fixed in Explanation "@en-GB;
	skos:inScheme <http://cv.iptc.org/newscodes/subjectcode/>;
	skos:broadMatch medtop:20001061;
	skos:broader	subj:15052000.

subj:15052002
	rdf:type skos:Concept;
	skos:prefLabel	"K120 jump"@en-GB;
	skos:definition	"Competitors jump from 90m and must clear 120m distance in their jump before scoring points for it "@en-GB;
	skos:inScheme <http://cv.iptc.org/newscodes/subjectcode/>;
	skos:broadMatch medtop:20001061;
	skos:broader	subj:15052000.

subj:15052003
	rdf:type skos:Concept;
	skos:prefLabel	"K180 (flying jump)"@en-GB;
	skos:definition	"Competitors jump from 180m and must clear 180m in their jump before scoring points for it "@en-GB;
	skos:inScheme <http://cv.iptc.org/newscodes/subjectcode/>;
	skos:broadMatch medtop:20001061;
	skos:broader	subj:15052000.

subj:15053000
	rdf:type skos:Concept;
	skos:prefLabel	"snow boarding"@en-GB;
	skos:definition	"Practiced with a single board (rather than two skis) "@en-GB;
	skos:inScheme <http://cv.iptc.org/newscodes/subjectcode/>;
	skos:exactMatch medtop:20001064;
	skos:broader	subj:15000000;
	skos:narrower	subj:15053001;
	skos:narrower	subj:15053002.

subj:15053001
	rdf:type skos:Concept;
	skos:prefLabel	"giant slalom"@en-GB;
	skos:definition	"Knock-out head-to-head downhill racing "@en-GB;
	skos:inScheme <http://cv.iptc.org/newscodes/subjectcode/>;
	skos:broadMatch medtop:20001064;
	skos:broader	subj:15053000.

subj:15053002
	rdf:type skos:Concept;
	skos:prefLabel	"half-pipe"@en-GB;
	skos:definition	"Over a semi-cylindrical tube of 100m competitors must perform a series of moves that are marked for style by 5 judges "@en-GB;
	skos:historyNote	"typo fixed in Explanation "@en-GB;
	skos:inScheme <http://cv.iptc.org/newscodes/subjectcode/>;
	skos:broadMatch medtop:20001064;
	skos:broader	subj:15053000.

subj:15054000
	rdf:type skos:Concept;
	skos:prefLabel	"soccer"@en-GB;
	skos:definition	"Two teams of eleven try to kick or head a ball into the opponents goal over a match usually of 90 minutes "@en-GB;
	skos:inScheme <http://cv.iptc.org/newscodes/subjectcode/>;
	skos:exactMatch medtop:20001065;
	skos:broader	subj:15000000.

subj:15055000
	rdf:type skos:Concept;
	skos:prefLabel	"softball"@en-GB;
	skos:definition	"Similar to baseball but with a larger and softer ball, a thinner bat, shorter gaps between bases and less innings "@en-GB;
	skos:historyNote	"typo fixed in Explanation "@en-GB;
	skos:inScheme <http://cv.iptc.org/newscodes/subjectcode/>;
	skos:exactMatch medtop:20001066;
	skos:broader	subj:15000000.

subj:15056000
	rdf:type skos:Concept;
	skos:prefLabel	"speed skating"@en-GB;
	skos:definition	"Timed races competed by two skaters at a time on an oval ice track "@en-GB;
	skos:inScheme <http://cv.iptc.org/newscodes/subjectcode/>;
	skos:exactMatch medtop:20001067;
	skos:broader	subj:15000000;
	skos:narrower	subj:15056001;
	skos:narrower	subj:15056002;
	skos:narrower	subj:15056003;
	skos:narrower	subj:15056004;
	skos:narrower	subj:15056005;
	skos:narrower	subj:15056006;
	skos:narrower	subj:15056007;
	skos:narrower	subj:15056008;
	skos:narrower	subj:15056009;
	skos:narrower	subj:15056010;
	skos:narrower	subj:15056011;
	skos:narrower	subj:15056012;
	skos:narrower	subj:15056013;
	skos:narrower	subj:15056014.

subj:15056001
	rdf:type skos:Concept;
	skos:prefLabel	"500 m"@en-GB;
	skos:definition	"Speed skating race over 500m "@en-GB;
	skos:inScheme <http://cv.iptc.org/newscodes/subjectcode/>;
	skos:broadMatch medtop:20001067;
	skos:broader	subj:15056000.

subj:15056002
	rdf:type skos:Concept;
	skos:prefLabel	"1000 m"@en-GB;
	skos:definition	"Speed skating race over 1000m "@en-GB;
	skos:inScheme <http://cv.iptc.org/newscodes/subjectcode/>;
	skos:broadMatch medtop:20001067;
	skos:broader	subj:15056000.

subj:15056003
	rdf:type skos:Concept;
	skos:prefLabel	"1500 m"@en-GB;
	skos:definition	"Speed skating race over 1500m "@en-GB;
	skos:inScheme <http://cv.iptc.org/newscodes/subjectcode/>;
	skos:broadMatch medtop:20001067;
	skos:broader	subj:15056000.

subj:15056004
	rdf:type skos:Concept;
	skos:prefLabel	"3000 m"@en-GB;
	skos:definition	"Speed skating race over 3000m "@en-GB;
	skos:inScheme <http://cv.iptc.org/newscodes/subjectcode/>;
	skos:broadMatch medtop:20001067;
	skos:broader	subj:15056000.

subj:15056005
	rdf:type skos:Concept;
	skos:prefLabel	"5000 m"@en-GB;
	skos:definition	"Speed skating race over 5000m "@en-GB;
	skos:inScheme <http://cv.iptc.org/newscodes/subjectcode/>;
	skos:broadMatch medtop:20001067;
	skos:broader	subj:15056000.

subj:15056006
	rdf:type skos:Concept;
	skos:prefLabel	"10000 m"@en-GB;
	skos:definition	"Speed skating race over 10000m "@en-GB;
	skos:inScheme <http://cv.iptc.org/newscodes/subjectcode/>;
	skos:broadMatch medtop:20001067;
	skos:broader	subj:15056000.

subj:15056007
	rdf:type skos:Concept;
	skos:prefLabel	"Short-track"@en-GB;
	skos:definition	"Races of four or more skaters on an oval ice track. Qualifying, semi-finals and finals determine winners. "@en-GB;
	skos:historyNote	"typo fixed in Explanation "@en-GB;
	skos:inScheme <http://cv.iptc.org/newscodes/subjectcode/>;
	skos:broadMatch medtop:20001067;
	skos:broader	subj:15056000.

subj:15056008
	rdf:type skos:Concept;
	skos:prefLabel	"st 500 m"@en-GB;
	skos:definition	"Short track speed skate race over 500m "@en-GB;
	skos:inScheme <http://cv.iptc.org/newscodes/subjectcode/>;
	skos:broadMatch medtop:20001067;
	skos:broader	subj:15056000.

subj:15056009
	rdf:type skos:Concept;
	skos:prefLabel	"st 1000m"@en-GB;
	skos:definition	"Short track speed skate race over 1000m "@en-GB;
	skos:inScheme <http://cv.iptc.org/newscodes/subjectcode/>;
	skos:broadMatch medtop:20001067;
	skos:broader	subj:15056000.

subj:15056010
	rdf:type skos:Concept;
	skos:prefLabel	"st 1500m"@en-GB;
	skos:definition	"Short track speed skate race over 1500m "@en-GB;
	skos:inScheme <http://cv.iptc.org/newscodes/subjectcode/>;
	skos:broadMatch medtop:20001067;
	skos:broader	subj:15056000.

subj:15056011
	rdf:type skos:Concept;
	skos:prefLabel	"st 3000m"@en-GB;
	skos:definition	"Short track speed skate race over 3000m "@en-GB;
	skos:inScheme <http://cv.iptc.org/newscodes/subjectcode/>;
	skos:broadMatch medtop:20001067;
	skos:broader	subj:15056000.

subj:15056012
	rdf:type skos:Concept;
	skos:prefLabel	"st 3000m relay"@en-GB;
	skos:definition	"Short track relay speed skate race over 3000m "@en-GB;
	skos:inScheme <http://cv.iptc.org/newscodes/subjectcode/>;
	skos:broadMatch medtop:20001067;
	skos:broader	subj:15056000.

subj:15056013
	rdf:type skos:Concept;
	skos:prefLabel	"st 5000m"@en-GB;
	skos:definition	"Short track speed skate race over 5000m "@en-GB;
	skos:inScheme <http://cv.iptc.org/newscodes/subjectcode/>;
	skos:broadMatch medtop:20001067;
	skos:broader	subj:15056000.

subj:15056014
	rdf:type skos:Concept;
	skos:prefLabel	"st 5000m relay"@en-GB;
	skos:definition	"Short track relay speed skate race over 5000m "@en-GB;
	skos:inScheme <http://cv.iptc.org/newscodes/subjectcode/>;
	skos:broadMatch medtop:20001067;
	skos:broader	subj:15056000.

subj:15057000
	rdf:type skos:Concept;
	skos:prefLabel	"speedway"@en-GB;
	skos:definition	"Fast track "@en-GB;
	skos:inScheme <http://cv.iptc.org/newscodes/subjectcode/>;
	skos:exactMatch medtop:20001007;
	skos:broader	subj:15000000.

subj:15058000
	rdf:type skos:Concept;
	skos:prefLabel	"sports organisations"@en-GB;
	skos:definition	"Organisations responsible for a specific sport "@en-GB;
	skos:historyNote	"typo fixed in Explanation "@en-GB;
	skos:inScheme <http://cv.iptc.org/newscodes/subjectcode/>;
	skos:exactMatch medtop:20001125;
	skos:broader	subj:15000000;
	skos:narrower	subj:15058001;
	skos:narrower	subj:15058002;
	skos:narrower	subj:15058003;
	skos:narrower	subj:15058004;
	skos:narrower	subj:15058005.

subj:15058001
	rdf:type skos:Concept;
	skos:prefLabel	"IOC"@en-GB;
	skos:definition	"International Olympic Committee "@en-GB;
	skos:inScheme <http://cv.iptc.org/newscodes/subjectcode/>;
	skos:broadMatch medtop:20001125;
	skos:broader	subj:15058000.

subj:15058002
	rdf:type skos:Concept;
	skos:prefLabel	"international federation"@en-GB;
	skos:definition	"A body responsible for the international coordination of a specific sport "@en-GB;
	skos:inScheme <http://cv.iptc.org/newscodes/subjectcode/>;
	skos:broadMatch medtop:20001125;
	skos:broader	subj:15058000.

subj:15058003
	rdf:type skos:Concept;
	skos:prefLabel	"continental federation"@en-GB;
	skos:definition	"A body responsible for the continental coordination of a specific sport "@en-GB;
	skos:inScheme <http://cv.iptc.org/newscodes/subjectcode/>;
	skos:broadMatch medtop:20001125;
	skos:broader	subj:15058000.

subj:15058004
	rdf:type skos:Concept;
	skos:prefLabel	"national federation"@en-GB;
	skos:definition	"A body responsible for the national coordination of a specific sport "@en-GB;
	skos:inScheme <http://cv.iptc.org/newscodes/subjectcode/>;
	skos:broadMatch medtop:20001125;
	skos:broader	subj:15058000.

subj:15058005
	rdf:type skos:Concept;
	skos:prefLabel	"GAISF"@en-GB;
	skos:definition	"General Association of International Sports Federations "@en-GB;
	skos:inScheme <http://cv.iptc.org/newscodes/subjectcode/>;
	skos:broadMatch medtop:20001125;
	skos:broader	subj:15058000.

subj:15059000
	rdf:type skos:Concept;
	skos:prefLabel	"squash"@en-GB;
	skos:definition	"A racket sport of strategy and endurance played by singles or doubles teams in a walled court with a small rubber ball "@en-GB;
	skos:historyNote	"typo fixed in Explanation "@en-GB;
	skos:inScheme <http://cv.iptc.org/newscodes/subjectcode/>;
	skos:exactMatch medtop:20001068;
	skos:broader	subj:15000000.

subj:15060000
	rdf:type skos:Concept;
	skos:prefLabel	"sumo wrestling"@en-GB;
	skos:definition	"A combat sport of speed and rapidity with much ceremony where two contestants try to throw or slap a competitor out of a marked area. Generally practiced in Japan by large men. "@en-GB;
	skos:inScheme <http://cv.iptc.org/newscodes/subjectcode/>;
	skos:exactMatch medtop:20001069;
	skos:broader	subj:15000000.

subj:15061000
	rdf:type skos:Concept;
	skos:prefLabel	"surfing"@en-GB;
	skos:definition	"Water sport where contestants catch and ride waves upright on a surfboard "@en-GB;
	skos:inScheme <http://cv.iptc.org/newscodes/subjectcode/>;
	skos:exactMatch medtop:20001070;
	skos:broader	subj:15000000.

subj:15062000
	rdf:type skos:Concept;
	skos:prefLabel	"swimming"@en-GB;
	skos:definition	"A water sport where contestants swim as fast as possible in a given style and win races by being the first to touch home "@en-GB;
	skos:inScheme <http://cv.iptc.org/newscodes/subjectcode/>;
	skos:exactMatch medtop:20001071;
	skos:broader	subj:15000000;
	skos:narrower	subj:15062001;
	skos:narrower	subj:15062002;
	skos:narrower	subj:15062003;
	skos:narrower	subj:15062004;
	skos:narrower	subj:15062005;
	skos:narrower	subj:15062006;
	skos:narrower	subj:15062007;
	skos:narrower	subj:15062008;
	skos:narrower	subj:15062009;
	skos:narrower	subj:15062010;
	skos:narrower	subj:15062011;
	skos:narrower	subj:15062012;
	skos:narrower	subj:15062013;
	skos:narrower	subj:15062014;
	skos:narrower	subj:15062015;
	skos:narrower	subj:15062016;
	skos:narrower	subj:15062017;
	skos:narrower	subj:15062018;
	skos:narrower	subj:15062019;
	skos:narrower	subj:15062020;
	skos:narrower	subj:15062021;
	skos:narrower	subj:15062022;
	skos:narrower	subj:15062023;
	skos:narrower	subj:15062024;
	skos:narrower	subj:15062025;
	skos:narrower	subj:15062026.

subj:15062001
	rdf:type skos:Concept;
	skos:prefLabel	"50 m freestyle"@en-GB;
	skos:definition	"Competitors cover 50m in any style, though front crawl is universally employed "@en-GB;
	skos:inScheme <http://cv.iptc.org/newscodes/subjectcode/>;
	skos:broadMatch medtop:20001071;
	skos:broader	subj:15062000.

subj:15062002
	rdf:type skos:Concept;
	skos:prefLabel	"100 m freestyle"@en-GB;
	skos:definition	"Competitors cover 100m in any style, though front crawl is universally employed "@en-GB;
	skos:inScheme <http://cv.iptc.org/newscodes/subjectcode/>;
	skos:broadMatch medtop:20001071;
	skos:broader	subj:15062000.

subj:15062003
	rdf:type skos:Concept;
	skos:prefLabel	"200 m freestyle"@en-GB;
	skos:definition	"Competitors cover 200m in any style, though front crawl is universally employed "@en-GB;
	skos:inScheme <http://cv.iptc.org/newscodes/subjectcode/>;
	skos:broadMatch medtop:20001071;
	skos:broader	subj:15062000.

subj:15062004
	rdf:type skos:Concept;
	skos:prefLabel	"400 m freestyle"@en-GB;
	skos:definition	"Competitors cover 400m in any style, though front crawl is universally employed "@en-GB;
	skos:inScheme <http://cv.iptc.org/newscodes/subjectcode/>;
	skos:broadMatch medtop:20001071;
	skos:broader	subj:15062000.

subj:15062005
	rdf:type skos:Concept;
	skos:prefLabel	"800 m freestyle"@en-GB;
	skos:definition	"Competitors cover 800m in any style, though front crawl is universally employed "@en-GB;
	skos:inScheme <http://cv.iptc.org/newscodes/subjectcode/>;
	skos:broadMatch medtop:20001071;
	skos:broader	subj:15062000.

subj:15062006
	rdf:type skos:Concept;
	skos:prefLabel	"1500 m freestyle"@en-GB;
	skos:definition	"Competitors cover 1500m in any style, though front crawl is universally employed "@en-GB;
	skos:inScheme <http://cv.iptc.org/newscodes/subjectcode/>;
	skos:broadMatch medtop:20001071;
	skos:broader	subj:15062000.

subj:15062007
	rdf:type skos:Concept;
	skos:prefLabel	"relay 4x50 m freestyle"@en-GB;
	skos:definition	"Teams of four swimmers cover 50m freestyle in a 200m race "@en-GB;
	skos:inScheme <http://cv.iptc.org/newscodes/subjectcode/>;
	skos:broadMatch medtop:20001071;
	skos:broader	subj:15062000.

subj:15062008
	rdf:type skos:Concept;
	skos:prefLabel	"relay 4x100 m freestyle"@en-GB;
	skos:definition	"Teams of four swimmers cover 100m freestyle in a 400m race "@en-GB;
	skos:inScheme <http://cv.iptc.org/newscodes/subjectcode/>;
	skos:broadMatch medtop:20001071;
	skos:broader	subj:15062000.

subj:15062009
	rdf:type skos:Concept;
	skos:prefLabel	"relay 4x200 m freestyle"@en-GB;
	skos:definition	"Teams of four swimmers cover 200m freestyle in a 800m race "@en-GB;
	skos:inScheme <http://cv.iptc.org/newscodes/subjectcode/>;
	skos:broadMatch medtop:20001071;
	skos:broader	subj:15062000.

subj:15062010
	rdf:type skos:Concept;
	skos:prefLabel	"50 m backstroke"@en-GB;
	skos:definition	"Competitors cover 50m in the backstroke style "@en-GB;
	skos:inScheme <http://cv.iptc.org/newscodes/subjectcode/>;
	skos:broadMatch medtop:20001071;
	skos:broader	subj:15062000.

subj:15062011
	rdf:type skos:Concept;
	skos:prefLabel	"100 m backstroke"@en-GB;
	skos:definition	"Competitors cover 100m in the backstroke style "@en-GB;
	skos:inScheme <http://cv.iptc.org/newscodes/subjectcode/>;
	skos:broadMatch medtop:20001071;
	skos:broader	subj:15062000.

subj:15062012
	rdf:type skos:Concept;
	skos:prefLabel	"200 m backstroke"@en-GB;
	skos:definition	"Competitors cover 200m in the backstroke style "@en-GB;
	skos:inScheme <http://cv.iptc.org/newscodes/subjectcode/>;
	skos:broadMatch medtop:20001071;
	skos:broader	subj:15062000.

subj:15062013
	rdf:type skos:Concept;
	skos:prefLabel	"50 m breaststroke"@en-GB;
	skos:definition	"A 50m race in the breaststroke style, on the front, effecting forward and outward push movements with the arms and backward and outward pushes with the legs "@en-GB;
	skos:inScheme <http://cv.iptc.org/newscodes/subjectcode/>;
	skos:broadMatch medtop:20001071;
	skos:broader	subj:15062000.

subj:15062014
	rdf:type skos:Concept;
	skos:prefLabel	"100 m breaststroke"@en-GB;
	skos:definition	"A 100m race in the breaststroke style, on the front, effecting forward and outward push movements with the arms and backward and outward pushes with the legs "@en-GB;
	skos:inScheme <http://cv.iptc.org/newscodes/subjectcode/>;
	skos:broadMatch medtop:20001071;
	skos:broader	subj:15062000.

subj:15062015
	rdf:type skos:Concept;
	skos:prefLabel	"200 m breaststroke"@en-GB;
	skos:definition	"A 200m race in the breaststroke style, on the front, effecting forward and outward push movements with the arms and backward and outward pushes with the legs "@en-GB;
	skos:inScheme <http://cv.iptc.org/newscodes/subjectcode/>;
	skos:broadMatch medtop:20001071;
	skos:broader	subj:15062000.

subj:15062016
	rdf:type skos:Concept;
	skos:prefLabel	"50 m butterfly"@en-GB;
	skos:definition	"A 50m butterfly race, swum on the front with the shoulders remaining parallel to the water both arms moving in simultaneous windmill fashion, the legs remain together and are moved in a flapping motion. The most physical of all styles. "@en-GB;
	skos:inScheme <http://cv.iptc.org/newscodes/subjectcode/>;
	skos:broadMatch medtop:20001071;
	skos:broader	subj:15062000.

subj:15062017
	rdf:type skos:Concept;
	skos:prefLabel	"100 m butterfly"@en-GB;
	skos:definition	"A 100m butterfly race, swum on the front with the shoulders remaining parallel to the water both arms moving in simultaneous windmill fashion, the legs remain together and are moved in a flapping motion. The most physical of all styles "@en-GB;
	skos:inScheme <http://cv.iptc.org/newscodes/subjectcode/>;
	skos:broadMatch medtop:20001071;
	skos:broader	subj:15062000.

subj:15062018
	rdf:type skos:Concept;
	skos:prefLabel	"200 m butterfly"@en-GB;
	skos:definition	"A 200m butterfly race, swum on the front with the shoulders remaining parallel to the water both arms moving in simultaneous windmill fashion, the legs remain together and are moved in a flapping motion. The most physical of all styles "@en-GB;
	skos:inScheme <http://cv.iptc.org/newscodes/subjectcode/>;
	skos:broadMatch medtop:20001071;
	skos:broader	subj:15062000.

subj:15062019
	rdf:type skos:Concept;
	skos:prefLabel	"100 m medley"@en-GB;
	skos:definition	"Swimmers complete four laps, each in a different style and in this order: butterfly, backstroke, breaststroke and freestyle, covering a total of 100m. "@en-GB;
	skos:inScheme <http://cv.iptc.org/newscodes/subjectcode/>;
	skos:broadMatch medtop:20001071;
	skos:broader	subj:15062000.

subj:15062020
	rdf:type skos:Concept;
	skos:prefLabel	"200 m medley"@en-GB;
	skos:definition	"Swimmers complete four laps, each in a different style and in this order: butterfly, backstroke, breaststroke and freestyle, covering a total of 200m. "@en-GB;
	skos:inScheme <http://cv.iptc.org/newscodes/subjectcode/>;
	skos:broadMatch medtop:20001071;
	skos:broader	subj:15062000.

subj:15062021
	rdf:type skos:Concept;
	skos:prefLabel	"400 m medley"@en-GB;
	skos:definition	"Swimmers complete eight laps, two in each style and in this order: butterfly, backstroke, breaststroke and freestyle, covering a total of 400m. "@en-GB;
	skos:inScheme <http://cv.iptc.org/newscodes/subjectcode/>;
	skos:broadMatch medtop:20001071;
	skos:broader	subj:15062000.

subj:15062022
	rdf:type skos:Concept;
	skos:prefLabel	"relay 4x50 m medlay"@en-GB;
	skos:definition	"A relay team of four, each of whom completes a single lap and each in a different style in this order: backstroke, breaststroke, butterfly and freestyle in a race of 200m total. "@en-GB;
	skos:inScheme <http://cv.iptc.org/newscodes/subjectcode/>;
	skos:broadMatch medtop:20001071;
	skos:broader	subj:15062000.

subj:15062023
	rdf:type skos:Concept;
	skos:prefLabel	"relay4x100 m medley"@en-GB;
	skos:definition	"A relay team of four, each of whom completes two laps and each in a different style in this order: backstroke, breaststroke, butterfly and freestyle in a race of 400m total. "@en-GB;
	skos:historyNote	"typo fixed in Explanation "@en-GB;
	skos:inScheme <http://cv.iptc.org/newscodes/subjectcode/>;
	skos:broadMatch medtop:20001071;
	skos:broader	subj:15062000.

subj:15062024
	rdf:type skos:Concept;
	skos:prefLabel	"short course"@en-GB;
	skos:definition	"Races competed in a 25m length pool "@en-GB;
	skos:inScheme <http://cv.iptc.org/newscodes/subjectcode/>;
	skos:broadMatch medtop:20001071;
	skos:broader	subj:15062000.

subj:15062025
	rdf:type skos:Concept;
	skos:prefLabel	"synchronised technical routine"@en-GB;
	skos:definition	"Contestants obtain points from 10 sitting judges by executing certain synchronised artistic shapes and movements in the water. In the technical programme, competitors must execute a range of specific moves in a given order. "@en-GB;
	skos:inScheme <http://cv.iptc.org/newscodes/subjectcode/>;
	skos:exactMatch medtop:20001082;
	skos:broader	subj:15062000.

subj:15062026
	rdf:type skos:Concept;
	skos:prefLabel	"synchronised free routine"@en-GB;
	skos:definition	"In the free programme, music, movements and their order of execution are not restricted. "@en-GB;
	skos:inScheme <http://cv.iptc.org/newscodes/subjectcode/>;
	skos:exactMatch medtop:20001081;
	skos:broader	subj:15062000.

subj:15063000
	rdf:type skos:Concept;
	skos:prefLabel	"table tennis"@en-GB;
	skos:definition	"A racket sport for two or four (in doubles), who compete at a table divided by a net using a small bat to play a lightweight ball "@en-GB;
	skos:historyNote	"typo fixed in Explanation "@en-GB;
	skos:inScheme <http://cv.iptc.org/newscodes/subjectcode/>;
	skos:exactMatch medtop:20001083;
	skos:broader	subj:15000000.

subj:15064000
	rdf:type skos:Concept;
	skos:prefLabel	"Taekwon-Do"@en-GB;
	skos:definition	"A martial art of Korean origin "@en-GB;
	skos:inScheme <http://cv.iptc.org/newscodes/subjectcode/>;
	skos:exactMatch medtop:20001084;
	skos:broader	subj:15000000;
	skos:narrower	subj:15064001;
	skos:narrower	subj:15064002;
	skos:narrower	subj:15064003;
	skos:narrower	subj:15064004;
	skos:narrower	subj:15064005;
	skos:narrower	subj:15064006;
	skos:narrower	subj:15064007;
	skos:narrower	subj:15064008.

subj:15064001
	rdf:type skos:Concept;
	skos:prefLabel	"under 49 kg"@en-GB;
	skos:definition	"Weight category in Taekwon-Do"@en-GB;
	skos:inScheme <http://cv.iptc.org/newscodes/subjectcode/>;
	skos:broadMatch medtop:20001084;
	skos:broader	subj:15064000.

subj:15064002
	rdf:type skos:Concept;
	skos:prefLabel	"under 58 kg"@en-GB;
	skos:definition	"Weight category in Taekwon-Do"@en-GB;
	skos:inScheme <http://cv.iptc.org/newscodes/subjectcode/>;
	skos:broadMatch medtop:20001084;
	skos:broader	subj:15064000.

subj:15064003
	rdf:type skos:Concept;
	skos:prefLabel	"49-57 kg"@en-GB;
	skos:definition	"Weight category in Taekwon-Do"@en-GB;
	skos:inScheme <http://cv.iptc.org/newscodes/subjectcode/>;
	skos:broadMatch medtop:20001084;
	skos:broader	subj:15064000.

subj:15064004
	rdf:type skos:Concept;
	skos:prefLabel	"58-68 kg"@en-GB;
	skos:definition	"Weight category in Taekwon-Do"@en-GB;
	skos:inScheme <http://cv.iptc.org/newscodes/subjectcode/>;
	skos:broadMatch medtop:20001084;
	skos:broader	subj:15064000.

subj:15064005
	rdf:type skos:Concept;
	skos:prefLabel	"57-67 kg"@en-GB;
	skos:definition	"Weight category in Taekwon-Do"@en-GB;
	skos:inScheme <http://cv.iptc.org/newscodes/subjectcode/>;
	skos:broadMatch medtop:20001084;
	skos:broader	subj:15064000.

subj:15064006
	rdf:type skos:Concept;
	skos:prefLabel	"68-80 kg"@en-GB;
	skos:definition	"Weight category in Taekwon-Do"@en-GB;
	skos:inScheme <http://cv.iptc.org/newscodes/subjectcode/>;
	skos:broadMatch medtop:20001084;
	skos:broader	subj:15064000.

subj:15064007
	rdf:type skos:Concept;
	skos:prefLabel	"over 67 kg"@en-GB;
	skos:definition	"Weight category in Taekwon-Do"@en-GB;
	skos:inScheme <http://cv.iptc.org/newscodes/subjectcode/>;
	skos:broadMatch medtop:20001084;
	skos:broader	subj:15064000.

subj:15064008
	rdf:type skos:Concept;
	skos:prefLabel	"over 80 kg"@en-GB;
	skos:definition	"Weight category in Taekwon-Do"@en-GB;
	skos:inScheme <http://cv.iptc.org/newscodes/subjectcode/>;
	skos:broadMatch medtop:20001084;
	skos:broader	subj:15064000.

subj:15065000
	rdf:type skos:Concept;
	skos:prefLabel	"tennis"@en-GB;
	skos:definition	"A sport where two players, four in doubles, equipped with a racket compete by hitting the ball over a net into the opponent's side of the court with the aim of putting it out of reach within the regulation lines, thus winning points. "@en-GB;
	skos:inScheme <http://cv.iptc.org/newscodes/subjectcode/>;
	skos:exactMatch medtop:20001085;
	skos:broader	subj:15000000;
	skos:narrower	subj:15065001.

subj:15065001
	rdf:type skos:Concept;
	skos:prefLabel	"soft tennis"@en-GB;
	skos:definition	"Tennis with a soft rubber ball. (Programme of National Sports Festival in Japan) "@en-GB;
	skos:inScheme <http://cv.iptc.org/newscodes/subjectcode/>;
	skos:broadMatch medtop:20000822;
	skos:broader	subj:15065000.

subj:15066000
	rdf:type skos:Concept;
	skos:prefLabel	"triathlon"@en-GB;
	skos:definition	"An endurance multi-sport where competitors first swim, then cycle and then run a road race. Distances vary according to the competition, the Olympic version being 1.5, 40 and 10km respectively. "@en-GB;
	skos:historyNote	"typo fixed in Explanation "@en-GB;
	skos:inScheme <http://cv.iptc.org/newscodes/subjectcode/>;
	skos:exactMatch medtop:20001087;
	skos:broader	subj:15000000;
	skos:narrower	subj:15066001;
	skos:narrower	subj:15066002;
	skos:narrower	subj:15066003.

subj:15066001
	rdf:type skos:Concept;
	skos:prefLabel	"triathlon swimming"@en-GB;
	skos:definition	"Triathlon event "@en-GB;
	skos:inScheme <http://cv.iptc.org/newscodes/subjectcode/>;
	skos:broadMatch medtop:20001087;
	skos:broader	subj:15066000.

subj:15066002
	rdf:type skos:Concept;
	skos:prefLabel	"triathlon cycling"@en-GB;
	skos:definition	"Triathlon event "@en-GB;
	skos:inScheme <http://cv.iptc.org/newscodes/subjectcode/>;
	skos:broadMatch medtop:20001087;
	skos:broader	subj:15066000.

subj:15066003
	rdf:type skos:Concept;
	skos:prefLabel	"triathlon run"@en-GB;
	skos:definition	"Triathlon event "@en-GB;
	skos:inScheme <http://cv.iptc.org/newscodes/subjectcode/>;
	skos:broadMatch medtop:20001087;
	skos:broader	subj:15066000.

subj:15067000
	rdf:type skos:Concept;
	skos:prefLabel	"volleyball"@en-GB;
	skos:definition	"Two teams of six record points by hitting a ball over a net into the opponent's half of the court, keeping it in the air at all times. Points are won when opponents fail to return the ball. "@en-GB;
	skos:inScheme <http://cv.iptc.org/newscodes/subjectcode/>;
	skos:exactMatch medtop:20001089;
	skos:broader	subj:15000000;
	skos:narrower	subj:15067001.

subj:15067001
	rdf:type skos:Concept;
	skos:prefLabel	"beach volleyball"@en-GB;
	skos:definition	"Two teams of two players compete on a sand court. Unlike indoor volleyball, points are scored only when the serving team wins a rally or forces an error. The sand surface makes it more physically demanding than volleyball. "@en-GB;
	skos:inScheme <http://cv.iptc.org/newscodes/subjectcode/>;
	skos:exactMatch medtop:20001090;
	skos:broader	subj:15067000.

subj:15068000
	rdf:type skos:Concept;
	skos:prefLabel	"water polo"@en-GB;
	skos:definition	"Played in a pool between two teams of 7, who must stay afloat and can only use one hand to pass the ball or swim with it before trying to throw it into the opponents net to score goals. "@en-GB;
	skos:historyNote	"typo fixed in Explanation "@en-GB;
	skos:inScheme <http://cv.iptc.org/newscodes/subjectcode/>;
	skos:exactMatch medtop:20001091;
	skos:broader	subj:15000000.

subj:15069000
	rdf:type skos:Concept;
	skos:prefLabel	"water skiing"@en-GB;
	skos:definition	"On one or two skis contestants are pulled by a power boat along the water's surface "@en-GB;
	skos:inScheme <http://cv.iptc.org/newscodes/subjectcode/>;
	skos:exactMatch medtop:20001092;
	skos:broader	subj:15000000;
	skos:narrower	subj:15069001;
	skos:narrower	subj:15069002;
	skos:narrower	subj:15069003;
	skos:narrower	subj:15069004.

subj:15069001
	rdf:type skos:Concept;
	skos:prefLabel	"slalom"@en-GB;
	skos:definition	"Speed event where contestants round a course marked out by buoys "@en-GB;
	skos:historyNote	"typo fixed in Explanation "@en-GB;
	skos:inScheme <http://cv.iptc.org/newscodes/subjectcode/>;
	skos:broadMatch medtop:20001092;
	skos:broader	subj:15069000.

subj:15069002
	rdf:type skos:Concept;
	skos:prefLabel	"trick"@en-GB;
	skos:definition	"Skiers perform a maximum of figures in a limited time period "@en-GB;
	skos:inScheme <http://cv.iptc.org/newscodes/subjectcode/>;
	skos:broadMatch medtop:20001092;
	skos:broader	subj:15069000.

subj:15069003
	rdf:type skos:Concept;
	skos:prefLabel	"jump"@en-GB;
	skos:definition	"Skiers perform as long a jump as possible from a ramp in the water "@en-GB;
	skos:inScheme <http://cv.iptc.org/newscodes/subjectcode/>;
	skos:broadMatch medtop:20001092;
	skos:broader	subj:15069000.

subj:15069004
	rdf:type skos:Concept;
	skos:prefLabel	"combined"@en-GB;
	skos:definition	"A combined event made up of the slalom, jump and trick "@en-GB;
	skos:inScheme <http://cv.iptc.org/newscodes/subjectcode/>;
	skos:broadMatch medtop:20001092;
	skos:broader	subj:15069000.

subj:15070000
	rdf:type skos:Concept;
	skos:prefLabel	"weightlifting"@en-GB;
	skos:definition	"A strength test where competitors lift as heavy a weight as possible "@en-GB;
	skos:inScheme <http://cv.iptc.org/newscodes/subjectcode/>;
	skos:exactMatch medtop:20001093;
	skos:broader	subj:15000000;
	skos:narrower	subj:15070001;
	skos:narrower	subj:15070002;
	skos:narrower	subj:15070003;
	skos:narrower	subj:15070004;
	skos:narrower	subj:15070005;
	skos:narrower	subj:15070006;
	skos:narrower	subj:15070007;
	skos:narrower	subj:15070008;
	skos:narrower	subj:15070009;
	skos:narrower	subj:15070010;
	skos:narrower	subj:15070011;
	skos:narrower	subj:15070012;
	skos:narrower	subj:15070013;
	skos:narrower	subj:15070014;
	skos:narrower	subj:15070015;
	skos:narrower	subj:15070016.

subj:15070001
	rdf:type skos:Concept;
	skos:prefLabel	"snatch"@en-GB;
	skos:definition	"The bar must be lifted from floor to above the head in one movement "@en-GB;
	skos:inScheme <http://cv.iptc.org/newscodes/subjectcode/>;
	skos:exactMatch medtop:20001096;
	skos:broader	subj:15070000.

subj:15070002
	rdf:type skos:Concept;
	skos:prefLabel	"clean and jerk"@en-GB;
	skos:definition	"The bar is first lifted to the shoulders and then jerk it above the head and keep it there while maintaining straight legs "@en-GB;
	skos:inScheme <http://cv.iptc.org/newscodes/subjectcode/>;
	skos:exactMatch medtop:20001094;
	skos:broader	subj:15070000.

subj:15070003
	rdf:type skos:Concept;
	skos:prefLabel	"48 kg"@en-GB;
	skos:definition	"Competitor weight category in weightlifting"@en-GB;
	skos:inScheme <http://cv.iptc.org/newscodes/subjectcode/>;
	skos:broadMatch medtop:20001093;
	skos:broader	subj:15070000.

subj:15070004
	rdf:type skos:Concept;
	skos:prefLabel	"53 kg"@en-GB;
	skos:definition	"Competitor weight category in weightlifting"@en-GB;
	skos:inScheme <http://cv.iptc.org/newscodes/subjectcode/>;
	skos:broadMatch medtop:20001093;
	skos:broader	subj:15070000.

subj:15070005
	rdf:type skos:Concept;
	skos:prefLabel	"63 kg"@en-GB;
	skos:definition	"Competitor weight category in weightlifting"@en-GB;
	skos:inScheme <http://cv.iptc.org/newscodes/subjectcode/>;
	skos:broadMatch medtop:20001093;
	skos:broader	subj:15070000.

subj:15070006
	rdf:type skos:Concept;
	skos:prefLabel	"75 kg"@en-GB;
	skos:definition	"Competitor weight category in weightlifting"@en-GB;
	skos:inScheme <http://cv.iptc.org/newscodes/subjectcode/>;
	skos:broadMatch medtop:20001093;
	skos:broader	subj:15070000.

subj:15070007
	rdf:type skos:Concept;
	skos:prefLabel	"over 75 kg"@en-GB;
	skos:definition	"Competitor weight category in weightlifting"@en-GB;
	skos:inScheme <http://cv.iptc.org/newscodes/subjectcode/>;
	skos:broadMatch medtop:20001093;
	skos:broader	subj:15070000.

subj:15070008
	rdf:type skos:Concept;
	skos:prefLabel	"56 kg"@en-GB;
	skos:definition	"Competitor weight category in weightlifting"@en-GB;
	skos:inScheme <http://cv.iptc.org/newscodes/subjectcode/>;
	skos:broadMatch medtop:20001093;
	skos:broader	subj:15070000.

subj:15070009
	rdf:type skos:Concept;
	skos:prefLabel	"62 kg"@en-GB;
	skos:definition	"Competitor weight category in weightlifting"@en-GB;
	skos:inScheme <http://cv.iptc.org/newscodes/subjectcode/>;
	skos:broadMatch medtop:20001093;
	skos:broader	subj:15070000.

subj:15070010
	rdf:type skos:Concept;
	skos:prefLabel	"69 kg"@en-GB;
	skos:definition	"Competitor weight category in weightlifting"@en-GB;
	skos:inScheme <http://cv.iptc.org/newscodes/subjectcode/>;
	skos:broadMatch medtop:20001093;
	skos:broader	subj:15070000.

subj:15070011
	rdf:type skos:Concept;
	skos:prefLabel	"77 kg"@en-GB;
	skos:definition	"Competitor weight category in weightlifting"@en-GB;
	skos:inScheme <http://cv.iptc.org/newscodes/subjectcode/>;
	skos:broadMatch medtop:20001093;
	skos:broader	subj:15070000.

subj:15070012
	rdf:type skos:Concept;
	skos:prefLabel	"85 kg"@en-GB;
	skos:definition	"Competitor weight category in weightlifting"@en-GB;
	skos:inScheme <http://cv.iptc.org/newscodes/subjectcode/>;
	skos:broadMatch medtop:20001093;
	skos:broader	subj:15070000.

subj:15070013
	rdf:type skos:Concept;
	skos:prefLabel	"94 kg"@en-GB;
	skos:definition	"Competitor weight category in weightlifting"@en-GB;
	skos:inScheme <http://cv.iptc.org/newscodes/subjectcode/>;
	skos:broadMatch medtop:20001093;
	skos:broader	subj:15070000.

subj:15070014
	rdf:type skos:Concept;
	skos:prefLabel	"105 kg"@en-GB;
	skos:definition	"Competitor weight category in weightlifting"@en-GB;
	skos:inScheme <http://cv.iptc.org/newscodes/subjectcode/>;
	skos:broadMatch medtop:20001093;
	skos:broader	subj:15070000.

subj:15070015
	rdf:type skos:Concept;
	skos:prefLabel	"over 105 kg"@en-GB;
	skos:definition	"Competitor weight category in weightlifting"@en-GB;
	skos:inScheme <http://cv.iptc.org/newscodes/subjectcode/>;
	skos:broadMatch medtop:20001093;
	skos:broader	subj:15070000.

subj:15070016
	rdf:type skos:Concept;
	skos:prefLabel	"powerlifting"@en-GB;
	skos:definition	"A strength test where competitors lift as heavy a weight as possible "@en-GB;
	skos:inScheme <http://cv.iptc.org/newscodes/subjectcode/>;
	skos:exactMatch medtop:20001095;
	skos:broader	subj:15070000.

subj:15071000
	rdf:type skos:Concept;
	skos:prefLabel	"windsurfing"@en-GB;
	skos:definition	"Contestants must complete a marked out course as fast as possible on a windsurf board "@en-GB;
	skos:inScheme <http://cv.iptc.org/newscodes/subjectcode/>;
	skos:exactMatch medtop:20001097;
	skos:broader	subj:15000000;
	skos:narrower	subj:15071001;
	skos:narrower	subj:15071002;
	skos:narrower	subj:15071003;
	skos:narrower	subj:15071004.

subj:15071001
	rdf:type skos:Concept;
	skos:prefLabel	"ocean"@en-GB;
	skos:definition	"Races on the open seas "@en-GB;
	skos:inScheme <http://cv.iptc.org/newscodes/subjectcode/>;
	skos:broadMatch medtop:20001097;
	skos:broader	subj:15071000.

subj:15071002
	rdf:type skos:Concept;
	skos:prefLabel	"lake"@en-GB;
	skos:definition	"Races competed on lakes "@en-GB;
	skos:inScheme <http://cv.iptc.org/newscodes/subjectcode/>;
	skos:broadMatch medtop:20001097;
	skos:broader	subj:15071000.

subj:15071003
	rdf:type skos:Concept;
	skos:prefLabel	"river"@en-GB;
	skos:definition	"Races competed on rivers "@en-GB;
	skos:inScheme <http://cv.iptc.org/newscodes/subjectcode/>;
	skos:broadMatch medtop:20001097;
	skos:broader	subj:15071000.

subj:15071004
	rdf:type skos:Concept;
	skos:prefLabel	"land"@en-GB;
	skos:definition	"Races competed on land with a board equipped with wheels "@en-GB;
	skos:historyNote	"typo fixed in Explanation "@en-GB;
	skos:inScheme <http://cv.iptc.org/newscodes/subjectcode/>;
	skos:broadMatch medtop:20001097;
	skos:broader	subj:15071000.

subj:15072000
	rdf:type skos:Concept;
	skos:prefLabel	"wrestling"@en-GB;
	skos:definition	"Combat sport where each wrestler attempts to win over his adversary, by holding both shoulders on the ground (fall) long enough to be in control. Points can also be decisive. "@en-GB;
	skos:inScheme <http://cv.iptc.org/newscodes/subjectcode/>;
	skos:exactMatch medtop:20001098;
	skos:broader	subj:15000000;
	skos:narrower	subj:15072001;
	skos:narrower	subj:15072002;
	skos:narrower	subj:15072003;
	skos:narrower	subj:15072004;
	skos:narrower	subj:15072005;
	skos:narrower	subj:15072006;
	skos:narrower	subj:15072007;
	skos:narrower	subj:15072008;
	skos:narrower	subj:15072009;
	skos:narrower	subj:15072010;
	skos:narrower	subj:15072011;
	skos:narrower	subj:15072012.

subj:15072001
	rdf:type skos:Concept;
	skos:prefLabel	"freestyle"@en-GB;
	skos:definition	"A style where leg holds are allowed "@en-GB;
	skos:inScheme <http://cv.iptc.org/newscodes/subjectcode/>;
	skos:exactMatch medtop:20001099;
	skos:broader	subj:15072000.

subj:15072002
	rdf:type skos:Concept;
	skos:prefLabel	"greco-roman"@en-GB;
	skos:definition	"A style where the only holds allowed are those between the head and the belt "@en-GB;
	skos:inScheme <http://cv.iptc.org/newscodes/subjectcode/>;
	skos:exactMatch medtop:20001100;
	skos:broader	subj:15072000.

subj:15072003
	rdf:type skos:Concept;
	skos:prefLabel	"over 130 kg"@en-GB;
	skos:definition	"Competitor weight category in wrestling"@en-GB;
	skos:inScheme <http://cv.iptc.org/newscodes/subjectcode/>;
	skos:broadMatch medtop:20001098;
	skos:broader	subj:15072000.

subj:15072004
	rdf:type skos:Concept;
	skos:prefLabel	"130 kg"@en-GB;
	skos:definition	"Competitor weight category in wrestling"@en-GB;
	skos:inScheme <http://cv.iptc.org/newscodes/subjectcode/>;
	skos:broadMatch medtop:20001098;
	skos:broader	subj:15072000.

subj:15072005
	rdf:type skos:Concept;
	skos:prefLabel	"97 kg"@en-GB;
	skos:definition	"Competitor weight category in wrestling"@en-GB;
	skos:inScheme <http://cv.iptc.org/newscodes/subjectcode/>;
	skos:broadMatch medtop:20001098;
	skos:broader	subj:15072000.

subj:15072006
	rdf:type skos:Concept;
	skos:prefLabel	"85 kg"@en-GB;
	skos:definition	"Competitor weight category in wrestling"@en-GB;
	skos:inScheme <http://cv.iptc.org/newscodes/subjectcode/>;
	skos:broadMatch medtop:20001098;
	skos:broader	subj:15072000.

subj:15072007
	rdf:type skos:Concept;
	skos:prefLabel	"76 kg"@en-GB;
	skos:definition	"Competitor weight category in wrestling"@en-GB;
	skos:inScheme <http://cv.iptc.org/newscodes/subjectcode/>;
	skos:broadMatch medtop:20001098;
	skos:broader	subj:15072000.

subj:15072008
	rdf:type skos:Concept;
	skos:prefLabel	"69 kg"@en-GB;
	skos:definition	"Competitor weight category in wrestling"@en-GB;
	skos:inScheme <http://cv.iptc.org/newscodes/subjectcode/>;
	skos:broadMatch medtop:20001098;
	skos:broader	subj:15072000.

subj:15072009
	rdf:type skos:Concept;
	skos:prefLabel	"63 kg"@en-GB;
	skos:definition	"Competitor weight category in wrestling"@en-GB;
	skos:inScheme <http://cv.iptc.org/newscodes/subjectcode/>;
	skos:broadMatch medtop:20001098;
	skos:broader	subj:15072000.

subj:15072010
	rdf:type skos:Concept;
	skos:prefLabel	"58 kg"@en-GB;
	skos:definition	"Competitor weight category in wrestling"@en-GB;
	skos:inScheme <http://cv.iptc.org/newscodes/subjectcode/>;
	skos:broadMatch medtop:20001098;
	skos:broader	subj:15072000.

subj:15072011
	rdf:type skos:Concept;
	skos:prefLabel	"54 kg"@en-GB;
	skos:definition	"Competitor weight category in wrestling"@en-GB;
	skos:inScheme <http://cv.iptc.org/newscodes/subjectcode/>;
	skos:broadMatch medtop:20001098;
	skos:broader	subj:15072000.

subj:15072012
	rdf:type skos:Concept;
	skos:prefLabel	"Swiss wrestling"@en-GB;
	skos:definition	"Traditional Swiss sport similar to wrestling with specific rules "@en-GB;
	skos:inScheme <http://cv.iptc.org/newscodes/subjectcode/>;
	skos:exactMatch medtop:20001101;
	skos:broader	subj:15072000.

subj:15073000
	rdf:type skos:Concept;
	skos:prefLabel	"sports event"@en-GB;
	skos:definition	"Sports meeting "@en-GB;
	skos:inScheme <http://cv.iptc.org/newscodes/subjectcode/>;
	skos:exactMatch medtop:20001108;
	skos:broader	subj:15000000;
	skos:narrower	subj:15073001;
	skos:narrower	subj:15073002;
	skos:narrower	subj:15073003;
	skos:narrower	subj:15073004;
	skos:narrower	subj:15073005;
	skos:narrower	subj:15073006;
	skos:narrower	subj:15073007;
	skos:narrower	subj:15073008;
	skos:narrower	subj:15073009;
	skos:narrower	subj:15073010;
	skos:narrower	subj:15073011;
	skos:narrower	subj:15073012;
	skos:narrower	subj:15073013;
	skos:narrower	subj:15073014;
	skos:narrower	subj:15073015;
	skos:narrower	subj:15073016;
	skos:narrower	subj:15073017;
	skos:narrower	subj:15073018;
	skos:narrower	subj:15073019;
	skos:narrower	subj:15073020;
	skos:narrower	subj:15073021;
	skos:narrower	subj:15073022;
	skos:narrower	subj:15073023;
	skos:narrower	subj:15073024;
	skos:narrower	subj:15073025;
	skos:narrower	subj:15073026;
	skos:narrower	subj:15073027;
	skos:narrower	subj:15073028;
	skos:narrower	subj:15073029;
	skos:narrower	subj:15073030;
	skos:narrower	subj:15073031;
	skos:narrower	subj:15073032;
	skos:narrower	subj:15073033;
	skos:narrower	subj:15073034;
	skos:narrower	subj:15073035;
	skos:narrower	subj:15073036;
	skos:narrower	subj:15073037;
	skos:narrower	subj:15073038;
	skos:narrower	subj:15073039;
	skos:narrower	subj:15073040;
	skos:narrower	subj:15073041;
	skos:narrower	subj:15073042;
	skos:narrower	subj:15073043;
	skos:narrower	subj:15073044;
	skos:narrower	subj:15073045;
	skos:narrower	subj:15073046;
	skos:narrower	subj:15073047.

subj:15073001
	rdf:type skos:Concept;
	skos:prefLabel	"Summer Olympics"@en-GB;
	skos:definition	"Summer Olympics "@en-GB;
	skos:inScheme <http://cv.iptc.org/newscodes/subjectcode/>;
	skos:broadMatch medtop:20001108;
	skos:broader	subj:15073000.

subj:15073002
	rdf:type skos:Concept;
	skos:prefLabel	"Winter Olympics"@en-GB;
	skos:definition	"Winter Olympics "@en-GB;
	skos:inScheme <http://cv.iptc.org/newscodes/subjectcode/>;
	skos:broadMatch medtop:20001108;
	skos:broader	subj:15073000.

subj:15073003
	rdf:type skos:Concept;
	skos:prefLabel	"Summer universiade"@en-GB;
	skos:definition	"Summer universiade "@en-GB;
	skos:inScheme <http://cv.iptc.org/newscodes/subjectcode/>;
	skos:broadMatch medtop:20001108;
	skos:broader	subj:15073000.

subj:15073004
	rdf:type skos:Concept;
	skos:prefLabel	"Winter Universiade"@en-GB;
	skos:definition	"Winter Universiade "@en-GB;
	skos:inScheme <http://cv.iptc.org/newscodes/subjectcode/>;
	skos:broadMatch medtop:20001108;
	skos:broader	subj:15073000.

subj:15073005
	rdf:type skos:Concept;
	skos:prefLabel	"Commonwealth Games"@en-GB;
	skos:definition	"Commonwealth Games "@en-GB;
	skos:inScheme <http://cv.iptc.org/newscodes/subjectcode/>;
	skos:broadMatch medtop:20001108;
	skos:broader	subj:15073000.

subj:15073006
	rdf:type skos:Concept;
	skos:prefLabel	"Winter Goodwill Games"@en-GB;
	skos:definition	"Winter Goodwill Games "@en-GB;
	skos:inScheme <http://cv.iptc.org/newscodes/subjectcode/>;
	skos:broadMatch medtop:20001108;
	skos:broader	subj:15073000.

subj:15073007
	rdf:type skos:Concept;
	skos:prefLabel	"Summer Asian Games"@en-GB;
	skos:definition	"Summer Asian Games "@en-GB;
	skos:inScheme <http://cv.iptc.org/newscodes/subjectcode/>;
	skos:broadMatch medtop:20001108;
	skos:broader	subj:15073000.

subj:15073008
	rdf:type skos:Concept;
	skos:prefLabel	"Winter Asian Games"@en-GB;
	skos:definition	"Winter Asian Games "@en-GB;
	skos:inScheme <http://cv.iptc.org/newscodes/subjectcode/>;
	skos:broadMatch medtop:20001108;
	skos:broader	subj:15073000.

subj:15073009
	rdf:type skos:Concept;
	skos:prefLabel	"Panamerican Games"@en-GB;
	skos:definition	"Panamerican Games "@en-GB;
	skos:inScheme <http://cv.iptc.org/newscodes/subjectcode/>;
	skos:broadMatch medtop:20001108;
	skos:broader	subj:15073000.

subj:15073010
	rdf:type skos:Concept;
	skos:prefLabel	"African Games"@en-GB;
	skos:definition	"African Games "@en-GB;
	skos:inScheme <http://cv.iptc.org/newscodes/subjectcode/>;
	skos:broadMatch medtop:20001108;
	skos:broader	subj:15073000.

subj:15073011
	rdf:type skos:Concept;
	skos:prefLabel	"Mediterranean Games"@en-GB;
	skos:definition	"Mediterranean Games "@en-GB;
	skos:inScheme <http://cv.iptc.org/newscodes/subjectcode/>;
	skos:broadMatch medtop:20001108;
	skos:broader	subj:15073000.

subj:15073012
	rdf:type skos:Concept;
	skos:prefLabel	"SouthEast Asiatic Games"@en-GB;
	skos:definition	"SouthEast Asiatic Games "@en-GB;
	skos:inScheme <http://cv.iptc.org/newscodes/subjectcode/>;
	skos:broadMatch medtop:20001108;
	skos:broader	subj:15073000.

subj:15073013
	rdf:type skos:Concept;
	skos:prefLabel	"PanPacific Games"@en-GB;
	skos:definition	"PanPacific Games "@en-GB;
	skos:inScheme <http://cv.iptc.org/newscodes/subjectcode/>;
	skos:broadMatch medtop:20001108;
	skos:broader	subj:15073000.

subj:15073014
	rdf:type skos:Concept;
	skos:prefLabel	"SouthPacific Games"@en-GB;
	skos:definition	"SouthPacific Games "@en-GB;
	skos:inScheme <http://cv.iptc.org/newscodes/subjectcode/>;
	skos:broadMatch medtop:20001108;
	skos:broader	subj:15073000.

subj:15073015
	rdf:type skos:Concept;
	skos:prefLabel	"PanArabic Games"@en-GB;
	skos:definition	"PanArabic Games "@en-GB;
	skos:inScheme <http://cv.iptc.org/newscodes/subjectcode/>;
	skos:broadMatch medtop:20001108;
	skos:broader	subj:15073000.

subj:15073016
	rdf:type skos:Concept;
	skos:prefLabel	"Summer Goodwill Games"@en-GB;
	skos:definition	"Summer Goodwill Games "@en-GB;
	skos:inScheme <http://cv.iptc.org/newscodes/subjectcode/>;
	skos:broadMatch medtop:20001108;
	skos:broader	subj:15073000.

subj:15073017
	rdf:type skos:Concept;
	skos:prefLabel	"World games"@en-GB;
	skos:definition	"A competition featuring world class athletes "@en-GB;
	skos:inScheme <http://cv.iptc.org/newscodes/subjectcode/>;
	skos:exactMatch medtop:20001123;
	skos:broader	subj:15073000.

subj:15073018
	rdf:type skos:Concept;
	skos:prefLabel	"World Cup"@en-GB;
	skos:definition	"Sports meeting with competitors from the five continents "@en-GB;
	skos:inScheme <http://cv.iptc.org/newscodes/subjectcode/>;
	skos:exactMatch medtop:20001122;
	skos:broader	subj:15073000.

subj:15073019
	rdf:type skos:Concept;
	skos:prefLabel	"intercontinental cup"@en-GB;
	skos:definition	"Sports meeting bringing together competitors from different continents "@en-GB;
	skos:historyNote	"typo fixed in Explanation "@en-GB;
	skos:inScheme <http://cv.iptc.org/newscodes/subjectcode/>;
	skos:broadMatch medtop:20001108;
	skos:broader	subj:15073000.

subj:15073020
	rdf:type skos:Concept;
	skos:prefLabel	"continental cup"@en-GB;
	skos:definition	"Sports meeting where competitors come from a single continent "@en-GB;
	skos:inScheme <http://cv.iptc.org/newscodes/subjectcode/>;
	skos:exactMatch medtop:20001110;
	skos:broader	subj:15073000.

subj:15073021
	rdf:type skos:Concept;
	skos:prefLabel	"international cup"@en-GB;
	skos:definition	"Sports meeting where competitors come from several nations "@en-GB;
	skos:inScheme <http://cv.iptc.org/newscodes/subjectcode/>;
	skos:exactMatch medtop:20001113;
	skos:broader	subj:15073000.

subj:15073022
	rdf:type skos:Concept;
	skos:prefLabel	"National Cup"@en-GB;
	skos:definition	"Sports meeting where competitors come from a single nation "@en-GB;
	skos:inScheme <http://cv.iptc.org/newscodes/subjectcode/>;
	skos:exactMatch medtop:20001116;
	skos:broader	subj:15073000.

subj:15073023
	rdf:type skos:Concept;
	skos:prefLabel	"interregional cup"@en-GB;
	skos:definition	"Sports meeting where competitors come from several regions "@en-GB;
	skos:inScheme <http://cv.iptc.org/newscodes/subjectcode/>;
	skos:broadMatch medtop:20001108;
	skos:broader	subj:15073000.

subj:15073024
	rdf:type skos:Concept;
	skos:prefLabel	"regional cup"@en-GB;
	skos:definition	"Sports meeting where competitors come from a single region "@en-GB;
	skos:inScheme <http://cv.iptc.org/newscodes/subjectcode/>;
	skos:exactMatch medtop:20001119;
	skos:broader	subj:15073000.

subj:15073025
	rdf:type skos:Concept;
	skos:prefLabel	"league cup"@en-GB;
	skos:definition	"A competition within a sports league "@en-GB;
	skos:inScheme <http://cv.iptc.org/newscodes/subjectcode/>;
	skos:broadMatch medtop:20001108;
	skos:broader	subj:15073000.

subj:15073026
	rdf:type skos:Concept;
	skos:prefLabel	"world championship"@en-GB;
	skos:definition	"A championship where competitors from the five continents take part "@en-GB;
	skos:inScheme <http://cv.iptc.org/newscodes/subjectcode/>;
	skos:exactMatch medtop:20001121;
	skos:broader	subj:15073000.

subj:15073027
	rdf:type skos:Concept;
	skos:prefLabel	"intercontinental championship"@en-GB;
	skos:definition	"A championship where competitors from the different continents take part "@en-GB;
	skos:inScheme <http://cv.iptc.org/newscodes/subjectcode/>;
	skos:broadMatch medtop:20001108;
	skos:broader	subj:15073000.

subj:15073028
	rdf:type skos:Concept;
	skos:prefLabel	"continental championship 1st level"@en-GB;
	skos:definition	"A championship where top level competitors from a single continent take part "@en-GB;
	skos:inScheme <http://cv.iptc.org/newscodes/subjectcode/>;
	skos:broadMatch medtop:20001109;
	skos:broader	subj:15073000.

subj:15073029
	rdf:type skos:Concept;
	skos:prefLabel	"continental championship 2nd level"@en-GB;
	skos:definition	"A championship where second string competitors from a single continent take part "@en-GB;
	skos:inScheme <http://cv.iptc.org/newscodes/subjectcode/>;
	skos:broadMatch medtop:20001109;
	skos:broader	subj:15073000.

subj:15073030
	rdf:type skos:Concept;
	skos:prefLabel	"continental championship 3rd level"@en-GB;
	skos:definition	"A championship where third string competitors from a single continent take part "@en-GB;
	skos:inScheme <http://cv.iptc.org/newscodes/subjectcode/>;
	skos:broadMatch medtop:20001109;
	skos:broader	subj:15073000.

subj:15073031
	rdf:type skos:Concept;
	skos:prefLabel	"national championship 1st level"@en-GB;
	skos:definition	"A championship where top level competitors from a single nation take part "@en-GB;
	skos:inScheme <http://cv.iptc.org/newscodes/subjectcode/>;
	skos:broadMatch medtop:20001115;
	skos:broader	subj:15073000.

subj:15073032
	rdf:type skos:Concept;
	skos:prefLabel	"national championship 2nd level"@en-GB;
	skos:definition	"A championship where second string competitors from a single continent take part "@en-GB;
	skos:inScheme <http://cv.iptc.org/newscodes/subjectcode/>;
	skos:broadMatch medtop:20001115;
	skos:broader	subj:15073000.

subj:15073033
	rdf:type skos:Concept;
	skos:prefLabel	"national championship3rdlevel"@en-GB;
	skos:definition	"A championship where third string competitors from a single continent take part "@en-GB;
	skos:inScheme <http://cv.iptc.org/newscodes/subjectcode/>;
	skos:broadMatch medtop:20001115;
	skos:broader	subj:15073000.

subj:15073034
	rdf:type skos:Concept;
	skos:prefLabel	"national championship 4th level"@en-GB;
	skos:definition	"A championship where fourth string competitors from a single continent take part "@en-GB;
	skos:inScheme <http://cv.iptc.org/newscodes/subjectcode/>;
	skos:broadMatch medtop:20001115;
	skos:broader	subj:15073000.

subj:15073035
	rdf:type skos:Concept;
	skos:prefLabel	"regional championship"@en-GB;
	skos:definition	"A championship where competitors from a single region take part "@en-GB;
	skos:inScheme <http://cv.iptc.org/newscodes/subjectcode/>;
	skos:exactMatch medtop:20001118;
	skos:broader	subj:15073000.

subj:15073036
	rdf:type skos:Concept;
	skos:prefLabel	"Grand Prix"@en-GB;
	skos:definition	"High level sports competition, most often motor racing "@en-GB;
	skos:inScheme <http://cv.iptc.org/newscodes/subjectcode/>;
	skos:broadMatch medtop:20001108;
	skos:broader	subj:15073000.

subj:15073037
	rdf:type skos:Concept;
	skos:prefLabel	"intercontinental tournament"@en-GB;
	skos:definition	"Tournament where competitors from several continents take part "@en-GB;
	skos:inScheme <http://cv.iptc.org/newscodes/subjectcode/>;
	skos:broadMatch medtop:20001108;
	skos:broader	subj:15073000.

subj:15073038
	rdf:type skos:Concept;
	skos:prefLabel	"continental tournament"@en-GB;
	skos:definition	"Tournament where competitors from a single continent take part "@en-GB;
	skos:inScheme <http://cv.iptc.org/newscodes/subjectcode/>;
	skos:broadMatch medtop:20001108;
	skos:broader	subj:15073000.

subj:15073039
	rdf:type skos:Concept;
	skos:prefLabel	"international tournament"@en-GB;
	skos:definition	"Tournament where competitors from several nations take part "@en-GB;
	skos:inScheme <http://cv.iptc.org/newscodes/subjectcode/>;
	skos:broadMatch medtop:20001108;
	skos:broader	subj:15073000.

subj:15073040
	rdf:type skos:Concept;
	skos:prefLabel	"national tournament"@en-GB;
	skos:definition	"Tournament where competitors from a single nation take part "@en-GB;
	skos:inScheme <http://cv.iptc.org/newscodes/subjectcode/>;
	skos:broadMatch medtop:20001108;
	skos:broader	subj:15073000.

subj:15073041
	rdf:type skos:Concept;
	skos:prefLabel	"inter-nations competition"@en-GB;
	skos:definition	"Tournament where athletes from several nations take part "@en-GB;
	skos:inScheme <http://cv.iptc.org/newscodes/subjectcode/>;
	skos:broadMatch medtop:20001108;
	skos:broader	subj:15073000.

subj:15073042
	rdf:type skos:Concept;
	skos:prefLabel	"inter-clubs competition"@en-GB;
	skos:definition	"Tournament where competitors from several clubs take part "@en-GB;
	skos:inScheme <http://cv.iptc.org/newscodes/subjectcode/>;
	skos:broadMatch medtop:20001108;
	skos:broader	subj:15073000.

subj:15073043
	rdf:type skos:Concept;
	skos:prefLabel	"friendly competition"@en-GB;
	skos:definition	"Sports played but not in a tournament "@en-GB;
	skos:inScheme <http://cv.iptc.org/newscodes/subjectcode/>;
	skos:broadMatch medtop:20001108;
	skos:broader	subj:15073000.

subj:15073044
	rdf:type skos:Concept;
	skos:prefLabel	"all-stars competition"@en-GB;
	skos:definition	"Competition between teams made up of invited stars "@en-GB;
	skos:inScheme <http://cv.iptc.org/newscodes/subjectcode/>;
	skos:broadMatch medtop:20001108;
	skos:broader	subj:15073000.

subj:15073045
	rdf:type skos:Concept;
	skos:prefLabel	"exhibition"@en-GB;
	skos:definition	"demonstration "@en-GB;
	skos:inScheme <http://cv.iptc.org/newscodes/subjectcode/>;
	skos:broadMatch medtop:20001108;
	skos:broader	subj:15073000.

subj:15073046
	rdf:type skos:Concept;
	skos:prefLabel	"Super Bowl"@en-GB;
	skos:definition	"The American football final that determines the champion "@en-GB;
	skos:inScheme <http://cv.iptc.org/newscodes/subjectcode/>;
	skos:broadMatch medtop:20001108;
	skos:broader	subj:15073000.

subj:15073047
	rdf:type skos:Concept;
	skos:prefLabel	"paralympic games"@en-GB;
	skos:definition	"Olympic style Games for athletes with a disability "@en-GB;
	skos:inScheme <http://cv.iptc.org/newscodes/subjectcode/>;
	skos:broadMatch medtop:20001108;
	skos:broader	subj:15073000.

subj:15074000
	rdf:type skos:Concept;
	skos:prefLabel	"rodeo"@en-GB;
	skos:definition	"A discipline where wild horses or bulls must be mounted and mastered "@en-GB;
	skos:inScheme <http://cv.iptc.org/newscodes/subjectcode/>;
	skos:exactMatch medtop:20001017;
	skos:broader	subj:15000000;
	skos:narrower	subj:15074001;
	skos:narrower	subj:15074002;
	skos:narrower	subj:15074003;
	skos:narrower	subj:15074004;
	skos:narrower	subj:15074005;
	skos:narrower	subj:15074006;
	skos:narrower	subj:15074007.

subj:15074001
	rdf:type skos:Concept;
	skos:prefLabel	"barrel racing"@en-GB;
	skos:definition	"Rodeo discipline "@en-GB;
	skos:inScheme <http://cv.iptc.org/newscodes/subjectcode/>;
	skos:exactMatch medtop:20001019;
	skos:broader	subj:15074000.

subj:15074002
	rdf:type skos:Concept;
	skos:prefLabel	"calf roping"@en-GB;
	skos:definition	"Rodeo discipline "@en-GB;
	skos:inScheme <http://cv.iptc.org/newscodes/subjectcode/>;
	skos:exactMatch medtop:20001022;
	skos:broader	subj:15074000.

subj:15074003
	rdf:type skos:Concept;
	skos:prefLabel	"bull riding"@en-GB;
	skos:definition	"Rodeo discipline "@en-GB;
	skos:inScheme <http://cv.iptc.org/newscodes/subjectcode/>;
	skos:exactMatch medtop:20001020;
	skos:broader	subj:15074000.

subj:15074004
	rdf:type skos:Concept;
	skos:prefLabel	"bulldogging"@en-GB;
	skos:definition	"Rodeo discipline "@en-GB;
	skos:inScheme <http://cv.iptc.org/newscodes/subjectcode/>;
	skos:exactMatch medtop:20001021;
	skos:broader	subj:15074000.

subj:15074005
	rdf:type skos:Concept;
	skos:prefLabel	"saddle bronc"@en-GB;
	skos:definition	"Rodeo discipline "@en-GB;
	skos:inScheme <http://cv.iptc.org/newscodes/subjectcode/>;
	skos:exactMatch medtop:20001024;
	skos:broader	subj:15074000.

subj:15074006
	rdf:type skos:Concept;
	skos:prefLabel	"bareback"@en-GB;
	skos:definition	"Rodeo discipline "@en-GB;
	skos:inScheme <http://cv.iptc.org/newscodes/subjectcode/>;
	skos:exactMatch medtop:20001018;
	skos:broader	subj:15074000.

subj:15074007
	rdf:type skos:Concept;
	skos:prefLabel	"goat roping"@en-GB;
	skos:definition	"Rodeo discipline "@en-GB;
	skos:inScheme <http://cv.iptc.org/newscodes/subjectcode/>;
	skos:exactMatch medtop:20001023;
	skos:broader	subj:15074000.

subj:15075000
	rdf:type skos:Concept;
	skos:prefLabel	"mini golf sport"@en-GB;
	skos:definition	"A game where balls must be holed on an artificial course in as few strokes from the club as possible "@en-GB;
	skos:inScheme <http://cv.iptc.org/newscodes/subjectcode/>;
	skos:exactMatch medtop:20000941;
	skos:broader	subj:15000000.

subj:15076000
	rdf:type skos:Concept;
	skos:prefLabel	"bandy"@en-GB;
	skos:definition	"Played outdoors on ice. The size of the ice rink is about the size of a soccer field. Skates like ice hockey. A small hard ball is used for playing. Players play with sticks, much like in ice hockey, but the sticks are shorter and more rounded. "@en-GB;
	skos:historyNote	"Explanation shortened "@en-GB;
	skos:inScheme <http://cv.iptc.org/newscodes/subjectcode/>;
	skos:exactMatch medtop:20000848;
	skos:broader	subj:15000000.

subj:15077000
	rdf:type skos:Concept;
	skos:prefLabel	"flying disc"@en-GB;
	skos:definition	"A group of events all played with a flying plastic disc. The exact regulation for the disc is different in different events but it has to be unbroken of solid plastic and a production model with no modification. Flying disc is sometimes called Frisbee. "@en-GB;
	skos:historyNote	"Explanation shortened "@en-GB;
	skos:inScheme <http://cv.iptc.org/newscodes/subjectcode/>;
	skos:exactMatch medtop:20000938;
	skos:broader	subj:15000000;
	skos:narrower	subj:15077001;
	skos:narrower	subj:15077002;
	skos:narrower	subj:15077003;
	skos:narrower	subj:15077004;
	skos:narrower	subj:15077005;
	skos:narrower	subj:15077006;
	skos:narrower	subj:15077007;
	skos:narrower	subj:15077008;
	skos:narrower	subj:15077009;
	skos:narrower	subj:15077010.

subj:15077001
	rdf:type skos:Concept;
	skos:prefLabel	"ultimate"@en-GB;
	skos:definition	"Team game. Played outdoors on soccer-size field with 7 players per team and indoors with 5 players per team. Games are played to a preset number of goals. Goals are scored by passing the disc to a team-member catching it inside the goal area. "@en-GB;
	skos:historyNote	"Explanation shortened "@en-GB;
	skos:inScheme <http://cv.iptc.org/newscodes/subjectcode/>;
	skos:broadMatch medtop:20000938;
	skos:broader	subj:15077000.

subj:15077002
	rdf:type skos:Concept;
	skos:prefLabel	"guts"@en-GB;
	skos:definition	"Team game where two teams of 5 players each face each other. Teams take turns to throw the disc towards the other team. Points are scored if the opposing team does not catch the disc. "@en-GB;
	skos:inScheme <http://cv.iptc.org/newscodes/subjectcode/>;
	skos:broadMatch medtop:20000938;
	skos:broader	subj:15077000.

subj:15077003
	rdf:type skos:Concept;
	skos:prefLabel	"overall"@en-GB;
	skos:definition	"Not an event in itself but in most competitions with individual events the winner of the competition will be awarded to the player with the highest combined score in the events. "@en-GB;
	skos:inScheme <http://cv.iptc.org/newscodes/subjectcode/>;
	skos:broadMatch medtop:20000938;
	skos:broader	subj:15077000.

subj:15077004
	rdf:type skos:Concept;
	skos:prefLabel	"distance"@en-GB;
	skos:definition	"The object is to throw the disc as far as possible. Each player get five throws per turn. Throws are made downwind. World record is over 200 meters. "@en-GB;
	skos:inScheme <http://cv.iptc.org/newscodes/subjectcode/>;
	skos:broadMatch medtop:20000938;
	skos:broader	subj:15077000.

subj:15077005
	rdf:type skos:Concept;
	skos:prefLabel	"discathon"@en-GB;
	skos:definition	"The object is to throw and run a park course of about 1 kilometre. Four players compete in each heat. They have two discs each. They may also carry a third disc in reserve. Where one thrown disc stops the second disc must be thrown. "@en-GB;
	skos:historyNote	"Explanation shortened "@en-GB;
	skos:inScheme <http://cv.iptc.org/newscodes/subjectcode/>;
	skos:broadMatch medtop:20000938;
	skos:broader	subj:15077000.

subj:15077006
	rdf:type skos:Concept;
	skos:prefLabel	"DDC"@en-GB;
	skos:definition	"Abbreviation for Double Disc Court. Two players per team in a square 13x13 metre. The teams start with one disc per team and throw at each other. Discs are thrown back and forth until one or both hit the ground. "@en-GB;
	skos:historyNote	"Explanation shortened "@en-GB;
	skos:inScheme <http://cv.iptc.org/newscodes/subjectcode/>;
	skos:broadMatch medtop:20000938;
	skos:broader	subj:15077000.

subj:15077007
	rdf:type skos:Concept;
	skos:prefLabel	"SCF"@en-GB;
	skos:definition	"Abbreviation for Self Caught Flights. Divided into two sub events called MTA (Maximum Time Aloft) and TRC (Throw Run Catch). In both sub events the player throws a disc and then runs to catch it with one hand before it hits the ground. "@en-GB;
	skos:historyNote	"Explanation shortened "@en-GB;
	skos:inScheme <http://cv.iptc.org/newscodes/subjectcode/>;
	skos:broadMatch medtop:20000938;
	skos:broader	subj:15077000.

subj:15077008
	rdf:type skos:Concept;
	skos:prefLabel	"freestyle"@en-GB;
	skos:definition	"A judged event where groups of two or three players perform as many tricks as possible. In competitions the judges can use either a ranking system or set scores on presentation, execution and difficulty. "@en-GB;
	skos:inScheme <http://cv.iptc.org/newscodes/subjectcode/>;
	skos:broadMatch medtop:20000938;
	skos:broader	subj:15077000.

subj:15077009
	rdf:type skos:Concept;
	skos:prefLabel	"accuracy"@en-GB;
	skos:definition	"Each player has 28 throws from various distances and angles to throw the disc through a goal 1.5 x 1.5 meters. World record is 25 of 28 possible. "@en-GB;
	skos:inScheme <http://cv.iptc.org/newscodes/subjectcode/>;
	skos:broadMatch medtop:20000938;
	skos:broader	subj:15077000.

subj:15077010
	rdf:type skos:Concept;
	skos:prefLabel	"disc golf"@en-GB;
	skos:definition	"Much like golf but played with discs instead of balls and clubs. Instead of a hole in the ground there is a metal basket with light metal chains to throw the disc at. Players often carry discs specialized for long throws, right or left bends. "@en-GB;
	skos:historyNote	"Explanation shortened "@en-GB;
	skos:inScheme <http://cv.iptc.org/newscodes/subjectcode/>;
	skos:broadMatch medtop:20000938;
	skos:broader	subj:15077000.

subj:15078000
	rdf:type skos:Concept;
	skos:prefLabel	"floorball"@en-GB;
	skos:definition	"Played indoors in a court the size of a basketball court. 6 players per team, of which one is a who plays in a kneeling position without a stick like in ice hockey. The other players use plastic clubs and a light plastic ball to pass and shoot goals. "@en-GB;
	skos:historyNote	"Explanation shortened "@en-GB;
	skos:inScheme <http://cv.iptc.org/newscodes/subjectcode/>;
	skos:exactMatch medtop:20000937;
	skos:broader	subj:15000000.

subj:15079000
	rdf:type skos:Concept;
	skos:prefLabel	"casting"@en-GB;
	skos:definition	"Using fishing equipment to hit a target and score points "@en-GB;
	skos:inScheme <http://cv.iptc.org/newscodes/subjectcode/>;
	skos:exactMatch medtop:20000883;
	skos:broader	subj:15000000.

subj:15080000
	rdf:type skos:Concept;
	skos:prefLabel	"tug-of-war"@en-GB;
	skos:definition	"Two teams pulling against each other on a rope "@en-GB;
	skos:inScheme <http://cv.iptc.org/newscodes/subjectcode/>;
	skos:exactMatch medtop:20001088;
	skos:broader	subj:15000000.

subj:15081000
	rdf:type skos:Concept;
	skos:prefLabel	"croquette"@en-GB;
	skos:definition	"Using mallets to hit a ball through hoops "@en-GB;
	skos:inScheme <http://cv.iptc.org/newscodes/subjectcode/>;
	skos:exactMatch medtop:20000889;
	skos:broader	subj:15000000.

subj:15082000
	rdf:type skos:Concept;
	skos:prefLabel	"dog racing"@en-GB;
	skos:definition	"Dogs racing around a track "@en-GB;
	skos:inScheme <http://cv.iptc.org/newscodes/subjectcode/>;
	skos:exactMatch medtop:20000919;
	skos:broader	subj:15000000;
	skos:narrower	subj:15082001;
	skos:narrower	subj:15082002.

subj:15082001
	rdf:type skos:Concept;
	skos:prefLabel	"sled"@en-GB;
	skos:definition	"Harnessed to a sled "@en-GB;
	skos:inScheme <http://cv.iptc.org/newscodes/subjectcode/>;
	skos:exactMatch medtop:20000921;
	skos:broader	subj:15082000.

subj:15082002
	rdf:type skos:Concept;
	skos:prefLabel	"oval track"@en-GB;
	skos:definition	"Pursuing an artificial rabbit around an oval track "@en-GB;
	skos:inScheme <http://cv.iptc.org/newscodes/subjectcode/>;
	skos:exactMatch medtop:20000920;
	skos:broader	subj:15082000.

subj:15083000
	rdf:type skos:Concept;
	skos:prefLabel	"skeleton"@en-GB;
	skos:definition	"In skeleton the competitor lays on his/hers stomach when racing down the course. The competitor must be on the sled when crossing the finishing line. The total time of all races in a competition is added together. "@en-GB;
	skos:historyNote	"Explanation shortened "@en-GB;
	skos:inScheme <http://cv.iptc.org/newscodes/subjectcode/>;
	skos:exactMatch medtop:20001055;
	skos:broader	subj:15000000.

subj:15084000
	rdf:type skos:Concept;
	skos:prefLabel	"Australian rules football"@en-GB;
	skos:definition	"Football played under Australian rules "@en-GB;
	skos:inScheme <http://cv.iptc.org/newscodes/subjectcode/>;
	skos:exactMatch medtop:20000846;
	skos:broader	subj:15000000.

subj:15085000
	rdf:type skos:Concept;
	skos:prefLabel	"Canadian football"@en-GB;
	skos:definition	"Football played under Canadian rules "@en-GB;
	skos:inScheme <http://cv.iptc.org/newscodes/subjectcode/>;
	skos:exactMatch medtop:20000876;
	skos:broader	subj:15000000.

subj:15086000
	rdf:type skos:Concept;
	skos:prefLabel	"duathlon"@en-GB;
	skos:definition	"Duathlon "@en-GB;
	skos:inScheme <http://cv.iptc.org/newscodes/subjectcode/>;
	skos:exactMatch medtop:20000922;
	skos:broader	subj:15000000.

subj:15087000
	rdf:type skos:Concept;
	skos:prefLabel	"hornuss"@en-GB;
	skos:definition	"Swiss team sport with 16 or 18 men per team. A rubber puck is hit towards the field of the adversary team which tries to hit the puck in the air with a wooden board thrown in the air "@en-GB;
	skos:inScheme <http://cv.iptc.org/newscodes/subjectcode/>;
	skos:exactMatch medtop:20000959;
	skos:broader	subj:15000000.

subj:15088000
	rdf:type skos:Concept;
	skos:prefLabel	"fist ball"@en-GB;
	skos:definition	"Men's team sport similar to volleyball (with a much lower net) executed mainly in gymnastics clubs "@en-GB;
	skos:inScheme <http://cv.iptc.org/newscodes/subjectcode/>;
	skos:exactMatch medtop:20000936;
	skos:broader	subj:15000000.

subj:15089000
	rdf:type skos:Concept;
	skos:prefLabel	"inline skating"@en-GB;
	skos:definition	"Competitive sports using inline skates "@en-GB;
	skos:inScheme <http://cv.iptc.org/newscodes/subjectcode/>;
	skos:exactMatch medtop:20000967;
	skos:broader	subj:15000000.

subj:15090000
	rdf:type skos:Concept;
	skos:prefLabel	"grass ski"@en-GB;
	skos:definition	"Alpine skiing on roller skis and grass "@en-GB;
	skos:inScheme <http://cv.iptc.org/newscodes/subjectcode/>;
	skos:exactMatch medtop:20001059;
	skos:broader	subj:15000000.

subj:15091000
	rdf:type skos:Concept;
	skos:prefLabel	"snowbiking"@en-GB;
	skos:definition	"Individual sport on snow on a snow bike, the athlete has two mini skis, previous name: ski bob "@en-GB;
	skos:inScheme <http://cv.iptc.org/newscodes/subjectcode/>;
	skos:broadMatch medtop:20000822;
	skos:broader	subj:15000000.

subj:15092000
	rdf:type skos:Concept;
	skos:prefLabel	"twirling"@en-GB;
	skos:definition	"Team competition with majorettes and a jury "@en-GB;
	skos:inScheme <http://cv.iptc.org/newscodes/subjectcode/>;
	skos:broadMatch medtop:20000822;
	skos:broader	subj:15000000.

subj:15093000
	rdf:type skos:Concept;
	skos:prefLabel	"kendo"@en-GB;
	skos:definition	"Japanese traditional martial art using a bamboo sword, sometimes called Japanese fencing. (Programme of National Sports Festival in Japan) "@en-GB;
	skos:inScheme <http://cv.iptc.org/newscodes/subjectcode/>;
	skos:exactMatch medtop:20000984;
	skos:broader	subj:15000000.

subj:15094000
	rdf:type skos:Concept;
	skos:prefLabel	"jukendo"@en-GB;
	skos:definition	"Japanese traditional martial art using a model rifle made of wood. ´Juken´ means a rifle or gun with blade (bayonet). (Programme of National Sports Festival in Japan) "@en-GB;
	skos:inScheme <http://cv.iptc.org/newscodes/subjectcode/>;
	skos:exactMatch medtop:20000977;
	skos:broader	subj:15000000.

subj:15095000
	rdf:type skos:Concept;
	skos:prefLabel	"naginata"@en-GB;
	skos:definition	"Japanese traditional martial art using a pole sword made of wood. ´Naginata´ means a spear with a curved blade. (Programme of National Sports Festival in Japan) "@en-GB;
	skos:inScheme <http://cv.iptc.org/newscodes/subjectcode/>;
	skos:exactMatch medtop:20001009;
	skos:broader	subj:15000000.

subj:15096000
	rdf:type skos:Concept;
	skos:prefLabel	"kyudo"@en-GB;
	skos:definition	"Japanese traditional martial art using a bamboo bow and arrows, sometimes called Japanese archery. (Programme of National Sports Festival in Japan) "@en-GB;
	skos:inScheme <http://cv.iptc.org/newscodes/subjectcode/>;
	skos:exactMatch medtop:20000985;
	skos:broader	subj:15000000.

subj:15097000
	rdf:type skos:Concept;
	skos:prefLabel	"kabaddi"@en-GB;
	skos:definition	"The attacking side scores by touching, and the side to guard scores by capturing. The attacker continues calling it ´kabaddi´. "@en-GB;
	skos:inScheme <http://cv.iptc.org/newscodes/subjectcode/>;
	skos:exactMatch medtop:20000978;
	skos:broader	subj:15000000.

subj:15098000
	rdf:type skos:Concept;
	skos:prefLabel	"sepak takraw"@en-GB;
	skos:definition	"The game like volleyball which must not use a hand. The ball made of rattan is used. (Programme of National Sports Festival in Japan) "@en-GB;
	skos:inScheme <http://cv.iptc.org/newscodes/subjectcode/>;
	skos:exactMatch medtop:20001047;
	skos:broader	subj:15000000.

subj:15099000
	rdf:type skos:Concept;
	skos:prefLabel	"wushu"@en-GB;
	skos:definition	"Generally, Chinese traditional martial art. (Programme of National Sports Festival in Japan) "@en-GB;
	skos:inScheme <http://cv.iptc.org/newscodes/subjectcode/>;
	skos:exactMatch medtop:20001102;
	skos:broader	subj:15000000.

subj:15100000
	rdf:type skos:Concept;
	skos:prefLabel	"darts"@en-GB;
	skos:definition	"Two players compete by throwing metal darts at a wall-mounted circular board divided radially into segments of different scores "@en-GB;
	skos:inScheme <http://cv.iptc.org/newscodes/subjectcode/>;
	skos:exactMatch medtop:20000912;
	skos:broader	subj:15000000.

subj:15101000
	rdf:type skos:Concept;
	skos:prefLabel	"bodybuilding"@en-GB;
	skos:definition	"A person displays pronounced muscle tone and exaggerated muscle mass and definition for overall aesthetic effect "@en-GB;
	skos:inScheme <http://cv.iptc.org/newscodes/subjectcode/>;
	skos:broadMatch medtop:20000822;
	skos:broader	subj:15000000.

subj:15102000
	rdf:type skos:Concept;
	skos:prefLabel	"sports disciplinary action"@en-GB;
	skos:definition	"Actions, including fines and suspensions levied by sports organisations and teams "@en-GB;
	skos:inScheme <http://cv.iptc.org/newscodes/subjectcode/>;
	skos:exactMatch medtop:20001103;
	skos:broader	subj:15000000.

subj:15103000
	rdf:type skos:Concept;
	skos:prefLabel	"sports awards"@en-GB;
	skos:definition	"Awards and honors given by sports organisations or won by sports figures "@en-GB;
	skos:inScheme <http://cv.iptc.org/newscodes/subjectcode/>;
	skos:broadMatch medtop:15000000;
	skos:broader	subj:15000000.

subj:16000000
	rdf:type skos:Concept;
	skos:prefLabel	"unrest, conflicts and war"@en-GB;
	skos:definition	"Acts of socially or politically motivated protest and/or violence. "@en-GB;
	skos:inScheme <http://cv.iptc.org/newscodes/subjectcode/>;
	skos:closeMatch medtop:16000000;
	skos:narrower	subj:16001000;
	skos:narrower	subj:16002000;
	skos:narrower	subj:16003000;
	skos:narrower	subj:16004000;
	skos:narrower	subj:16005000;
	skos:narrower	subj:16006000;
	skos:narrower	subj:16007000;
	skos:narrower	subj:16008000;
	skos:narrower	subj:16009000;
	skos:narrower	subj:16010000;
	skos:narrower	subj:16011000;
	skos:narrower	subj:16012000.

subj:16001000
	rdf:type skos:Concept;
	skos:prefLabel	"act of terror"@en-GB;
	skos:definition	"Act of violence, often deadly, designed to raise fear and anxiety in a population "@en-GB;
	skos:inScheme <http://cv.iptc.org/newscodes/subjectcode/>;
	skos:exactMatch medtop:20000053;
	skos:broader	subj:16000000.

subj:16002000
	rdf:type skos:Concept;
	skos:prefLabel	"armed conflict"@en-GB;
	skos:definition	"Disputes between opposing groups involving the use of weaponry, but not formally declared a war "@en-GB;
	skos:inScheme <http://cv.iptc.org/newscodes/subjectcode/>;
	skos:exactMatch medtop:20000056;
	skos:broader	subj:16000000.

subj:16003000
	rdf:type skos:Concept;
	skos:prefLabel	"civil unrest"@en-GB;
	skos:definition	"Dissatisfaction among the general population as evidenced by rallies, strikes, demonstrations or sabotage "@en-GB;
	skos:inScheme <http://cv.iptc.org/newscodes/subjectcode/>;
	skos:exactMatch medtop:20000065;
	skos:broader	subj:16000000;
	skos:narrower	subj:16003001;
	skos:narrower	subj:16003002;
	skos:narrower	subj:16003003;
	skos:narrower	subj:16003004;
	skos:narrower	subj:16003005.

subj:16003001
	rdf:type skos:Concept;
	skos:prefLabel	"revolutions"@en-GB;
	skos:definition	"An often violent change in a nation's system of government by internal forces that results in systematic social change. "@en-GB;
	skos:inScheme <http://cv.iptc.org/newscodes/subjectcode/>;
	skos:exactMatch medtop:20000068;
	skos:broader	subj:16003000.

subj:16003002
	rdf:type skos:Concept;
	skos:prefLabel	"rebellions"@en-GB;
	skos:definition	"Armed uprising by citizens of a nation with the intent to overthrow the government, without necessarily achieving social change "@en-GB;
	skos:inScheme <http://cv.iptc.org/newscodes/subjectcode/>;
	skos:exactMatch medtop:20000067;
	skos:broader	subj:16003000.

subj:16003003
	rdf:type skos:Concept;
	skos:prefLabel	"political dissent"@en-GB;
	skos:definition	"Disagreement between political groups, usually organized and sometimes resulting in imprisonment of the dissenters "@en-GB;
	skos:inScheme <http://cv.iptc.org/newscodes/subjectcode/>;
	skos:exactMatch medtop:20000648;
	skos:broader	subj:16003000.

subj:16003004
	rdf:type skos:Concept;
	skos:prefLabel	"religious conflict"@en-GB;
	skos:definition	"Conflicts involving religious differences "@en-GB;
	skos:inScheme <http://cv.iptc.org/newscodes/subjectcode/>;
	skos:exactMatch medtop:20000688;
	skos:broader	subj:16003000.

subj:16003005
	rdf:type skos:Concept;
	skos:prefLabel	"social conflict"@en-GB;
	skos:definition	"Conflicts involving social differences "@en-GB;
	skos:inScheme <http://cv.iptc.org/newscodes/subjectcode/>;
	skos:broadMatch medtop:16000000;
	skos:broader	subj:16003000.

subj:16004000
	rdf:type skos:Concept;
	skos:prefLabel	"coup d'etat"@en-GB;
	skos:definition	"The overthrow of an established government by an organized group, often the military or a political party "@en-GB;
	skos:inScheme <http://cv.iptc.org/newscodes/subjectcode/>;
	skos:exactMatch medtop:20000070;
	skos:broader	subj:16000000.

subj:16005000
	rdf:type skos:Concept;
	skos:prefLabel	"guerrilla activity"@en-GB;
	skos:definition	"Anti-government actions by clandestine groups using hit-and-run techniques or sabotage, kidnapping and the like "@en-GB;
	skos:inScheme <http://cv.iptc.org/newscodes/subjectcode/>;
	skos:exactMatch medtop:20000057;
	skos:broader	subj:16000000;
	skos:narrower	subj:16005001;
	skos:narrower	subj:16005002.

subj:16005001
	rdf:type skos:Concept;
	skos:prefLabel	"bioterrorism"@en-GB;
	skos:definition	"Use of biological agent to raise the level of fear within a population, whether deaths occur or not. "@en-GB;
	skos:inScheme <http://cv.iptc.org/newscodes/subjectcode/>;
	skos:exactMatch medtop:20000054;
	skos:broader	subj:16005000.

subj:16005002
	rdf:type skos:Concept;
	skos:prefLabel	"bombings"@en-GB;
	skos:definition	"Use of explosive devices against people, buildings or structures "@en-GB;
	skos:inScheme <http://cv.iptc.org/newscodes/subjectcode/>;
	skos:exactMatch medtop:20000055;
	skos:broader	subj:16005000.

subj:16006000
	rdf:type skos:Concept;
	skos:prefLabel	"massacre"@en-GB;
	skos:definition	"The death of a large group of people over a brief period of time "@en-GB;
	skos:inScheme <http://cv.iptc.org/newscodes/subjectcode/>;
	skos:exactMatch medtop:20000071;
	skos:broader	subj:16000000;
	skos:narrower	subj:16006001.

subj:16006001
	rdf:type skos:Concept;
	skos:prefLabel	"genocide"@en-GB;
	skos:definition	"Systematic killing of one clan, tribe or ethnic type by another "@en-GB;
	skos:inScheme <http://cv.iptc.org/newscodes/subjectcode/>;
	skos:exactMatch medtop:20000072;
	skos:broader	subj:16006000.

subj:16007000
	rdf:type skos:Concept;
	skos:prefLabel	"riots"@en-GB;
	skos:definition	"Violent, destructive demonstrations often involving injury to individuals and destruction of property "@en-GB;
	skos:inScheme <http://cv.iptc.org/newscodes/subjectcode/>;
	skos:exactMatch medtop:20000069;
	skos:broader	subj:16000000.

subj:16008000
	rdf:type skos:Concept;
	skos:prefLabel	"demonstration"@en-GB;
	skos:definition	"A public show of feeling or opinion, as by a mass meeting or parade "@en-GB;
	skos:historyNote	"name changed from: violent demonstration "@en-GB;
	skos:inScheme <http://cv.iptc.org/newscodes/subjectcode/>;
	skos:exactMatch medtop:20000066;
	skos:broader	subj:16000000.

subj:16009000
	rdf:type skos:Concept;
	skos:prefLabel	"war"@en-GB;
	skos:definition	"A formal declaration of hostilities by one country against another "@en-GB;
	skos:inScheme <http://cv.iptc.org/newscodes/subjectcode/>;
	skos:exactMatch medtop:20000062;
	skos:broader	subj:16000000;
	skos:narrower	subj:16009001;
	skos:narrower	subj:16009002;
	skos:narrower	subj:16009003.

subj:16009001
	rdf:type skos:Concept;
	skos:prefLabel	"civil war"@en-GB;
	skos:definition	"Armed conflict between members of the same nation or geographical region, in some cases with a desire to divide the nation or region. "@en-GB;
	skos:inScheme <http://cv.iptc.org/newscodes/subjectcode/>;
	skos:exactMatch medtop:20000063;
	skos:broader	subj:16009000.

subj:16009002
	rdf:type skos:Concept;
	skos:prefLabel	"international military intervention"@en-GB;
	skos:definition	"Temporary use of international forces by invitation or by a decision of an outside body in another country or region for the purpose of resolving a crisis. "@en-GB;
	skos:inScheme <http://cv.iptc.org/newscodes/subjectcode/>;
	skos:exactMatch medtop:20000058;
	skos:broader	subj:16009000.

subj:16009003
	rdf:type skos:Concept;
	skos:prefLabel	"prisoners and detainees"@en-GB;
	skos:definition	"People captured and imprisoned by their enemy during war or armed conflict "@en-GB;
	skos:inScheme <http://cv.iptc.org/newscodes/subjectcode/>;
	skos:exactMatch medtop:20000080;
	skos:broader	subj:16009000.

subj:16010000
	rdf:type skos:Concept;
	skos:prefLabel	"conflict (general)"@en-GB;
	skos:definition	"A dispute which can be at several levels, "@en-GB;
	skos:inScheme <http://cv.iptc.org/newscodes/subjectcode/>;
	skos:broadMatch medtop:16000000;
	skos:broader	subj:16000000;
	skos:narrower	subj:16010001.

subj:16010001
	rdf:type skos:Concept;
	skos:prefLabel	"peacekeeping force"@en-GB;
	skos:definition	"Varied national military forces under unified international command to maintain order in disputed areas. "@en-GB;
	skos:inScheme <http://cv.iptc.org/newscodes/subjectcode/>;
	skos:exactMatch medtop:20000059;
	skos:broader	subj:16010000.

subj:16011000
	rdf:type skos:Concept;
	skos:prefLabel	"crisis"@en-GB;
	skos:definition	"Conflict of all kinds that rises to a level where, depending on events, governments can fall, war be declared or stock markets crash, or not "@en-GB;
	skos:inScheme <http://cv.iptc.org/newscodes/subjectcode/>;
	skos:closeMatch medtop:20000647;
	skos:broader	subj:16000000.

subj:16012000
	rdf:type skos:Concept;
	skos:prefLabel	"weaponry"@en-GB;
	skos:definition	"Armaments of all types used to conduct war "@en-GB;
	skos:inScheme <http://cv.iptc.org/newscodes/subjectcode/>;
	skos:exactMatch medtop:20000602;
	skos:broader	subj:16000000.

subj:17000000
	rdf:type skos:Concept;
	skos:prefLabel	"weather"@en-GB;
	skos:definition	"The study, reporting and prediction of meteorological phenomena. "@en-GB;
	skos:inScheme <http://cv.iptc.org/newscodes/subjectcode/>;
	skos:exactMatch medtop:17000000;
	skos:narrower	subj:17001000;
	skos:narrower	subj:17002000;
	skos:narrower	subj:17003000;
	skos:narrower	subj:17004000;
	skos:narrower	subj:17005000.

subj:17001000
	rdf:type skos:Concept;
	skos:prefLabel	"forecast"@en-GB;
	skos:definition	"Prediction of the course of the weather in the future either near term or long term "@en-GB;
	skos:inScheme <http://cv.iptc.org/newscodes/subjectcode/>;
	skos:exactMatch medtop:20001128;
	skos:broader	subj:17000000.

subj:17002000
	rdf:type skos:Concept;
	skos:prefLabel	"global change"@en-GB;
	skos:definition	"The determination whether the Earth is getting warm, or colder, whether seas are rising or falling and the like "@en-GB;
	skos:inScheme <http://cv.iptc.org/newscodes/subjectcode/>;
	skos:exactMatch medtop:20000418;
	skos:broader	subj:17000000.

subj:17003000
	rdf:type skos:Concept;
	skos:prefLabel	"report"@en-GB;
	skos:definition	"Any distributed announcement about the weather "@en-GB;
	skos:inScheme <http://cv.iptc.org/newscodes/subjectcode/>;
	skos:broadMatch medtop:17000000;
	skos:broader	subj:17000000;
	skos:narrower	subj:17003001.

subj:17003001
	rdf:type skos:Concept;
	skos:prefLabel	"weather news"@en-GB;
	skos:definition	"General information about weather events "@en-GB;
	skos:inScheme <http://cv.iptc.org/newscodes/subjectcode/>;
	skos:broadMatch medtop:17000000;
	skos:broader	subj:17003000.

subj:17004000
	rdf:type skos:Concept;
	skos:prefLabel	"statistic"@en-GB;
	skos:definition	"Numerical facts about the weather such as temperature, barometric pressure, river levels, humidity, high and low tides and the like "@en-GB;
	skos:inScheme <http://cv.iptc.org/newscodes/subjectcode/>;
	skos:exactMatch medtop:20001130;
	skos:broader	subj:17000000.

subj:17005000
	rdf:type skos:Concept;
	skos:prefLabel	"warning"@en-GB;
	skos:definition	"Alerts to the general populace about severe weather coming their way "@en-GB;
	skos:inScheme <http://cv.iptc.org/newscodes/subjectcode/>;
	skos:exactMatch medtop:20001131;
	skos:broader	subj:17000000.
