@prefix rdf:   <http://www.w3.org/1999/02/22-rdf-syntax-ns#> .
@prefix owl:   <http://www.w3.org/2002/07/owl#> .
@prefix xsd:   <http://www.w3.org/2001/XMLSchema#> .
@prefix rdfs:  <http://www.w3.org/2000/01/rdf-schema#> .
@prefix wot:   <http://xmlns.com/wot/0.1/> .
@prefix vs:    <http://www.w3.org/2003/06/sw-vocab-status/ns#> .
@prefix foaf:  <http://xmlns.com/foaf/0.1/> .
@prefix dc:    <http://purl.org/dc/elements/1.1/> .

foaf:knows  a             owl:ObjectProperty ;
        rdfs:comment      "\nA person known by this person (indicating some level of reciprocated interaction between the parties).\n" ;
        rdfs:domain       foaf:Person ;
        rdfs:isDefinedBy  foaf: ;
        rdfs:label        "knows" ;
        rdfs:range        foaf:Person ;
        vs:term_status    "testing" .

foaf:firstName  a         owl:DatatypeProperty ;
        rdfs:comment      "The first name of a person." ;
        rdfs:domain       foaf:Person ;
        rdfs:isDefinedBy  foaf: ;
        rdfs:label        "firstName" ;
        rdfs:range        rdfs:Literal ;
        vs:term_status    "testing" .

foaf:icqChatID  a           owl:InverseFunctionalProperty , owl:DatatypeProperty ;
        rdfs:comment        "An ICQ chat ID" ;
        rdfs:domain         foaf:Agent ;
        rdfs:isDefinedBy    foaf: ;
        rdfs:label          "ICQ chat ID" ;
        rdfs:range          rdfs:Literal ;
        rdfs:subPropertyOf  foaf:nick ;
        vs:term_status      "testing" .

foaf:birthday  a          owl:FunctionalProperty , owl:DatatypeProperty ;
        rdfs:comment      "\nThe birthday of this Agent, represented in mm-dd string form, eg. '12-31'.\n" ;
        rdfs:domain       foaf:Agent ;
        rdfs:isDefinedBy  foaf: ;
        rdfs:label        "birthday" ;
        rdfs:range        xsd:date ;
        vs:term_status    "unstable" .

foaf:givenname  a         owl:DatatypeProperty ;
        rdfs:comment      "The given name of some person." ;
        rdfs:isDefinedBy  foaf: ;
        rdfs:label        "Given name" ;
        vs:term_status    "testing" .

foaf:accountServiceHomepage
        a                 owl:ObjectProperty ;
        rdfs:comment      "\nIndicates a homepage of the service provide for this online account.\n" ;
        rdfs:domain       foaf:OnlineAccount ;
        rdfs:isDefinedBy  foaf: ;
        rdfs:label        "account service homepage" ;
        rdfs:range        foaffoafiaf- ;
        vs:term_status    "unstable" .

foaf:isPrimaryTopicOf
        a                   owl:ObjectProperty , owl:InverseFunctionalProperty ;
        rdfs:comment        "\nA document that this thing is the primary topic of.\n" ;
        rdfs:isDefinedBy    foaf: ;
        rdfs:label          "is primary topic of" ;
        rdfs:range          foaffoafiaf- ;
        rdfs:subPropertyOf  foaf:page ;
        owl:inverseOf       foaf:primaryTopic ;
        vs:term_status      "testing" .

foaf:phone  a             owl:ObjectProperty ;
        rdfs:comment      "\nA phone, specified using fully qualified tel: URI scheme (refs: http://www.w3.org/Addressing/schemes.html#tel).\n" ;
        rdfs:isDefinedBy  foaf: ;
        rdfs:label        "phone" ;
        vs:term_status    "testing" .

foaf:openid  a              owl:ObjectProperty , owl:InverseFunctionalProperty ;
        rdfs:comment        "An OpenID for an Agent." ;
        rdfs:domain         foaf:Agent ;
        rdfs:isDefinedBy    foaf: ;
        rdfs:label          "openid" ;
        rdfs:range          foaffoafiaf- ;
        rdfs:subPropertyOf  foaf:isPrimaryTopicOf ;
        vs:term_status      "unstable" .

foaf:depicts  a           owl:ObjectProperty ;
        rdfs:comment      "A thing depicted in this representation." ;
        rdfs:domain       foaf:Image ;
        rdfs:isDefinedBy  foaf: ;
        rdfs:label        "depicts" ;
        owl:inverseOf     foaf:depiction ;
        vs:term_status    "testing" .

foaf:Project  a           owl:Class ;
        rdfs:comment      "A project (a collective endeavour of some kind)." ;
        rdfs:isDefinedBy  foaf: ;
        rdfs:label        "Project" ;
        owl:disjointWith  foaf:Person , foaffoafiaf- ;
        vs:term_status    "unstable" .

foaf:Image  a             owl:Class ;
        rdfs:comment      "An image." ;
        rdfs:isDefinedBy  foaf: ;
        rdfs:label        "Image" ;
        vs:term_status    "testing" .

foaf:page  a              owl:ObjectProperty ;
        rdfs:comment      "A page or document about this thing." ;
        rdfs:isDefinedBy  foaf: ;
        rdfs:label        "page" ;
        rdfs:range        foaffoafiaf- ;
        owl:inverseOf     foaf:topic ;
        vs:term_status    "testing" .

foaf:OnlineEcommerceAccount
        a                 owl:Class ;
        rdfs:comment      "An online e-commerce account." ;
        rdfs:isDefinedBy  foaf: ;
        rdfs:label        "Online E-commerce Account" ;
        rdfs:subClassOf   foaf:OnlineAccount ;
        vs:term_status    "unstable" .

foaf:membershipClass  a   rdf:Property , owl:AnnotationProperty ;
        rdfs:comment      "\nIndicates the class of individuals that are a member of a Group\n" ;
        rdfs:isDefinedBy  foaf: ;
        rdfs:label        "membershipClass" ;
        vs:term_status    "unstable" .

foaf:yahooChatID  a         owl:DatatypeProperty , owl:InverseFunctionalProperty ;
        rdfs:comment        "A Yahoo chat ID" ;
        rdfs:domain         foaf:Agent ;
        rdfs:isDefinedBy    foaf: ;
        rdfs:label          "Yahoo chat ID" ;
        rdfs:range          rdfs:Literal ;
        rdfs:subPropertyOf  foaf:nick ;
        vs:term_status      "testing" .

foaf:homepage  a            owl:ObjectProperty , owl:InverseFunctionalProperty ;
        rdfs:comment        "A homepage for some thing." ;
        rdfs:isDefinedBy    foaf: ;
        rdfs:label          "homepage" ;
        rdfs:range          foaffoafiaf- ;
        rdfs:subPropertyOf  foaf:page , foaf:isPrimaryTopicOf ;
        vs:term_status      "stable" .

wot:assurance  a  owl:AnnotationProperty .

foaf:topic_interest  a    owl:ObjectProperty ;
        rdfs:comment      "A thing of interest to this person." ;
        rdfs:domain       foaf:Person ;
        rdfs:isDefinedBy  foaf: ;
        rdfs:label        "interest_topic" ;
        vs:term_status    "testing" .

foaf:dnaChecksum  a       owl:DatatypeProperty ;
        rdfs:comment      "A checksum for the DNA of some thing. Joke." ;
        rdfs:isDefinedBy  foaf: ;
        rdfs:label        "DNA checksum" ;
        rdfs:range        rdfs:Literal ;
        vs:term_status    "unstable" .

foaf:gender  a            owl:FunctionalProperty , owl:DatatypeProperty ;
        rdfs:comment      "\nThe gender of this Agent (typically but not necessarily 'male' or 'female').\n" ;
        rdfs:domain       foaf:Agent ;
        rdfs:isDefinedBy  foaf: ;
        rdfs:label        "gender" ;
        rdfs:range        [ a          owl:DataRange ;
                            owl:oneOf  ( "male"^^xsd:string "female"^^xsd:string )
                          ] ;
        vs:term_status    "testing" .

foaf:mbox_sha1sum  a      owl:InverseFunctionalProperty , owl:DatatypeProperty ;
        rdfs:comment      "\nThe sha1sum of the URI of an Internet mailbox associated with exactly one owner, the first owner of the mailbox.\n" ;
        rdfs:domain       foaf:Agent ;
        rdfs:isDefinedBy  foaf: ;
        rdfs:label        "sha1sum of a personal mailbox URI name" ;
        rdfs:range        rdfs:Literal ;
        vs:term_status    "testing" .

foaf:logo  a              owl:ObjectProperty ;
        rdfs:comment      "A logo representing some thing." ;
        rdfs:isDefinedBy  foaf: ;
        rdfs:label        "logo" ;
        vs:term_status    "testing" .

dc:description  a  owl:AnnotationProperty .

foaf:img  a                 owl:ObjectProperty ;
        rdfs:comment        "\nAn image that can be used to represent some thing (ie. those depictions which are particularly representative of something, eg. one's photo on a homepage).\n" ;
        rdfs:domain         foaf:Person ;
        rdfs:isDefinedBy    foaf: ;
        rdfs:label          "image" ;
        rdfs:range          foaf:Image ;
        rdfs:subPropertyOf  foaf:depiction ;
        vs:term_status      "testing" .

foaf:fundedBy  a          owl:ObjectProperty ;
        rdfs:comment      "An organization funding a project or person." ;
        rdfs:isDefinedBy  foaf: ;
        rdfs:label        "funded by" ;
        vs:term_status    "unstable" .

foaf:interest  a          owl:ObjectProperty ;
        rdfs:comment      "A page about a topic of interest to this person." ;
        rdfs:domain       foaf:Person ;
        rdfs:isDefinedBy  foaf: ;
        rdfs:label        "interest" ;
        rdfs:range        foaffoafiaf- ;
        vs:term_status    "testing" .

foaf:msnChatID  a           owl:DatatypeProperty , owl:InverseFunctionalProperty ;
        rdfs:comment        "An MSN chat ID" ;
        rdfs:domain         foaf:Agent ;
        rdfs:isDefinedBy    foaf: ;
        rdfs:label          "MSN chat ID" ;
        rdfs:range          rdfs:Literal ;
        rdfs:subPropertyOf  foaf:nick ;
        vs:term_status      "testing" .

foaf:sha1  a              owl:DatatypeProperty ;
        rdfs:comment      "A sha1sum hash, in hex." ;
        rdfs:domain       foaffoafiaf- ;
        rdfs:isDefinedBy  foaf: ;
        rdfs:label        "sha1sum (hex)" ;
        vs:term_status    "unstable" .

foaf:PersonalProfileDocument
        a                owl:Class ;
        rdfs:comment     "A personal profile RDF document." ;
        rdfs:label       "PersonalProfileDocument" ;
        rdfs:subClassOf  foaffoafiaf- ;
        vs:term_status   "testing" .

foaf:workInfoHomepage
        a                 owl:ObjectProperty ;
        rdfs:comment      "\nA work info homepage of some person; a page about their work for some organization.\n" ;
        rdfs:domain       foaf:Person ;
        rdfs:isDefinedBy  foaf: ;
        rdfs:label        "work info homepage" ;
        rdfs:range        foaffoafiaf- ;
        vs:term_status    "testing" .

foaf:currentProject  a    owl:ObjectProperty ;
        rdfs:comment      "A current project this person works on." ;
        rdfs:domain       foaf:Person ;
        rdfs:isDefinedBy  foaf: ;
        rdfs:label        "current project" ;
        vs:term_status    "testing" .

foaf:mbox  a              owl:InverseFunctionalProperty , owl:ObjectProperty ;
        rdfs:comment      "\nA personal mailbox, ie. an Internet mailbox associated with exactly one owner, the first owner of this mailbox. This is a 'static inverse functional property', in that there is (across time and change) at most one individual that ever has any particular value for foaf:mbox.\n" ;
        rdfs:domain       foaf:Agent ;
        rdfs:isDefinedBy  foaf: ;
        rdfs:label        "personal mailbox" ;
        vs:term_status    "stable" .

vs:term_status  a  owl:AnnotationProperty .

foaf:schoolHomepage  a    owl:ObjectProperty ;
        rdfs:comment      "A homepage of a school attended by the person." ;
        rdfs:domain       foaf:Person ;
        rdfs:isDefinedBy  foaf: ;
        rdfs:label        "schoolHomepage" ;
        rdfs:range        foaffoafiaf- ;
        vs:term_status    "testing" .

foaf:   a               owl:Ontology ;
        rdfs:comment    "\nThis is a modified version of the official FOAF specification, optimized for editing tools such as TopBraid. Changes include: - removed { ?p rdf:type rdf:Property } on properties that are also owl:DatatypeProperty etc - removed { ?p rdfs:domain owl:Thing } to prevent these properties from showing up on all forms - removed { ?p rdfs:range owl:Thing } especially for inverse properties for the same reason - removed subclass relationships into external ontologies such as wordnet to keep the class tree flat Edited 2008-02-07 by Holger Knublauch\n" ;
        dc:date         "$Date: 2007-06-16 23:18:26 $" ;
        dc:description  "\nThe Friend of a Friend (FOAF) RDF vocabulary, described using W3C RDF Schema and the Web Ontology Language.\n" ;
        dc:title        "Friend of a Friend (FOAF) vocabulary" ;
        owl:imports     <http://www.topbraidcomposer.org/owl/2006/07/tbcgeo.owl> .

foaf:Organization  a      owl:Class ;
        rdfs:comment      "An organization." ;
        rdfs:isDefinedBy  foaf: ;
        rdfs:label        "Organization" ;
        rdfs:subClassOf   foaf:Agent ;
        owl:disjointWith  foaf:Person , foaffoafiaf- ;
        vs:term_status    "stable" .

foaf:maker  a             owl:ObjectProperty ;
        rdfs:comment      "An agent that made this thing." ;
        rdfs:isDefinedBy  foaf: ;
        rdfs:label        "maker" ;
        rdfs:range        foaf:Agent ;
        owl:inverseOf     foaf:made ;
        vs:term_status    "stable" .

foaf:holdsAccount  a      owl:ObjectProperty ;
        rdfs:comment      "Indicates an account held by this agent." ;
        rdfs:domain       foaf:Agent ;
        rdfs:isDefinedBy  foaf: ;
        rdfs:label        "holds account" ;
        rdfs:range        foaf:OnlineAccount ;
        vs:term_status    "unstable" .

foaf:OnlineChatAccount
        a                 owl:Class ;
        rdfs:comment      "An online chat account." ;
        rdfs:isDefinedBy  foaf: ;
        rdfs:label        "Online Chat Account" ;
        rdfs:subClassOf   foaf:OnlineAccount ;
        vs:term_status    "unstable" .

foaf:jabberID  a          owl:InverseFunctionalProperty , owl:DatatypeProperty ;
        rdfs:comment      "A jabber ID for something." ;
        rdfs:domain       foaf:Agent ;
        rdfs:isDefinedBy  foaf: ;
        rdfs:label        "jabber ID" ;
        rdfs:range        rdfs:Literal ;
        vs:term_status    "testing" .

foaf:pastProject  a       owl:ObjectProperty ;
        rdfs:comment      "A project this person has previously worked on." ;
        rdfs:domain       foaf:Person ;
        rdfs:isDefinedBy  foaf: ;
        rdfs:label        "past project" ;
        vs:term_status    "testing" .

foaf:accountName  a       owl:DatatypeProperty ;
        rdfs:comment      "\nIndicates the name (identifier) associated with this online account.\n" ;
        rdfs:domain       foaf:OnlineAccount ;
        rdfs:isDefinedBy  foaf: ;
        rdfs:label        "account name" ;
        rdfs:range        rdfs:Literal ;
        vs:term_status    "unstable" .

foaf:name  a                rdf:Property , owl:DatatypeProperty ;
        rdfs:comment        "A name for some thing." ;
        rdfs:isDefinedBy    foaf: ;
        rdfs:label          "name" ;
        rdfs:range          rdfs:Literal ;
        rdfs:subPropertyOf  rdfs:label ;
        vs:term_status      "testing" .

foaf:OnlineAccount  a     owl:Class ;
        rdfs:comment      "An online account." ;
        rdfs:isDefinedBy  foaf: ;
        rdfs:label        "Online Account" ;
        rdfs:subClassOf   owl:Thing ;
        vs:term_status    "unstable" .

<http://www.w3.org/2003/01/geo/wgs84_pos#SpatialThing>
        a       owl:Class .

foaf:tipjar  a              owl:ObjectProperty ;
        rdfs:comment        "\nA tipjar document for this agent, describing means for payment and reward.\n" ;
        rdfs:domain         foaf:Agent ;
        rdfs:isDefinedBy    foaf: ;
        rdfs:label          "tipjar" ;
        rdfs:range          foaffoafiaf- ;
        rdfs:subPropertyOf  foaf:page ;
        vs:term_status      "testing" .

wot:src_assurance  a  owl:AnnotationProperty .

foaf:myersBriggs  a       owl:ObjectProperty ;
        rdfs:comment      "A Myers Briggs (MBTI) personality classification." ;
        rdfs:domain       foaf:Person ;
        rdfs:isDefinedBy  foaf: ;
        rdfs:label        "myersBriggs" ;
        rdfs:range        rdfs:Literal ;
        vs:term_status    "testing" .

foaf:Agent  a             owl:Class ;
        rdfs:comment      "\nAn agent (eg. person, group, software or physical artifact).\n" ;
        rdfs:label        "Agent" ;
        owl:disjointWith  foaffoafiaf- ;
        vs:term_status    "stable" .

foaf:primaryTopic  a      owl:ObjectProperty , owl:FunctionalProperty ;
        rdfs:comment      "The primary topic of some page or document." ;
        rdfs:domain       foaffoafiaf- ;
        rdfs:isDefinedBy  foaf: ;
        rdfs:label        "primary topic" ;
        owl:inverseOf     foaf:isPrimaryTopicOf ;
        vs:term_status    "testing" .

dc:date  a      owl:AnnotationProperty .

foaf:OnlineGamingAccount
        a                 owl:Class ;
        rdfs:comment      "An online gaming account." ;
        rdfs:isDefinedBy  foaf: ;
        rdfs:label        "Online Gaming Account" ;
        rdfs:subClassOf   foaf:OnlineAccount ;
        vs:term_status    "unstable" .

foaf:depiction  a         owl:ObjectProperty ;
        rdfs:comment      "A depiction of some thing." ;
        rdfs:isDefinedBy  foaf: ;
        rdfs:label        "depiction" ;
        rdfs:range        foaf:Image ;
        owl:inverseOf     foaf:depicts ;
        vs:term_status    "testing" .

foaf:workplaceHomepage
        a                 owl:ObjectProperty ;
        rdfs:comment      "\nA workplace homepage of some person; the homepage of an organization they work for.\n" ;
        rdfs:domain       foaf:Person ;
        rdfs:isDefinedBy  foaf: ;
        rdfs:label        "workplace homepage" ;
        rdfs:range        foaf:Document ;
        vs:term_status    "testing" .

foaf:title  a             owl:DatatypeProperty ;
        rdfs:comment      "Title (Mr, Mrs, Ms, Dr. etc)" ;
        rdfs:isDefinedBy  foaf: ;
        rdfs:label        "title" ;
        vs:term_status    "testing" .

foaf:weblog  a              owl:InverseFunctionalProperty , owl:ObjectProperty ;
        rdfs:comment        "\nA weblog of some thing (whether person, group, company etc.).\n" ;
        rdfs:domain         foaf:Agent ;
        rdfs:isDefinedBy    foaf: ;
        rdfs:label          "weblog" ;
        rdfs:range          foaf:Document ;
        rdfs:subPropertyOf  foaf:page ;
        vs:term_status      "testing" .

foaf:thumbnail  a         owl:ObjectProperty ;
        rdfs:comment      "A derived thumbnail image." ;
        rdfs:domain       foaf:Image ;
        rdfs:isDefinedBy  foaf: ;
        rdfs:label        "thumbnail" ;
        rdfs:range        foaf:Image ;
        vs:term_status    "testing" .

foaf:Person  a            owl:Class ;
        rdfs:comment      "A person." ;
        rdfs:isDefinedBy  foaf: ;
        rdfs:label        "Person" ;
        rdfs:subClassOf   <http://www.w3.org/2003/01/geo/wgs84_pos#SpatialThing> , foaf:Agent ;
        owl:disjointWith  foaf:Project , foaf:Document , foaf:Organization ;
        vs:term_status    "stable" .

foaf:nick  a              owl:DatatypeProperty ;
        rdfs:comment      "\nA short informal nickname characterising an agent (includes login identifiers, IRC and other chat nicknames).\n" ;
        rdfs:isDefinedBy  foaf: ;
        rdfs:label        "nickname" ;
        vs:term_status    "testing" .

foaf:made  a              owl:ObjectProperty ;
        rdfs:comment      "Something that was made by this agent." ;
        rdfs:domain       foaf:Agent ;
        rdfs:isDefinedBy  foaf: ;
        rdfs:label        "made" ;
        owl:inverseOf     foaf:maker ;
        vs:term_status    "stable" .

foaf:based_near  a        owl:ObjectProperty ;
        rdfs:comment      "\nA location that something is based near, for some broadly human notion of near.\n" ;
        rdfs:domain       <http://www.w3.org/2003/01/geo/wgs84_pos#SpatialThing> ;
        rdfs:isDefinedBy  foaf: ;
        rdfs:label        "based near" ;
        rdfs:range        <http://www.w3.org/2003/01/geo/wgs84_pos#SpatialThing> ;
        vs:term_status    "unstable" .

foaf:surname  a           owl:DatatypeProperty ;
        rdfs:comment      "The surname of some person." ;
        rdfs:domain       foaf:Person ;
        rdfs:isDefinedBy  foaf: ;
        rdfs:label        "Surname" ;
        rdfs:range        rdfs:Literal ;
        vs:term_status    "testing" .

foaf:plan  a              owl:DatatypeProperty ;
        rdfs:comment      "\nA .plan comment, in the tradition of finger and '.plan' files.\n" ;
        rdfs:domain       foaf:Person ;
        rdfs:isDefinedBy  foaf: ;
        rdfs:label        "plan" ;
        rdfs:range        rdfs:Literal ;
        vs:term_status    "testing" .

foaf:aimChatID  a           owl:DatatypeProperty , owl:InverseFunctionalProperty ;
        rdfs:comment        "An AIM chat ID" ;
        rdfs:domain         foaf:Agent ;
        rdfs:isDefinedBy    foaf: ;
        rdfs:label          "AIM chat ID" ;
        rdfs:range          rdfs:Literal ;
        rdfs:subPropertyOf  foaf:nick ;
        vs:term_status      "testing" .

foaf:Group  a            owl:Class ;
        rdfs:comment     "A class of Agents." ;
        rdfs:label       "Group" ;
        rdfs:subClassOf  foaf:Agent ;
        vs:term_status   "stable" .

foaf:geekcode  a          owl:DatatypeProperty ;
        rdfs:comment      "\nA textual geekcode for this person, see http://www.geekcode.com/geek.html\n" ;
        rdfs:domain       foaf:Person ;
        rdfs:isDefinedBy  foaf: ;
        rdfs:label        "geekcode" ;
        rdfs:range        rdfs:Literal ;
        vs:term_status    "testing" .

dc:title  a     owl:AnnotationProperty .

foaf:Document  a          owl:Class ;
        rdfs:comment      "A document." ;
        rdfs:isDefinedBy  foaf: ;
        rdfs:label        "Document" ;
        owl:disjointWith  foaf:Person , foaf:Organization , foaf:Project ;
        vs:term_status    "testing" .

foaf:topic  a             owl:ObjectProperty ;
        rdfs:comment      "A topic of some page or document." ;
        rdfs:domain       foaf:Document ;
        rdfs:isDefinedBy  foaf: ;
        rdfs:label        "topic" ;
        owl:inverseOf     foaf:page ;
        vs:term_status    "testing" .

foaf:family_name  a       owl:DatatypeProperty ;
        rdfs:comment      "The family_name of some person." ;
        rdfs:domain       foaf:Person ;
        rdfs:isDefinedBy  foaf: ;
        rdfs:label        "family_name" ;
        rdfs:range        rdfs:Literal ;
        vs:term_status    "testing" .

foaf:member  a            owl:ObjectProperty ;
        rdfs:comment      "Indicates a member of a Group" ;
        rdfs:domain       foaf:Group ;
        rdfs:isDefinedBy  foaf: ;
        rdfs:label        "member" ;
        rdfs:range        foaf:Agent ;
        vs:term_status    "stable" .

foaf:theme  a             owl:ObjectProperty ;
        rdfs:comment      "A theme." ;
        rdfs:isDefinedBy  foaf: ;
        rdfs:label        "theme" ;
        vs:term_status    "unstable" .

foaf:publications  a      owl:ObjectProperty ;
        rdfs:comment      "A link to the publications of this person." ;
        rdfs:domain       foaf:Person ;
        rdfs:isDefinedBy  foaf: ;
        rdfs:label        "publications" ;
        rdfs:range        foaf:Document ;
        vs:term_status    "unstable" .