{"@graph":[{"@id":"","@type":"skos:Concept","uri":"","rdf:type":["sioc:topic","foaf:topic"],"foaf:topic":"","rdfs:label":"","skos:definition":"","skos:inScheme":"","skos:broader":[],"skos:narrower":[],"skos:prefLabel":""},{"@id":"https://foafiaf-asteriusj.c9users.io/owl/foafiaf#Values","@type":"skos:ConceptScheme","skos:HasTopConcept":["value:01","value:02","value:03","value:04","value:05","value:06","value:07","value:08","value:09"],"foaf:topic":"Our Shared values","rdfs:label":"OUR SHARED VALUES","skos:definition":"We, as community members of the Rockford Region, desire to achieve our vision for transformational change and will uphold the following shared values as the foundation for a civil and cultivating environment"},{"@id":"value:01","@type":"skos:Concept","rdf:type":["sioc:topic","foaf:topic"],"foaf:topic":"Inclusion","rdfs:label":"Inclusion","owl:sameAs":"","skos:exactMatch":"","skos:inScheme":"https://foafiaf-asteriusj.c9users.io/owl/foafiaf#Values","skos:narrower":[],"skos:definition":"Cultivate and support an environment that fully engages our community’s differences and diversity to ensure that individuals and organizations are heard, valued and supported.","skos:altLabel":"Inclusion: Cultivate and support an environment that fully engages our community’s differences and diversity to ensure that individuals and organizations are heard, valued and supported.","skos:prefLabel":"Inclusion"},{"@id":"value:02","@type":"skos:Concept","rdf:type":["sioc:topic","foaf:topic"],"foaf:topic":"Caring","rdfs:label":"Caring","owl:sameAs":"","skos:exactMatch":"","skos:inScheme":"https://foafiaf-asteriusj.c9users.io/owl/foafiaf#Values","skos:narrower":[],"skos:definition":"Show concern for the welfare of each person and foster a community culture that thinks and acts as one interactive and interdependent region.","skos:altLabel":"Caring: Show concern for the welfare of each person and foster a community culture that thinks and acts as one interactive and interdependent region.","skos:prefLabel":"Caring"},{"@id":"value:03","@type":"skos:Concept","rdf:type":["sioc:topic","foaf:topic"],"foaf:topic":"Respect","rdfs:label":"Respect","owl:sameAs":"","skos:exactMatch":"","skos:inScheme":"https://foafiaf-asteriusj.c9users.io/owl/foafiaf#Values","skos:narrower":[],"skos:definition":"Embrace the knowledge and experiences of others by being attentive, listening well and celebrating diversity as a strength and source of shared learning.","skos:altLabel":"Respect: Embrace the knowledge and experiences of others by being attentive, listening well and celebrating diversity as a strength and source of shared learning.","skos:prefLabel":"Respect"},{"@id":"value:04","@type":"skos:Concept","rdf:type":["sioc:topic","foaf:topic"],"foaf:topic":"Transparency","rdfs:label":"Transparency","owl:sameAs":"","skos:exactMatch":"","skos:inScheme":"https://foafiaf-asteriusj.c9users.io/owl/foafiaf#Values","skos:narrower":[],"skos:definition":"Foster an open process for maximum participant input and access to all information to enhance understanding and community ownership.","skos:altLabel":"Transparency: Foster an open process for maximum participant input and access to all information to enhance understanding and community ownership.","skos:prefLabel":"Transparency"},{"@id":"value:05","@type":"skos:Concept","rdf:type":["sioc:topic","foaf:topic"],"foaf:topic":"Trustworthiness","rdfs:label":"Trustworthiness","owl:sameAs":"","skos:exactMatch":"","skos:inScheme":"https://foafiaf-asteriusj.c9users.io/owl/foafiaf#Values","skos:narrower":[],"skos:definition":"Strive for integrity and reliable communication. Become committed to the highest levels of honesty and truthfulness.","skos:altLabel":"Trustworthiness: Strive for integrity and reliable communication. Become committed to the highest levels of honesty and truthfulness.","skos:prefLabel":"Trustworthiness"},{"@id":"value:06","@type":"skos:Concept","rdf:type":["sioc:topic","foaf:topic"],"foaf:topic":"Unity","rdfs:label":"Unity","owl:sameAs":"","skos:exactMatch":"","skos:inScheme":"https://foafiaf-asteriusj.c9users.io/owl/foafiaf#Values","skos:narrower":[],"skos:definition":"Place the greater good of all parts of our region and its transformation ahead of self or organizational interests.","skos:altLabel":"Unity: Place the greater good of all parts of our region and its transformation ahead of self or organizational interests.","skos:prefLabel":"Unity"},{"@id":"value:07","@type":"skos:Concept","rdf:type":["sioc:topic","foaf:topic"],"foaf:topic":"Ideation","rdfs:label":"Ideation","owl:sameAs":"","skos:exactMatch":"","skos:inScheme":"https://foafiaf-asteriusj.c9users.io/owl/foafiaf#Values","skos:narrower":[],"skos:definition":"Balance our brainstorming and decision-making process with all points of view and measurable information.","skos:altLabel":"Ideation: Balance our brainstorming and decision-making process with all points of view and measurable information.","skos:prefLabel":"Ideation"},{"@id":"value:08","@type":"skos:Concept","rdf:type":["sioc:topic","foaf:topic"],"foaf:topic":"Responsibility","rdfs:label":"Responsibility","owl:sameAs":"","skos:exactMatch":"","skos:inScheme":"https://foafiaf-asteriusj.c9users.io/owl/foafiaf#Values","skos:narrower":[],"skos:definition":"Pursue excellence and accountability of self and others by not shifting blame or taking improper credit. Participate to the fullest of our ability.","skos:altLabel":"Responsibility: Pursue excellence and accountability of self and others by not shifting blame or taking improper credit. Participate to the fullest of our ability.","skos:prefLabel":"Responsibility"},{"@id":"value:09","@type":"skos:Concept","rdf:type":["sioc:topic","foaf:topic"],"foaf:topic":"Interconnectedness","rdfs:label":"Interconnectedness","owl:sameAs":"","skos:exactMatch":"","skos:inScheme":"https://foafiaf-asteriusj.c9users.io/owl/foafiaf#Values","skos:narrower":[],"skos:definition":"Won’t compromise any jurisdiction’s or organization’s identity or decision authority, but rather look to partner and integrate shared values, goals and philosophies.","skos:altLabel":"Interconnectedness Won’t compromise any jurisdiction’s or organization’s identity or decision authority, but rather look to partner and integrate shared values, goals and philosophies.","skos:prefLabel":"Interconnectedness"},{"@id":"spoke:0","@type":"skos:ConceptScheme","rdt:type":"https://foafiaf-asteriusj.c9users.io/owl/foafiaf#Spokes","skos:HasTopConcept":["spoke:01","spoke:02","spoke:03","spoke:04","spoke:05"]},{"@id":"spoke:01","@type":"skos:Concept","rdf:type":["sioc:topic","foaf:topic"],"foaf:topic":"Funding Our Future","rdfs:label":"FUNDING OUR FUTURE","owl:sameAs":"","skos:exactMatch":"","skos:inScheme":"https://foafiaf-asteriusj.c9users.io/owl/foafiaf#Spokes","skos:broader":["spoke:0"],"skos:narrower":[],"skos:definition":{"@value":"","@language":"en-gb"},"skos:prefLabel":{"@value":"FUNDING OUR FUTURE: ","@language":"en-gb"}},{"@id":"spoke:02","@type":"skos:Concept","rdf:type":["sioc:topic","foaf:topic"],"foaf:topic":"Reframing a 21st Century Community","rdfs:label":"REFRAMING A 21ST CENTURY COMMUNITY","owl:sameAs":"","skos:exactMatch":"","skos:inScheme":"https://foafiaf-asteriusj.c9users.io/owl/foafiaf#Spokes","skos:broader":["spoke:0"],"skos:narrower":[],"skos:definition":{"@value":"","@language":"en-gb"},"skos:prefLabel":{"@value":"REFRAMING A 21ST CENTURY COMMUNITY: ","@language":"en-gb"}},{"@id":"spoke:03","@type":"skos:Concept","rdf:type":["sioc:topic","foaf:topic"],"foaf:topic":"Renewal","rdfs:label":"RENEWAL","owl:sameAs":"","skos:exactMatch":"","skos:inScheme":"https://foafiaf-asteriusj.c9users.io/owl/foafiaf#Spokes","skos:broader":["spoke:0"],"skos:narrower":[],"skos:definition":{"@value":"","@language":"en-gb"},"skos:prefLabel":{"@value":"RENEWAL: ","@language":"en-gb"}},{"@id":"spoke:04","@type":"skos:Concept","rdf:type":["sioc:topic","foaf:topic"],"foaf:topic":"Revitalization","rdfs:label":"REVITALIZATION","owl:sameAs":"","skos:exactMatch":"","skos:inScheme":"https://foafiaf-asteriusj.c9users.io/owl/foafiaf#Spokes","skos:broader":["spoke:0"],"skos:narrower":[],"skos:definition":{"@value":"","@language":"en-gb"},"skos:prefLabel":{"@value":"REVITALIZATION: ","@language":"en-gb"}},{"@id":"spoke:05","@type":"skos:Concept","rdf:type":["sioc:topic","foaf:topic"],"foaf:topic":"Sense of Place","rdfs:label":"SENSE OF PLACE","owl:sameAs":"","skos:exactMatch":"","skos:inScheme":"https://foafiaf-asteriusj.c9users.io/owl/foafiaf#Spokes","skos:broader":["spoke:0"],"skos:narrower":[],"skos:definition":{"@value":"","@language":"en-gb"},"skos:prefLabel":{"@value":"SENSE OF PLACE: ","@language":"en-gb"}},{"@id":"segment:0","@type":"skos:ConceptScheme","rdf:type":"https://foafiaf-asteriusj.c9users.io/owl/foafiaf#Segments","skos:HasTopConcept":["segment:01","segment:02","segment:03","segment:04","_Segment_HealthyLifestyles","segment:05","segment:06","segment:07","segment:08","segment:09","segment:10","segment:11","segment:12","segment:13","segment:14"]},{"@id":"_Segment_HealthyLifestyles","@type":"skos:Concept","rdf:type":["sioc:topic","foaf:topic"],"foaf:topic":"Healthy Lifestyles","rdfs:label":"Healthy Lifestyles","owl:sameAs":"","skos:exactMatch":"","skos:inScheme":"https://foafiaf-asteriusj.c9users.io/owl/foafiaf#Segments","skos:broader":["segment:0","spoke:03"],"skos:narrower":[],"skos:definition":{"@value":"","@language":"en-gb"},"skos:prefLabel":{"@value":"HealthyLifestyles: ","@language":"en-gb"}},{"@id":"strategy:0","rdf:type":"https://foafiaf-asteriusj.c9users.io/owl/foafiaf#Strategies","@type":"skos:ConceptScheme","skos:HasTopConcept":["_Strategy_EatforHealth","_Strategy_MoveMore","_Strategy_LoveandBeLoved"]},{"@id":"_Strategy_EatforHealth","@type":"skos:Concept","rdf:type":["sioc:topic","foaf:topic"],"foaf:topic":"Eat for Health Objective","rdfs:label":"Eat for Health","title":"We are a community where healthy food choices are accessible to all and the easy choice.","owl:sameAs":"","skos:exactMatch":"","skos:inScheme":"https://foafiaf-asteriusj.c9users.io/owl/foafiaf#Strategies","skos:broader":["strategy:0","_Segment_HealthyLifestyles"],"skos:narrower":[],"skos:definition":{"@value":"","@language":"en-gb"},"skos:prefLabel":{"@value":"Eat for Health ","@language":"en-gb"}},{"@id":"_Strategy_MoveMore","@type":"skos:Concept","rdf:type":["sioc:topic","foaf:topic"],"foaf:topic":"Move More Objective","rdfs:label":"Move More","title":"We are a community of active living where all have access to recreational opportunities.","owl:sameAs":"","skos:exactMatch":"","skos:inScheme":"https://foafiaf-asteriusj.c9users.io/owl/foafiaf#Strategies","skos:broader":["strategy:0","_Segment_HealthyLifestyles"],"skos:narrower":[],"skos:definition":{"@value":"","@language":"en-gb"},"skos:prefLabel":{"@value":"Move More ","@language":"en-gb"}},{"@id":"_Strategy_LoveandBeLoved","@type":"skos:Concept","rdf:type":["sioc:topic","foaf:topic"],"foaf:topic":"Love and Be Loved Objective","rdfs:label":"Love and Be Loved","title":"We have healthy social and emotional development for everyone at all stages of life.","owl:sameAs":"","skos:exactMatch":"","skos:inScheme":"https://foafiaf-asteriusj.c9users.io/owl/foafiaf#Strategies","skos:broader":["strategy:0","_Segment_HealthyLifestyles"],"skos:narrower":[],"skos:definition":{"@value":"","@language":"en-gb"},"skos:prefLabel":{"@value":"Love and Be Loved","@language":"en-gb"}}],"@id":"urn:x-arq:DefaultGraphNode","@context":[{"foaf":"http://xmlns.com/foaf/0.1/"},{"org":"http://www.w3.org/ns/org#"},{"dbo":"http://dbpedia.org/ontology/"},{"dbp":"http://dbpedia.org/property/"},{"dbr":"http://dbpedia.org/resource/"},{"dct":"http://purl.org/dc/terms"},{"owl":"http://www.w3.org/2002/07/owl#"},{"geo":"http://www.w3.org/2003/01/geo/wgs84_pos#"},{"url":"http://schema.org/url"},{"rdf":"http://www.w3.org/1999/02/22-rdf-syntax-ns#"},{"rdfs":"http://www.w3.org/2000/01/rdf-schema#"},{"skos":"http://www.w3.org/2004/02/skos/core#"},{"vision":"https://foafiaf-asteriusj.c9users.io/owl/foafiaf#Visions"},{"segment":"https://foafiaf-asteriusj.c9users.io/owl/foafiaf#Values"},{"spoke":"https://foafiaf-asteriusj.c9users.io/owl/foafiaf#Segments"},{"value":"https://foafiaf-asteriusj.c9users.io/owl/foafiaf#Spokes"},{"sector":"https://foafiaf-asteriusj.c9users.io/owl/foafiaf#Sectors/"},{"skill":"https://foafiaf-asteriusj.c9users.io/owl/foafiaf#Skills"},{"interest":"https://foafiaf-asteriusj.c9users.io/owl/foafiaf#Interests"},{"foaf":"http://xmlns.com/foaf/0.1/"},{"org":"http://www.w3.org/ns/org#"},{"dbo":"http://dbpedia.org/ontology/"},{"dbp":"http://dbpedia.org/property/"},{"dbr":"http://dbpedia.org/resource/"},{"dct":"http://purl.org/dc/terms"},{"owl":"http://www.w3.org/2002/07/owl#"},{"geo":"http://www.w3.org/2003/01/geo/wgs84_pos#"},{"url":"http://schema.org/url"},{"rdf":"http://www.w3.org/1999/02/22-rdf-syntax-ns#"},{"skos":"http://www.w3.org/2004/02/skos/core#"},{"vision":"https://foafiaf-asteriusj.c9users.io/owl/foafiaf#Visions"},{"segment":"https://foafiaf-asteriusj.c9users.io/owl/foafiaf#Values"},{"spoke":"https://foafiaf-asteriusj.c9users.io/owl/foafiaf#Segments"},{"value":"https://foafiaf-asteriusj.c9users.io/owl/foafiaf#Spokes"},{"sector":"https://foafiaf-asteriusj.c9users.io/owl/foafiaf#Sectors/"},{"skill":"https://foafiaf-asteriusj.c9users.io/owl/foafiaf#Skills"},{"interest":"https://foafiaf-asteriusj.c9users.io/owl/foafiaf#Interests"},{"foaf":"http://xmlns.com/foaf/0.1/"},{"org":"http://www.w3.org/ns/org#"},{"dbo":"http://dbpedia.org/ontology/"},{"dbp":"http://dbpedia.org/property/"},{"dbr":"http://dbpedia.org/resource/"},{"dct":"http://purl.org/dc/terms"},{"owl":"http://www.w3.org/2002/07/owl#"},{"geo":"http://www.w3.org/2003/01/geo/wgs84_pos#"},{"url":"http://schema.org/url"},{"rdf":"http://www.w3.org/1999/02/22-rdf-syntax-ns#"},{"skos":"http://www.w3.org/2004/02/skos/core#"},{"vision":"https://foafiaf-asteriusj.c9users.io/owl/foafiaf#Visions"},{"segment":"https://foafiaf-asteriusj.c9users.io/owl/foafiaf#Values"},{"spoke":"https://foafiaf-asteriusj.c9users.io/owl/foafiaf#Segments"},{"value":"https://foafiaf-asteriusj.c9users.io/owl/foafiaf#Spokes"},{"sector":"https://foafiaf-asteriusj.c9users.io/owl/foafiaf#Sectors/"},{"skill":"https://foafiaf-asteriusj.c9users.io/owl/foafiaf#Skills"},{"interest":"https://foafiaf-asteriusj.c9users.io/owl/foafiaf#Interests"},{"foaf":"http://xmlns.com/foaf/0.1/"},{"org":"http://www.w3.org/ns/org#"},{"dbo":"http://dbpedia.org/ontology/"},{"dbp":"http://dbpedia.org/property/"},{"dbr":"http://dbpedia.org/resource/"},{"dct":"http://purl.org/dc/terms"},{"owl":"http://www.w3.org/2002/07/owl#"},{"geo":"http://www.w3.org/2003/01/geo/wgs84_pos#"},{"url":"http://schema.org/url"},{"rdf":"http://www.w3.org/1999/02/22-rdf-syntax-ns#"},{"skos":"http://www.w3.org/2004/02/skos/core#"},{"strategy":"https://foafiaf-asteriusj.c9users.io/owl/foafiaf#Strategies"},{"vision":"https://foafiaf-asteriusj.c9users.io/owl/foafiaf#Visions"},{"segment":"https://foafiaf-asteriusj.c9users.io/owl/foafiaf#Values"},{"spoke":"https://foafiaf-asteriusj.c9users.io/owl/foafiaf#Segments"},{"value":"https://foafiaf-asteriusj.c9users.io/owl/foafiaf#Spokes"},{"sector":"https://foafiaf-asteriusj.c9users.io/owl/foafiaf#Sectors/"},{"skill":"https://foafiaf-asteriusj.c9users.io/owl/foafiaf#Skills"},{"interest":"https://foafiaf-asteriusj.c9users.io/owl/foafiaf#Interests"}]}