{
  "@graph": [
    {
      "@id": "",
      "@type": "skos:Concept",
      "uri": "",
      "rdf:type": [
        "sioc:topic",
        "foaf:topic"
      ],
      "foaf:topic": "",
      "rdfs:label": "",
      "skos:definition": "",
      "skos:inScheme": "",
      "skos:broader": [
        
      ],
      "skos:narrower": [
        
      ],
      "skos:prefLabel": ""
    },
    {
      "@id": "https://foafiaf-asteriusj.c9users.io/owl/foafiaf#Values",
      "@type": "skos:ConceptScheme",
      "skos:HasTopConcept": [
        "value:01",
        "value:02",
        "value:03",
        "value:04",
        "value:05",
        "value:06",
        "value:07",
        "value:08",
        "value:09"
      ],
      "foaf:topic": "Our Shared values",
      "rdfs:label": "OUR SHARED VALUES",
      "skos:definition": "We, as community members of the Rockford Region, desire to achieve our vision for transformational change and will uphold the following shared values as the foundation for a civil and cultivating environment"
    },
    {
      "@id": "value:01",
      "@type": "skos:Concept",
      "rdf:type": [
        "sioc:topic",
        "foaf:topic"
      ],
      "foaf:topic": "Inclusion",
      "rdfs:label": "Inclusion",
      "owl:sameAs": "",
      "skos:exactMatch": "",
      "skos:inScheme": "https://foafiaf-asteriusj.c9users.io/owl/foafiaf#Values",
      "skos:narrower": [
        
      ],
      "skos:definition": "Cultivate and support an environment that fully engages our community’s differences and diversity to ensure that individuals and organizations are heard, valued and supported.",
      "skos:altLabel": "Inclusion: Cultivate and support an environment that fully engages our community’s differences and diversity to ensure that individuals and organizations are heard, valued and supported.",
      "skos:prefLabel": "Inclusion"
    },
    {
      "@id": "value:02",
      "@type": "skos:Concept",
      "rdf:type": [
        "sioc:topic",
        "foaf:topic"
      ],
      "foaf:topic": "Caring",
      "rdfs:label": "Caring",
      "owl:sameAs": "",
      "skos:exactMatch": "",
      "skos:inScheme": "https://foafiaf-asteriusj.c9users.io/owl/foafiaf#Values",
      "skos:narrower": [
        
      ],
      "skos:definition": "Show concern for the welfare of each person and foster a community culture that thinks and acts as one interactive and interdependent region.",
      "skos:altLabel": "Caring: Show concern for the welfare of each person and foster a community culture that thinks and acts as one interactive and interdependent region.",
      "skos:prefLabel": "Caring"
    },
    {
      "@id": "value:03",
      "@type": "skos:Concept",
      "rdf:type": [
        "sioc:topic",
        "foaf:topic"
      ],
      "foaf:topic": "Respect",
      "rdfs:label": "Respect",
      "owl:sameAs": "",
      "skos:exactMatch": "",
      "skos:inScheme": "https://foafiaf-asteriusj.c9users.io/owl/foafiaf#Values",
      "skos:narrower": [
        
      ],
      "skos:definition": "Embrace the knowledge and experiences of others by being attentive, listening well and celebrating diversity as a strength and source of shared learning.",
      "skos:altLabel": "Respect: Embrace the knowledge and experiences of others by being attentive, listening well and celebrating diversity as a strength and source of shared learning.",
      "skos:prefLabel": "Respect"
    },
    {
      "@id": "value:04",
      "@type": "skos:Concept",
      "rdf:type": [
        "sioc:topic",
        "foaf:topic"
      ],
      "foaf:topic": "Transparency",
      "rdfs:label": "Transparency",
      "owl:sameAs": "",
      "skos:exactMatch": "",
      "skos:inScheme": "https://foafiaf-asteriusj.c9users.io/owl/foafiaf#Values",
      "skos:narrower": [
        
      ],
      "skos:definition": "Foster an open process for maximum participant input and access to all information to enhance understanding and community ownership.",
      "skos:altLabel": "Transparency: Foster an open process for maximum participant input and access to all information to enhance understanding and community ownership.",
      "skos:prefLabel": "Transparency"
    },
    {
      "@id": "value:05",
      "@type": "skos:Concept",
      "rdf:type": [
        "sioc:topic",
        "foaf:topic"
      ],
      "foaf:topic": "Trustworthiness",
      "rdfs:label": "Trustworthiness",
      "owl:sameAs": "",
      "skos:exactMatch": "",
      "skos:inScheme": "https://foafiaf-asteriusj.c9users.io/owl/foafiaf#Values",
      "skos:narrower": [
        
      ],
      "skos:definition": "Strive for integrity and reliable communication. Become committed to the highest levels of honesty and truthfulness.",
      "skos:altLabel": "Trustworthiness: Strive for integrity and reliable communication. Become committed to the highest levels of honesty and truthfulness.",
      "skos:prefLabel": "Trustworthiness"
    },
    {
      "@id": "value:06",
      "@type": "skos:Concept",
      "rdf:type": [
        "sioc:topic",
        "foaf:topic"
      ],
      "foaf:topic": "Unity",
      "rdfs:label": "Unity",
      "owl:sameAs": "",
      "skos:exactMatch": "",
      "skos:inScheme": "https://foafiaf-asteriusj.c9users.io/owl/foafiaf#Values",
      "skos:narrower": [
        
      ],
      "skos:definition": "Place the greater good of all parts of our region and its transformation ahead of self or organizational interests.",
      "skos:altLabel": "Unity: Place the greater good of all parts of our region and its transformation ahead of self or organizational interests.",
      "skos:prefLabel": "Unity"
    },
    {
      "@id": "value:07",
      "@type": "skos:Concept",
      "rdf:type": [
        "sioc:topic",
        "foaf:topic"
      ],
      "foaf:topic": "Ideation",
      "rdfs:label": "Ideation",
      "owl:sameAs": "",
      "skos:exactMatch": "",
      "skos:inScheme": "https://foafiaf-asteriusj.c9users.io/owl/foafiaf#Values",
      "skos:narrower": [
        
      ],
      "skos:definition": "Balance our brainstorming and decision-making process with all points of view and measurable information.",
      "skos:altLabel": "Ideation: Balance our brainstorming and decision-making process with all points of view and measurable information.",
      "skos:prefLabel": "Ideation"
    },
    {
      "@id": "value:08",
      "@type": "skos:Concept",
      "rdf:type": [
        "sioc:topic",
        "foaf:topic"
      ],
      "foaf:topic": "Responsibility",
      "rdfs:label": "Responsibility",
      "owl:sameAs": "",
      "skos:exactMatch": "",
      "skos:inScheme": "https://foafiaf-asteriusj.c9users.io/owl/foafiaf#Values",
      "skos:narrower": [
        
      ],
      "skos:definition": "Pursue excellence and accountability of self and others by not shifting blame or taking improper credit. Participate to the fullest of our ability.",
      "skos:altLabel": "Responsibility: Pursue excellence and accountability of self and others by not shifting blame or taking improper credit. Participate to the fullest of our ability.",
      "skos:prefLabel": "Responsibility"
    },
    {
      "@id": "value:09",
      "@type": "skos:Concept",
      "rdf:type": [
        "sioc:topic",
        "foaf:topic"
      ],
      "foaf:topic": "Interconnectedness",
      "rdfs:label": "Interconnectedness",
      "owl:sameAs": "",
      "skos:exactMatch": "",
      "skos:inScheme": "https://foafiaf-asteriusj.c9users.io/owl/foafiaf#Values",
      "skos:narrower": [
        
      ],
      "skos:definition": "Won’t compromise any jurisdiction’s or organization’s identity or decision authority, but rather look to partner and integrate shared values, goals and philosophies.",
      "skos:altLabel": "Interconnectedness Won’t compromise any jurisdiction’s or organization’s identity or decision authority, but rather look to partner and integrate shared values, goals and philosophies.",
      "skos:prefLabel": "Interconnectedness"
    }
  ],
  "@id": "urn:x-arq:DefaultGraphNode",
  "@context": {
    "foaf": "http://xmlns.com/foaf/0.1/",
    "org": "http://www.w3.org/ns/org#",
    "dbo": "http://dbpedia.org/ontology/",
    "dbp": "http://dbpedia.org/property/",
    "dbr": "http://dbpedia.org/resource/",
    "dct": "http://purl.org/dc/terms",
    "owl": "http://www.w3.org/2002/07/owl#",
    "geo": "http://www.w3.org/2003/01/geo/wgs84_pos#",
    "url": "http://schema.org/url",
    "rdf": "http://www.w3.org/1999/02/22-rdf-syntax-ns#",
    "rdfs": "http://www.w3.org/2000/01/rdf-schema#",
    "skos": "http://www.w3.org/2004/02/skos/core#",
    "vision": "https://foafiaf-asteriusj.c9users.io/owl/foafiaf#Visions",
    "segment": "https://foafiaf-asteriusj.c9users.io/owl/foafiaf#Values",
    "spoke": "https://foafiaf-asteriusj.c9users.io/owl/foafiaf#Segments",
    "value": "https://foafiaf-asteriusj.c9users.io/owl/foafiaf#Spokes",
    "sector": "https://foafiaf-asteriusj.c9users.io/owl/foafiaf#Sectors/",
    "skill" : "https://foafiaf-asteriusj.c9users.io/owl/foafiaf#Skills",
    "interest" : "https://foafiaf-asteriusj.c9users.io/owl/foafiaf#Interests"
  }
}